@prefix dcterms:      <http://purl.org/dc/terms/> .
@prefix owl:          <http://www.w3.org/2002/07/owl#> .
@prefix prov:         <http://www.w3.org/ns/prov#> .
@prefix rdf:          <http://www.w3.org/1999/02/22-rdf-syntax-ns#> .
@prefix rdfs:         <http://www.w3.org/2000/01/rdf-schema#> .
@prefix reg:          <http://purl.org/linked-data/registry#> .
@prefix sdo:          <https://schema.org/> .
@prefix skos:         <http://www.w3.org/2004/02/skos/core#> .


skos:prefLabel  rdfs:label  "preferred label"@en .

skos:member  rdfs:label  "has member"@en .

dcterms:identifier  rdfs:label  "Identifier"@en .

skos:hasTopConcept  rdfs:label  "has top concept"@en .

<http://www.w3.org/1999/02/22-rdf-syntax-ns#type>
        rdfs:label  "type" .

skos:Concept  rdfs:label  "Concept"@en .

rdfs:isDefinedBy  rdfs:label  "is defined by" .

skos:topConceptOf  rdfs:label  "is top concept in scheme"@en .

skos:definition  rdfs:label  "definition"@en .

<https://linked.data.gov.au/org/gsq>
        rdfs:label  "Geological Survey of Queensland" .

skos:inScheme  rdfs:label  "is in scheme"@en .

dcterms:provenance  rdfs:label  "Provenance"@en .

skos:altLabel  rdfs:label  "alternative label"@en .

skos:notation  rdfs:label  "notation"@en .

skos:Collection  rdfs:label  "Collection"@en .

dcterms:created  rdfs:label  "Date Created"@en .

skos:ConceptScheme  rdfs:label  "Concept Scheme"@en .

dcterms:modified  rdfs:label  "Date Modified"@en .

dcterms:creator  rdfs:label  "Creator"@en .

dcterms:publisher  rdfs:label  "Publisher"@en .

owl:Ontology  a       rdfs:Class ;
        rdfs:comment  "The class of ontologies" ;
        rdfs:label    "Ontology" .

reg:status  rdfs:label  "status"@en .

<http://def.isotc211.org/iso19135/-1/2015/CoreModel/code/RE_ItemStatus/submitted>
        rdfs:label  "submitted" .

<https://linked.data.gov.au/org/gswa>
        rdfs:label  "Geological Survey of Western Australia" .

skos:broader  rdfs:label  "has broader"@en .

sdo:name  rdfs:comment  "The name of the item." ;
        rdfs:label    "name" .

sdo:url  rdfs:comment  "URL of the item." ;
        rdfs:label    "url" .

sdo:Organization  rdfs:comment  "An organization such as a school, NGO, corporation, club, etc." ;
        rdfs:label    "Organization" .

dcterms:source  rdfs:label  "Source"@en .

skos:editorialNote  rdfs:label  "editorial note"@en .

<https://linked.data.gov.au/org/cgi>
        rdfs:label  "Commission for Geoscience Information" .

skos:narrower  rdfs:label  "has narrower"@en .

<https://linked.data.gov.au/org/cgi-gtwg>
        rdfs:label  "CGI Geoscience Terminology Working Group" .

skos:changeNote  rdfs:label  "change note"@en .

sdo:affiliation  rdfs:comment  "An organization that this person is affiliated with. For example, a school/university, a club, or a team." ;
        rdfs:label    "affiliation" .

prov:entity  rdfs:label  "entity" .

prov:qualifiedDerivation
        rdfs:comment  "If this Entity prov:wasDerivedFrom Entity :e, then it can qualify how it was derived using prov:qualifiedDerivation [ a prov:Derivation;  prov:entity :e; :foo :bar ]."@en ;
        rdfs:label    "qualified derivation" .

prov:hadRole  rdfs:comment  "This property has multiple RDFS domains to suit multiple OWL Profiles. See <a href=\"#owl-profile\">PROV-O OWL Profile</a>." , "The _optional_ Role that an Entity assumed in the context of an Activity. For example, :baking prov:used :spoon; prov:qualified [ a prov:Usage; prov:entity :spoon; prov:hadRole roles:mixing_implement ]."@en ;
        rdfs:label    "had role" .

skos:exactMatch  rdfs:label  "has exact match"@en .

<http://www.w3.org/2006/time#months>
        rdfs:label  "months duration" .

rdfs:label  rdfs:label  "label" .

<http://www.w3.org/2006/time#hasTemporalDuration>
        rdfs:label  "has temporal duration" .

<http://www.w3.org/2006/time#minute>
        rdfs:label  "minute" .

<http://www.w3.org/2006/time#day>
        rdfs:label  "day" .

<http://www.w3.org/2006/time#after>
        rdfs:label  "after" .

<http://www.w3.org/2006/time#unitHour>
        rdfs:label  "Hour (unit of temporal duration)" , "hour" .

<http://www.w3.org/2006/time#inDateTime>
        rdfs:label  "in date-time description" .

<http://www.w3.org/2006/time#intervalBefore>
        rdfs:label  "interval before" .

<http://www.w3.org/2006/time#timeZone>
        rdfs:label  "in time zone" .

<http://www.w3.org/2006/time#TimeZone>
        rdfs:label  "Time Zone" .

<http://www.w3.org/2006/time#inTimePosition>
        rdfs:label  "Time position" .

<http://www.w3.org/2006/time#monthOfYear>
        rdfs:label  "month of year" .

<http://www.w3.org/2006/time#unitMonth>
        rdfs:label  "Month (unit of temporal duration)" , "month" .

<http://www.w3.org/2006/time#xsdDateTime>
        rdfs:label  "has XSD date-time" .

<http://www.w3.org/2006/time#TemporalDuration>
        rdfs:label  "Temporal duration" .

<http://www.w3.org/2006/time#intervalMetBy>
        rdfs:label  "interval met by" .

<http://www.w3.org/2006/time#intervalContains>
        rdfs:label  "interval contains" .

<http://www.w3.org/2006/time#TimePosition>
        rdfs:label  "Time position" .

<http://www.w3.org/2006/time#seconds>
        rdfs:label  "seconds duration" .

<http://www.w3.org/2006/time#Thursday>
        rdfs:label  "Thursday" .

<http://www.w3.org/2006/time#TemporalUnit>
        rdfs:label  "Temporal unit" .

<http://www.w3.org/2006/time#unitMinute>
        rdfs:label  "minute" , "Minute (unit of temporal duration)" .

<http://www.w3.org/2006/time#inXSDgYearMonth>
        rdfs:label  "in XSD g-YearMonth" .

<http://www.w3.org/2006/time#ProperInterval>
        rdfs:label  "Proper interval" .

<http://www.w3.org/2006/time#Friday>
        rdfs:label  "Friday" .

<http://www.w3.org/2006/time#DayOfWeek>
        rdfs:label  "Day of week" .

<http://www.w3.org/2006/time#hasTime>
        rdfs:label  "has time" .

<http://www.w3.org/2006/time#hasDurationDescription>
        rdfs:label  "has duration description" .

<http://www.w3.org/2006/time#unitWeek>
        rdfs:label  "week" , "Week (unit of temporal duration)" .

<http://www.w3.org/2006/time#inTemporalPosition>
        rdfs:label  "Temporal position" .

<http://www.w3.org/2006/time#minutes>
        rdfs:label  "minutes" .

<http://www.w3.org/2006/time#unitSecond>
        rdfs:label  "Second (unit of temporal duration)" , "second" .

<http://www.w3.org/2006/time#TemporalEntity>
        rdfs:label  "Temporal entity" .

<http://www.w3.org/2006/time#dayOfYear>
        rdfs:label  "day of year" .

<http://www.w3.org/2006/time#intervalAfter>
        rdfs:label  "interval after" .

<http://www.w3.org/2006/time>
        rdfs:label  "OWL-Time" .

<http://www.w3.org/2006/time#intervalDuring>
        rdfs:label  "interval during" .

<http://www.w3.org/2006/time#before>
        rdfs:label  "before" .

<http://www.w3.org/2006/time#intervalFinishedBy>
        rdfs:label  "interval finished by" .

<http://www.w3.org/2006/time#unitType>
        rdfs:label  "temporal unit type" .

<http://www.w3.org/2006/time#DurationDescription>
        rdfs:label  "Duration description" .

<http://www.w3.org/2006/time#intervalFinishes>
        rdfs:label  "interval finishes" .

<http://www.w3.org/2006/time#hasDateTimeDescription>
        rdfs:label  "has Date-Time description" .

<http://www.w3.org/2006/time#unitDay>
        rdfs:label  "day" , "Day (unit of temporal duration)" .

<http://www.w3.org/2006/time#TemporalPosition>
        rdfs:label  "Temporal position" .

<http://www.w3.org/2006/time#inXSDDate>
        rdfs:label  "in XSD date" .

<http://www.w3.org/2006/time#unitYear>
        rdfs:label  "year" , "Year (unit of temporal duration)" .

<http://www.w3.org/2006/time#numericPosition>
        rdfs:label  "Numeric value of temporal position" .

<http://www.w3.org/2006/time#days>
        rdfs:label  "days duration" .

<http://www.w3.org/2006/time#nominalPosition>
        rdfs:label  "Name of temporal position" .

<http://www.w3.org/2006/time#hasBeginning>
        rdfs:label  "has beginning" .

<http://www.w3.org/2006/time#Instant>
        rdfs:label  "Time instant" .

<http://www.w3.org/2006/time#GeneralDurationDescription>
        rdfs:label  "Generalized duration description" .

<http://www.w3.org/2006/time#hasXSDDuration>
        rdfs:label  "has XSD duration" .

<http://www.w3.org/2006/time#week>
        rdfs:label  "week" .

<http://www.w3.org/2006/time#Year>
        rdfs:label  "Year" .

<http://www.w3.org/2006/time#Wednesday>
        rdfs:label  "Wednesday" .

<http://www.w3.org/2006/time#years>
        rdfs:label  "years duration" .

<http://www.w3.org/2006/time#Tuesday>
        rdfs:label  "Tuesday" .

<http://www.w3.org/2006/time#month>
        rdfs:label  "month" .

<http://www.w3.org/2006/time#numericDuration>
        rdfs:label  "Numeric value of temporal duration" .

<http://www.w3.org/2006/time#inXSDDateTimeStamp>
        rdfs:label  "in XSD Date-Time-Stamp" .

<http://www.w3.org/2006/time#MonthOfYear>
        rdfs:label  "Month of year" .

<http://www.w3.org/2006/time#Duration>
        rdfs:label  "Time duration" .

<http://www.w3.org/2006/time#hasEnd>
        rdfs:label  "has end" .

<http://www.w3.org/2006/time#Interval>
        rdfs:label  "Time interval" .

<http://www.w3.org/2006/time#intervalEquals>
        rdfs:label  "interval equals" .

<http://www.w3.org/2006/time#Monday>
        rdfs:label  "Monday" .

<http://www.w3.org/2006/time#year>
        rdfs:label  "year" .

<http://www.w3.org/2006/time#generalMonth>
        rdfs:label  "Generalized month" .

<http://www.w3.org/2006/time#generalDay>
        rdfs:label  "Generalized day" .

<http://www.w3.org/2006/time#hours>
        rdfs:label  "hours duration" .

<http://www.w3.org/2006/time#hasTRS>
        rdfs:label  "Temporal reference system used" .

<http://www.w3.org/2006/time#intervalIn>
        rdfs:label  "interval in" .

<http://www.w3.org/2006/time#dayOfWeek>
        rdfs:label  "day of week" .

<http://www.w3.org/2006/time#inside>
        rdfs:label  "has time instant inside" .

<http://www.w3.org/2006/time#TRS>
        rdfs:label  "Temporal Reference System" .

<http://www.w3.org/2006/time#intervalStartedBy>
        rdfs:label  "interval started by" .

<http://www.w3.org/2006/time#inXSDgYear>
        rdfs:label  "in XSD g-Year" .

<http://www.w3.org/2006/time#DateTimeDescription>
        rdfs:label  "Date-Time description" .

<http://www.w3.org/2006/time#weeks>
        rdfs:label  "weeks duration" .

<http://www.w3.org/2006/time#intervalStarts>
        rdfs:label  "interval starts" .

<http://www.w3.org/2006/time#generalYear>
        rdfs:label  "Generalized year" .

<http://www.w3.org/2006/time#Sunday>
        rdfs:label  "Sunday" .

<http://www.w3.org/2006/time#hasDuration>
        rdfs:label  "has duration" .

<http://www.w3.org/2006/time#intervalOverlaps>
        rdfs:label  "interval overlaps" .

<http://www.w3.org/2006/time#intervalOverlappedBy>
        rdfs:label  "interval overlapped by" .

<http://www.w3.org/2006/time#intervalMeets>
        rdfs:label  "interval meets" .

<http://www.w3.org/2006/time#hour>
        rdfs:label  "hour" .

<http://www.w3.org/2006/time#DateTimeInterval>
        rdfs:label  "Date-time interval" .

<http://www.w3.org/2006/time#intervalDisjoint>
        rdfs:label  "interval disjoint" .

<http://www.w3.org/2006/time#inXSDDateTime>
        rdfs:label  "in XSD Date-Time" .

<http://www.w3.org/2006/time#GeneralDateTimeDescription>
        rdfs:label  "Generalized date-time description" .

<http://www.w3.org/2006/time#Saturday>
        rdfs:label  "Saturday" .

<http://www.w3.org/2006/time#second>
        rdfs:label  "second" .

rdfs:comment  rdfs:label  "comment" .

prov:derivedByInsertionFrom
        rdfs:comment  "The dictionary was derived from the other by insertion. prov:qualifiedInsertion shows details of the insertion, in particular the inserted key-entity pairs." ;
        rdfs:label    "derivedByInsertionFrom" .

prov:RightsHolder  rdfs:comment  "Role with the function of owning or managing rights over a resource. The Agent assigned to this role is associated with a RightsAssignment Activity"@en ;
        rdfs:label    "RightsHolder"@en .

prov:Entity  rdfs:comment  "An entity is a physical, digital, conceptual, or other kind of thing with some fixed aspects; entities may be real or imaginary. "@en ;
        rdfs:label    "Entity" .

prov:wasAttributedTo  rdfs:comment  "Attribution is the ascribing of an entity to an agent."@en ;
        rdfs:label    "was attributed to" .

prov:hadActivity  rdfs:comment  "The _optional_ Activity of an Influence, which used, generated, invalidated, or was the responsibility of some Entity. This property is _not_ used by ActivityInfluence (use prov:activity instead)."@en , "This property has multiple RDFS domains to suit multiple OWL Profiles. See <a href=\"#owl-profile\">PROV-O OWL Profile</a>." ;
        rdfs:label    "had activity" .

prov:dm  rdfs:comment  "A reference to the principal section of the PROV-DM document that describes this concept."@en .

prov:Plan  rdfs:comment  "A plan is an entity that represents a set of actions or steps intended by one or more agents to achieve some goals." , "There exist no prescriptive requirement on the nature of plans, their representation, the actions or steps they consist of, or their intended goals. Since plans may evolve over time, it may become necessary to track their provenance, so plans themselves are entities. Representing the plan explicitly in the provenance can be useful for various tasks: for example, to validate the execution as represented in the provenance record, to manage expectation failures, or to provide explanations."@en ;
        rdfs:label    "Plan" .

prov:Bundle  rdfs:comment  "Note that there are kinds of bundles (e.g. handwritten letters, audio recordings, etc.) that are not expressed in PROV-O, but can be still be described by PROV-O."@en , "A bundle is a named set of provenance descriptions, and is itself an Entity, so allowing provenance of provenance to be expressed."@en ;
        rdfs:label    "Bundle" .

prov:actedOnBehalfOf  rdfs:comment  "An object property to express the accountability of an agent towards another agent. The subordinate agent acted on behalf of the responsible agent in an actual activity. "@en ;
        rdfs:label    "acted on behalf of" .

prov:Influence  rdfs:comment  "An instance of prov:Influence provides additional descriptions about the binary prov:wasInfluencedBy relation from some influenced Activity, Entity, or Agent to the influencing Activity, Entity, or Agent. For example, :stomach_ache prov:wasInfluencedBy :spoon; prov:qualifiedInfluence [ a prov:Influence; prov:entity :spoon; :foo :bar ] . Because prov:Influence is a broad relation, the more specific relations (Communication, Delegation, End, etc.) should be used when applicable."@en , "Because prov:Influence is a broad relation, its most specific subclasses (e.g. prov:Communication, prov:Delegation, prov:End, prov:Revision, etc.) should be used when applicable."@en , "Influence is the capacity of an entity, activity, or agent to have an effect on the character, development, or behavior of another by means of usage, start, end, generation, invalidation, communication, derivation, attribution, association, or delegation."@en ;
        rdfs:label    "Influence" .

prov:ServiceDescription
        rdfs:comment  "Type for a generic provenance query service. Mainly for use in RDF provenance query service descriptions, to facilitate discovery in linked data environments." ;
        rdfs:label    "Service Description" .

prov:Contributor  rdfs:comment  "Role with the function of having responsibility for making contributions to a resource. The Agent assigned to this role is associated with a Modify or Create Activities"@en ;
        rdfs:label    "Contributor"@en .

prov:EntityInfluence  rdfs:comment  "EntityInfluence provides additional descriptions of an Entity's binary influence upon any other kind of resource. Instances of EntityInfluence use the prov:entity property to cite the influencing Entity."@en , "It is not recommended that the type EntityInfluence be asserted without also asserting one of its more specific subclasses."@en ;
        rdfs:label    "Entity Influence" .

prov:editorsDefinition
        rdfs:comment  "When the prov-o term does not have a definition drawn from prov-dm, and the prov-o editor provides one."@en .

prov:wasQuotedFrom  rdfs:comment  "An entity is derived from an original entity by copying, or 'quoting', some or all of it."@en ;
        rdfs:label    "was quoted from" .

prov:Association  rdfs:comment  "An instance of prov:Association provides additional descriptions about the binary prov:wasAssociatedWith relation from an prov:Activity to some prov:Agent that had some responsiblity for it. For example, :baking prov:wasAssociatedWith :baker; prov:qualifiedAssociation [ a prov:Association; prov:agent :baker; :foo :bar ]."@en , "An activity association is an assignment of responsibility to an agent for an activity, indicating that the agent had a role in the activity. It further allows for a plan to be specified, which is the plan intended by the agent to achieve some goals in the context of this activity."@en ;
        rdfs:label    "Association" .

prov:Creator  rdfs:comment  "Role with the function of creating a resource. The Agent assigned to this role is associated with a Create Activity"@en ;
        rdfs:label    "Creator"@en .

prov:Start  rdfs:comment  "An instance of prov:Start provides additional descriptions about the binary prov:wasStartedBy relation from some started prov:Activity to an prov:Entity that started it. For example, :foot_race prov:wasStartedBy :bang; prov:qualifiedStart [ a prov:Start; prov:entity :bang; :foo :bar; prov:atTime '2012-03-09T08:05:08-05:00'^^xsd:dateTime ] ."@en , "Start is when an activity is deemed to have been started by an entity, known as trigger. The activity did not exist before its start. Any usage, generation, or invalidation involving an activity follows the activity's start. A start may refer to a trigger entity that set off the activity, or to an activity, known as starter, that generated the trigger."@en ;
        rdfs:label    "Start" .

prov:derivedByRemovalFrom
        rdfs:comment  "The dictionary was derived from the other by removal. prov:qualifiedRemoval shows details of the removal, in particular the removed key-entity pairs." ;
        rdfs:label    "derivedByRemovalFrom" .

prov:endedAtTime  rdfs:comment  "The time at which an activity ended. See also prov:startedAtTime."@en ;
        rdfs:label    "ended at time" .

prov:EmptyDictionary  rdfs:comment  "An empty dictionary (i.e. has no members)." ;
        rdfs:label    "Empty Dictionary" .

prov:PrimarySource  rdfs:comment  "A primary source for a topic refers to something produced by some agent with direct experience and knowledge about the topic, at the time of the topic's study, without benefit from hindsight.\n\nBecause of the directness of primary sources, they 'speak for themselves' in ways that cannot be captured through the filter of secondary sources. As such, it is important for secondary sources to reference those primary sources from which they were derived, so that their reliability can be investigated.\n\nA primary source relation is a particular case of derivation of secondary materials from their primary sources. It is recognized that the determination of primary sources can be up to interpretation, and should be done according to conventions accepted within the application's domain."@en , "An instance of prov:PrimarySource provides additional descriptions about the binary prov:hadPrimarySource relation from some secondary prov:Entity to an earlier, primary prov:Entity. For example, :blog prov:hadPrimarySource :newsArticle; prov:qualifiedPrimarySource [ a prov:PrimarySource; prov:entity :newsArticle; :foo :bar ] ."@en ;
        rdfs:label    "Primary Source" .

prov:Role  rdfs:comment  "A role is the function of an entity or agent with respect to an activity, in the context of a usage, generation, invalidation, association, start, and end."@en ;
        rdfs:label    "Role" .

prov:qualifiedAssociation
        rdfs:comment  "If this Activity prov:wasAssociatedWith Agent :ag, then it can qualify the Association using prov:qualifiedAssociation [ a prov:Association;  prov:agent :ag; :foo :bar ]."@en ;
        rdfs:label    "qualified association" .

prov:pingback  rdfs:comment  "Relates a resource to a provenance pingback service that may receive additional provenance links about the resource."@en ;
        rdfs:label    "provenance pingback" .

prov:AgentInfluence  rdfs:comment  "It is not recommended that the type AgentInfluence be asserted without also asserting one of its more specific subclasses."@en , "AgentInfluence provides additional descriptions of an Agent's binary influence upon any other kind of resource. Instances of AgentInfluence use the prov:agent property to cite the influencing Agent."@en ;
        rdfs:label    "Agent Influence" .

prov:InstantaneousEvent
        rdfs:comment  "The PROV data model is implicitly based on a notion of instantaneous events (or just events), that mark transitions in the world. Events include generation, usage, or invalidation of entities, as well as starting or ending of activities. This notion of event is not first-class in the data model, but it is useful for explaining its other concepts and its semantics."@en , "An instantaneous event, or event for short, happens in the world and marks a change in the world, in its activities and in its entities. The term 'event' is commonly used in process algebra with a similar meaning. Events represent communications or interactions; they are assumed to be atomic and instantaneous."@en ;
        rdfs:label    "Instantaneous Event" .

prov:Location  rdfs:comment  "A location can be an identifiable geographic place (ISO 19112), but it can also be a non-geographic place such as a directory, row, or column. As such, there are numerous ways in which location can be expressed, such as by a coordinate, address, landmark, and so forth."@en ;
        rdfs:label    "Location" .

prov:atLocation  rdfs:comment  "This property has multiple RDFS domains to suit multiple OWL Profiles. See <a href=\"#owl-profile\">PROV-O OWL Profile</a>." , "The Location of any resource."@en ;
        rdfs:label    "atLocation" .

prov:Derivation  rdfs:comment  "The more specific forms of prov:Derivation (i.e., prov:Revision, prov:Quotation, prov:PrimarySource) should be asserted if they apply."@en , "A derivation is a transformation of an entity into another, an update of an entity resulting in a new one, or the construction of a new entity based on a pre-existing entity."@en , "An instance of prov:Derivation provides additional descriptions about the binary prov:wasDerivedFrom relation from some derived prov:Entity to another prov:Entity from which it was derived. For example, :chewed_bubble_gum prov:wasDerivedFrom :unwrapped_bubble_gum; prov:qualifiedDerivation [ a prov:Derivation; prov:entity :unwrapped_bubble_gum; :foo :bar ]."@en ;
        rdfs:label    "Derivation" .

prov:Removal  rdfs:comment  "Removal is a derivation that transforms a dictionary into another, by removing one or more key-entity pairs." ;
        rdfs:label    "Removal" .

prov:Submit  rdfs:comment  "Activity that identifies the issuance (e.g., publication) of a resource. "@en ;
        rdfs:label    "Submit"@en .

prov:wasGeneratedBy  rdfs:label  "was generated by" , "was generatedby" .

prov:Publisher  rdfs:comment  "Role with the function of publishing a resource. The Agent assigned to this role is associated with a Publish Activity"@en ;
        rdfs:label    "Publisher"@en .

prov:qualifiedEnd  rdfs:comment  "If this Activity prov:wasEndedBy Entity :e1, then it can qualify how it was ended using prov:qualifiedEnd [ a prov:End;  prov:entity :e1; :foo :bar ]."@en ;
        rdfs:label    "qualified end" .

prov:SoftwareAgent  rdfs:comment  "A software agent is running software."@en ;
        rdfs:label    "Software Agent" , "SoftwareAgent" .

prov:ActivityInfluence
        rdfs:comment  "ActivityInfluence provides additional descriptions of an Activity's binary influence upon any other kind of resource. Instances of ActivityInfluence use the prov:activity property to cite the influencing Activity."@en , "It is not recommended that the type ActivityInfluence be asserted without also asserting one of its more specific subclasses."@en ;
        rdfs:label    "Activity Influence" .

prov:Dictionary  rdfs:comment  "This concept allows for the provenance of the dictionary, but also of its constituents to be expressed. Such a notion of dictionary corresponds to a wide variety of concrete data structures, such as a maps or associative arrays." , "A given dictionary forms a given structure for its members. A different structure (obtained either by insertion or removal of members) constitutes a different dictionary." , "A dictionary is an entity that provides a structure to some constituents, which are themselves entities. These constituents are said to be member of the dictionary." ;
        rdfs:label    "Dictionary" .

prov:specializationOf
        rdfs:comment  "An entity that is a specialization of another shares all aspects of the latter, and additionally presents more specific aspects of the same thing as the latter. In particular, the lifetime of the entity being specialized contains that of any specialization. Examples of aspects include a time period, an abstraction, and a context associated with the entity."@en ;
        rdfs:label    "specialization of" , "specializationOf" .

prov:DirectQueryService
        rdfs:comment  "Type for a generic provenance query service. Mainly for use in RDF provenance query service descriptions, to facilitate discovery in linked data environments." ;
        rdfs:label    "Provenance Service" .

prov:hadPrimarySource
        rdfs:label  "had primary source" .

prov:qualifiedGeneration
        rdfs:comment  "If this Activity prov:generated Entity :e, then it can qualify how it performed the Generation using prov:qualifiedGeneration [ a prov:Generation;  prov:entity :e; :foo :bar ]."@en ;
        rdfs:label    "qualified generation" .

prov:qualifiedForm  rdfs:comment  "This annotation property links a subproperty of prov:wasInfluencedBy with the subclass of prov:Influence and the qualifying property that are used to qualify it. \n\nExample annotation:\n\n    prov:wasGeneratedBy prov:qualifiedForm prov:qualifiedGeneration, prov:Generation .\n\nThen this unqualified assertion:\n\n    :entity1 prov:wasGeneratedBy :activity1 .\n\ncan be qualified by adding:\n\n   :entity1 prov:qualifiedGeneration :entity1Gen .\n   :entity1Gen \n       a prov:Generation, prov:Influence;\n       prov:activity :activity1;\n       :customValue 1337 .\n\nNote how the value of the unqualified influence (prov:wasGeneratedBy :activity1) is mirrored as the value of the prov:activity (or prov:entity, or prov:agent) property on the influence class."@en .

prov:End  rdfs:comment  "An instance of prov:End provides additional descriptions about the binary prov:wasEndedBy relation from some ended prov:Activity to an prov:Entity that ended it. For example, :ball_game prov:wasEndedBy :buzzer; prov:qualifiedEnd [ a prov:End; prov:entity :buzzer; :foo :bar; prov:atTime '2012-03-09T08:05:08-05:00'^^xsd:dateTime ]."@en , "End is when an activity is deemed to have been ended by an entity, known as trigger. The activity no longer exists after its end. Any usage, generation, or invalidation involving an activity precedes the activity's end. An end may refer to a trigger entity that terminated the activity, or to an activity, known as ender that generated the trigger."@en ;
        rdfs:label    "End" .

prov:Accept  rdfs:comment  "Activity that identifies the acceptance of a resource (e.g., an article in a conference)"@en ;
        rdfs:label    "Accept"@en .

prov:n  rdfs:comment  "A reference to the principal section of the PROV-DM document that describes this concept."@en , "A reference to the principal section of the PROV-M document that describes this concept."@en .

prov:hadPlan  rdfs:comment  "The _optional_ Plan adopted by an Agent in Association with some Activity. Plan specifications are out of the scope of this specification."@en ;
        rdfs:label    "had plan" .

prov:Publish  rdfs:comment  "Activity that identifies the publication of a resource"@en ;
        rdfs:label    "Publish"@en .

prov:generatedAtTime  rdfs:comment  "The time at which an entity was completely created and is available for use."@en ;
        rdfs:label    "generated at time" .

prov:qualifiedCommunication
        rdfs:comment  "If this Activity prov:wasInformedBy Activity :a, then it can qualify how it was influenced using prov:qualifiedCommunication [ a prov:Communication;  prov:activity :a; :foo :bar ]."@en ;
        rdfs:label    "qualified communication" .

prov:Attribution  rdfs:comment  "Attribution is the ascribing of an entity to an agent.\n\nWhen an entity e is attributed to agent ag, entity e was generated by some unspecified activity that in turn was associated to agent ag. Thus, this relation is useful when the activity is not known, or irrelevant."@en , "An instance of prov:Attribution provides additional descriptions about the binary prov:wasAttributedTo relation from an prov:Entity to some prov:Agent that had some responsible for it. For example, :cake prov:wasAttributedTo :baker; prov:qualifiedAttribution [ a prov:Attribution; prov:entity :baker; :foo :bar ]."@en ;
        rdfs:label    "Attribution" .

prov:describesService
        rdfs:comment  "relates a generic provenance query service resource (type prov:ServiceDescription) to a specific query service description (e.g. a prov:DirectQueryService or a sd:Service)."@en ;
        rdfs:label    "describes service" .

prov:Create  rdfs:comment  "Activity that identifies the creation of a resource"@en ;
        rdfs:label    "Create"@en .

prov:has_anchor  rdfs:comment  "Indicates anchor URI for a potentially dynamic resource instance."@en ;
        rdfs:label    "has anchor" .

prov:Generation  rdfs:comment  "Generation is the completion of production of a new entity by an activity. This entity did not exist before generation and becomes available for usage after this generation."@en , "An instance of prov:Generation provides additional descriptions about the binary prov:wasGeneratedBy relation from a generated prov:Entity to the prov:Activity that generated it. For example, :cake prov:wasGeneratedBy :baking; prov:qualifiedGeneration [ a prov:Generation; prov:activity :baking; :foo :bar ]."@en ;
        rdfs:label    "Generation" .

<http://www.w3.org/ns/prov-dictionary#>
        rdfs:comment  "This document is published by the Provenance Working Group (http://www.w3.org/2011/prov/wiki/Main_Page). \n\nIf you wish to make comments regarding this document, please send them to public-prov-comments@w3.org (subscribe public-prov-comments-request@w3.org, archives http://lists.w3.org/Archives/Public/public-prov-comments/). All feedback is welcome."@en ;
        rdfs:label    "W3C PROVenance Interchange Ontology (PROV-O) Dictionary Extension"@en .

prov:hadUsage  rdfs:comment  "The _optional_ Usage involved in an Entity's Derivation."@en ;
        rdfs:label    "had usage" , "hadUsage" .

prov:asInBundle  rdfs:comment  "prov:asInBundle is used to specify which bundle the general entity of a prov:mentionOf property is described.\n\nWhen :x prov:mentionOf :y and :y is described in Bundle :b, the triple :x prov:asInBundle :b is also asserted to cite the Bundle in which :y was described."@en ;
        rdfs:label    "asInBundle" .

prov:qualifiedInsertion
        rdfs:comment  "The dictionary was derived from the other by insertion. prov:qualifiedInsertion shows details of the insertion, in particular the inserted key-entity pairs." ;
        rdfs:label    "qualifiedInsertion" .

prov:inverse  rdfs:comment  "PROV-O does not define all property inverses. The directionalities defined in PROV-O should be given preference over those not defined. However, if users wish to name the inverse of a PROV-O property, the local name given by prov:inverse should be used."@en .

prov:wasInvalidatedBy
        rdfs:label  "was invalidated by" .

prov:wasInformedBy  rdfs:comment  "An activity a2 is dependent on or informed by another activity a1, by way of some unspecified entity that is generated by a1 and used by a2."@en ;
        rdfs:label    "was informed by" .

prov:wasStartedBy  rdfs:comment  "Start is when an activity is deemed to have started. A start may refer to an entity, known as trigger, that initiated the activity."@en ;
        rdfs:label    "was started by" .

prov:wasDerivedFrom  rdfs:comment  "The more specific subproperties of prov:wasDerivedFrom (i.e., prov:wasQuotedFrom, prov:wasRevisionOf, prov:hadPrimarySource) should be used when applicable."@en , "A derivation is a transformation of an entity into another, an update of an entity resulting in a new one, or the construction of a new entity based on a pre-existing entity."@en ;
        rdfs:label    "was derived from" .

<http://www.w3.org/ns/prov-o#>
        rdfs:comment  "This document is published by the Provenance Working Group (http://www.w3.org/2011/prov/wiki/Main_Page). \n\nIf you wish to make comments regarding this document, please send them to public-prov-comments@w3.org (subscribe public-prov-comments-request@w3.org, archives http://lists.w3.org/Archives/Public/public-prov-comments/). All feedback is welcome."@en ;
        rdfs:label    "W3C PROVenance Interchange Ontology (PROV-O)"@en .

prov:Quotation  rdfs:comment  "A quotation is the repeat of (some or all of) an entity, such as text or image, by someone who may or may not be its original author. Quotation is a particular case of derivation."@en , "An instance of prov:Quotation provides additional descriptions about the binary prov:wasQuotedFrom relation from some taken prov:Entity from an earlier, larger prov:Entity. For example, :here_is_looking_at_you_kid prov:wasQuotedFrom :casablanca_script; prov:qualifiedQuotation [ a prov:Quotation; prov:entity :casablanca_script; :foo :bar ]."@en ;
        rdfs:label    "Quotation" .

prov:qualifiedUsage  rdfs:comment  "If this Activity prov:used Entity :e, then it can qualify how it used it using prov:qualifiedUsage [ a prov:Usage; prov:entity :e; :foo :bar ]."@en ;
        rdfs:label    "qualified usage" .

prov:Organization  rdfs:comment  "An organization is a social or legal institution such as a company, society, etc." ;
        rdfs:label    "Organization" .

<http://www.w3.org/ns/prov-aq#>
        rdfs:comment  "This document is published by the Provenance Working Group (http://www.w3.org/2011/prov/wiki/Main_Page). \n\nIf you wish to make comments regarding this document, please send them to public-prov-comments@w3.org (subscribe public-prov-comments-request@w3.org, archives http://lists.w3.org/Archives/Public/public-prov-comments/). All feedback is welcome."@en , "0.2" ;
        rdfs:label    "PROV Access and Query Ontology"@en .

prov:Replace  rdfs:comment  "Activity that identifies the replacement of a resource."@en ;
        rdfs:label    "Replace"@en .

prov:used  rdfs:comment  "A prov:Entity that was used by this prov:Activity. For example, :baking prov:used :spoon, :egg, :oven ."@en ;
        rdfs:label    "used" .

prov:hadGeneration  rdfs:comment  "The _optional_ Generation involved in an Entity's Derivation."@en ;
        rdfs:label    "had generation" .

prov:invalidatedAtTime
        rdfs:comment  "The time at which an entity was invalidated (i.e., no longer usable)."@en ;
        rdfs:label    "invalidated at time" .

prov:influencer  rdfs:comment  "Subproperties of prov:influencer are used to cite the object of an unqualified PROV-O triple whose predicate is a subproperty of prov:wasInfluencedBy (e.g. prov:used, prov:wasGeneratedBy). prov:influencer is used much like rdf:object is used."@en ;
        rdfs:label    "influencer" .

prov:wasRevisionOf  rdfs:comment  "A revision is a derivation that revises an entity into a revised version."@en ;
        rdfs:label    "was revision of" .

prov:Insertion  rdfs:comment  "Insertion is a derivation that transforms a dictionary into another, by insertion of one or more key-entity pairs." ;
        rdfs:label    "Insertion" .

prov:dictionary  rdfs:comment  "The property used by a prov:Insertion and prov:Removal to cite the prov:Dictionary that was prov:derivedByInsertionFrom or prov:derivedByRemovalFrom another dictionary." ;
        rdfs:label    "dictionary" .

prov:removedKey  rdfs:comment  "The key removed in a Removal." ;
        rdfs:label    "removedKey" .

prov:insertedKeyEntityPair
        rdfs:comment  "An object property to refer to the prov:KeyEntityPair inserted into a prov:Dictionary." ;
        rdfs:label    "insertedKeyEntityPair" .

prov:qualifiedRevision
        rdfs:comment  "If this Entity prov:wasRevisionOf Entity :e, then it can qualify how it was revised using prov:qualifiedRevision [ a prov:Revision;  prov:entity :e; :foo :bar ]."@en ;
        rdfs:label    "qualified revision" .

prov:unqualifiedForm  rdfs:comment  "Classes and properties used to qualify relationships are annotated with prov:unqualifiedForm to indicate the property used to assert an unqualified provenance relation."@en .

prov:qualifiedInfluence
        rdfs:comment  "Because prov:qualifiedInfluence is a broad relation, the more specific relations (qualifiedCommunication, qualifiedDelegation, qualifiedEnd, etc.) should be used when applicable."@en ;
        rdfs:label    "qualified influence" .

prov:Activity  rdfs:comment  "An activity is something that occurs over a period of time and acts upon or with entities; it may include consuming, processing, transforming, modifying, relocating, using, or generating entities." ;
        rdfs:label    "Activity" .

prov:component  rdfs:comment  "Classify prov-o terms into six components according to prov-dm, including 'agents-responsibility', 'alternate', 'annotations', 'collections', 'derivations', and 'entities-activities'. This classification is used so that readers of prov-o specification can find its correspondence with the prov-dm specification."@en .

prov:Copyright  rdfs:comment  "Activity that identifies the Copyrighting activity associated to a resource."@en ;
        rdfs:label    "Copyright"@en .

prov:EmptyCollection  rdfs:comment  "An empty collection is a collection without members."@en ;
        rdfs:label    "Empty Collection"@en .

prov:qualifiedPrimarySource
        rdfs:comment  "If this Entity prov:hadPrimarySource Entity :e, then it can qualify how using prov:qualifiedPrimarySource [ a prov:PrimarySource; prov:entity :e; :foo :bar ]."@en ;
        rdfs:label    "qualified primary source" .

<http://www.w3.org/ns/prov-dc#>
        rdfs:comment  "This document is published by the Provenance Working Group (http://www.w3.org/2011/prov/wiki/Main_Page). \n\nIf you wish to make comments regarding this document, please send them to public-prov-comments@w3.org (subscribe public-prov-comments-request@w3.org, archives http://lists.w3.org/Archives/Public/public-prov-comments/). All feedback is welcome."@en ;
        rdfs:label    "Dublin Core extensions of the W3C PROVenance Interchange Ontology (PROV-O) "@en .

prov:wasAssociatedWith
        rdfs:comment  "An prov:Agent that had some (unspecified) responsibility for the occurrence of this prov:Activity."@en ;
        rdfs:label    "was associated with" .

prov:mentionOf  rdfs:comment  "prov:mentionOf is used to specialize an entity as described in another bundle. It is to be used in conjuction with prov:asInBundle.\n\nprov:asInBundle is used to cite the Bundle in which the generalization was mentioned."@en ;
        rdfs:label    "mentionOf" .

prov:invalidated  rdfs:label  "invalidated" .

prov:Communication  rdfs:comment  "An instance of prov:Communication provides additional descriptions about the binary prov:wasInformedBy relation from an informed prov:Activity to the prov:Activity that informed it. For example, :you_jumping_off_bridge prov:wasInformedBy :everyone_else_jumping_off_bridge; prov:qualifiedCommunication [ a prov:Communication; prov:activity :everyone_else_jumping_off_bridge; :foo :bar ]."@en , "Communication is the exchange of an entity by two activities, one activity using the entity generated by the other." ;
        rdfs:label    "Communication" .

prov:value  rdfs:comment  "Provides a value that is a direct representation of an entity."@en ;
        rdfs:label    "value" .

prov:Invalidation  rdfs:comment  "An instance of prov:Invalidation provides additional descriptions about the binary prov:wasInvalidatedBy relation from an invalidated prov:Entity to the prov:Activity that invalidated it. For example, :uncracked_egg prov:wasInvalidatedBy :baking; prov:qualifiedInvalidation [ a prov:Invalidation; prov:activity :baking; :foo :bar ]."@en , "Invalidation is the start of the destruction, cessation, or expiry of an existing entity by an activity. The entity is no longer available for use (or further invalidation) after invalidation. Any generation or usage of an entity precedes its invalidation." ;
        rdfs:label    "Invalidation" .

prov:definition  rdfs:comment  "A definition quoted from PROV-DM or PROV-CONSTRAINTS that describes the concept expressed with this OWL term."@en .

prov:Delegation  rdfs:comment  "An instance of prov:Delegation provides additional descriptions about the binary prov:actedOnBehalfOf relation from a performing prov:Agent to some prov:Agent for whom it was performed. For example, :mixing prov:wasAssociatedWith :toddler . :toddler prov:actedOnBehalfOf :mother; prov:qualifiedDelegation [ a prov:Delegation; prov:entity :mother; :foo :bar ]."@en , "Delegation is the assignment of authority and responsibility to an agent (by itself or by another agent) to carry out a specific activity as a delegate or representative, while the agent it acts on behalf of retains some responsibility for the outcome of the delegated work.\n\nFor example, a student acted on behalf of his supervisor, who acted on behalf of the department chair, who acted on behalf of the university; all those agents are responsible in some way for the activity that took place but we do not say explicitly who bears responsibility and to what degree."@en ;
        rdfs:label    "Delegation" .

prov:hadMember  rdfs:label  "had member" .

prov:pairKey  rdfs:comment  "The key of a KeyEntityPair, which is an element of a prov:Dictionary." ;
        rdfs:label    "pairKey" .

prov:has_provenance  rdfs:comment  "Indicates a provenance-URI for a resource; the resource identified by this property presents a provenance record about its subject or anchor resource."@en ;
        rdfs:label    "has provenance" .

prov:Revision  rdfs:comment  "A revision is a derivation for which the resulting entity is a revised version of some original. The implication here is that the resulting entity contains substantial content from the original. Revision is a particular case of derivation."@en , "An instance of prov:Revision provides additional descriptions about the binary prov:wasRevisionOf relation from some newer prov:Entity to an earlier prov:Entity. For example, :draft_2 prov:wasRevisionOf :draft_1; prov:qualifiedRevision [ a prov:Revision; prov:entity :draft_1; :foo :bar ]."@en ;
        rdfs:label    "Revision" .

prov:Person  rdfs:comment  "Person agents are people."@en ;
        rdfs:label    "Person" .

prov:generated  rdfs:label  "generated" .

prov:hadDictionaryMember
        rdfs:comment  "Describes the key-entity pair that was member of a prov:Dictionary. A dictionary can have multiple members." ;
        rdfs:label    "hadDictionaryMember" .

prov:Usage  rdfs:comment  "An instance of prov:Usage provides additional descriptions about the binary prov:used relation from some prov:Activity to an prov:Entity that it used. For example, :keynote prov:used :podium; prov:qualifiedUsage [ a prov:Usage; prov:entity :podium; :foo :bar ]."@en , "Usage is the beginning of utilizing an entity by an activity. Before usage, the activity had not begun to utilize this entity and could not have been affected by the entity."@en ;
        rdfs:label    "Usage" .

prov:qualifiedAttribution
        rdfs:comment  "If this Entity prov:wasAttributedTo Agent :ag, then it can qualify how it was influenced using prov:qualifiedAttribution [ a prov:Attribution;  prov:agent :ag; :foo :bar ]."@en ;
        rdfs:label    "qualified attribution" .

prov:Modify  rdfs:comment  "Activity that identifies the modification of a resource. "@en ;
        rdfs:label    "Modify"@en .

prov:RightsAssignment
        rdfs:comment  "Activity that identifies the rights assignment of a resource."@en ;
        rdfs:label    "RightsAssignment"@en .

prov:editorialNote  rdfs:comment  "A note by the OWL development team about how this term expresses the PROV-DM concept, or how it should be used in context of semantic web or linked data."@en .

prov:qualifiedInvalidation
        rdfs:comment  "If this Entity prov:wasInvalidatedBy Activity :a, then it can qualify how it was invalidated using prov:qualifiedInvalidation [ a prov:Invalidation;  prov:activity :a; :foo :bar ]."@en ;
        rdfs:label    "qualified invalidation" .

prov:has_query_service
        rdfs:comment  "Indicates a provenance query service that can access provenance related to its subject or anchor resource."@en ;
        rdfs:label    "has provenance service" .

prov:wasInfluencedBy  rdfs:comment  "This property has multiple RDFS domains to suit multiple OWL Profiles. See <a href=\"#owl-profile\">PROV-O OWL Profile</a>." , "Because prov:wasInfluencedBy is a broad relation, its more specific subproperties (e.g. prov:wasInformedBy, prov:actedOnBehalfOf, prov:wasEndedBy, etc.) should be used when applicable."@en ;
        rdfs:label    "was influenced by" .

prov:startedAtTime  rdfs:comment  "The time at which an activity started. See also prov:endedAtTime."@en ;
        rdfs:label    "started at time" .

prov:KeyEntityPair  rdfs:comment  "A key-entity pair. Part of a prov:Dictionary through prov:hadDictionaryMember. The key is any RDF Literal, the value is a prov:Entity." ;
        rdfs:label    "Key-Entity Pair" .

prov:qualifiedStart  rdfs:comment  "If this Activity prov:wasStartedBy Entity :e1, then it can qualify how it was started using prov:qualifiedStart [ a prov:Start;  prov:entity :e1; :foo :bar ]."@en ;
        rdfs:label    "qualified start" .

prov:provenanceUriTemplate
        rdfs:comment  "Relates a provenance service to a URI template string for constructing provenance-URIs."@en ;
        rdfs:label    "provenanceUriTemplate" .

prov:Agent  rdfs:comment  "An agent is something that bears some form of responsibility for an activity taking place, for the existence of an entity, or for another agent's activity. "@en ;
        rdfs:label    "Agent" .

prov:pairEntity  rdfs:comment  "The value of a KeyEntityPair." ;
        rdfs:label    "pairKey" .

prov:atTime  rdfs:comment  "The time at which an InstantaneousEvent occurred, in the form of xsd:dateTime."@en ;
        rdfs:label    "at time" .

prov:wasEndedBy  rdfs:comment  "End is when an activity is deemed to have ended. An end may refer to an entity, known as trigger, that terminated the activity."@en ;
        rdfs:label    "was ended by" .

prov:Contribute  rdfs:comment  "Activity that identifies any contribution of an agent to a resource. "@en ;
        rdfs:label    "Contribute\n"@en .

prov:qualifiedRemoval
        rdfs:comment  "The dictionary was derived from the other by removal. prov:qualifiedRemoval shows details of the removal, in particular the removed keys." ;
        rdfs:label    "qualifiedRemoval" .

prov:activity  rdfs:label  "activity" .

prov:order  rdfs:comment  "The position that this OWL term should be listed within documentation. The scope of the documentation (e.g., among all terms, among terms within a prov:category, among properties applying to a particular class, etc.) is unspecified."@en .

<http://www.w3.org/ns/prov-links#>
        rdfs:comment  "This document is published by the Provenance Working Group (http://www.w3.org/2011/prov/wiki/Main_Page). If you wish to make comments regarding this document, please send them to public-prov-comments@w3.org (subscribe public-prov-comments-request@w3.org, archives http://lists.w3.org/Archives/Public/public-prov-comments/\n). All feedback is welcome."@en ;
        rdfs:label    "W3C PROV Linking Across Provenance Bundles Ontology (PROV-LINKS)"@en .

prov:constraints  rdfs:comment  "A reference to the principal section of the PROV-CONSTRAINTS document that describes this concept."@en .

prov:qualifiedDelegation
        rdfs:comment  "If this Agent prov:actedOnBehalfOf Agent :ag, then it can qualify how with prov:qualifiedResponsibility [ a prov:Responsibility;  prov:agent :ag; :foo :bar ]."@en ;
        rdfs:label    "qualified delegation" .

prov:agent  rdfs:label  "agent" .

prov:influenced  rdfs:label  "influenced" .

prov:qualifiedQuotation
        rdfs:comment  "If this Entity prov:wasQuotedFrom Entity :e, then it can qualify how using prov:qualifiedQuotation [ a prov:Quotation;  prov:entity :e; :foo :bar ]."@en ;
        rdfs:label    "qualified quotation" .

prov:Collection  rdfs:comment  "A collection is an entity that provides a structure to some constituents, which are themselves entities. These constituents are said to be member of the collections."@en ;
        rdfs:label    "Collection" .

prov:category  rdfs:comment  "Classify prov-o terms into three categories, including 'starting-point', 'qualifed', and 'extended'. This classification is used by the prov-o html document to gently introduce prov-o terms to its users. "@en .

prov:alternateOf  rdfs:comment  "Two alternate entities present aspects of the same thing. These aspects may be the same or different, and the alternate entities may or may not overlap in time."@en ;
        rdfs:label    "alternate of" .

<https://linked.data.gov.au/def/vocab-derivation-modes/extension>
        rdfs:label  "Extension" .

<https://linked.data.gov.au/def/vocab-derivation-modes/relabelling>
        rdfs:label  "Relabelling" .

<https://linked.data.gov.au/def/vocab-derivation-modes/none>
        rdfs:label  "None" .

<https://linked.data.gov.au/def/vocab-derivation-modes/subsetting>
        rdfs:label  "Subsetting" .

<https://linked.data.gov.au/def/vocab-derivation-modes/subsetting-and-extension>
        rdfs:label  "Subset & Extension" .

<https://linked.data.gov.au/def/vocab-derivation-modes/direct>
        rdfs:label  "Direct" .

<https://linked.data.gov.au/def/vocab-derivation-modes/not-applicable>
        rdfs:label  "Not Applicable" .

owl:equivalentProperty
        a             <http://www.w3.org/1999/02/22-rdf-syntax-ns#Property> ;
        rdfs:comment  "The property that determines that two given properties are equivalent" ;
        rdfs:label    "equivalent property" .

owl:AsymmetricProperty
        a             rdfs:Class ;
        rdfs:comment  "The class of asymmetric properties" ;
        rdfs:label    "Asymmetric Property" .

rdfs:Class  rdfs:label  "Class" .

owl:imports  a        owl:OntologyProperty ;
        rdfs:comment  "The property that is used for importing other ontologies into a given ontology" ;
        rdfs:label    "imports" .

rdfs:domain  rdfs:label  "domain" .

owl:sameAs  a         <http://www.w3.org/1999/02/22-rdf-syntax-ns#Property> ;
        rdfs:comment  "The property that determines that two given individuals are equal" ;
        rdfs:label    "same as" .

rdfs:range  rdfs:label  "range" .

owl:Thing  a          owl:Class ;
        rdfs:comment  "The class of OWL individuals" ;
        rdfs:label    "Thing" .

owl:priorVersion  a   owl:OntologyProperty , owl:AnnotationProperty ;
        rdfs:comment  "The annotation property that indicates the predecessor ontology of a given ontology" ;
        rdfs:label    "prior version" .

owl:targetIndividual  a  <http://www.w3.org/1999/02/22-rdf-syntax-ns#Property> ;
        rdfs:comment  "The property that determines the object of a negative object property assertion" ;
        rdfs:label    "target individual" .

owl:NegativePropertyAssertion
        a             rdfs:Class ;
        rdfs:comment  "The class of negative property assertions" ;
        rdfs:label    "Negative Property Assertion" .

owl:hasSelf  a        <http://www.w3.org/1999/02/22-rdf-syntax-ns#Property> ;
        rdfs:comment  "The property that determines the property that a self restriction refers to" ;
        rdfs:label    "has self" ;
        rdfs:range    rdfs:Resource .

owl:backwardCompatibleWith
        a             owl:OntologyProperty , owl:AnnotationProperty ;
        rdfs:comment  "The annotation property that indicates that a given ontology is backward compatible with another ontology" ;
        rdfs:label    "backward compatible with" .

owl:OntologyProperty  a  rdfs:Class ;
        rdfs:comment  "The class of ontology properties" ;
        rdfs:label    "Ontology Property" .

owl:cardinality  a    <http://www.w3.org/1999/02/22-rdf-syntax-ns#Property> ;
        rdfs:comment  "The property that determines the cardinality of an exact cardinality restriction" ;
        rdfs:label    "cardinality" .

owl:Axiom  a          rdfs:Class ;
        rdfs:comment  "The class of annotated axioms for which the RDF serialization consists of an annotated subject, predicate and object" ;
        rdfs:label    "Axiom" .

owl:onClass  a        <http://www.w3.org/1999/02/22-rdf-syntax-ns#Property> ;
        rdfs:comment  "The property that determines the class that a qualified object cardinality restriction refers to" ;
        rdfs:label    "on class" .

owl:bottomDataProperty
        a             owl:DatatypeProperty ;
        rdfs:comment  "The data property that does not relate any individual to any data value" ;
        rdfs:label    "bottom data property" .

owl:DatatypeProperty  a  rdfs:Class ;
        rdfs:comment  "The class of data properties" ;
        rdfs:label    "Datatype Property" .

owl:Restriction  a    rdfs:Class ;
        rdfs:comment  "The class of property restrictions" ;
        rdfs:label    "Restriction" .

owl:distinctMembers  a  <http://www.w3.org/1999/02/22-rdf-syntax-ns#Property> ;
        rdfs:comment  "The property that determines the collection of pairwise different individuals in a owl:AllDifferent axiom" ;
        rdfs:label    "distinct members" .

owl:maxQualifiedCardinality
        a             <http://www.w3.org/1999/02/22-rdf-syntax-ns#Property> ;
        rdfs:comment  "The property that determines the cardinality of a maximum qualified cardinality restriction" ;
        rdfs:label    "max qualified cardinality" .

owl:propertyDisjointWith
        a             <http://www.w3.org/1999/02/22-rdf-syntax-ns#Property> ;
        rdfs:comment  "The property that determines that two given properties are disjoint" ;
        rdfs:label    "property disjoint with" .

owl:bottomObjectProperty
        a             owl:ObjectProperty ;
        rdfs:comment  "The object property that does not relate any two individuals" ;
        rdfs:label    "bottom object property" .

owl:onDataRange  a    <http://www.w3.org/1999/02/22-rdf-syntax-ns#Property> ;
        rdfs:comment  "The property that determines the data range that a qualified data cardinality restriction refers to" ;
        rdfs:label    "on data range" .

owl:hasKey  a         <http://www.w3.org/1999/02/22-rdf-syntax-ns#Property> ;
        rdfs:comment  "The property that determines the collection of properties that jointly build a key" ;
        rdfs:label    "has key" .

<http://www.w3.org/1999/02/22-rdf-syntax-ns#List>
        rdfs:label  "List" .

owl:onProperty  a     <http://www.w3.org/1999/02/22-rdf-syntax-ns#Property> ;
        rdfs:comment  "The property that determines the property that a property restriction refers to" ;
        rdfs:label    "on property" .

owl:minQualifiedCardinality
        a             <http://www.w3.org/1999/02/22-rdf-syntax-ns#Property> ;
        rdfs:comment  "The property that determines the cardinality of a minimum qualified cardinality restriction" ;
        rdfs:label    "min qualified cardinality" .

owl:incompatibleWith  a  owl:OntologyProperty , owl:AnnotationProperty ;
        rdfs:comment  "The annotation property that indicates that a given ontology is incompatible with another ontology" ;
        rdfs:label    "incompatible with" .

owl:Annotation  a     rdfs:Class ;
        rdfs:comment  "The class of annotated annotations for which the RDF serialization consists of an annotated subject, predicate and object" ;
        rdfs:label    "Annotation" .

owl:datatypeComplementOf
        a             <http://www.w3.org/1999/02/22-rdf-syntax-ns#Property> ;
        rdfs:comment  "The property that determines that a given data range is the complement of another data range with respect to the data domain" ;
        rdfs:label    "datatype complement of" .

owl:minCardinality  a  <http://www.w3.org/1999/02/22-rdf-syntax-ns#Property> ;
        rdfs:comment  "The property that determines the cardinality of a minimum cardinality restriction" ;
        rdfs:label    "min cardinality" .

owl:targetValue  a    <http://www.w3.org/1999/02/22-rdf-syntax-ns#Property> ;
        rdfs:comment  "The property that determines the value of a negative data property assertion" ;
        rdfs:label    "target value" .

owl:inverseOf  a      <http://www.w3.org/1999/02/22-rdf-syntax-ns#Property> ;
        rdfs:comment  "The property that determines that two given properties are inverse" ;
        rdfs:label    "inverse of" .

owl:ObjectProperty  a  rdfs:Class ;
        rdfs:comment  "The class of object properties" ;
        rdfs:label    "Object Property" .

owl:Nothing  a        owl:Class ;
        rdfs:comment  "This is the empty class" ;
        rdfs:label    "Nothing" .

owl:AllDifferent  a   rdfs:Class ;
        rdfs:comment  "The class of collections of pairwise different individuals" ;
        rdfs:label    "All Different" .

owl:equivalentClass  a  <http://www.w3.org/1999/02/22-rdf-syntax-ns#Property> ;
        rdfs:comment  "The property that determines that two given classes are equivalent, and that is used to specify datatype definitions" ;
        rdfs:label    "equivalent class" .

owl:maxCardinality  a  <http://www.w3.org/1999/02/22-rdf-syntax-ns#Property> ;
        rdfs:comment  "The property that determines the cardinality of a maximum cardinality restriction" ;
        rdfs:label    "max cardinality" .

owl:topObjectProperty
        a             owl:ObjectProperty ;
        rdfs:comment  "The object property that relates every two individuals" ;
        rdfs:label    "top object property" .

owl:annotatedTarget  a  <http://www.w3.org/1999/02/22-rdf-syntax-ns#Property> ;
        rdfs:comment  "The property that determines the object of an annotated axiom or annotated annotation" ;
        rdfs:label    "annotated target" .

owl:withRestrictions  a  <http://www.w3.org/1999/02/22-rdf-syntax-ns#Property> ;
        rdfs:comment  "The property that determines the collection of facet-value pairs that define a datatype restriction" ;
        rdfs:label    "with restrictions" .

rdfs:Datatype  rdfs:label  "Datatype" .

owl:members  a        <http://www.w3.org/1999/02/22-rdf-syntax-ns#Property> ;
        rdfs:comment  "The property that determines the collection of members in either a owl:AllDifferent, owl:AllDisjointClasses or owl:AllDisjointProperties axiom" ;
        rdfs:label    "members" .

owl:onProperties  a   <http://www.w3.org/1999/02/22-rdf-syntax-ns#Property> ;
        rdfs:comment  "The property that determines the n-tuple of properties that a property restriction on an n-ary data range refers to" ;
        rdfs:label    "on properties" .

owl:assertionProperty
        a             <http://www.w3.org/1999/02/22-rdf-syntax-ns#Property> ;
        rdfs:comment  "The property that determines the predicate of a negative property assertion" ;
        rdfs:label    "assertion property" .

<http://www.w3.org/1999/02/22-rdf-syntax-ns#Property>
        rdfs:label  "Property" .

owl:AllDisjointClasses
        a             rdfs:Class ;
        rdfs:comment  "The class of collections of pairwise disjoint classes" ;
        rdfs:label    "All Disjoint Classes" .

owl:qualifiedCardinality
        a             <http://www.w3.org/1999/02/22-rdf-syntax-ns#Property> ;
        rdfs:comment  "The property that determines the cardinality of an exact qualified cardinality restriction" ;
        rdfs:label    "qualified cardinality" .

owl:sourceIndividual  a  <http://www.w3.org/1999/02/22-rdf-syntax-ns#Property> ;
        rdfs:comment  "The property that determines the subject of a negative property assertion" ;
        rdfs:label    "source individual" .

owl:propertyChainAxiom
        a             <http://www.w3.org/1999/02/22-rdf-syntax-ns#Property> ;
        rdfs:comment  "The property that determines the n-tuple of properties that build a sub property chain of a given property" ;
        rdfs:label    "property chain axiom" .

owl:disjointUnionOf  a  <http://www.w3.org/1999/02/22-rdf-syntax-ns#Property> ;
        rdfs:comment  "The property that determines that a given class is equivalent to the disjoint union of a collection of other classes" ;
        rdfs:label    "disjoint union of" .

owl:topDataProperty  a  owl:DatatypeProperty ;
        rdfs:comment  "The data property that relates every individual to every data value" ;
        rdfs:label    "top data property" .

owl:differentFrom  a  <http://www.w3.org/1999/02/22-rdf-syntax-ns#Property> ;
        rdfs:comment  "The property that determines that two given individuals are different" ;
        rdfs:label    "different from" .

owl:versionInfo  a    owl:AnnotationProperty ;
        rdfs:comment  "The annotation property that provides version information for an ontology or another OWL construct" ;
        rdfs:label    "version info" .

rdfs:Resource  rdfs:label  "Resource" .

owl:AnnotationProperty
        a             rdfs:Class ;
        rdfs:comment  "The class of annotation properties" ;
        rdfs:label    "Annotation Property" .

owl:Class  a          rdfs:Class ;
        rdfs:comment  "The class of OWL classes" ;
        rdfs:label    "Class" .

rdfs:subClassOf  rdfs:label  "subClassOf" .

rdfs:seeAlso  rdfs:label  "seeAlso" .

owl:FunctionalProperty
        a             rdfs:Class ;
        rdfs:comment  "The class of functional properties" ;
        rdfs:label    "Functional Property" .

owl:annotatedProperty
        a             <http://www.w3.org/1999/02/22-rdf-syntax-ns#Property> ;
        rdfs:comment  "The property that determines the predicate of an annotated axiom or annotated annotation" ;
        rdfs:label    "annotated property" .

owl:DataRange  a      rdfs:Class ;
        rdfs:comment  "The class of OWL data ranges, which are special kinds of datatypes. Note: The use of the IRI owl:DataRange has been deprecated as of OWL 2. The IRI rdfs:Datatype SHOULD be used instead" ;
        rdfs:label    "Data Range" .

owl:oneOf  a          <http://www.w3.org/1999/02/22-rdf-syntax-ns#Property> ;
        rdfs:comment  "The property that determines the collection of individuals or data values that build an enumeration" ;
        rdfs:label    "one of" .

owl:DeprecatedProperty
        a             rdfs:Class ;
        rdfs:comment  "The class of deprecated properties" ;
        rdfs:label    "Deprecated Property" .

owl:AllDisjointProperties
        a             rdfs:Class ;
        rdfs:comment  "The class of collections of pairwise disjoint properties" ;
        rdfs:label    "All Disjoint Properties" .

owl:unionOf  a        <http://www.w3.org/1999/02/22-rdf-syntax-ns#Property> ;
        rdfs:comment  "The property that determines the collection of classes or data ranges that build a union" ;
        rdfs:label    "union of" .

owl:disjointWith  a   <http://www.w3.org/1999/02/22-rdf-syntax-ns#Property> ;
        rdfs:comment  "The property that determines that two given classes are disjoint" ;
        rdfs:label    "disjoint with" .

owl:InverseFunctionalProperty
        a             rdfs:Class ;
        rdfs:comment  "The class of inverse-functional properties" ;
        rdfs:label    "Inverse Functional Property" .

owl:complementOf  a   <http://www.w3.org/1999/02/22-rdf-syntax-ns#Property> ;
        rdfs:comment  "The property that determines that a given class is the complement of another class" ;
        rdfs:label    "complement of" .

owl:TransitiveProperty
        a             rdfs:Class ;
        rdfs:comment  "The class of transitive properties" ;
        rdfs:label    "Transitive Property" .

owl:deprecated  a     owl:AnnotationProperty ;
        rdfs:comment  "The annotation property that indicates that a given entity has been deprecated" ;
        rdfs:label    "deprecated" .

owl:hasValue  a       <http://www.w3.org/1999/02/22-rdf-syntax-ns#Property> ;
        rdfs:comment  "The property that determines the individual that a has-value restriction refers to" ;
        rdfs:label    "has value" .

owl:onDatatype  a     <http://www.w3.org/1999/02/22-rdf-syntax-ns#Property> ;
        rdfs:comment  "The property that determines the datatype that a datatype restriction refers to" ;
        rdfs:label    "on datatype" .

owl:versionIRI  a     owl:OntologyProperty ;
        rdfs:comment  "The property that identifies the version IRI of an ontology" ;
        rdfs:label    "version IRI" .

owl:intersectionOf  a  <http://www.w3.org/1999/02/22-rdf-syntax-ns#Property> ;
        rdfs:comment  "The property that determines the collection of classes or data ranges that build an intersection" ;
        rdfs:label    "intersection of" .

owl:IrreflexiveProperty
        a             rdfs:Class ;
        rdfs:comment  "The class of irreflexive properties" ;
        rdfs:label    "Irreflexive Property" .

owl:NamedIndividual  a  rdfs:Class ;
        rdfs:comment  "The class of named individuals" ;
        rdfs:label    "Named Individual" .

owl:SymmetricProperty
        a             rdfs:Class ;
        rdfs:comment  "The class of symmetric properties" ;
        rdfs:label    "Symmetric Property" .

owl:someValuesFrom  a  <http://www.w3.org/1999/02/22-rdf-syntax-ns#Property> ;
        rdfs:comment  "The property that determines the class that an existential property restriction refers to" ;
        rdfs:label    "some values from" .

rdfs:Literal  rdfs:label  "Literal" .

owl:annotatedSource  a  <http://www.w3.org/1999/02/22-rdf-syntax-ns#Property> ;
        rdfs:comment  "The property that determines the subject of an annotated axiom or annotated annotation" ;
        rdfs:label    "annotated source" .

owl:allValuesFrom  a  <http://www.w3.org/1999/02/22-rdf-syntax-ns#Property> ;
        rdfs:comment  "The property that determines the class that a universal property restriction refers to" ;
        rdfs:label    "all values from" .

owl:ReflexiveProperty
        a             rdfs:Class ;
        rdfs:comment  "The class of reflexive properties" ;
        rdfs:label    "Reflexive Property" .

owl:DeprecatedClass  a  rdfs:Class ;
        rdfs:comment  "The class of deprecated classes" ;
        rdfs:label    "Deprecated Class" .

dcterms:Frequency  rdfs:label  "Frequency"@en .

dcterms:  rdfs:label  "DCMI Metadata Terms - other"@en .

dcterms:Standard  rdfs:label  "Standard"@en .

dcterms:LocationPeriodOrJurisdiction
        rdfs:label  "Location, Period, or Jurisdiction"@en .

dcterms:Period  rdfs:label  "DCMI Period"@en .

dcterms:extent  rdfs:label  "Extent"@en .

dcterms:W3CDTF  rdfs:label  "W3C-DTF"@en .

dcterms:IMT  rdfs:label  "IMT"@en .

dcterms:AgentClass  rdfs:label  "Agent Class"@en .

dcterms:conformsTo  rdfs:label  "Conforms To"@en .

dcterms:type  rdfs:label  "Type"@en .

dcterms:description  rdfs:label  "Description"@en .

dcterms:accrualPolicy
        rdfs:label  "Accrual Policy"@en .

dcterms:issued  rdfs:label  "Date Issued"@en .

dcterms:abstract  rdfs:label  "Abstract"@en .

dcterms:NLM  rdfs:label  "NLM"@en .

dcterms:bibliographicCitation
        rdfs:label  "Bibliographic Citation"@en .

dcterms:alternative  rdfs:label  "Alternative Title"@en .

dcterms:contributor  rdfs:label  "Contributor"@en .

dcterms:dateCopyrighted
        rdfs:label  "Date Copyrighted"@en .

dcterms:language  rdfs:label  "Language"@en .

dcterms:LinguisticSystem
        rdfs:label  "Linguistic System"@en .

dcterms:title  rdfs:label  "Title"@en .

dcterms:rightsHolder  rdfs:label  "Rights Holder"@en .

dcterms:license  rdfs:label  "License"@en .

dcterms:isRequiredBy  rdfs:label  "Is Required By"@en .

rdfs:subPropertyOf  rdfs:label  "subPropertyOf" .

dcterms:relation  rdfs:label  "Relation"@en .

dcterms:RFC3066  rdfs:label  "RFC 3066"@en .

dcterms:rights  rdfs:label  "Rights"@en .

dcterms:TGN  rdfs:label  "TGN"@en .

dcterms:URI  rdfs:label  "URI"@en .

dcterms:replaces  rdfs:label  "Replaces"@en .

dcterms:audience  rdfs:label  "Audience"@en .

dcterms:Location  rdfs:label  "Location"@en .

dcterms:PeriodOfTime  rdfs:label  "Period of Time"@en .

dcterms:LicenseDocument
        rdfs:label  "License Document"@en .

dcterms:hasFormat  rdfs:label  "Has Format"@en .

dcterms:hasVersion  rdfs:label  "Has Version"@en .

dcterms:Agent  rdfs:label  "Agent"@en .

dcterms:MediaTypeOrExtent
        rdfs:label  "Media Type or Extent"@en .

dcterms:accessRights  rdfs:label  "Access Rights"@en .

dcterms:medium  rdfs:label  "Medium"@en .

dcterms:format  rdfs:label  "Format"@en .

dcterms:MethodOfAccrual
        rdfs:label  "Method of Accrual"@en .

dcterms:PhysicalResource
        rdfs:label  "Physical Resource"@en .

dcterms:DDC  rdfs:label  "DDC"@en .

dcterms:FileFormat  rdfs:label  "File Format"@en .

dcterms:MediaType  rdfs:label  "Media Type"@en .

dcterms:LCC  rdfs:label  "LCC"@en .

dcterms:available  rdfs:label  "Date Available"@en .

dcterms:date  rdfs:label  "Date"@en .

dcterms:MethodOfInstruction
        rdfs:label  "Method of Instruction"@en .

dcterms:references  rdfs:label  "References"@en .

dcterms:hasPart  rdfs:label  "Has Part"@en .

dcterms:RFC5646  rdfs:label  "RFC 5646"@en .

dcterms:dateSubmitted
        rdfs:label  "Date Submitted"@en .

dcterms:SizeOrDuration
        rdfs:label  "Size or Duration"@en .

dcterms:coverage  rdfs:label  "Coverage"@en .

dcterms:LCSH  rdfs:label  "LCSH"@en .

dcterms:BibliographicResource
        rdfs:label  "Bibliographic Resource"@en .

dcterms:UDC  rdfs:label  "UDC"@en .

dcterms:spatial  rdfs:label  "Spatial Coverage"@en .

dcterms:MESH  rdfs:label  "MeSH"@en .

dcterms:instructionalMethod
        rdfs:label  "Instructional Method"@en .

dcterms:Policy  rdfs:label  "Policy"@en .

dcterms:ProvenanceStatement
        rdfs:label  "Provenance Statement"@en .

dcterms:valid  rdfs:label  "Date Valid"@en .

dcterms:ISO3166  rdfs:label  "ISO 3166"@en .

dcterms:accrualPeriodicity
        rdfs:label  "Accrual Periodicity"@en .

dcterms:tableOfContents
        rdfs:label  "Table Of Contents"@en .

dcterms:RFC1766  rdfs:label  "RFC 1766"@en .

dcterms:isReferencedBy
        rdfs:label  "Is Referenced By"@en .

dcterms:isReplacedBy  rdfs:label  "Is Replaced By"@en .

dcterms:subject  rdfs:label  "Subject"@en .

dcterms:Box  rdfs:label  "DCMI Box"@en .

dcterms:ISO639-3  rdfs:label  "ISO 639-3"@en .

dcterms:RFC4646  rdfs:label  "RFC 4646"@en .

dcterms:isPartOf  rdfs:label  "Is Part Of"@en .

dcterms:educationLevel
        rdfs:label  "Audience Education Level"@en .

dcterms:RightsStatement
        rdfs:label  "Rights Statement"@en .

dcterms:PhysicalMedium
        rdfs:label  "Physical Medium"@en .

dcterms:ISO639-2  rdfs:label  "ISO 639-2"@en .

dcterms:temporal  rdfs:label  "Temporal Coverage"@en .

dcterms:mediator  rdfs:label  "Mediator"@en .

dcterms:requires  rdfs:label  "Requires"@en .

dcterms:accrualMethod
        rdfs:label  "Accrual Method"@en .

dcterms:Point  rdfs:label  "DCMI Point"@en .

dcterms:dateAccepted  rdfs:label  "Date Accepted"@en .

dcterms:DCMIType  rdfs:label  "DCMI Type Vocabulary"@en .

dcterms:Jurisdiction  rdfs:label  "Jurisdiction"@en .

dcterms:isVersionOf  rdfs:label  "Is Version Of"@en .

dcterms:isFormatOf  rdfs:label  "Is Format Of"@en .

skos:scopeNote  rdfs:label  "scope note"@en .

skos:note  rdfs:label  "note"@en .

<http://www.w3.org/2004/02/skos/core>
        rdfs:label  "SKOS Vocabulary"@en .

skos:mappingRelation  rdfs:label  "is in mapping relation with"@en .

<http://www.w3.org/1999/02/22-rdf-syntax-ns#first>
        rdfs:label  "first" .

skos:example  rdfs:label  "example"@en .

skos:semanticRelation
        rdfs:label  "is in semantic relation with"@en .

skos:memberList  rdfs:label  "has member list"@en .

skos:OrderedCollection
        rdfs:label  "Ordered Collection"@en .

skos:relatedMatch  rdfs:label  "has related match"@en .

skos:related  rdfs:label  "has related"@en .

skos:hiddenLabel  rdfs:label  "hidden label"@en .

skos:broaderTransitive
        rdfs:label  "has broader transitive"@en .

skos:closeMatch  rdfs:label  "has close match"@en .

skos:broadMatch  rdfs:label  "has broader match"@en .

skos:narrowMatch  rdfs:label  "has narrower match"@en .

skos:narrowerTransitive
        rdfs:label  "has narrower transitive"@en .

skos:historyNote  rdfs:label  "history note"@en .

<http://www.w3.org/1999/02/22-rdf-syntax-ns#rest>
        rdfs:label  "rest" .

<http://www.w3.org/1999/02/22-rdf-syntax-ns#nil>
        rdfs:label  "nil" .

<http://www.w3.org/1999/02/22-rdf-syntax-ns#PlainLiteral>
        rdfs:label  "PlainLiteral" .

<http://www.w3.org/1999/02/22-rdf-syntax-ns#langString>
        rdfs:label  "langString" .

<http://www.w3.org/1999/02/22-rdf-syntax-ns#subject>
        rdfs:label  "subject" .

<http://www.w3.org/1999/02/22-rdf-syntax-ns#predicate>
        rdfs:label  "predicate" .

<http://www.w3.org/1999/02/22-rdf-syntax-ns#object>
        rdfs:label  "object" .

<http://www.w3.org/1999/02/22-rdf-syntax-ns#XMLLiteral>
        rdfs:label  "XMLLiteral" .

<http://www.w3.org/1999/02/22-rdf-syntax-ns#Bag>
        rdfs:label  "Bag" .

<http://www.w3.org/1999/02/22-rdf-syntax-ns#Alt>
        rdfs:label  "Alt" .

<http://www.w3.org/1999/02/22-rdf-syntax-ns#HTML>
        rdfs:label  "HTML" .

<http://www.w3.org/1999/02/22-rdf-syntax-ns#value>
        rdfs:label  "value" .

<http://www.w3.org/1999/02/22-rdf-syntax-ns#Statement>
        rdfs:label  "Statement" .

<http://www.w3.org/1999/02/22-rdf-syntax-ns#language>
        rdfs:label  "language" .

<http://www.w3.org/1999/02/22-rdf-syntax-ns#JSON>
        rdfs:label  "JSON" .

rdfs:Container  rdfs:label  "Container" .

<http://www.w3.org/1999/02/22-rdf-syntax-ns#direction>
        rdfs:label  "direction" .

<http://www.w3.org/1999/02/22-rdf-syntax-ns#Seq>
        rdfs:label  "Seq" .

<http://www.w3.org/1999/02/22-rdf-syntax-ns#CompoundLiteral>
        rdfs:label  "CompoundLiteral" .

<http://def.isotc211.org/iso19135/-1/2015/CoreModel/code/RE_ItemStatus/addition>
        rdfs:label  "addition" .

<http://def.isotc211.org/iso19135/-1/2015/CoreModel/code/RE_ItemStatus/invalid>
        rdfs:label  "invalid" .

<http://def.isotc211.org/iso19135/-1/2015/CoreModel/code/RE_ItemStatus/original>
        rdfs:label  "original" .

<http://def.isotc211.org/iso19135/-1/2015/CoreModel/code/RE_ItemStatus/stable>
        rdfs:label  "stable" .

<http://def.isotc211.org/iso19135/-1/2015/CoreModel/code/RE_ItemStatus/retired>
        rdfs:label  "retired" .

<http://def.isotc211.org/iso19135/-1/2015/CoreModel/code/RE_ItemStatus/superseded>
        rdfs:label  "superseded" .

<http://def.isotc211.org/iso19135/-1/2015/CoreModel/code/RE_ItemStatus/valid>
        rdfs:label  "valid" .

<http://def.isotc211.org/iso19135/-1/2015/CoreModel/code/RE_ItemStatus/experimental>
        rdfs:label  "experimental" .

reg:definition  rdfs:label  "definition"@en .

reg:RegisterItem  rdfs:label  "RegisterItem"@en .

<http://dbpedia.org/ontology/Language>
        rdfs:label  "Language" .

reg:statusReserved  rdfs:label  "reserved"@en .

reg:Status  rdfs:label  "Status"@en .

reg:SPARQLConstructQuery
        rdfs:label  "SPARQL CONSTRUCT query"@en .

reg:SPARQLQuery  rdfs:label  "SPARQL query"@en .

reg:itemClass  rdfs:label  "item class"@en .

reg:MonitorSpec  rdfs:label  "Monitor Spec"@en .

reg:owner  rdfs:label  "owner"@en .

reg:statusRetired  rdfs:label  "retired"@en .

reg:statusDeprecated  rdfs:label  "deprecated"@en .

<http://dbpedia.org/ontology/languageCode>
        rdfs:label  "Language code" .

reg:Delegated  rdfs:label  "Delegated"@en .

reg:validationQuery  rdfs:label  "validation query"@en .

reg:query  rdfs:label  "query"@en .

reg:entity  rdfs:label  "entity"@en .

reg:containedItemClass
        rdfs:label  "contained item class"@en .

reg:statusNotAccepted
        rdfs:label  "notAccepted"@en .

reg:inverseMembershipPredicate
        rdfs:label  "inverse membership predicate"@en .

reg:operatingLanguage
        rdfs:label  "operating language"@en .

reg:Topic  rdfs:label  "Topic"@en .

reg:priorState  rdfs:label  "next state"@en .

reg:statusValid  rdfs:label  "valid"@en .

reg:StatusScheme  rdfs:label  "Status Scheme"@en .

reg:category  rdfs:label  "category"@en .

reg:predecessor  rdfs:label  "predecessor"@en .

reg:sourceGraph  rdfs:label  "source graph"@en .

reg:NamespaceForward  rdfs:label  "Namespace Forward"@en .

reg:enumerationPredicate
        rdfs:label  "enumeration predicate"@en .

reg:sourceDataset  rdfs:label  "source dataset"@en .

reg:statusExperimental
        rdfs:label  "experimental"@en .

reg:governancePolicy  rdfs:label  "governance policy"@en .

reg:Register  rdfs:label  "Register"@en .

reg:delegationTarget  rdfs:label  "delegation target"@en .

reg:alias  rdfs:label  "alias"@en .

reg:statusAccepted  rdfs:label  "accepted"@en .

reg:EntityReference  rdfs:label  "Entity Reference"@en .

reg:tag  rdfs:label  "tag"@en .

reg:subregister  rdfs:label  "subregister"@en .

reg:presentation  rdfs:label  "presentation"@en .

reg:statusAny  rdfs:label  "any"@en .

reg:entityVersion  rdfs:label  "entity version"@en .

reg:manager  rdfs:label  "manager"@en .

reg:notifies  rdfs:label  "notifies"@en .

reg:statusInvalid  rdfs:label  "invalid"@en .

reg:statusSuperseded  rdfs:label  "superseded"@en .

reg:annotation  rdfs:label  "annotation"@en .

reg:SPARQLAskQuery  rdfs:label  "SPARQL ASK query"@en .

reg:forwardingCode  rdfs:label  "forwarding code"@en .

reg:FederatedRegister
        rdfs:label  "Federated Register"@en .

<http://purl.org/linked-data/registry>
        rdfs:label  "Registry ontology"@en .

reg:ignores  rdfs:label  "ignores"@en .

reg:register  rdfs:label  "register"@en .

reg:DelegatedRegister
        rdfs:label  "Delegated Register"@en .

reg:nextState  rdfs:label  "next state"@en .

reg:successor  rdfs:label  "successor"@en .

reg:monitors  rdfs:label  "monitors"@en .

reg:submitter  rdfs:label  "submitter"@en .

reg:enumerationObject
        rdfs:label  "enumeration object"@en .

reg:SPARQLSelectQuery
        rdfs:label  "SPARQL SELECT query"@en .

reg:representationOf  rdfs:label  "representation of"@en .

reg:statusSubmitted  rdfs:label  "submitted"@en .

reg:enumerationSubject
        rdfs:label  "enumeration subject"@en .

reg:notation  rdfs:label  "notation"@en .

reg:release  rdfs:label  "release"@en .

reg:statusStable  rdfs:label  "stable"@en .

sdo:MultiPlayer  rdfs:comment  "Play mode: MultiPlayer. Requiring or allowing multiple human players to play simultaneously." ;
        rdfs:label    "MultiPlayer" .

sdo:Plumber  rdfs:comment  "A plumbing service." ;
        rdfs:label    "Plumber" .

sdo:MedicalEntity  rdfs:comment  "The most generic type of entity related to health and the practice of medicine." ;
        rdfs:label    "MedicalEntity" .

sdo:jobTitle  rdfs:comment  "The job title of the person (for example, Financial Manager)." ;
        rdfs:label    "job title" .

sdo:codeValue  rdfs:comment  "A short textual code that uniquely identifies the value." ;
        rdfs:label    "code value" .

sdo:Endocrine  rdfs:comment  "A specific branch of medical science that pertains to diagnosis and treatment of disorders of endocrine glands and their secretions." ;
        rdfs:label    "Endocrine" .

sdo:RoofingContractor
        rdfs:comment  "A roofing contractor." ;
        rdfs:label    "RoofingContractor" .

sdo:termDuration  rdfs:comment  "The amount of time in a term as defined by the institution. A term is a length of time where students take one or more classes. Semesters and quarters are common units for term." ;
        rdfs:label    "term duration" .

sdo:BikeStore  rdfs:comment  "A bike store." ;
        rdfs:label    "BikeStore" .

sdo:MerchantReturnUnspecified
        rdfs:comment  "Specifies that a product return policy is not provided." ;
        rdfs:label    "MerchantReturnUnspecified" .

sdo:courseMode  rdfs:comment  "The medium or means of delivery of the course instance or the mode of study, either as a text label (e.g. \"online\", \"onsite\" or \"blended\"; \"synchronous\" or \"asynchronous\"; \"full-time\" or \"part-time\") or as a URL reference to a term from a controlled vocabulary (e.g. https://ceds.ed.gov/element/001311#Asynchronous )." ;
        rdfs:label    "course mode" .

sdo:BodyMeasurementInsideLeg
        rdfs:comment  "Inside leg (measured between crotch and soles of feet). Used, for example, to fit pants." ;
        rdfs:label    "BodyMeasurementInsideLeg" .

sdo:CDFormat  rdfs:comment  "CDFormat." ;
        rdfs:label    "CDFormat" .

sdo:Flight  rdfs:comment  "An airline flight." ;
        rdfs:label    "Flight" .

sdo:Action  rdfs:comment  "An action performed by a direct agent and indirect participants upon a direct object. Optionally happens at a location with the help of an inanimate instrument. The execution of the action may produce a result. Specific action sub-type documentation specifies the exact expectation of each argument/role.\\n\\nSee also [blog post](http://blog.schema.org/2014/04/announcing-schemaorg-actions.html) and [Actions overview document](https://schema.org/docs/actions.html)." ;
        rdfs:label    "Action" .

sdo:scheduleTimezone  rdfs:comment  "Indicates the timezone for which the time(s) indicated in the [[Schedule]] are given. The value provided should be among those listed in the IANA Time Zone Database." ;
        rdfs:label    "schedule timezone" .

sdo:GamePlayMode  rdfs:comment  "Indicates whether this game is multi-player, co-op or single-player." ;
        rdfs:label    "GamePlayMode" .

sdo:VegetarianDiet  rdfs:comment  "A diet exclusive of animal meat." ;
        rdfs:label    "VegetarianDiet" .

sdo:CleaningFee  rdfs:comment  "Represents the cleaning fee part of the total price for an offered product, for example a vacation rental." ;
        rdfs:label    "CleaningFee" .

sdo:bioChemSimilarity
        rdfs:comment  "A similar BioChemEntity, e.g., obtained by fingerprint similarity algorithms." ;
        rdfs:label    "bio chemSimilarity" .

sdo:TripleBlindedTrial
        rdfs:comment  "A trial design in which neither the researcher, the person administering the therapy nor the patient knows the details of the treatment the patient was randomly assigned to." ;
        rdfs:label    "TripleBlindedTrial" .

sdo:ElementarySchool  rdfs:comment  "An elementary school." ;
        rdfs:label    "ElementarySchool" .

sdo:backstory  rdfs:comment  "For an [[Article]], typically a [[NewsArticle]], the backstory property provides a textual summary giving a brief explanation of why and how an article was created. In a journalistic setting this could include information about reporting process, methods, interviews, data sources, etc." ;
        rdfs:label    "backstory" .

sdo:Nonprofit501c7  rdfs:comment  "Nonprofit501c7: Non-profit type referring to Social and Recreational Clubs." ;
        rdfs:label    "Nonprofit501c7" .

sdo:Physician  rdfs:comment  "A doctor's office." ;
        rdfs:label    "Physician" .

sdo:WearableSizeSystemContinental
        rdfs:comment  "Continental size system for wearables." ;
        rdfs:label    "WearableSizeSystemContinental" .

sdo:OrderItem  rdfs:comment  "An order item is a line of an order. It includes the quantity and shipping details of a bought offer." ;
        rdfs:label    "OrderItem" .

sdo:StoreCreditRefund
        rdfs:comment  "Specifies that the customer receives a store credit as refund when returning a product" ;
        rdfs:label    "StoreCreditRefund" .

sdo:postOfficeBoxNumber
        rdfs:comment  "The post office box number for PO box addresses." ;
        rdfs:label    "post officeBoxNumber" .

sdo:representativeOfPage
        rdfs:comment  "Indicates whether this image is representative of the content of the page." ;
        rdfs:label    "representative ofPage" .

sdo:DigitalDocumentPermissionType
        rdfs:comment  "A type of permission which can be granted for accessing a digital document." ;
        rdfs:label    "DigitalDocumentPermissionType" .

sdo:EducationalOccupationalCredential
        rdfs:comment  "An educational or occupational credential. A diploma, academic degree, certification, qualification, badge, etc., that may be awarded to a person or other entity that meets the requirements defined by the credentialer." ;
        rdfs:label    "EducationalOccupationalCredential" .

sdo:GardenStore  rdfs:comment  "A garden store." ;
        rdfs:label    "GardenStore" .

sdo:HealthInsurancePlan
        rdfs:comment  "A US-style health insurance plan, including PPOs, EPOs, and HMOs. " ;
        rdfs:label    "HealthInsurancePlan" .

sdo:reviews  rdfs:comment  "Review of the item." ;
        rdfs:label    "reviews" .

sdo:EmployeeRole  rdfs:comment  "A subclass of OrganizationRole used to describe employee relationships." ;
        rdfs:label    "EmployeeRole" .

sdo:securityClearanceRequirement
        rdfs:comment  "A description of any security clearance requirements of the job." ;
        rdfs:label    "security clearanceRequirement" .

sdo:hasCourseInstance
        rdfs:comment  "An offering of the course at a specific time and place or through specific media or mode of study or to a specific section of students." ;
        rdfs:label    "has courseInstance" .

sdo:artist  rdfs:comment  "The primary artist for a work\n    \tin a medium other than pencils or digital line art--for example, if the\n    \tprimary artwork is done in watercolors or digital paints." ;
        rdfs:label    "artist" .

sdo:EventPostponed  rdfs:comment  "The event has been postponed and no new date has been set. The event's previousStartDate should be set." ;
        rdfs:label    "EventPostponed" .

sdo:Installment  rdfs:comment  "Represents the installment pricing component of the total price for an offered product." ;
        rdfs:label    "Installment" .

sdo:Radiography  rdfs:comment  "Radiography is an imaging technique that uses electromagnetic radiation other than visible light, especially X-rays, to view the internal structure of a non-uniformly composed and opaque object such as the human body." ;
        rdfs:label    "Radiography" .

sdo:vehicleInteriorColor
        rdfs:comment  "The color or color combination of the interior of the vehicle." ;
        rdfs:label    "vehicle interiorColor" .

sdo:numberOfPages  rdfs:comment  "The number of pages in the book." ;
        rdfs:label    "number ofPages" .

sdo:duplicateTherapy  rdfs:comment  "A therapy that duplicates or overlaps this one." ;
        rdfs:label    "duplicate therapy" .

sdo:event  rdfs:comment  "Upcoming or past event associated with this place, organization, or action." ;
        rdfs:label    "event" .

sdo:QuoteAction  rdfs:comment  "An agent quotes/estimates/appraises an object/product/service with a price at a location/store." ;
        rdfs:label    "QuoteAction" .

sdo:contraindication  rdfs:comment  "A contraindication for this therapy." ;
        rdfs:label    "contraindication" .

sdo:ActiveActionStatus
        rdfs:comment  "An in-progress action (e.g, while watching the movie, or driving to a location)." ;
        rdfs:label    "ActiveActionStatus" .

sdo:utterances  rdfs:comment  "Text of an utterances (spoken words, lyrics etc.) that occurs at a certain section of a media object, represented as a [[HyperTocEntry]]." ;
        rdfs:label    "utterances" .

sdo:checkinTime  rdfs:comment  "The earliest someone may check into a lodging establishment." ;
        rdfs:label    "checkin time" .

sdo:Casino  rdfs:comment  "A casino." ;
        rdfs:label    "Casino" .

sdo:nonProprietaryName
        rdfs:comment  "The generic name of this drug or supplement." ;
        rdfs:label    "non proprietaryName" .

sdo:legislationLegalForce
        rdfs:comment  "Whether the legislation is currently in force, not in force, or partially in force." ;
        rdfs:label    "legislation legalForce" .

sdo:PaymentStatusType
        rdfs:comment  "A specific payment status. For example, PaymentDue, PaymentComplete, etc." ;
        rdfs:label    "PaymentStatusType" .

sdo:observationDate  rdfs:comment  "The observationDate of an [[Observation]]." ;
        rdfs:label    "observation date" .

sdo:GlutenFreeDiet  rdfs:comment  "A diet exclusive of gluten." ;
        rdfs:label    "GlutenFreeDiet" .

sdo:StagedContent  rdfs:comment  "Content coded 'staged content' in a [[MediaReview]], considered in the context of how it was published or shared.\n\nFor a [[VideoObject]] to be 'staged content': A video that has been created using actors or similarly contrived.\n\nFor an [[ImageObject]] to be 'staged content': An image that was created using actors or similarly contrived, such as a screenshot of a fake tweet.\n\nFor an [[ImageObject]] with embedded text to be 'staged content': An image that was created using actors or similarly contrived, such as a screenshot of a fake tweet.\n\nFor an [[AudioObject]] to be 'staged content': Audio that has been created using actors or similarly contrived.\n" ;
        rdfs:label    "StagedContent" .

sdo:keywords  rdfs:comment  "Keywords or tags used to describe this content. Multiple entries in a keywords list are typically delimited by commas." ;
        rdfs:label    "keywords" .

sdo:WebPage  rdfs:comment  "A web page. Every web page is implicitly assumed to be declared to be of type WebPage, so the various properties about that webpage, such as <code>breadcrumb</code> may be used. We recommend explicit declaration if these properties are specified, but if they are found outside of an itemscope, they will be assumed to be about the page." ;
        rdfs:label    "WebPage" .

sdo:subEvents  rdfs:comment  "Events that are a part of this event. For example, a conference event includes many presentations, each subEvents of the conference." ;
        rdfs:label    "sub events" .

sdo:DoseSchedule  rdfs:comment  "A specific dosing schedule for a drug or supplement." ;
        rdfs:label    "DoseSchedule" .

sdo:Question  rdfs:comment  "A specific question - e.g. from a user seeking answers online, or collected in a Frequently Asked Questions (FAQ) document." ;
        rdfs:label    "Question" .

sdo:OnlineFull  rdfs:comment  "Game server status: OnlineFull. Server is online but unavailable. The maximum number of players has reached." ;
        rdfs:label    "OnlineFull" .

sdo:assemblyVersion  rdfs:comment  "Associated product/technology version. e.g., .NET Framework 4.5." ;
        rdfs:label    "assembly version" .

sdo:validUntil  rdfs:comment  "The date when the item is no longer valid." ;
        rdfs:label    "valid until" .

sdo:purchaseDate  rdfs:comment  "The date the item e.g. vehicle was purchased by the current owner." ;
        rdfs:label    "purchase date" .

sdo:accommodationFloorPlan
        rdfs:comment  "A floorplan of some [[Accommodation]]." ;
        rdfs:label    "accommodation floorPlan" .

sdo:firstPerformance  rdfs:comment  "The date and place the work was first performed." ;
        rdfs:label    "first performance" .

sdo:suggestedAge  rdfs:comment  "The age or age range for the intended audience or person, for example 3-12 months for infants, 1-5 years for toddlers." ;
        rdfs:label    "suggested age" .

sdo:MedicalEnumeration
        rdfs:comment  "Enumerations related to health and the practice of medicine: A concept that is used to attribute a quality to another concept, as a qualifier, a collection of items or a listing of all of the elements of a set in medicine practice." ;
        rdfs:label    "MedicalEnumeration" .

sdo:ReservationPackage
        rdfs:comment  "A group of multiple reservations with common values for all sub-reservations." ;
        rdfs:label    "ReservationPackage" .

sdo:interactionStatistic
        rdfs:comment  "The number of interactions for the CreativeWork using the WebSite or SoftwareApplication. The most specific child type of InteractionCounter should be used." ;
        rdfs:label    "interaction statistic" .

sdo:WearableSizeGroupHusky
        rdfs:comment  "Size group \"Husky\" (or \"Stocky\") for wearables." ;
        rdfs:label    "WearableSizeGroupHusky" .

sdo:printEdition  rdfs:comment  "The edition of the print product in which the NewsArticle appears." ;
        rdfs:label    "print edition" .

sdo:target  rdfs:comment  "Indicates a target EntryPoint for an Action." ;
        rdfs:label    "target" .

sdo:Class  rdfs:comment  "A class, also often called a 'Type'; equivalent to rdfs:Class." ;
        rdfs:label    "Class" .

sdo:EUEnergyEfficiencyCategoryC
        rdfs:comment  "Represents EU Energy Efficiency Class C as defined in EU energy labeling regulations." ;
        rdfs:label    "EUEnergyEfficiencyCategoryC" .

sdo:realEstateAgent  rdfs:comment  "A sub property of participant. The real estate agent involved in the action." ;
        rdfs:label    "real estateAgent" .

sdo:RadioClip  rdfs:comment  "A short radio program or a segment/part of a radio program." ;
        rdfs:label    "RadioClip" .

sdo:byArtist  rdfs:comment  "The artist that performed this album or recording." ;
        rdfs:label    "by artist" .

sdo:availability  rdfs:comment  "The availability of this item&#x2014;for example In stock, Out of stock, Pre-order, etc." ;
        rdfs:label    "availability" .

sdo:termsOfService  rdfs:comment  "Human-readable terms of service documentation." ;
        rdfs:label    "terms ofService" .

sdo:Manuscript  rdfs:comment  "A book, document, or piece of music written by hand rather than typed or printed." ;
        rdfs:label    "Manuscript" .

sdo:streetAddress  rdfs:comment  "The street address. For example, 1600 Amphitheatre Pkwy." ;
        rdfs:label    "street address" .

sdo:comment  rdfs:comment  "Comments, typically from users." ;
        rdfs:label    "comment" .

sdo:boardingPolicy  rdfs:comment  "The type of boarding policy used by the airline (e.g. zone-based or group-based)." ;
        rdfs:label    "boarding policy" .

sdo:startDate  rdfs:comment  "The start date and time of the item (in [ISO 8601 date format](http://en.wikipedia.org/wiki/ISO_8601))." ;
        rdfs:label    "start date" .

sdo:rxcui  rdfs:comment  "The RxCUI drug identifier from RXNORM." ;
        rdfs:label    "rxcui" .

sdo:quest  rdfs:comment  "The task that a player-controlled character, or group of characters may complete in order to gain a reward." ;
        rdfs:label    "quest" .

sdo:founder  rdfs:comment  "A person who founded this organization." ;
        rdfs:label    "founder" .

sdo:superEvent  rdfs:comment  "An event that this event is a part of. For example, a collection of individual music performances might each have a music festival as their superEvent." ;
        rdfs:label    "super event" .

sdo:material  rdfs:comment  "A material that something is made from, e.g. leather, wool, cotton, paper." ;
        rdfs:label    "material" .

sdo:linkRelationship  rdfs:comment  "Indicates the relationship type of a Web link. " ;
        rdfs:label    "link relationship" .

sdo:PaymentPastDue  rdfs:comment  "The payment is due and considered late." ;
        rdfs:label    "PaymentPastDue" .

sdo:circle  rdfs:comment  "A circle is the circular region of a specified radius centered at a specified latitude and longitude. A circle is expressed as a pair followed by a radius in meters." ;
        rdfs:label    "circle" .

sdo:parents  rdfs:comment  "A parents of the person." ;
        rdfs:label    "parents" .

sdo:Landform  rdfs:comment  "A landform or physical feature.  Landform elements include mountains, plains, lakes, rivers, seascape and oceanic waterbody interface features such as bays, peninsulas, seas and so forth, including sub-aqueous terrain features such as submersed mountain ranges, volcanoes, and the great ocean basins." ;
        rdfs:label    "Landform" .

sdo:SatiricalArticle  rdfs:comment  "An [[Article]] whose content is primarily [[satirical]](https://en.wikipedia.org/wiki/Satire) in nature, i.e. unlikely to be literally true. A satirical article is sometimes but not necessarily also a [[NewsArticle]]. [[ScholarlyArticle]]s are also sometimes satirized." ;
        rdfs:label    "SatiricalArticle" .

sdo:reservationFor  rdfs:comment  "The thing -- flight, event, restaurant,etc. being reserved." ;
        rdfs:label    "reservation for" .

sdo:ReturnLabelSourceEnumeration
        rdfs:comment  "Enumerates several types of return labels for product returns." ;
        rdfs:label    "ReturnLabelSourceEnumeration" .

sdo:encoding  rdfs:comment  "A media object that encodes this CreativeWork. This property is a synonym for associatedMedia." ;
        rdfs:label    "encoding" .

sdo:AppendAction  rdfs:comment  "The act of inserting at the end if an ordered collection." ;
        rdfs:label    "AppendAction" .

sdo:refundType  rdfs:comment  "A refund type, from an enumerated list." ;
        rdfs:label    "refund type" .

sdo:scheduledPaymentDate
        rdfs:comment  "The date the invoice is scheduled to be paid." ;
        rdfs:label    "scheduled paymentDate" .

sdo:SearchAction  rdfs:comment  "The act of searching for an object.\\n\\nRelated actions:\\n\\n* [[FindAction]]: SearchAction generally leads to a FindAction, but not necessarily." ;
        rdfs:label    "SearchAction" .

sdo:lesserOrEqual  rdfs:comment  "This ordering relation for qualitative values indicates that the subject is lesser than or equal to the object." ;
        rdfs:label    "lesser orEqual" .

sdo:ReadPermission  rdfs:comment  "Permission to read or view the document." ;
        rdfs:label    "ReadPermission" .

sdo:WearableSizeGroupRegular
        rdfs:comment  "Size group \"Regular\" for wearables." ;
        rdfs:label    "WearableSizeGroupRegular" .

sdo:image  rdfs:comment  "An image of the item. This can be a [[URL]] or a fully described [[ImageObject]]." ;
        rdfs:label    "image" .

sdo:gameLocation  rdfs:comment  "Real or fictional location of the game (or part of game)." ;
        rdfs:label    "game location" .

sdo:validThrough  rdfs:comment  "The date after when the item is not valid. For example the end of an offer, salary period, or a period of opening hours." ;
        rdfs:label    "valid through" .

sdo:price  rdfs:comment  "The offer price of a product, or of a price component when attached to PriceSpecification and its subtypes.\\n\\nUsage guidelines:\\n\\n* Use the [[priceCurrency]] property (with standard formats: [ISO 4217 currency format](http://en.wikipedia.org/wiki/ISO_4217) e.g. \"USD\"; [Ticker symbol](https://en.wikipedia.org/wiki/List_of_cryptocurrencies) for cryptocurrencies e.g. \"BTC\"; well known names for [Local Exchange Tradings Systems](https://en.wikipedia.org/wiki/Local_exchange_trading_system) (LETS) and other currency types e.g. \"Ithaca HOUR\") instead of including [ambiguous symbols](http://en.wikipedia.org/wiki/Dollar_sign#Currencies_that_use_the_dollar_or_peso_sign) such as '$' in the value.\\n* Use '.' (Unicode 'FULL STOP' (U+002E)) rather than ',' to indicate a decimal point. Avoid using these symbols as a readability separator.\\n* Note that both [RDFa](http://www.w3.org/TR/xhtml-rdfa-primer/#using-the-content-attribute) and Microdata syntax allow the use of a \"content=\" attribute for publishing simple machine-readable values alongside more human-friendly formatting.\\n* Use values from 0123456789 (Unicode 'DIGIT ZERO' (U+0030) to 'DIGIT NINE' (U+0039)) rather than superficially similiar Unicode symbols.\n      " ;
        rdfs:label    "price" .

sdo:broadcastServiceTier
        rdfs:comment  "The type of service required to have access to the channel (e.g. Standard or Premium)." ;
        rdfs:label    "broadcast serviceTier" .

sdo:TVEpisode  rdfs:comment  "A TV episode which can be part of a series or season." ;
        rdfs:label    "TVEpisode" .

sdo:StatusEnumeration
        rdfs:comment  "Lists or enumerations dealing with status types." ;
        rdfs:label    "StatusEnumeration" .

sdo:hasMenuItem  rdfs:comment  "A food or drink item contained in a menu or menu section." ;
        rdfs:label    "has menuItem" .

sdo:nationality  rdfs:comment  "Nationality of the person." ;
        rdfs:label    "nationality" .

sdo:BookStore  rdfs:comment  "A bookstore." ;
        rdfs:label    "BookStore" .

sdo:serviceOperator  rdfs:comment  "The operating organization, if different from the provider.  This enables the representation of services that are provided by an organization, but operated by another organization like a subcontractor." ;
        rdfs:label    "service operator" .

sdo:PhysicalActivity  rdfs:comment  "Any bodily activity that enhances or maintains physical fitness and overall health and wellness. Includes activity that is part of daily living and routine, structured exercise, and exercise prescribed as part of a medical treatment or recovery plan." ;
        rdfs:label    "PhysicalActivity" .

sdo:referencesOrder  rdfs:comment  "The Order(s) related to this Invoice. One or more Orders may be combined into a single Invoice." ;
        rdfs:label    "references order" .

sdo:BusinessEvent  rdfs:comment  "Event type: Business event." ;
        rdfs:label    "BusinessEvent" .

sdo:TreatmentIndication
        rdfs:comment  "An indication for treating an underlying condition, symptom, etc." ;
        rdfs:label    "TreatmentIndication" .

sdo:Withdrawn  rdfs:comment  "Withdrawn." ;
        rdfs:label    "Withdrawn" .

sdo:advanceBookingRequirement
        rdfs:comment  "The amount of time that is required between accepting the offer and the actual usage of the resource or service." ;
        rdfs:label    "advance bookingRequirement" .

sdo:iswcCode  rdfs:comment  "The International Standard Musical Work Code for the composition." ;
        rdfs:label    "iswc code" .

sdo:Dermatology  rdfs:comment  "A specific branch of medical science that pertains to diagnosis and treatment of disorders of skin." ;
        rdfs:label    "Dermatology" .

sdo:isPlanForApartment
        rdfs:comment  "Indicates some accommodation that this floor plan describes." ;
        rdfs:label    "is planForApartment" .

sdo:Optician  rdfs:comment  "A store that sells reading glasses and similar devices for improving vision." ;
        rdfs:label    "Optician" .

sdo:RsvpResponseMaybe
        rdfs:comment  "The invitee may or may not attend." ;
        rdfs:label    "RsvpResponseMaybe" .

sdo:prepTime  rdfs:comment  "The length of time it takes to prepare the items to be used in instructions or a direction, in [ISO 8601 duration format](http://en.wikipedia.org/wiki/ISO_8601)." ;
        rdfs:label    "prep time" .

sdo:legislationPassedBy
        rdfs:comment  "The person or organization that originally passed or made the law : typically parliament (for primary legislation) or government (for secondary legislation). This indicates the \"legal author\" of the law, as opposed to its physical author." ;
        rdfs:label    "legislation passedBy" .

sdo:AmpStory  rdfs:comment  "A creative work with a visual storytelling format intended to be viewed online, particularly on mobile devices." ;
        rdfs:label    "AmpStory" .

sdo:LaserDiscFormat  rdfs:comment  "LaserDiscFormat." ;
        rdfs:label    "LaserDiscFormat" .

sdo:supersededBy  rdfs:comment  "Relates a term (i.e. a property, class or enumeration) to one that supersedes it." ;
        rdfs:label    "superseded by" .

sdo:softwareVersion  rdfs:comment  "Version of the software instance." ;
        rdfs:label    "software version" .

sdo:reportNumber  rdfs:comment  "The number or other unique designator assigned to a Report by the publishing organization." ;
        rdfs:label    "report number" .

sdo:ContactPoint  rdfs:comment  "A contact point&#x2014;for example, a Customer Complaints department." ;
        rdfs:label    "ContactPoint" .

sdo:BefriendAction  rdfs:comment  "The act of forming a personal connection with someone (object) mutually/bidirectionally/symmetrically.\\n\\nRelated actions:\\n\\n* [[FollowAction]]: Unlike FollowAction, BefriendAction implies that the connection is reciprocal." ;
        rdfs:label    "BefriendAction" .

sdo:track  rdfs:comment  "A music recording (track)&#x2014;usually a single song. If an ItemList is given, the list should contain items of type MusicRecording." ;
        rdfs:label    "track" .

sdo:TraditionalChinese
        rdfs:comment  "A system of medicine based on common theoretical concepts that originated in China and evolved over thousands of years, that uses herbs, acupuncture, exercise, massage, dietary therapy, and other methods to treat a wide range of conditions." ;
        rdfs:label    "TraditionalChinese" .

sdo:paymentMethodId  rdfs:comment  "An identifier for the method of payment used (e.g. the last 4 digits of the credit card)." ;
        rdfs:label    "payment methodId" .

sdo:expectedPrognosis
        rdfs:comment  "The likely outcome in either the short term or long term of the medical condition." ;
        rdfs:label    "expected prognosis" .

sdo:containsPlace  rdfs:comment  "The basic containment relation between a place and another that it contains." ;
        rdfs:label    "contains place" .

sdo:dosageForm  rdfs:comment  "A dosage form in which this drug/supplement is available, e.g. 'tablet', 'suspension', 'injection'." ;
        rdfs:label    "dosage form" .

sdo:height  rdfs:comment  "The height of the item." ;
        rdfs:label    "height" .

sdo:parent  rdfs:comment  "A parent of this person." ;
        rdfs:label    "parent" .

sdo:Ear  rdfs:comment  "Ear function assessment with clinical examination." ;
        rdfs:label    "Ear" .

sdo:EntryPoint  rdfs:comment  "An entry point, within some Web-based protocol." ;
        rdfs:label    "EntryPoint" .

sdo:RepaymentSpecification
        rdfs:comment  "A structured value representing repayment." ;
        rdfs:label    "RepaymentSpecification" .

sdo:typeOfGood  rdfs:comment  "The product that this structured value is referring to." ;
        rdfs:label    "type ofGood" .

sdo:QuantitativeValue
        rdfs:comment  " A point value or interval for product characteristics and other purposes." ;
        rdfs:label    "QuantitativeValue" .

sdo:ComedyClub  rdfs:comment  "A comedy club." ;
        rdfs:label    "ComedyClub" .

sdo:medicalSpecialty  rdfs:comment  "A medical specialty of the provider." ;
        rdfs:label    "medical specialty" .

sdo:ParkingFacility  rdfs:comment  "A parking lot or other parking facility." ;
        rdfs:label    "ParkingFacility" .

sdo:alternativeOf  rdfs:comment  "Another gene which is a variation of this one." ;
        rdfs:label    "alternative of" .

sdo:defaultValue  rdfs:comment  "The default value of the input.  For properties that expect a literal, the default is a literal value, for properties that expect an object, it's an ID reference to one of the current values." ;
        rdfs:label    "default value" .

sdo:game  rdfs:comment  "Video game which is played on this server." ;
        rdfs:label    "game" .

sdo:brand  rdfs:comment  "The brand(s) associated with a product or service, or the brand(s) maintained by an organization or business person." ;
        rdfs:label    "brand" .

sdo:unitText  rdfs:comment  "A string or text indicating the unit of measurement. Useful if you cannot provide a standard unit code for\n<a href='unitCode'>unitCode</a>." ;
        rdfs:label    "unit text" .

sdo:Discontinued  rdfs:comment  "Indicates that the item has been discontinued." ;
        rdfs:label    "Discontinued" .

sdo:Chiropractic  rdfs:comment  "A system of medicine focused on the relationship between the body's structure, mainly the spine, and its functioning." ;
        rdfs:label    "Chiropractic" .

sdo:TrainStation  rdfs:comment  "A train station." ;
        rdfs:label    "TrainStation" .

sdo:sportsTeam  rdfs:comment  "A sub property of participant. The sports team that participated on this action." ;
        rdfs:label    "sports team" .

sdo:Thursday  rdfs:comment  "The day of the week between Wednesday and Friday." ;
        rdfs:label    "Thursday" .

sdo:SinglePlayer  rdfs:comment  "Play mode: SinglePlayer. Which is played by a lone player." ;
        rdfs:label    "SinglePlayer" .

sdo:WearableSizeGroupTall
        rdfs:comment  "Size group \"Tall\" for wearables." ;
        rdfs:label    "WearableSizeGroupTall" .

sdo:VeterinaryCare  rdfs:comment  "A vet's office." ;
        rdfs:label    "VeterinaryCare" .

sdo:RealEstateListing
        rdfs:comment  "A [[RealEstateListing]] is a listing that describes one or more real-estate [[Offer]]s (whose [[businessFunction]] is typically to lease out, or to sell).\n  The [[RealEstateListing]] type itself represents the overall listing, as manifested in some [[WebPage]].\n  " ;
        rdfs:label    "RealEstateListing" .

sdo:ComputerLanguage  rdfs:comment  "This type covers computer programming languages such as Scheme and Lisp, as well as other language-like computer representations. Natural languages are best represented with the [[Language]] type." ;
        rdfs:label    "ComputerLanguage" .

sdo:SportingGoodsStore
        rdfs:comment  "A sporting goods store." ;
        rdfs:label    "SportingGoodsStore" .

sdo:weightTotal  rdfs:comment  "The permitted total weight of the loaded vehicle, including passengers and cargo and the weight of the empty vehicle.\\n\\nTypical unit code(s): KGM for kilogram, LBR for pound\\n\\n* Note 1: You can indicate additional information in the [[name]] of the [[QuantitativeValue]] node.\\n* Note 2: You may also link to a [[QualitativeValue]] node that provides additional information using [[valueReference]].\\n* Note 3: Note that you can use [[minValue]] and [[maxValue]] to indicate ranges." ;
        rdfs:label    "weight total" .

sdo:mechanismOfAction
        rdfs:comment  "The specific biochemical interaction through which this drug or supplement produces its pharmacological effect." ;
        rdfs:label    "mechanism ofAction" .

sdo:minimumPaymentDue
        rdfs:comment  "The minimum payment required at this time." ;
        rdfs:label    "minimum paymentDue" .

sdo:ReturnFeesEnumeration
        rdfs:comment  "Enumerates several kinds of policies for product return fees." ;
        rdfs:label    "ReturnFeesEnumeration" .

sdo:MusicVideoObject  rdfs:comment  "A music video file." ;
        rdfs:label    "MusicVideoObject" .

sdo:itemCondition  rdfs:comment  "A predefined value from OfferItemCondition specifying the condition of the product or service, or the products or services included in the offer. Also used for product return policies to specify the condition of products accepted for returns." ;
        rdfs:label    "item condition" .

sdo:lesser  rdfs:comment  "This ordering relation for qualitative values indicates that the subject is lesser than the object." ;
        rdfs:label    "lesser" .

sdo:leiCode  rdfs:comment  "An organization identifier that uniquely identifies a legal entity as defined in ISO 17442." ;
        rdfs:label    "lei code" .

sdo:DownloadAction  rdfs:comment  "The act of downloading an object." ;
        rdfs:label    "DownloadAction" .

sdo:hoursAvailable  rdfs:comment  "The hours during which this service or contact is available." ;
        rdfs:label    "hours available" .

sdo:alumniOf  rdfs:comment  "An organization that the person is an alumni of." ;
        rdfs:label    "alumni of" .

sdo:departurePlatform
        rdfs:comment  "The platform from which the train departs." ;
        rdfs:label    "departure platform" .

sdo:PostalAddress  rdfs:comment  "The mailing address." ;
        rdfs:label    "PostalAddress" .

sdo:frequency  rdfs:comment  "How often the dose is taken, e.g. 'daily'." ;
        rdfs:label    "frequency" .

sdo:MonetaryAmountDistribution
        rdfs:comment  "A statistical distribution of monetary amounts." ;
        rdfs:label    "MonetaryAmountDistribution" .

sdo:WearableSizeSystemMX
        rdfs:comment  "Mexican size system for wearables." ;
        rdfs:label    "WearableSizeSystemMX" .

sdo:targetProduct  rdfs:comment  "Target Operating System / Product to which the code applies.  If applies to several versions, just the product name can be used." ;
        rdfs:label    "target product" .

sdo:proprietaryName  rdfs:comment  "Proprietary name given to the diet plan, typically by its originator or creator." ;
        rdfs:label    "proprietary name" .

sdo:HomeAndConstructionBusiness
        rdfs:comment  "A construction business.\\n\\nA HomeAndConstructionBusiness is a [[LocalBusiness]] that provides services around homes and buildings.\\n\\nAs a [[LocalBusiness]] it can be described as a [[provider]] of one or more [[Service]]\\(s)." ;
        rdfs:label    "HomeAndConstructionBusiness" .

sdo:diagnosis  rdfs:comment  "One or more alternative conditions considered in the differential diagnosis process as output of a diagnosis process." ;
        rdfs:label    "diagnosis" .

sdo:subOrganization  rdfs:comment  "A relationship between two organizations where the first includes the second, e.g., as a subsidiary. See also: the more specific 'department' property." ;
        rdfs:label    "sub organization" .

sdo:PhysicalTherapy  rdfs:comment  "A process of progressive physical care and rehabilitation aimed at improving a health condition." ;
        rdfs:label    "PhysicalTherapy" .

sdo:PhysicalActivityCategory
        rdfs:comment  "Categories of physical activity, organized by physiologic classification." ;
        rdfs:label    "PhysicalActivityCategory" .

sdo:seasonNumber  rdfs:comment  "Position of the season within an ordered group of seasons." ;
        rdfs:label    "season number" .

sdo:locationCreated  rdfs:comment  "The location where the CreativeWork was created, which may not be the same as the location depicted in the CreativeWork." ;
        rdfs:label    "location created" .

sdo:supportingData  rdfs:comment  "Supporting data for a SoftwareApplication." ;
        rdfs:label    "supporting data" .

sdo:accessibilityFeature
        rdfs:comment  "Content features of the resource, such as accessible media, alternatives and supported enhancements for accessibility ([WebSchemas wiki lists possible values](http://www.w3.org/wiki/WebSchemas/Accessibility))." ;
        rdfs:label    "accessibility feature" .

sdo:yearBuilt  rdfs:comment  "The year an [[Accommodation]] was constructed. This corresponds to the [YearBuilt field in RESO](https://ddwiki.reso.org/display/DDW17/YearBuilt+Field). " ;
        rdfs:label    "year built" .

sdo:enginePower  rdfs:comment  "The power of the vehicle's engine.\n    Typical unit code(s): KWT for kilowatt, BHP for brake horsepower, N12 for metric horsepower (PS, with 1 PS = 735,49875 W)\\n\\n* Note 1: There are many different ways of measuring an engine's power. For an overview, see  [http://en.wikipedia.org/wiki/Horsepower#Engine_power_test_codes](http://en.wikipedia.org/wiki/Horsepower#Engine_power_test_codes).\\n* Note 2: You can link to information about how the given value has been determined using the [[valueReference]] property.\\n* Note 3: You can use [[minValue]] and [[maxValue]] to indicate ranges." ;
        rdfs:label    "engine power" .

sdo:ConvenienceStore  rdfs:comment  "A convenience store." ;
        rdfs:label    "ConvenienceStore" .

sdo:WorkersUnion  rdfs:comment  "A Workers Union (also known as a Labor Union, Labour Union, or Trade Union) is an organization that promotes the interests of its worker members by collectively bargaining with management, organizing, and political lobbying." ;
        rdfs:label    "WorkersUnion" .

sdo:hasDeliveryMethod
        rdfs:comment  "Method used for delivery or shipping." ;
        rdfs:label    "has deliveryMethod" .

sdo:broadcastDisplayName
        rdfs:comment  "The name displayed in the channel guide. For many US affiliates, it is the network name." ;
        rdfs:label    "broadcast displayName" .

sdo:coverageStartTime
        rdfs:comment  "The time when the live blog will begin covering the Event. Note that coverage may begin before the Event's start time. The LiveBlogPosting may also be created before coverage begins." ;
        rdfs:label    "coverage startTime" .

sdo:GraphicNovel  rdfs:comment  "Book format: GraphicNovel. May represent a bound collection of ComicIssue instances." ;
        rdfs:label    "GraphicNovel" .

sdo:DecontextualizedContent
        rdfs:comment  "Content coded 'missing context' in a [[MediaReview]], considered in the context of how it was published or shared.\n\nFor a [[VideoObject]] to be 'missing context': Presenting unaltered video in an inaccurate manner that misrepresents the footage. For example, using incorrect dates or locations, altering the transcript or sharing brief clips from a longer video to mislead viewers. (A video rated 'original' can also be missing context.)\n\nFor an [[ImageObject]] to be 'missing context': Presenting unaltered images in an inaccurate manner to misrepresent the image and mislead the viewer. For example, a common tactic is using an unaltered image but saying it came from a different time or place. (An image rated 'original' can also be missing context.)\n\nFor an [[ImageObject]] with embedded text to be 'missing context': An unaltered image presented in an inaccurate manner to misrepresent the image and mislead the viewer. For example, a common tactic is using an unaltered image but saying it came from a different time or place. (An 'original' image with inaccurate text would generally fall in this category.)\n\nFor an [[AudioObject]] to be 'missing context': Unaltered audio presented in an inaccurate manner that misrepresents it. For example, using incorrect dates or locations, or sharing brief clips from a longer recording to mislead viewers. (Audio rated “original” can also be missing context.)\n" ;
        rdfs:label    "DecontextualizedContent" .

sdo:interpretedAsClaim
        rdfs:comment  "Used to indicate a specific claim contained, implied, translated or refined from the content of a [[MediaObject]] or other [[CreativeWork]]. The interpreting party can be indicated using [[claimInterpreter]]." ;
        rdfs:label    "interpreted asClaim" .

sdo:Virus  rdfs:comment  "Pathogenic virus that causes viral infection." ;
        rdfs:label    "Virus" .

sdo:OrderAction  rdfs:comment  "An agent orders an object/product/service to be delivered/sent." ;
        rdfs:label    "OrderAction" .

sdo:step  rdfs:comment  "A single step item (as HowToStep, text, document, video, etc.) or a HowToSection." ;
        rdfs:label    "step" .

sdo:Female  rdfs:comment  "The female gender." ;
        rdfs:label    "Female" .

sdo:Blog  rdfs:comment  "A [blog](https://en.wikipedia.org/wiki/Blog), sometimes known as a \"weblog\". Note that the individual posts ([[BlogPosting]]s) in a [[Blog]] are often colloqually referred to by the same term." ;
        rdfs:label    "Blog" .

sdo:Suite  rdfs:comment  "A suite in a hotel or other public accommodation, denotes a class of luxury accommodations, the key feature of which is multiple rooms (Source: Wikipedia, the free encyclopedia, see <a href=\"http://en.wikipedia.org/wiki/Suite_(hotel)\">http://en.wikipedia.org/wiki/Suite_(hotel)</a>).\n<br /><br />\nSee also the <a href=\"/docs/hotels.html\">dedicated document on the use of schema.org for marking up hotels and other forms of accommodations</a>.\n" ;
        rdfs:label    "Suite" .

sdo:PlasticSurgery  rdfs:comment  "A specific branch of medical science that pertains to therapeutic or cosmetic repair or re-formation of missing, injured or malformed tissues or body parts by manual and instrumental means." ;
        rdfs:label    "PlasticSurgery" .

sdo:TipAction  rdfs:comment  "The act of giving money voluntarily to a beneficiary in recognition of services rendered." ;
        rdfs:label    "TipAction" .

sdo:exampleOfWork  rdfs:comment  "A creative work that this work is an example/instance/realization/derivation of." ;
        rdfs:label    "example ofWork" .

sdo:Poster  rdfs:comment  "A large, usually printed placard, bill, or announcement, often illustrated, that is posted to advertise or publicize something." ;
        rdfs:label    "Poster" .

sdo:regionDrained  rdfs:comment  "The anatomical or organ system drained by this vessel; generally refers to a specific part of an organ." ;
        rdfs:label    "region drained" .

sdo:TextDigitalDocument
        rdfs:comment  "A file composed primarily of text." ;
        rdfs:label    "TextDigitalDocument" .

sdo:OrderStatus  rdfs:comment  "Enumerated status values for Order." ;
        rdfs:label    "OrderStatus" .

sdo:requiredCollateral
        rdfs:comment  "Assets required to secure loan or credit repayments. It may take form of third party pledge, goods, financial instruments (cash, securities, etc.)" ;
        rdfs:label    "required collateral" .

sdo:InvestmentFund  rdfs:comment  "A company or fund that gathers capital from a number of investors to create a pool of money that is then re-invested into stocks, bonds and other assets." ;
        rdfs:label    "InvestmentFund" .

sdo:Hostel  rdfs:comment  "A hostel - cheap accommodation, often in shared dormitories.\n<br /><br />\nSee also the <a href=\"/docs/hotels.html\">dedicated document on the use of schema.org for marking up hotels and other forms of accommodations</a>.\n" ;
        rdfs:label    "Hostel" .

sdo:clinicalPharmacology
        rdfs:comment  "Description of the absorption and elimination of drugs, including their concentration (pharmacokinetics, pK) and biological effects (pharmacodynamics, pD)." ;
        rdfs:label    "clinical pharmacology" .

sdo:DeactivateAction  rdfs:comment  "The act of stopping or deactivating a device or application (e.g. stopping a timer or turning off a flashlight)." ;
        rdfs:label    "DeactivateAction" .

sdo:dateDeleted  rdfs:comment  "The datetime the item was removed from the DataFeed." ;
        rdfs:label    "date deleted" .

sdo:departureGate  rdfs:comment  "Identifier of the flight's departure gate." ;
        rdfs:label    "departure gate" .

sdo:WearableMeasurementChestOrBust
        rdfs:comment  "Measurement of the chest/bust section, for example of a suit" ;
        rdfs:label    "WearableMeasurementChestOrBust" .

sdo:WearableSizeGroupInfants
        rdfs:comment  "Size group \"Infants\" for wearables." ;
        rdfs:label    "WearableSizeGroupInfants" .

sdo:EducationEvent  rdfs:comment  "Event type: Education event." ;
        rdfs:label    "EducationEvent" .

sdo:EvidenceLevelB  rdfs:comment  "Data derived from a single randomized trial, or nonrandomized studies." ;
        rdfs:label    "EvidenceLevelB" .

sdo:valueMaxLength  rdfs:comment  "Specifies the allowed range for number of characters in a literal value." ;
        rdfs:label    "value maxLength" .

sdo:Role  rdfs:comment  "Represents additional information about a relationship or property. For example a Role can be used to say that a 'member' role linking some SportsTeam to a player occurred during a particular time period. Or that a Person's 'actor' role in a Movie was for some particular characterName. Such properties can be attached to a Role entity, which is then associated with the main entities using ordinary properties like 'member' or 'actor'.\\n\\nSee also [blog post](http://blog.schema.org/2014/06/introducing-role.html)." ;
        rdfs:label    "Role" .

sdo:Event  rdfs:comment  "An event happening at a certain time and location, such as a concert, lecture, or festival. Ticketing information may be added via the [[offers]] property. Repeated events may be structured as separate Event objects." ;
        rdfs:label    "Event" .

sdo:performerIn  rdfs:comment  "Event that this person is a performer or participant in." ;
        rdfs:label    "performer in" .

sdo:inLanguage  rdfs:comment  "The language of the content or performance or used in an action. Please use one of the language codes from the [IETF BCP 47 standard](http://tools.ietf.org/html/bcp47). See also [[availableLanguage]]." ;
        rdfs:label    "in language" .

sdo:FoodEstablishment
        rdfs:comment  "A food-related business." ;
        rdfs:label    "FoodEstablishment" .

sdo:accountId  rdfs:comment  "The identifier for the account the payment will be applied to." ;
        rdfs:label    "account id" .

sdo:EmergencyService  rdfs:comment  "An emergency service, such as a fire station or ER." ;
        rdfs:label    "EmergencyService" .

sdo:newsUpdatesAndGuidelines
        rdfs:comment  "Indicates a page with news updates and guidelines. This could often be (but is not required to be) the main page containing [[SpecialAnnouncement]] markup on a site." ;
        rdfs:label    "news updatesAndGuidelines" .

sdo:MediaObject  rdfs:comment  "A media object, such as an image, video, or audio object embedded in a web page or a downloadable dataset i.e. DataDownload. Note that a creative work may have many media objects associated with it on the same web page. For example, a page about a single song (MusicRecording) may have a music video (VideoObject), and a high and low bandwidth audio stream (2 AudioObject's)." ;
        rdfs:label    "MediaObject" .

sdo:videoQuality  rdfs:comment  "The quality of the video." ;
        rdfs:label    "video quality" .

sdo:seeks  rdfs:comment  "A pointer to products or services sought by the organization or person (demand)." ;
        rdfs:label    "seeks" .

sdo:PodcastSeries  rdfs:comment  "A podcast is an episodic series of digital audio or video files which a user can download and listen to." ;
        rdfs:label    "PodcastSeries" .

sdo:NoteDigitalDocument
        rdfs:comment  "A file containing a note, primarily for the author." ;
        rdfs:label    "NoteDigitalDocument" .

sdo:PawnShop  rdfs:comment  "A shop that will buy, or lend money against the security of, personal possessions." ;
        rdfs:label    "PawnShop" .

sdo:engineDisplacement
        rdfs:comment  "The volume swept by all of the pistons inside the cylinders of an internal combustion engine in a single movement. \\n\\nTypical unit code(s): CMQ for cubic centimeter, LTR for liters, INQ for cubic inches\\n* Note 1: You can link to information about how the given value has been determined using the [[valueReference]] property.\\n* Note 2: You can use [[minValue]] and [[maxValue]] to indicate ranges." ;
        rdfs:label    "engine displacement" .

sdo:recipeCuisine  rdfs:comment  "The cuisine of the recipe (for example, French or Ethiopian)." ;
        rdfs:label    "recipe cuisine" .

sdo:healthPlanNetworkId
        rdfs:comment  "Name or unique ID of network. (Networks are often reused across different insurance plans)." ;
        rdfs:label    "health planNetworkId" .

sdo:paymentDueDate  rdfs:comment  "The date that payment is due." ;
        rdfs:label    "payment dueDate" .

sdo:MedicalStudyStatus
        rdfs:comment  "The status of a medical study. Enumerated type." ;
        rdfs:label    "MedicalStudyStatus" .

sdo:cvdNumC19OverflowPats
        rdfs:comment  "numc19overflowpats - ED/OVERFLOW: Patients with suspected or confirmed COVID-19 who are in the ED or any overflow location awaiting an inpatient bed." ;
        rdfs:label    "cvd numC19OverflowPats" .

sdo:activeIngredient  rdfs:comment  "An active ingredient, typically chemical compounds and/or biologic substances." ;
        rdfs:label    "active ingredient" .

sdo:JewelryStore  rdfs:comment  "A jewelry store." ;
        rdfs:label    "JewelryStore" .

sdo:isGift  rdfs:comment  "Was the offer accepted as a gift for someone other than the buyer." ;
        rdfs:label    "is gift" .

sdo:MarryAction  rdfs:comment  "The act of marrying a person." ;
        rdfs:label    "MarryAction" .

sdo:FinancialProduct  rdfs:comment  "A product provided to consumers and businesses by financial institutions such as banks, insurance companies, brokerage firms, consumer finance companies, and investment companies which comprise the financial services industry." ;
        rdfs:label    "FinancialProduct" .

sdo:ImageGallery  rdfs:comment  "Web page type: Image gallery page." ;
        rdfs:label    "ImageGallery" .

sdo:MedicalCause  rdfs:comment  "The causative agent(s) that are responsible for the pathophysiologic process that eventually results in a medical condition, symptom or sign. In this schema, unless otherwise specified this is meant to be the proximate cause of the medical condition, symptom or sign. The proximate cause is defined as the causative agent that most directly results in the medical condition, symptom or sign. For example, the HIV virus could be considered a cause of AIDS. Or in a diagnostic context, if a patient fell and sustained a hip fracture and two days later sustained a pulmonary embolism which eventuated in a cardiac arrest, the cause of the cardiac arrest (the proximate cause) would be the pulmonary embolism and not the fall. Medical causes can include cardiovascular, chemical, dermatologic, endocrine, environmental, gastroenterologic, genetic, hematologic, gynecologic, iatrogenic, infectious, musculoskeletal, neurologic, nutritional, obstetric, oncologic, otolaryngologic, pharmacologic, psychiatric, pulmonary, renal, rheumatologic, toxic, traumatic, or urologic causes; medical conditions can be causes as well." ;
        rdfs:label    "MedicalCause" .

sdo:SolveMathAction  rdfs:comment  "The action that takes in a math expression and directs users to a page potentially capable of solving/simplifying that expression." ;
        rdfs:label    "SolveMathAction" .

sdo:BroadcastFrequencySpecification
        rdfs:comment  "The frequency in MHz and the modulation used for a particular BroadcastService." ;
        rdfs:label    "BroadcastFrequencySpecification" .

sdo:seatRow  rdfs:comment  "The row location of the reserved seat (e.g., B)." ;
        rdfs:label    "seat row" .

sdo:codeSampleType  rdfs:comment  "What type of code sample: full (compile ready) solution, code snippet, inline code, scripts, template." ;
        rdfs:label    "code sampleType" .

sdo:postOp  rdfs:comment  "A description of the postoperative procedures, care, and/or followups for this device." ;
        rdfs:label    "post op" .

sdo:Nonprofit501c2  rdfs:comment  "Nonprofit501c2: Non-profit type referring to Title-holding Corporations for Exempt Organizations." ;
        rdfs:label    "Nonprofit501c2" .

sdo:orderStatus  rdfs:comment  "The current status of the order." ;
        rdfs:label    "order status" .

sdo:SteeringPositionValue
        rdfs:comment  "A value indicating a steering position." ;
        rdfs:label    "SteeringPositionValue" .

sdo:duration  rdfs:comment  "The duration of the item (movie, audio recording, event, etc.) in [ISO 8601 date format](http://en.wikipedia.org/wiki/ISO_8601)." ;
        rdfs:label    "duration" .

sdo:homeLocation  rdfs:comment  "A contact location for a person's residence." ;
        rdfs:label    "home location" .

sdo:ArchiveOrganization
        rdfs:comment  "An organization with archival holdings. An organization which keeps and preserves archival material and typically makes it accessible to the public."@en ;
        rdfs:label    "ArchiveOrganization"@en .

sdo:MedicalCode  rdfs:comment  "A code for a medical entity." ;
        rdfs:label    "MedicalCode" .

sdo:free  rdfs:comment  "A flag to signal that the item, event, or place is accessible for free." ;
        rdfs:label    "free" .

sdo:countryOfLastProcessing
        rdfs:comment  "The place where the item (typically [[Product]]) was last processed and tested before importation." ;
        rdfs:label    "country ofLastProcessing" .

sdo:suggestedMinAge  rdfs:comment  "Minimum recommended age in years for the audience or user." ;
        rdfs:label    "suggested minAge" .

sdo:NutritionInformation
        rdfs:comment  "Nutritional information about the recipe." ;
        rdfs:label    "NutritionInformation" .

sdo:encodings  rdfs:comment  "A media object that encodes this CreativeWork." ;
        rdfs:label    "encodings" .

sdo:Nonprofit501c9  rdfs:comment  "Nonprofit501c9: Non-profit type referring to Voluntary Employee Beneficiary Associations." ;
        rdfs:label    "Nonprofit501c9" .

sdo:gracePeriod  rdfs:comment  "The period of time after any due date that the borrower has to fulfil its obligations before a default (failure to pay) is deemed to have occurred." ;
        rdfs:label    "grace period" .

sdo:LoseAction  rdfs:comment  "The act of being defeated in a competitive activity." ;
        rdfs:label    "LoseAction" .

sdo:infectiousAgentClass
        rdfs:comment  "The class of infectious agent (bacteria, prion, etc.) that causes the disease." ;
        rdfs:label    "infectious agentClass" .

sdo:Pond  rdfs:comment  "A pond." ;
        rdfs:label    "Pond" .

sdo:EventSeries  rdfs:comment  "A series of [[Event]]s. Included events can relate with the series using the [[superEvent]] property.\n\nAn EventSeries is a collection of events that share some unifying characteristic. For example, \"The Olympic Games\" is a series, which\nis repeated regularly. The \"2012 London Olympics\" can be presented both as an [[Event]] in the series \"Olympic Games\", and as an\n[[EventSeries]] that included a number of sporting competitions as Events.\n\nThe nature of the association between the events in an [[EventSeries]] can vary, but typical examples could\ninclude a thematic event series (e.g. topical meetups or classes), or a series of regular events that share a location, attendee group and/or organizers.\n\nEventSeries has been defined as a kind of Event to make it easy for publishers to use it in an Event context without\nworrying about which kinds of series are really event-like enough to call an Event. In general an EventSeries\nmay seem more Event-like when the period of time is compact and when aspects such as location are fixed, but\nit may also sometimes prove useful to describe a longer-term series as an Event.\n   " ;
        rdfs:label    "EventSeries" .

sdo:beforeMedia  rdfs:comment  "A media object representing the circumstances before performing this direction." ;
        rdfs:label    "before media" .

sdo:InternationalTrial
        rdfs:comment  "An international trial." ;
        rdfs:label    "InternationalTrial" .

sdo:WearableSizeGroupMisses
        rdfs:comment  "Size group \"Misses\" (also known as \"Missy\") for wearables." ;
        rdfs:label    "WearableSizeGroupMisses" .

sdo:requiredGender  rdfs:comment  "Audiences defined by a person's gender." ;
        rdfs:label    "required gender" .

sdo:BoardingPolicyType
        rdfs:comment  "A type of boarding policy used by an airline." ;
        rdfs:label    "BoardingPolicyType" .

sdo:RealEstateAgent  rdfs:comment  "A real-estate agent." ;
        rdfs:label    "RealEstateAgent" .

sdo:Pediatric  rdfs:comment  "A specific branch of medical science that specializes in the care of infants, children and adolescents." ;
        rdfs:label    "Pediatric" .

sdo:BoatReservation  rdfs:comment  "A reservation for boat travel.\n\nNote: This type is for information about actual reservations, e.g. in confirmation emails or HTML pages with individual confirmations of reservations. For offers of tickets, use [[Offer]]." ;
        rdfs:label    "BoatReservation" .

sdo:availableThrough  rdfs:comment  "After this date, the item will no longer be available for pickup." ;
        rdfs:label    "available through" .

sdo:identifyingExam  rdfs:comment  "A physical examination that can identify this sign." ;
        rdfs:label    "identifying exam" .

sdo:includedDataCatalog
        rdfs:comment  "A data catalog which contains this dataset (this property was previously 'catalog', preferred name is now 'includedInDataCatalog')." ;
        rdfs:label    "included dataCatalog" .

sdo:itemListOrder  rdfs:comment  "Type of ordering (e.g. Ascending, Descending, Unordered)." ;
        rdfs:label    "item listOrder" .

sdo:lender  rdfs:comment  "A sub property of participant. The person that lends the object being borrowed." ;
        rdfs:label    "lender" .

sdo:InteractAction  rdfs:comment  "The act of interacting with another person or organization." ;
        rdfs:label    "InteractAction" .

sdo:WholesaleStore  rdfs:comment  "A wholesale store." ;
        rdfs:label    "WholesaleStore" .

sdo:PlanAction  rdfs:comment  "The act of planning the execution of an event/task/action/reservation/plan to a future date." ;
        rdfs:label    "PlanAction" .

sdo:CausesHealthAspect
        rdfs:comment  "Information about the causes and main actions that gave rise to the topic." ;
        rdfs:label    "CausesHealthAspect" .

sdo:recipeCategory  rdfs:comment  "The category of the recipe—for example, appetizer, entree, etc." ;
        rdfs:label    "recipe category" .

sdo:PropertyValueSpecification
        rdfs:comment  "A Property value specification." ;
        rdfs:label    "PropertyValueSpecification" .

sdo:strengthUnit  rdfs:comment  "The units of an active ingredient's strength, e.g. mg." ;
        rdfs:label    "strength unit" .

sdo:award  rdfs:comment  "An award won by or for this item." ;
        rdfs:label    "award" .

sdo:ContagiousnessHealthAspect
        rdfs:comment  "Content about contagion mechanisms and contagiousness information over the topic." ;
        rdfs:label    "ContagiousnessHealthAspect" .

sdo:hasMap  rdfs:comment  "A URL to a map of the place." ;
        rdfs:label    "has map" .

sdo:carrier  rdfs:comment  "'carrier' is an out-dated term indicating the 'provider' for parcel delivery and flights." ;
        rdfs:label    "carrier" .

sdo:OccupationalActivity
        rdfs:comment  "Any physical activity engaged in for job-related purposes. Examples may include waiting tables, maid service, carrying a mailbag, picking fruits or vegetables, construction work, etc." ;
        rdfs:label    "OccupationalActivity" .

sdo:publishingPrinciples
        rdfs:comment  "The publishingPrinciples property indicates (typically via [[URL]]) a document describing the editorial principles of an [[Organization]] (or individual e.g. a [[Person]] writing a blog) that relate to their activities as a publisher, e.g. ethics or diversity policies. When applied to a [[CreativeWork]] (e.g. [[NewsArticle]]) the principles are those of the party primarily responsible for the creation of the [[CreativeWork]].\n\nWhile such policies are most typically expressed in natural language, sometimes related information (e.g. indicating a [[funder]]) can be expressed using schema.org terminology.\n" ;
        rdfs:label    "publishing principles" .

sdo:WebContent  rdfs:comment  "WebContent is a type representing all [[WebPage]], [[WebSite]] and [[WebPageElement]] content. It is sometimes the case that detailed distinctions between Web pages, sites and their parts is not always important or obvious. The  [[WebContent]] type makes it easier to describe Web-addressable content without requiring such distinctions to always be stated. (The intent is that the existing types [[WebPage]], [[WebSite]] and [[WebPageElement]] will eventually be declared as subtypes of [[WebContent]])." ;
        rdfs:label    "WebContent" .

sdo:GovernmentOrganization
        rdfs:comment  "A governmental organization or agency." ;
        rdfs:label    "GovernmentOrganization" .

sdo:EngineSpecification
        rdfs:comment  "Information about the engine of the vehicle. A vehicle can have multiple engines represented by multiple engine specification entities." ;
        rdfs:label    "EngineSpecification" .

sdo:Ayurvedic  rdfs:comment  "A system of medicine that originated in India over thousands of years and that focuses on integrating and balancing the body, mind, and spirit." ;
        rdfs:label    "Ayurvedic" .

sdo:SingleRelease  rdfs:comment  "SingleRelease." ;
        rdfs:label    "SingleRelease" .

sdo:AdultEntertainment
        rdfs:comment  "An adult entertainment establishment." ;
        rdfs:label    "AdultEntertainment" .

sdo:WearableMeasurementCup
        rdfs:comment  "Measurement of the cup, for example of a bra" ;
        rdfs:label    "WearableMeasurementCup" .

sdo:Obstetric  rdfs:comment  "A specific branch of medical science that specializes in the care of women during the prenatal and postnatal care and with the delivery of the child." ;
        rdfs:label    "Obstetric" .

sdo:InviteAction  rdfs:comment  "The act of asking someone to attend an event. Reciprocal of RsvpAction." ;
        rdfs:label    "InviteAction" .

sdo:OpeningHoursSpecification
        rdfs:comment  "A structured value providing information about the opening hours of a place or a certain service inside a place.\\n\\n\nThe place is __open__ if the [[opens]] property is specified, and __closed__ otherwise.\\n\\nIf the value for the [[closes]] property is less than the value for the [[opens]] property then the hour range is assumed to span over the next day.\n      " ;
        rdfs:label    "OpeningHoursSpecification" .

sdo:musicalKey  rdfs:comment  "The key, mode, or scale this composition uses." ;
        rdfs:label    "musical key" .

sdo:itinerary  rdfs:comment  "Destination(s) ( [[Place]] ) that make up a trip. For a trip where destination order is important use [[ItemList]] to specify that order (see examples)." ;
        rdfs:label    "itinerary" .

sdo:Intangible  rdfs:comment  "A utility class that serves as the umbrella for a number of 'intangible' things such as quantities, structured values, etc." ;
        rdfs:label    "Intangible" .

sdo:encodingFormat  rdfs:comment  "Media type typically expressed using a MIME format (see [IANA site](http://www.iana.org/assignments/media-types/media-types.xhtml) and [MDN reference](https://developer.mozilla.org/en-US/docs/Web/HTTP/Basics_of_HTTP/MIME_types)) e.g. application/zip for a SoftwareApplication binary, audio/mpeg for .mp3 etc.).\n\nIn cases where a [[CreativeWork]] has several media type representations, [[encoding]] can be used to indicate each [[MediaObject]] alongside particular [[encodingFormat]] information.\n\nUnregistered or niche encoding and file formats can be indicated instead via the most appropriate URL, e.g. defining Web page or a Wikipedia/Wikidata entry." ;
        rdfs:label    "encoding format" .

sdo:MedicalDevicePurpose
        rdfs:comment  "Categories of medical devices, organized by the purpose or intended use of the device." ;
        rdfs:label    "MedicalDevicePurpose" .

sdo:copyrightYear  rdfs:comment  "The year during which the claimed copyright for the CreativeWork was first asserted." ;
        rdfs:label    "copyright year" .

sdo:timeToComplete  rdfs:comment  "The expected length of time to complete the program if attending full-time." ;
        rdfs:label    "time toComplete" .

sdo:eligibilityToWorkRequirement
        rdfs:comment  "The legal requirements such as citizenship, visa and other documentation required for an applicant to this job." ;
        rdfs:label    "eligibility toWorkRequirement" .

sdo:Legislation  rdfs:comment  "A legal document such as an act, decree, bill, etc. (enforceable or not) or a component of a legal act (like an article)." ;
        rdfs:label    "Legislation" .

sdo:Comment  rdfs:comment  "A comment on an item - for example, a comment on a blog post. The comment's content is expressed via the [[text]] property, and its topic via [[about]], properties shared with all CreativeWorks." ;
        rdfs:label    "Comment" .

sdo:suggestedMaxAge  rdfs:comment  "Maximum recommended age in years for the audience or user." ;
        rdfs:label    "suggested maxAge" .

sdo:BusinessAudience  rdfs:comment  "A set of characteristics belonging to businesses, e.g. who compose an item's target audience." ;
        rdfs:label    "BusinessAudience" .

sdo:contributor  rdfs:comment  "A secondary contributor to the CreativeWork or Event." ;
        rdfs:label    "contributor" .

sdo:BackOrder  rdfs:comment  "Indicates that the item is available on back order." ;
        rdfs:label    "BackOrder" .

sdo:InvestmentOrDeposit
        rdfs:comment  "A type of financial product that typically requires the client to transfer funds to a financial service in return for potential beneficial financial return." ;
        rdfs:label    "InvestmentOrDeposit" .

sdo:evidenceOrigin  rdfs:comment  "Source of the data used to formulate the guidance, e.g. RCT, consensus opinion, etc." ;
        rdfs:label    "evidence origin" .

sdo:OutletStore  rdfs:comment  "An outlet store." ;
        rdfs:label    "OutletStore" .

sdo:HobbyShop  rdfs:comment  "A store that sells materials useful or necessary for various hobbies." ;
        rdfs:label    "HobbyShop" .

sdo:TherapeuticProcedure
        rdfs:comment  "A medical procedure intended primarily for therapeutic purposes, aimed at improving a health condition." ;
        rdfs:label    "TherapeuticProcedure" .

sdo:HearingImpairedSupported
        rdfs:comment  "Uses devices to support users with hearing impairments." ;
        rdfs:label    "HearingImpairedSupported" .

sdo:nonprofitStatus  rdfs:comment  "nonprofit Status indicates the legal status of a non-profit organization in its primary place of business." ;
        rdfs:label    "nonprofit status" .

sdo:runsTo  rdfs:comment  "The vasculature the lymphatic structure runs, or efferents, to." ;
        rdfs:label    "runs to" .

sdo:WearableMeasurementOutsideLeg
        rdfs:comment  "Measurement of the outside leg, for example of pants" ;
        rdfs:label    "WearableMeasurementOutsideLeg" .

sdo:MeetingRoom  rdfs:comment  "A meeting room, conference room, or conference hall is a room provided for singular events such as business conferences and meetings (Source: Wikipedia, the free encyclopedia, see <a href=\"http://en.wikipedia.org/wiki/Conference_hall\">http://en.wikipedia.org/wiki/Conference_hall</a>).\n<br /><br />\nSee also the <a href=\"/docs/hotels.html\">dedicated document on the use of schema.org for marking up hotels and other forms of accommodations</a>.\n" ;
        rdfs:label    "MeetingRoom" .

sdo:hasEnergyEfficiencyCategory
        rdfs:comment  "Defines the energy efficiency Category (which could be either a rating out of range of values or a yes/no certification) for a product according to an international energy efficiency standard." ;
        rdfs:label    "has energyEfficiencyCategory" .

sdo:MedicalScholarlyArticle
        rdfs:comment  "A scholarly article in the medical domain." ;
        rdfs:label    "MedicalScholarlyArticle" .

sdo:Osteopathic  rdfs:comment  "A system of medicine focused on promoting the body's innate ability to heal itself." ;
        rdfs:label    "Osteopathic" .

sdo:events  rdfs:comment  "Upcoming or past events associated with this place or organization." ;
        rdfs:label    "events" .

sdo:tracks  rdfs:comment  "A music recording (track)&#x2014;usually a single song." ;
        rdfs:label    "tracks" .

sdo:Book  rdfs:comment  "A book." ;
        rdfs:label    "Book" .

sdo:MotorcycleRepair  rdfs:comment  "A motorcycle repair shop." ;
        rdfs:label    "MotorcycleRepair" .

sdo:PaymentComplete  rdfs:comment  "The payment has been received and processed." ;
        rdfs:label    "PaymentComplete" .

sdo:PropertyValue  rdfs:comment  "A property-value pair, e.g. representing a feature of a product or place. Use the 'name' property for the name of the property. If there is an additional human-readable version of the value, put that into the 'description' property.\\n\\n Always use specific schema.org properties when a) they exist and b) you can populate them. Using PropertyValue as a substitute will typically not trigger the same effect as using the original, specific property.\n    " ;
        rdfs:label    "PropertyValue" .

sdo:artEdition  rdfs:comment  "The number of copies when multiple copies of a piece of artwork are produced - e.g. for a limited edition of 20 prints, 'artEdition' refers to the total number of copies (in this example \"20\")." ;
        rdfs:label    "art edition" .

sdo:competitor  rdfs:comment  "A competitor in a sports event." ;
        rdfs:label    "competitor" .

sdo:FullRefund  rdfs:comment  "Specifies that a refund can be done in the full amount the customer paid for the product" ;
        rdfs:label    "FullRefund" .

sdo:AdvertiserContentArticle
        rdfs:comment  "An [[Article]] that an external entity has paid to place or to produce to its specifications. Includes [advertorials](https://en.wikipedia.org/wiki/Advertorial), sponsored content, native advertising and other paid content." ;
        rdfs:label    "AdvertiserContentArticle" .

sdo:WearableSizeGroupPlus
        rdfs:comment  "Size group \"Plus\" for wearables." ;
        rdfs:label    "WearableSizeGroupPlus" .

sdo:citation  rdfs:comment  "A citation or reference to another creative work, such as another publication, web page, scholarly article, etc." ;
        rdfs:label    "citation" .

sdo:schoolClosuresInfo
        rdfs:comment  "Information about school closures." ;
        rdfs:label    "school closuresInfo" .

sdo:RestrictedDiet  rdfs:comment  "A diet restricted to certain foods or preparations for cultural, religious, health or lifestyle reasons. " ;
        rdfs:label    "RestrictedDiet" .

sdo:PriceComponentTypeEnumeration
        rdfs:comment  "Enumerates different price components that together make up the total price for an offered product." ;
        rdfs:label    "PriceComponentTypeEnumeration" .

sdo:ArchiveComponent  rdfs:comment  "An intangible type to be applied to any archive content, carrying with it a set of properties required to describe archival items and collections."@en ;
        rdfs:label    "ArchiveComponent"@en .

sdo:UserDownloads  rdfs:comment  "UserInteraction and its subtypes is an old way of talking about users interacting with pages. It is generally better to use [[Action]]-based vocabulary, alongside types such as [[Comment]]." ;
        rdfs:label    "UserDownloads" .

sdo:WearableMeasurementHips
        rdfs:comment  "Measurement of the hip section, for example of a skirt" ;
        rdfs:label    "WearableMeasurementHips" .

sdo:HealthAndBeautyBusiness
        rdfs:comment  "Health and beauty." ;
        rdfs:label    "HealthAndBeautyBusiness" .

sdo:ReturnAtKiosk  rdfs:comment  "Specifies that product returns must be made at a kiosk." ;
        rdfs:label    "ReturnAtKiosk" .

sdo:location  rdfs:comment  "The location of, for example, where an event is happening, where an organization is located, or where an action takes place." ;
        rdfs:label    "location" .

sdo:MinimumAdvertisedPrice
        rdfs:comment  "Represents the minimum advertised price (\"MAP\") (as dictated by the manufacturer) of an offered product." ;
        rdfs:label    "MinimumAdvertisedPrice" .

sdo:naics  rdfs:comment  "The North American Industry Classification System (NAICS) code for a particular organization or business person." ;
        rdfs:label    "naics" .

sdo:orderItemNumber  rdfs:comment  "The identifier of the order item." ;
        rdfs:label    "order itemNumber" .

sdo:vehicleSeatingCapacity
        rdfs:comment  "The number of passengers that can be seated in the vehicle, both in terms of the physical space available, and in terms of limitations set by law.\\n\\nTypical unit code(s): C62 for persons." ;
        rdfs:label    "vehicle seatingCapacity" .

sdo:Quotation  rdfs:comment  "A quotation. Often but not necessarily from some written work, attributable to a real world author and - if associated with a fictional character - to any fictional Person. Use [[isBasedOn]] to link to source/origin. The [[recordedIn]] property can be used to reference a Quotation from an [[Event]]." ;
        rdfs:label    "Quotation" .

sdo:Accommodation  rdfs:comment  "An accommodation is a place that can accommodate human beings, e.g. a hotel room, a camping pitch, or a meeting room. Many accommodations are for overnight stays, but this is not a mandatory requirement.\nFor more specific types of accommodations not defined in schema.org, one can use additionalType with external vocabularies.\n<br /><br />\nSee also the <a href=\"/docs/hotels.html\">dedicated document on the use of schema.org for marking up hotels and other forms of accommodations</a>.\n" ;
        rdfs:label    "Accommodation" .

sdo:director  rdfs:comment  "A director of e.g. tv, radio, movie, video gaming etc. content, or of an event. Directors can be associated with individual items or with a series, episode, clip." ;
        rdfs:label    "director" .

sdo:healthPlanPharmacyCategory
        rdfs:comment  "The category or type of pharmacy associated with this cost sharing." ;
        rdfs:label    "health planPharmacyCategory" .

sdo:Abdomen  rdfs:comment  "Abdomen clinical examination." ;
        rdfs:label    "Abdomen" .

sdo:globalLocationNumber
        rdfs:comment  "The [Global Location Number](http://www.gs1.org/gln) (GLN, sometimes also referred to as International Location Number or ILN) of the respective organization, person, or place. The GLN is a 13-digit number used to identify parties and physical locations." ;
        rdfs:label    "global locationNumber" .

sdo:itemDefectReturnLabelSource
        rdfs:comment  "The method (from an enumeration) by which the customer obtains a return shipping label for a defect product." ;
        rdfs:label    "item defectReturnLabelSource" .

sdo:Nonprofit501c21  rdfs:comment  "Nonprofit501c21: Non-profit type referring to Black Lung Benefit Trusts." ;
        rdfs:label    "Nonprofit501c21" .

sdo:mapType  rdfs:comment  "Indicates the kind of Map, from the MapCategoryType Enumeration." ;
        rdfs:label    "map type" .

sdo:productGroupID  rdfs:comment  "Indicates a textual identifier for a ProductGroup." ;
        rdfs:label    "product groupID" .

sdo:seller  rdfs:comment  "An entity which offers (sells / leases / lends / loans) the services / goods.  A seller may also be a provider." ;
        rdfs:label    "seller" .

sdo:InStoreOnly  rdfs:comment  "Indicates that the item is available only at physical locations." ;
        rdfs:label    "InStoreOnly" .

sdo:followee  rdfs:comment  "A sub property of object. The person or organization being followed." ;
        rdfs:label    "followee" .

sdo:Optometric  rdfs:comment  "The science or practice of testing visual acuity and prescribing corrective lenses." ;
        rdfs:label    "Optometric" .

sdo:ReadAction  rdfs:comment  "The act of consuming written content." ;
        rdfs:label    "ReadAction" .

sdo:serviceOutput  rdfs:comment  "The tangible thing generated by the service, e.g. a passport, permit, etc." ;
        rdfs:label    "service output" .

sdo:seatSection  rdfs:comment  "The section location of the reserved seat (e.g. Orchestra)." ;
        rdfs:label    "seat section" .

sdo:CompoundPriceSpecification
        rdfs:comment  "A compound price specification is one that bundles multiple prices that all apply in combination for different dimensions of consumption. Use the name property of the attached unit price specification for indicating the dimension of a price component (e.g. \"electricity\" or \"final cleaning\")." ;
        rdfs:label    "CompoundPriceSpecification" .

sdo:TypesHealthAspect
        rdfs:comment  "Categorization and other types related to a topic." ;
        rdfs:label    "TypesHealthAspect" .

sdo:sku  rdfs:comment  "The Stock Keeping Unit (SKU), i.e. a merchant-specific identifier for a product or service, or the product to which the offer refers." ;
        rdfs:label    "sku" .

sdo:validFrom  rdfs:comment  "The date when the item becomes valid." ;
        rdfs:label    "valid from" .

sdo:Hackathon  rdfs:comment  "A [hackathon](https://en.wikipedia.org/wiki/Hackathon) event." ;
        rdfs:label    "Hackathon" .

sdo:SatireOrParodyContent
        rdfs:comment  "Content coded 'satire or parody content' in a [[MediaReview]], considered in the context of how it was published or shared.\n\nFor a [[VideoObject]] to be 'satire or parody content': A video that was created as political or humorous commentary and is presented in that context. (Reshares of satire/parody content that do not include relevant context are more likely to fall under the “missing context” rating.)\n\nFor an [[ImageObject]] to be 'satire or parody content': An image that was created as political or humorous commentary and is presented in that context. (Reshares of satire/parody content that do not include relevant context are more likely to fall under the “missing context” rating.)\n\nFor an [[ImageObject]] with embedded text to be 'satire or parody content': An image that was created as political or humorous commentary and is presented in that context. (Reshares of satire/parody content that do not include relevant context are more likely to fall under the “missing context” rating.)\n\nFor an [[AudioObject]] to be 'satire or parody content': Audio that was created as political or humorous commentary and is presented in that context. (Reshares of satire/parody content that do not include relevant context are more likely to fall under the “missing context” rating.)\n" ;
        rdfs:label    "SatireOrParodyContent" .

sdo:photo  rdfs:comment  "A photograph of this place." ;
        rdfs:label    "photo" .

sdo:associatedArticle
        rdfs:comment  "A NewsArticle associated with the Media Object." ;
        rdfs:label    "associated article" .

sdo:exerciseType  rdfs:comment  "Type(s) of exercise or activity, such as strength training, flexibility training, aerobics, cardiac rehabilitation, etc." ;
        rdfs:label    "exercise type" .

sdo:ZoneBoardingPolicy
        rdfs:comment  "The airline boards by zones of the plane." ;
        rdfs:label    "ZoneBoardingPolicy" .

sdo:BusStop  rdfs:comment  "A bus stop." ;
        rdfs:label    "BusStop" .

sdo:Nonprofit501c28  rdfs:comment  "Nonprofit501c28: Non-profit type referring to National Railroad Retirement Investment Trusts." ;
        rdfs:label    "Nonprofit501c28" .

sdo:riskFactor  rdfs:comment  "A modifiable or non-modifiable factor that increases the risk of a patient contracting this condition, e.g. age,  coexisting condition." ;
        rdfs:label    "risk factor" .

sdo:isBasedOnUrl  rdfs:comment  "A resource that was used in the creation of this resource. This term can be repeated for multiple sources. For example, http://example.com/great-multiplication-intro.html." ;
        rdfs:label    "is basedOnUrl" .

sdo:WearableSizeSystemCN
        rdfs:comment  "Chinese size system for wearables." ;
        rdfs:label    "WearableSizeSystemCN" .

sdo:EatAction  rdfs:comment  "The act of swallowing solid objects." ;
        rdfs:label    "EatAction" .

sdo:ConfirmAction  rdfs:comment  "The act of notifying someone that a future event/action is going to happen as expected.\\n\\nRelated actions:\\n\\n* [[CancelAction]]: The antonym of ConfirmAction." ;
        rdfs:label    "ConfirmAction" .

sdo:ProfilePage  rdfs:comment  "Web page type: Profile page." ;
        rdfs:label    "ProfilePage" .

sdo:drug  rdfs:comment  "Specifying a drug or medicine used in a medication procedure." ;
        rdfs:label    "drug" .

sdo:claimReviewed  rdfs:comment  "A short summary of the specific claims reviewed in a ClaimReview." ;
        rdfs:label    "claim reviewed" .

sdo:eligibleTransactionVolume
        rdfs:comment  "The transaction volume, in a monetary unit, for which the offer or price specification is valid, e.g. for indicating a minimal purchasing volume, to express free shipping above a certain order volume, or to limit the acceptance of credit cards to purchases to a certain minimal amount." ;
        rdfs:label    "eligible transactionVolume" .

sdo:paymentStatus  rdfs:comment  "The status of payment; whether the invoice has been paid or not." ;
        rdfs:label    "payment status" .

sdo:BodyOfWater  rdfs:comment  "A body of water, such as a sea, ocean, or lake." ;
        rdfs:label    "BodyOfWater" .

sdo:programType  rdfs:comment  "The type of educational or occupational program. For example, classroom, internship, alternance, etc.." ;
        rdfs:label    "program type" .

sdo:quarantineGuidelines
        rdfs:comment  "Guidelines about quarantine rules, e.g. in the context of a pandemic." ;
        rdfs:label    "quarantine guidelines" .

sdo:Volcano  rdfs:comment  "A volcano, like Fuji san." ;
        rdfs:label    "Volcano" .

sdo:OccupationalExperienceRequirements
        rdfs:comment  "Indicates employment-related experience requirements, e.g. [[monthsOfExperience]]." ;
        rdfs:label    "OccupationalExperienceRequirements" .

sdo:DrawAction  rdfs:comment  "The act of producing a visual/graphical representation of an object, typically with a pen/pencil and paper as instruments." ;
        rdfs:label    "DrawAction" .

sdo:MusculoskeletalExam
        rdfs:comment  "Musculoskeletal system clinical examination." ;
        rdfs:label    "MusculoskeletalExam" .

sdo:minValue  rdfs:comment  "The lower value of some characteristic or property." ;
        rdfs:label    "min value" .

sdo:OTC  rdfs:comment  "The character of a medical substance, typically a medicine, of being available over the counter or not." ;
        rdfs:label    "OTC" .

sdo:NewsArticle  rdfs:comment  "A NewsArticle is an article whose content reports news, or provides background context and supporting materials for understanding the news.\n\nA more detailed overview of [schema.org News markup](/docs/news.html) is also available.\n" ;
        rdfs:label    "NewsArticle" .

sdo:OccupationalTherapy
        rdfs:comment  "A treatment of people with physical, emotional, or social problems, using purposeful activity to help them overcome or learn to deal with their problems." ;
        rdfs:label    "OccupationalTherapy" .

sdo:arrivalGate  rdfs:comment  "Identifier of the flight's arrival gate." ;
        rdfs:label    "arrival gate" .

sdo:isSimilarTo  rdfs:comment  "A pointer to another, functionally similar product (or multiple products)." ;
        rdfs:label    "is similarTo" .

sdo:DiscussionForumPosting
        rdfs:comment  "A posting to a discussion forum." ;
        rdfs:label    "DiscussionForumPosting" .

sdo:archivedAt  rdfs:comment  "Indicates a page or other link involved in archival of a [[CreativeWork]]. In the case of [[MediaReview]], the items in a [[MediaReviewItem]] may often become inaccessible, but be archived by archival, journalistic, activist, or law enforcement organizations. In such cases, the referenced page may not directly publish the content." ;
        rdfs:label    "archived at" .

sdo:colleagues  rdfs:comment  "A colleague of the person." ;
        rdfs:label    "colleagues" .

sdo:webCheckinTime  rdfs:comment  "The time when a passenger can check into the flight online." ;
        rdfs:label    "web checkinTime" .

sdo:Longitudinal  rdfs:comment  "Unlike cross-sectional studies, longitudinal studies track the same people, and therefore the differences observed in those people are less likely to be the result of cultural differences across generations. Longitudinal studies are also used in medicine to uncover predictors of certain diseases." ;
        rdfs:label    "Longitudinal" .

sdo:Thing  rdfs:comment  "The most generic type of item." ;
        rdfs:label    "Thing" .

sdo:BroadcastService  rdfs:comment  "A delivery service through which content is provided via broadcast over the air or online." ;
        rdfs:label    "BroadcastService" .

sdo:SportsOrganization
        rdfs:comment  "Represents the collection of all sports organizations, including sports teams, governing bodies, and sports associations." ;
        rdfs:label    "SportsOrganization" .

sdo:costOrigin  rdfs:comment  "Additional details to capture the origin of the cost data. For example, 'Medicare Part B'." ;
        rdfs:label    "cost origin" .

sdo:alternateName  rdfs:comment  "An alias for the item." ;
        rdfs:label    "alternate name" .

sdo:additionalType  rdfs:comment  "An additional type for the item, typically used for adding more specific types from external vocabularies in microdata syntax. This is a relationship between something and a class that the thing is in. In RDFa syntax, it is better to use the native RDFa syntax - the 'typeof' attribute - for multiple types. Schema.org tools may have only weaker understanding of extra types, in particular those defined externally." ;
        rdfs:label    "additional type" .

sdo:recipe  rdfs:comment  "A sub property of instrument. The recipe/instructions used to perform the action." ;
        rdfs:label    "recipe" .

sdo:firstAppearance  rdfs:comment  "Indicates the first known occurence of a [[Claim]] in some [[CreativeWork]]." ;
        rdfs:label    "first appearance" .

sdo:PhotographAction  rdfs:comment  "The act of capturing still images of objects using a camera." ;
        rdfs:label    "PhotographAction" .

sdo:returnLabelSource
        rdfs:comment  "The method (from an enumeration) by which the customer obtains a return shipping label for a product returned for any reason." ;
        rdfs:label    "return labelSource" .

sdo:Code  rdfs:comment  "Computer programming source code. Example: Full (compile ready) solutions, code snippet samples, scripts, templates." ;
        rdfs:label    "Code" .

sdo:VisualArtsEvent  rdfs:comment  "Event type: Visual arts event." ;
        rdfs:label    "VisualArtsEvent" .

sdo:BodyMeasurementHead
        rdfs:comment  "Maximum girth of head above the ears. Used, for example, to fit hats." ;
        rdfs:label    "BodyMeasurementHead" .

sdo:benefitsSummaryUrl
        rdfs:comment  "The URL that goes directly to the summary of benefits and coverage for the specific standard plan or plan variation." ;
        rdfs:label    "benefits summaryUrl" .

sdo:healthPlanId  rdfs:comment  "The 14-character, HIOS-generated Plan ID number. (Plan IDs must be unique, even across different markets.)" ;
        rdfs:label    "health planId" .

sdo:petsAllowed  rdfs:comment  "Indicates whether pets are allowed to enter the accommodation or lodging business. More detailed information can be put in a text value." ;
        rdfs:label    "pets allowed" .

sdo:inker  rdfs:comment  "The individual who traces over the pencil drawings in ink after pencils are complete." ;
        rdfs:label    "inker" .

sdo:ItemListOrderAscending
        rdfs:comment  "An ItemList ordered with lower values listed first." ;
        rdfs:label    "ItemListOrderAscending" .

sdo:WearableSizeSystemEurope
        rdfs:comment  "European size system for wearables." ;
        rdfs:label    "WearableSizeSystemEurope" .

sdo:acquiredFrom  rdfs:comment  "The organization or person from which the product was acquired." ;
        rdfs:label    "acquired from" .

sdo:BioChemEntity  rdfs:comment  "Any biological, chemical, or biochemical thing. For example: a protein; a gene; a chemical; a synthetic chemical." ;
        rdfs:label    "BioChemEntity" .

sdo:GroceryStore  rdfs:comment  "A grocery store." ;
        rdfs:label    "GroceryStore" .

sdo:isResizable  rdfs:comment  "Whether the 3DModel allows resizing. For example, room layout applications often do not allow 3DModel elements to be resized to reflect reality." ;
        rdfs:label    "is resizable" .

sdo:author  rdfs:comment  "The author of this content or rating. Please note that author is special in that HTML 5 provides a special mechanism for indicating authorship via the rel tag. That is equivalent to this and may be used interchangeably." ;
        rdfs:label    "author" .

sdo:EUEnergyEfficiencyCategoryA3Plus
        rdfs:comment  "Represents EU Energy Efficiency Class A+++ as defined in EU energy labeling regulations." ;
        rdfs:label    "EUEnergyEfficiencyCategoryA3Plus" .

sdo:DataFeed  rdfs:comment  "A single feed providing structured information about one or more entities or topics." ;
        rdfs:label    "DataFeed" .

sdo:SRP  rdfs:comment  "Represents the suggested retail price (\"SRP\") of an offered product." ;
        rdfs:label    "SRP" .

sdo:negativeNotes  rdfs:comment  "Indicates, in the context of a [[Review]] (e.g. framed as 'pro' vs 'con' considerations), negative considerations - either as unstructured text, or a list." ;
        rdfs:label    "negative notes" .

sdo:evidenceLevel  rdfs:comment  "Strength of evidence of the data used to formulate the guideline (enumerated)." ;
        rdfs:label    "evidence level" .

sdo:TypeAndQuantityNode
        rdfs:comment  "A structured value indicating the quantity, unit of measurement, and business function of goods included in a bundle offer." ;
        rdfs:label    "TypeAndQuantityNode" .

sdo:WebSite  rdfs:comment  "A WebSite is a set of related web pages and other items typically served from a single web domain and accessible via URLs." ;
        rdfs:label    "WebSite" .

sdo:HinduDiet  rdfs:comment  "A diet conforming to Hindu dietary practices, in particular, beef-free." ;
        rdfs:label    "HinduDiet" .

sdo:makesOffer  rdfs:comment  "A pointer to products or services offered by the organization or person." ;
        rdfs:label    "makes offer" .

sdo:providerMobility  rdfs:comment  "Indicates the mobility of a provided service (e.g. 'static', 'dynamic')." ;
        rdfs:label    "provider mobility" .

sdo:Nonprofit501c12  rdfs:comment  "Nonprofit501c12: Non-profit type referring to Benevolent Life Insurance Associations, Mutual Ditch or Irrigation Companies, Mutual or Cooperative Telephone Companies." ;
        rdfs:label    "Nonprofit501c12" .

sdo:owns  rdfs:comment  "Products owned by the organization or person." ;
        rdfs:label    "owns" .

sdo:alcoholWarning  rdfs:comment  "Any precaution, guidance, contraindication, etc. related to consumption of alcohol while taking this drug." ;
        rdfs:label    "alcohol warning" .

sdo:countriesNotSupported
        rdfs:comment  "Countries for which the application is not supported. You can also provide the two-letter ISO 3166-1 alpha-2 country code." ;
        rdfs:label    "countries notSupported" .

sdo:lowPrice  rdfs:comment  "The lowest price of all offers available.\\n\\nUsage guidelines:\\n\\n* Use values from 0123456789 (Unicode 'DIGIT ZERO' (U+0030) to 'DIGIT NINE' (U+0039)) rather than superficially similiar Unicode symbols.\\n* Use '.' (Unicode 'FULL STOP' (U+002E)) rather than ',' to indicate a decimal point. Avoid using these symbols as a readability separator." ;
        rdfs:label    "low price" .

sdo:biologicalRole  rdfs:comment  "A role played by the BioChemEntity within a biological context." ;
        rdfs:label    "biological role" .

sdo:Gastroenterologic
        rdfs:comment  "A specific branch of medical science that pertains to diagnosis and treatment of disorders of digestive system." ;
        rdfs:label    "Gastroenterologic" .

sdo:TreatmentsHealthAspect
        rdfs:comment  "Treatments or related therapies for a Topic." ;
        rdfs:label    "TreatmentsHealthAspect" .

sdo:trainName  rdfs:comment  "The name of the train (e.g. The Orient Express)." ;
        rdfs:label    "train name" .

sdo:longitude  rdfs:comment  "The longitude of a location. For example ```-122.08585``` ([WGS 84](https://en.wikipedia.org/wiki/World_Geodetic_System))." ;
        rdfs:label    "longitude" .

sdo:NonprofitType  rdfs:comment  "NonprofitType enumerates several kinds of official non-profit types of which a non-profit organization can be." ;
        rdfs:label    "NonprofitType" .

sdo:letterer  rdfs:comment  "The individual who adds lettering, including speech balloons and sound effects, to artwork." ;
        rdfs:label    "letterer" .

sdo:totalPrice  rdfs:comment  "The total price for the reservation or ticket, including applicable taxes, shipping, etc.\\n\\nUsage guidelines:\\n\\n* Use values from 0123456789 (Unicode 'DIGIT ZERO' (U+0030) to 'DIGIT NINE' (U+0039)) rather than superficially similiar Unicode symbols.\\n* Use '.' (Unicode 'FULL STOP' (U+002E)) rather than ',' to indicate a decimal point. Avoid using these symbols as a readability separator." ;
        rdfs:label    "total price" .

sdo:contactPoints  rdfs:comment  "A contact point for a person or organization." ;
        rdfs:label    "contact points" .

sdo:hasVariant  rdfs:comment  "Indicates a [[Product]] that is a member of this [[ProductGroup]] (or [[ProductModel]])." ;
        rdfs:label    "has variant" .

sdo:NotYetRecruiting  rdfs:comment  "Not yet recruiting." ;
        rdfs:label    "NotYetRecruiting" .

sdo:foodWarning  rdfs:comment  "Any precaution, guidance, contraindication, etc. related to consumption of specific foods while taking this drug." ;
        rdfs:label    "food warning" .

sdo:JobPosting  rdfs:comment  "A listing that describes a job opening in a certain organization." ;
        rdfs:label    "JobPosting" .

sdo:participant  rdfs:comment  "Other co-agents that participated in the action indirectly. e.g. John wrote a book with *Steve*." ;
        rdfs:label    "participant" .

sdo:dataset  rdfs:comment  "A dataset contained in this catalog." ;
        rdfs:label    "dataset" .

sdo:RefurbishedCondition
        rdfs:comment  "Indicates that the item is refurbished." ;
        rdfs:label    "RefurbishedCondition" .

sdo:MedicalWebPage  rdfs:comment  "A web page that provides medical information." ;
        rdfs:label    "MedicalWebPage" .

sdo:PaymentService  rdfs:comment  "A Service to transfer funds from a person or organization to a beneficiary person or organization." ;
        rdfs:label    "PaymentService" .

sdo:MusicAlbumReleaseType
        rdfs:comment  "The kind of release which this album is: single, EP or album." ;
        rdfs:label    "MusicAlbumReleaseType" .

sdo:RearWheelDriveConfiguration
        rdfs:comment  "Real-wheel drive is a transmission layout where the engine drives the rear wheels." ;
        rdfs:label    "RearWheelDriveConfiguration" .

sdo:EUEnergyEfficiencyCategoryB
        rdfs:comment  "Represents EU Energy Efficiency Class B as defined in EU energy labeling regulations." ;
        rdfs:label    "EUEnergyEfficiencyCategoryB" .

sdo:DigitalAudioTapeFormat
        rdfs:comment  "DigitalAudioTapeFormat." ;
        rdfs:label    "DigitalAudioTapeFormat" .

sdo:gtin12  rdfs:comment  "The GTIN-12 code of the product, or the product to which the offer refers. The GTIN-12 is the 12-digit GS1 Identification Key composed of a U.P.C. Company Prefix, Item Reference, and Check Digit used to identify trade items. See [GS1 GTIN Summary](http://www.gs1.org/barcodes/technical/idkeys/gtin) for more details." ;
        rdfs:label    "gtin12" .

sdo:isrcCode  rdfs:comment  "The International Standard Recording Code for the recording." ;
        rdfs:label    "isrc code" .

sdo:ListenAction  rdfs:comment  "The act of consuming audio content." ;
        rdfs:label    "ListenAction" .

sdo:Mosque  rdfs:comment  "A mosque." ;
        rdfs:label    "Mosque" .

sdo:WearableSizeSystemGS1
        rdfs:comment  "GS1 (formerly NRF) size system for wearables." ;
        rdfs:label    "WearableSizeSystemGS1" .

sdo:SoundtrackAlbum  rdfs:comment  "SoundtrackAlbum." ;
        rdfs:label    "SoundtrackAlbum" .

sdo:Boolean  rdfs:comment  "Boolean: True or False." ;
        rdfs:label    "Boolean" .

sdo:healthPlanCoinsuranceOption
        rdfs:comment  "Whether the coinsurance applies before or after deductible, etc." ;
        rdfs:label    "health planCoinsuranceOption" .

sdo:currency  rdfs:comment  "The currency in which the monetary amount is expressed.\\n\\nUse standard formats: [ISO 4217 currency format](http://en.wikipedia.org/wiki/ISO_4217) e.g. \"USD\"; [Ticker symbol](https://en.wikipedia.org/wiki/List_of_cryptocurrencies) for cryptocurrencies e.g. \"BTC\"; well known names for [Local Exchange Tradings Systems](https://en.wikipedia.org/wiki/Local_exchange_trading_system) (LETS) and other currency types e.g. \"Ithaca HOUR\"." ;
        rdfs:label    "currency" .

sdo:MedicalEvidenceLevel
        rdfs:comment  "Level of evidence for a medical guideline. Enumerated type." ;
        rdfs:label    "MedicalEvidenceLevel" .

sdo:rangeIncludes  rdfs:comment  "Relates a property to a class that constitutes (one of) the expected type(s) for values of the property." ;
        rdfs:label    "range includes" .

sdo:penciler  rdfs:comment  "The individual who draws the primary narrative artwork." ;
        rdfs:label    "penciler" .

sdo:Invoice  rdfs:comment  "A statement of the money due for goods or services; a bill." ;
        rdfs:label    "Invoice" .

sdo:recordedAt  rdfs:comment  "The Event where the CreativeWork was recorded. The CreativeWork may capture all or part of the event." ;
        rdfs:label    "recorded at" .

sdo:OfflineTemporarily
        rdfs:comment  "Game server status: OfflineTemporarily. Server is offline now but it can be online soon." ;
        rdfs:label    "OfflineTemporarily" .

sdo:House  rdfs:comment  "A house is a building or structure that has the ability to be occupied for habitation by humans or other creatures (Source: Wikipedia, the free encyclopedia, see <a href=\"http://en.wikipedia.org/wiki/House\">http://en.wikipedia.org/wiki/House</a>)." ;
        rdfs:label    "House" .

sdo:LodgingReservation
        rdfs:comment  "A reservation for lodging at a hotel, motel, inn, etc.\\n\\nNote: This type is for information about actual reservations, e.g. in confirmation emails or HTML pages with individual confirmations of reservations." ;
        rdfs:label    "LodgingReservation" .

sdo:accessibilityHazard
        rdfs:comment  "A characteristic of the described resource that is physiologically dangerous to some users. Related to WCAG 2.0 guideline 2.3 ([WebSchemas wiki lists possible values](http://www.w3.org/wiki/WebSchemas/Accessibility))." ;
        rdfs:label    "accessibility hazard" .

sdo:interestRate  rdfs:comment  "The interest rate, charged or paid, applicable to the financial product. Note: This is different from the calculated annualPercentageRate." ;
        rdfs:label    "interest rate" .

sdo:nerve  rdfs:comment  "The underlying innervation associated with the muscle." ;
        rdfs:label    "nerve" .

sdo:possibleTreatment
        rdfs:comment  "A possible treatment to address this condition, sign or symptom." ;
        rdfs:label    "possible treatment" .

sdo:DateTime  rdfs:comment  "A combination of date and time of day in the form [-]CCYY-MM-DDThh:mm:ss[Z|(+|-)hh:mm] (see Chapter 5.4 of ISO 8601)." ;
        rdfs:label    "DateTime" .

sdo:cvdNumVent  rdfs:comment  "numvent - MECHANICAL VENTILATORS: Total number of ventilators available." ;
        rdfs:label    "cvd numVent" .

sdo:LiveAlbum  rdfs:comment  "LiveAlbum." ;
        rdfs:label    "LiveAlbum" .

sdo:PreventionHealthAspect
        rdfs:comment  "Information about actions or measures that can be taken to avoid getting the topic or reaching a critical situation related to the topic." ;
        rdfs:label    "PreventionHealthAspect" .

sdo:BasicIncome  rdfs:comment  "BasicIncome: this is a benefit for basic income." ;
        rdfs:label    "BasicIncome" .

sdo:MixedEventAttendanceMode
        rdfs:comment  "MixedEventAttendanceMode - an event that is conducted as a combination of both offline and online modes." ;
        rdfs:label    "MixedEventAttendanceMode" .

sdo:XPathType  rdfs:comment  "Text representing an XPath (typically but not necessarily version 1.0)." ;
        rdfs:label    "XPathType" .

sdo:ReturnShippingFees
        rdfs:comment  "Specifies that the customer must pay the return shipping costs when returning a product" ;
        rdfs:label    "ReturnShippingFees" .

sdo:touristType  rdfs:comment  "Attraction suitable for type(s) of tourist. eg. Children, visitors from a particular country, etc. " ;
        rdfs:label    "tourist type" .

sdo:DaySpa  rdfs:comment  "A day spa." ;
        rdfs:label    "DaySpa" .

sdo:Podiatric  rdfs:comment  "Podiatry is the care of the human foot, especially the diagnosis and treatment of foot disorders." ;
        rdfs:label    "Podiatric" .

sdo:Dentist  rdfs:comment  "A dentist." ;
        rdfs:label    "Dentist" .

sdo:legislationTransposes
        rdfs:comment  "Indicates that this legislation (or part of legislation) fulfills the objectives set by another legislation, by passing appropriate implementation measures. Typically, some legislations of European Union's member states or regions transpose European Directives. This indicates a legally binding link between the 2 legislations." ;
        rdfs:label    "legislation transposes" .

sdo:workHours  rdfs:comment  "The typical working hours for this job (e.g. 1st shift, night shift, 8am-5pm)." ;
        rdfs:label    "work hours" .

sdo:GiveAction  rdfs:comment  "The act of transferring ownership of an object to a destination. Reciprocal of TakeAction.\\n\\nRelated actions:\\n\\n* [[TakeAction]]: Reciprocal of GiveAction.\\n* [[SendAction]]: Unlike SendAction, GiveAction implies that ownership is being transferred (e.g. I may send my laptop to you, but that doesn't mean I'm giving it to you)." ;
        rdfs:label    "GiveAction" .

sdo:availableFrom  rdfs:comment  "When the item is available for pickup from the store, locker, etc." ;
        rdfs:label    "available from" .

sdo:MoveAction  rdfs:comment  "The act of an agent relocating to a place.\\n\\nRelated actions:\\n\\n* [[TransferAction]]: Unlike TransferAction, the subject of the move is a living Person or Organization rather than an inanimate object." ;
        rdfs:label    "MoveAction" .

sdo:WearableSizeSystemDE
        rdfs:comment  "German size system for wearables." ;
        rdfs:label    "WearableSizeSystemDE" .

sdo:endorsee  rdfs:comment  "A sub property of participant. The person/organization being supported." ;
        rdfs:label    "endorsee" .

sdo:awards  rdfs:comment  "Awards won by or for this item." ;
        rdfs:label    "awards" .

sdo:copyrightNotice  rdfs:comment  "Text of a notice appropriate for describing the copyright aspects of this Creative Work, ideally indicating the owner of the copyright for the Work." ;
        rdfs:label    "copyright notice" .

sdo:endTime  rdfs:comment  "The endTime of something. For a reserved event or service (e.g. FoodEstablishmentReservation), the time that it is expected to end. For actions that span a period of time, when the action was performed. e.g. John wrote a book from January to *December*. For media, including audio and video, it's the time offset of the end of a clip within a larger file.\\n\\nNote that Event uses startDate/endDate instead of startTime/endTime, even when describing dates with times. This situation may be clarified in future revisions." ;
        rdfs:label    "end time" .

sdo:HairSalon  rdfs:comment  "A hair salon." ;
        rdfs:label    "HairSalon" .

sdo:sugarContent  rdfs:comment  "The number of grams of sugar." ;
        rdfs:label    "sugar content" .

sdo:programmingModel  rdfs:comment  "Indicates whether API is managed or unmanaged." ;
        rdfs:label    "programming model" .

sdo:MediaReview  rdfs:comment  "A [[MediaReview]] is a more specialized form of Review dedicated to the evaluation of media content online, typically in the context of fact-checking and misinformation.\n    For more general reviews of media in the broader sense, use [[UserReview]], [[CriticReview]] or other [[Review]] types. This definition is\n    a work in progress. While the [[MediaManipulationRatingEnumeration]] list reflects significant community review amongst fact-checkers and others working\n    to combat misinformation, the specific structures for representing media objects, their versions and publication context, is still evolving. Similarly, best practices for the relationship between [[MediaReview]] and [[ClaimReview]] markup has not yet been finalized." ;
        rdfs:label    "MediaReview" .

sdo:pattern  rdfs:comment  "A pattern that something has, for example 'polka dot', 'striped', 'Canadian flag'. Values are typically expressed as text, although links to controlled value schemes are also supported." ;
        rdfs:label    "pattern" .

sdo:namedPosition  rdfs:comment  "A position played, performed or filled by a person or organization, as part of an organization. For example, an athlete in a SportsTeam might play in the position named 'Quarterback'." ;
        rdfs:label    "named position" .

sdo:ActionAccessSpecification
        rdfs:comment  "A set of requirements that a must be fulfilled in order to perform an Action." ;
        rdfs:label    "ActionAccessSpecification" .

sdo:attendee  rdfs:comment  "A person or organization attending the event." ;
        rdfs:label    "attendee" .

sdo:benefits  rdfs:comment  "Description of benefits associated with the job." ;
        rdfs:label    "benefits" .

sdo:TravelAgency  rdfs:comment  "A travel agency." ;
        rdfs:label    "TravelAgency" .

sdo:SportsEvent  rdfs:comment  "Event type: Sports event." ;
        rdfs:label    "SportsEvent" .

sdo:accessCode  rdfs:comment  "Password, PIN, or access code needed for delivery (e.g. from a locker)." ;
        rdfs:label    "access code" .

sdo:Artery  rdfs:comment  "A type of blood vessel that specifically carries blood away from the heart." ;
        rdfs:label    "Artery" .

sdo:priceValidUntil  rdfs:comment  "The date after which the price is no longer available." ;
        rdfs:label    "price validUntil" .

sdo:hasDriveThroughService
        rdfs:comment  "Indicates whether some facility (e.g. [[FoodEstablishment]], [[CovidTestingFacility]]) offers a service that can be used by driving through in a car. In the case of [[CovidTestingFacility]] such facilities could potentially help with social distancing from other potentially-infected users." ;
        rdfs:label    "has driveThroughService" .

sdo:UserTweets  rdfs:comment  "UserInteraction and its subtypes is an old way of talking about users interacting with pages. It is generally better to use [[Action]]-based vocabulary, alongside types such as [[Comment]]." ;
        rdfs:label    "UserTweets" .

sdo:Zoo  rdfs:comment  "A zoo." ;
        rdfs:label    "Zoo" .

sdo:commentCount  rdfs:comment  "The number of comments this CreativeWork (e.g. Article, Question or Answer) has received. This is most applicable to works published in Web sites with commenting system; additional comments may exist elsewhere." ;
        rdfs:label    "comment count" .

sdo:coursePrerequisites
        rdfs:comment  "Requirements for taking the Course. May be completion of another [[Course]] or a textual description like \"permission of instructor\". Requirements may be a pre-requisite competency, referenced using [[AlignmentObject]]." ;
        rdfs:label    "course prerequisites" .

sdo:duringMedia  rdfs:comment  "A media object representing the circumstances while performing this direction." ;
        rdfs:label    "during media" .

sdo:openingHoursSpecification
        rdfs:comment  "The opening hours of a certain place." ;
        rdfs:label    "opening hoursSpecification" .

sdo:targetPlatform  rdfs:comment  "Type of app development: phone, Metro style, desktop, XBox, etc." ;
        rdfs:label    "target platform" .

sdo:bioChemInteraction
        rdfs:comment  "A BioChemEntity that is known to interact with this item." ;
        rdfs:label    "bio chemInteraction" .

sdo:employee  rdfs:comment  "Someone working for this organization." ;
        rdfs:label    "employee" .

sdo:issuedThrough  rdfs:comment  "The service through with the permit was granted." ;
        rdfs:label    "issued through" .

sdo:aspect  rdfs:comment  "An aspect of medical practice that is considered on the page, such as 'diagnosis', 'treatment', 'causes', 'prognosis', 'etiology', 'epidemiology', etc." ;
        rdfs:label    "aspect" .

sdo:MedicalTherapy  rdfs:comment  "Any medical intervention designed to prevent, treat, and cure human diseases and medical conditions, including both curative and palliative therapies. Medical therapies are typically processes of care relying upon pharmacotherapy, behavioral therapy, supportive therapy (with fluid or nutrition for example), or detoxification (e.g. hemodialysis) aimed at improving or preventing a health condition." ;
        rdfs:label    "MedicalTherapy" .

sdo:addressCountry  rdfs:comment  "The country. For example, USA. You can also provide the two-letter [ISO 3166-1 alpha-2 country code](http://en.wikipedia.org/wiki/ISO_3166-1)." ;
        rdfs:label    "address country" .

sdo:PlaceboControlledTrial
        rdfs:comment  "A placebo-controlled trial design." ;
        rdfs:label    "PlaceboControlledTrial" .

sdo:NightClub  rdfs:comment  "A nightclub or discotheque." ;
        rdfs:label    "NightClub" .

sdo:isAcceptingNewPatients
        rdfs:comment  "Whether the provider is accepting new patients." ;
        rdfs:label    "is acceptingNewPatients" .

sdo:ReturnAction  rdfs:comment  "The act of returning to the origin that which was previously received (concrete objects) or taken (ownership)." ;
        rdfs:label    "ReturnAction" .

sdo:ScholarlyArticle  rdfs:comment  "A scholarly article." ;
        rdfs:label    "ScholarlyArticle" .

sdo:Neurologic  rdfs:comment  "A specific branch of medical science that studies the nerves and nervous system and its respective disease states." ;
        rdfs:label    "Neurologic" .

sdo:Nonprofit501e  rdfs:comment  "Nonprofit501e: Non-profit type referring to Cooperative Hospital Service Organizations." ;
        rdfs:label    "Nonprofit501e" .

sdo:cvdNumBeds  rdfs:comment  "numbeds - HOSPITAL INPATIENT BEDS: Inpatient beds, including all staffed, licensed, and overflow (surge) beds used for inpatients." ;
        rdfs:label    "cvd numBeds" .

sdo:educationalLevel  rdfs:comment  "The level in terms of progression through an educational or training context. Examples of educational levels include 'beginner', 'intermediate' or 'advanced', and formal sets of level indicators." ;
        rdfs:label    "educational level" .

sdo:InsuranceAgency  rdfs:comment  "An Insurance agency." ;
        rdfs:label    "InsuranceAgency" .

sdo:ReactAction  rdfs:comment  "The act of responding instinctively and emotionally to an object, expressing a sentiment." ;
        rdfs:label    "ReactAction" .

sdo:Menu  rdfs:comment  "A structured representation of food or drink items available from a FoodEstablishment." ;
        rdfs:label    "Menu" .

sdo:processorRequirements
        rdfs:comment  "Processor architecture required to run the application (e.g. IA64)." ;
        rdfs:label    "processor requirements" .

sdo:ticketedSeat  rdfs:comment  "The seat associated with the ticket." ;
        rdfs:label    "ticketed seat" .

sdo:EditedOrCroppedContent
        rdfs:comment  "Content coded 'edited or cropped content' in a [[MediaReview]], considered in the context of how it was published or shared.\n\nFor a [[VideoObject]] to be 'edited or cropped content': The video has been edited or rearranged. This category applies to time edits, including editing multiple videos together to alter the story being told or editing out large portions from a video.\n\nFor an [[ImageObject]] to be 'edited or cropped content': Presenting a part of an image from a larger whole to mislead the viewer.\n\nFor an [[ImageObject]] with embedded text to be 'edited or cropped content': Presenting a part of an image from a larger whole to mislead the viewer.\n\nFor an [[AudioObject]] to be 'edited or cropped content': The audio has been edited or rearranged. This category applies to time edits, including editing multiple audio clips together to alter the story being told or editing out large portions from the recording.\n" ;
        rdfs:label    "EditedOrCroppedContent" .

sdo:MedicalIntangible
        rdfs:comment  "A utility class that serves as the umbrella for a number of 'intangible' things in the medical space." ;
        rdfs:label    "MedicalIntangible" .

sdo:InternetCafe  rdfs:comment  "An internet cafe." ;
        rdfs:label    "InternetCafe" .

sdo:FoodService  rdfs:comment  "A food service, like breakfast, lunch, or dinner." ;
        rdfs:label    "FoodService" .

sdo:businessDays  rdfs:comment  "Days of the week when the merchant typically operates, indicated via opening hours markup." ;
        rdfs:label    "business days" .

sdo:VeganDiet  rdfs:comment  "A diet exclusive of all animal products." ;
        rdfs:label    "VeganDiet" .

sdo:healthPlanCostSharing
        rdfs:comment  "Whether The costs to the patient for services under this network or formulary." ;
        rdfs:label    "health planCostSharing" .

sdo:deathDate  rdfs:comment  "Date of death." ;
        rdfs:label    "death date" .

sdo:Place  rdfs:comment  "Entities that have a somewhat fixed, physical extension." ;
        rdfs:label    "Place" .

sdo:birthDate  rdfs:comment  "Date of birth." ;
        rdfs:label    "birth date" .

sdo:Chapter  rdfs:comment  "One of the sections into which a book is divided. A chapter usually has a section number or a name." ;
        rdfs:label    "Chapter" .

sdo:MedicalDevice  rdfs:comment  "Any object used in a medical capacity, such as to diagnose or treat a patient." ;
        rdfs:label    "MedicalDevice" .

sdo:merchantReturnDays
        rdfs:comment  "Specifies either a fixed return date or the number of days (from the delivery date) that a product can be returned. Used when the [[returnPolicyCategory]] property is specified as [[MerchantReturnFiniteReturnWindow]]." ;
        rdfs:label    "merchant returnDays" .

sdo:messageAttachment
        rdfs:comment  "A CreativeWork attached to the message." ;
        rdfs:label    "message attachment" .

sdo:AggregateOffer  rdfs:comment  "When a single product is associated with multiple offers (for example, the same pair of shoes is offered by different merchants), then AggregateOffer can be used.\\n\\nNote: AggregateOffers are normally expected to associate multiple offers that all share the same defined [[businessFunction]] value, or default to http://purl.org/goodrelations/v1#Sell if businessFunction is not explicitly defined." ;
        rdfs:label    "AggregateOffer" .

sdo:Nonprofit501c6  rdfs:comment  "Nonprofit501c6: Non-profit type referring to Business Leagues, Chambers of Commerce, Real Estate Boards." ;
        rdfs:label    "Nonprofit501c6" .

sdo:Trip  rdfs:comment  "A trip or journey. An itinerary of visits to one or more places." ;
        rdfs:label    "Trip" .

sdo:ShoeStore  rdfs:comment  "A shoe store." ;
        rdfs:label    "ShoeStore" .

sdo:parentOrganization
        rdfs:comment  "The larger organization that this organization is a [[subOrganization]] of, if any." ;
        rdfs:label    "parent organization" .

sdo:musicArrangement  rdfs:comment  "An arrangement derived from the composition." ;
        rdfs:label    "music arrangement" .

sdo:restockingFee  rdfs:comment  "Use [[MonetaryAmount]] to specify a fixed restocking fee for product returns, or use [[Number]] to specify a percentage of the product price paid by the customer." ;
        rdfs:label    "restocking fee" .

sdo:fileFormat  rdfs:comment  "Media type, typically MIME format (see [IANA site](http://www.iana.org/assignments/media-types/media-types.xhtml)) of the content e.g. application/zip of a SoftwareApplication binary. In cases where a CreativeWork has several media type representations, 'encoding' can be used to indicate each MediaObject alongside particular fileFormat information. Unregistered or niche file formats can be indicated instead via the most appropriate URL, e.g. defining Web page or a Wikipedia entry." ;
        rdfs:label    "file format" .

sdo:isRelatedTo  rdfs:comment  "A pointer to another, somehow related product (or multiple products)." ;
        rdfs:label    "is relatedTo" .

sdo:EnrollingByInvitation
        rdfs:comment  "Enrolling participants by invitation only." ;
        rdfs:label    "EnrollingByInvitation" .

sdo:taxID  rdfs:comment  "The Tax / Fiscal ID of the organization or person, e.g. the TIN in the US or the CIF/NIF in Spain." ;
        rdfs:label    "tax id" .

sdo:publisher  rdfs:comment  "The publisher of the creative work." ;
        rdfs:label    "publisher" .

sdo:partOfSystem  rdfs:comment  "The anatomical or organ system that this structure is part of." ;
        rdfs:label    "part ofSystem" .

sdo:tributary  rdfs:comment  "The anatomical or organ system that the vein flows into; a larger structure that the vein connects to." ;
        rdfs:label    "tributary" .

sdo:contentReferenceTime
        rdfs:comment  "The specific time described by a creative work, for works (e.g. articles, video objects etc.) that emphasise a particular moment within an Event." ;
        rdfs:label    "content referenceTime" .

sdo:GenderType  rdfs:comment  "An enumeration of genders." ;
        rdfs:label    "GenderType" .

sdo:Product  rdfs:comment  "Any offered product or service. For example: a pair of shoes; a concert ticket; the rental of a car; a haircut; or an episode of a TV show streamed online." ;
        rdfs:label    "Product" .

sdo:DonateAction  rdfs:comment  "The act of providing goods, services, or money without compensation, often for philanthropic reasons." ;
        rdfs:label    "DonateAction" .

sdo:loanTerm  rdfs:comment  "The duration of the loan or credit agreement." ;
        rdfs:label    "loan term" .

sdo:deliveryAddress  rdfs:comment  "Destination address." ;
        rdfs:label    "delivery address" .

sdo:transitTimeLabel  rdfs:comment  "Label to match an [[OfferShippingDetails]] with a [[DeliveryTimeSettings]] (within the context of a [[shippingSettingsLink]] cross-reference)." ;
        rdfs:label    "transit timeLabel" .

sdo:JoinAction  rdfs:comment  "An agent joins an event/group with participants/friends at a location.\\n\\nRelated actions:\\n\\n* [[RegisterAction]]: Unlike RegisterAction, JoinAction refers to joining a group/team of people.\\n* [[SubscribeAction]]: Unlike SubscribeAction, JoinAction does not imply that you'll be receiving updates.\\n* [[FollowAction]]: Unlike FollowAction, JoinAction does not imply that you'll be polling for updates." ;
        rdfs:label    "JoinAction" .

sdo:RefundTypeEnumeration
        rdfs:comment  "Enumerates several kinds of product return refund types." ;
        rdfs:label    "RefundTypeEnumeration" .

sdo:DiscoverAction  rdfs:comment  "The act of discovering/finding an object." ;
        rdfs:label    "DiscoverAction" .

sdo:MonetaryAmount  rdfs:comment  "A monetary value or range. This type can be used to describe an amount of money such as $50 USD, or a range as in describing a bank account being suitable for a balance between £1,000 and £1,000,000 GBP, or the value of a salary, etc. It is recommended to use [[PriceSpecification]] Types to describe the price of an Offer, Invoice, etc." ;
        rdfs:label    "MonetaryAmount" .

sdo:infectiousAgent  rdfs:comment  "The actual infectious agent, such as a specific bacterium." ;
        rdfs:label    "infectious agent" .

sdo:TravelAction  rdfs:comment  "The act of traveling from an fromLocation to a destination by a specified mode of transport, optionally with participants." ;
        rdfs:label    "TravelAction" .

sdo:GovernmentOffice  rdfs:comment  "A government office&#x2014;for example, an IRS or DMV office." ;
        rdfs:label    "GovernmentOffice" .

sdo:GeoCoordinates  rdfs:comment  "The geographic coordinates of a place or event." ;
        rdfs:label    "GeoCoordinates" .

sdo:AutomotiveBusiness
        rdfs:comment  "Car repair, sales, or parts." ;
        rdfs:label    "AutomotiveBusiness" .

sdo:DigitalFormat  rdfs:comment  "DigitalFormat." ;
        rdfs:label    "DigitalFormat" .

sdo:HowToTool  rdfs:comment  "A tool used (but not consumed) when performing instructions for how to achieve a result." ;
        rdfs:label    "HowToTool" .

sdo:hasPart  rdfs:comment  "Indicates an item or CreativeWork that is part of this item, or CreativeWork (in some sense)." ;
        rdfs:label    "has part" .

sdo:businessFunction  rdfs:comment  "The business function (e.g. sell, lease, repair, dispose) of the offer or component of a bundle (TypeAndQuantityNode). The default is http://purl.org/goodrelations/v1#Sell." ;
        rdfs:label    "business function" .

sdo:copyrightHolder  rdfs:comment  "The party holding the legal copyright to the CreativeWork." ;
        rdfs:label    "copyright holder" .

sdo:preOp  rdfs:comment  "A description of the workup, testing, and other preparations required before implanting this device." ;
        rdfs:label    "pre op" .

sdo:netWorth  rdfs:comment  "The total financial value of the person as calculated by subtracting assets from liabilities." ;
        rdfs:label    "net worth" .

sdo:itemOffered  rdfs:comment  "An item being offered (or demanded). The transactional nature of the offer or demand is documented using [[businessFunction]], e.g. sell, lease etc. While several common expected types are listed explicitly in this definition, others can be used. Using a second type, such as Product or a subtype of Product, can clarify the nature of the offer." ;
        rdfs:label    "item offered" .

sdo:PerformAction  rdfs:comment  "The act of participating in performance arts." ;
        rdfs:label    "PerformAction" .

sdo:availableService  rdfs:comment  "A medical service available from this provider." ;
        rdfs:label    "available service" .

sdo:associatedPathophysiology
        rdfs:comment  "If applicable, a description of the pathophysiology associated with the anatomical system, including potential abnormal changes in the mechanical, physical, and biochemical functions of the system." ;
        rdfs:label    "associated pathophysiology" .

sdo:ScreeningHealthAspect
        rdfs:comment  "Content about how to screen or further filter a topic." ;
        rdfs:label    "ScreeningHealthAspect" .

sdo:nsn  rdfs:comment  "Indicates the [NATO stock number](https://en.wikipedia.org/wiki/NATO_Stock_Number) (nsn) of a [[Product]]. " ;
        rdfs:label    "nsn" .

sdo:salaryCurrency  rdfs:comment  "The currency (coded using [ISO 4217](http://en.wikipedia.org/wiki/ISO_4217) ) used for the main salary information in this job posting or for this employee." ;
        rdfs:label    "salary currency" .

sdo:broadcastTimezone
        rdfs:comment  "The timezone in [ISO 8601 format](http://en.wikipedia.org/wiki/ISO_8601) for which the service bases its broadcasts" ;
        rdfs:label    "broadcast timezone" .

sdo:AgreeAction  rdfs:comment  "The act of expressing a consistency of opinion with the object. An agent agrees to/about an object (a proposition, topic or theme) with participants." ;
        rdfs:label    "AgreeAction" .

sdo:Seat  rdfs:comment  "Used to describe a seat, such as a reserved seat in an event reservation." ;
        rdfs:label    "Seat" .

sdo:EmployerAggregateRating
        rdfs:comment  "An aggregate rating of an Organization related to its role as an employer." ;
        rdfs:label    "EmployerAggregateRating" .

sdo:DigitalDocument  rdfs:comment  "An electronic file or document." ;
        rdfs:label    "DigitalDocument" .

sdo:occupationLocation
        rdfs:comment  " The region/country for which this occupational description is appropriate. Note that educational requirements and qualifications can vary between jurisdictions." ;
        rdfs:label    "occupation location" .

sdo:BedAndBreakfast  rdfs:comment  "Bed and breakfast.\n<br /><br />\nSee also the <a href=\"/docs/hotels.html\">dedicated document on the use of schema.org for marking up hotels and other forms of accommodations</a>.\n" ;
        rdfs:label    "BedAndBreakfast" .

sdo:acceptedAnswer  rdfs:comment  "The answer(s) that has been accepted as best, typically on a Question/Answer site. Sites vary in their selection mechanisms, e.g. drawing on community opinion and/or the view of the Question author." ;
        rdfs:label    "accepted answer" .

sdo:subReservation  rdfs:comment  "The individual reservations included in the package. Typically a repeated property." ;
        rdfs:label    "sub reservation" .

sdo:experienceInPlaceOfEducation
        rdfs:comment  "Indicates whether a [[JobPosting]] will accept experience (as indicated by [[OccupationalExperienceRequirements]]) in place of its formal educational qualifications (as indicated by [[educationRequirements]]). If true, indicates that satisfying one of these requirements is sufficient." ;
        rdfs:label    "experience inPlaceOfEducation" .

sdo:Number  rdfs:comment  "Data type: Number.\\n\\nUsage guidelines:\\n\\n* Use values from 0123456789 (Unicode 'DIGIT ZERO' (U+0030) to 'DIGIT NINE' (U+0039)) rather than superficially similiar Unicode symbols.\\n* Use '.' (Unicode 'FULL STOP' (U+002E)) rather than ',' to indicate a decimal point. Avoid using these symbols as a readability separator." ;
        rdfs:label    "Number" .

sdo:ComicStory  rdfs:comment  "The term \"story\" is any indivisible, re-printable\n    \tunit of a comic, including the interior stories, covers, and backmatter. Most\n    \tcomics have at least two stories: a cover (ComicCoverArt) and an interior story." ;
        rdfs:label    "ComicStory" .

sdo:WesternConventional
        rdfs:comment  "The conventional Western system of medicine, that aims to apply the best available evidence gained from the scientific method to clinical decision making. Also known as conventional or Western medicine." ;
        rdfs:label    "WesternConventional" .

sdo:Nonprofit501c10  rdfs:comment  "Nonprofit501c10: Non-profit type referring to Domestic Fraternal Societies and Associations." ;
        rdfs:label    "Nonprofit501c10" .

sdo:ActiveNotRecruiting
        rdfs:comment  "Active, but not recruiting new participants." ;
        rdfs:label    "ActiveNotRecruiting" .

sdo:taxonomicRange  rdfs:comment  "The taxonomic grouping of the organism that expresses, encodes, or in someway related to the BioChemEntity." ;
        rdfs:label    "taxonomic range" .

sdo:UserPlays  rdfs:comment  "UserInteraction and its subtypes is an old way of talking about users interacting with pages. It is generally better to use [[Action]]-based vocabulary, alongside types such as [[Comment]]." ;
        rdfs:label    "UserPlays" .

sdo:TelevisionChannel
        rdfs:comment  "A unique instance of a television BroadcastService on a CableOrSatelliteService lineup." ;
        rdfs:label    "TelevisionChannel" .

sdo:roofLoad  rdfs:comment  "The permitted total weight of cargo and installations (e.g. a roof rack) on top of the vehicle.\\n\\nTypical unit code(s): KGM for kilogram, LBR for pound\\n\\n* Note 1: You can indicate additional information in the [[name]] of the [[QuantitativeValue]] node.\\n* Note 2: You may also link to a [[QualitativeValue]] node that provides additional information using [[valueReference]]\\n* Note 3: Note that you can use [[minValue]] and [[maxValue]] to indicate ranges." ;
        rdfs:label    "roof load" .

sdo:Energy  rdfs:comment  "Properties that take Energy as values are of the form '&lt;Number&gt; &lt;Energy unit of measure&gt;'." ;
        rdfs:label    "Energy" .

sdo:SoftwareApplication
        rdfs:comment  "A software application." ;
        rdfs:label    "SoftwareApplication" .

sdo:seasons  rdfs:comment  "A season in a media series." ;
        rdfs:label    "seasons" .

sdo:Resort  rdfs:comment  "A resort is a place used for relaxation or recreation, attracting visitors for holidays or vacations. Resorts are places, towns or sometimes commercial establishment operated by a single company (Source: Wikipedia, the free encyclopedia, see <a href=\"http://en.wikipedia.org/wiki/Resort\">http://en.wikipedia.org/wiki/Resort</a>).\n<br /><br />\nSee also the <a href=\"/docs/hotels.html\">dedicated document on the use of schema.org for marking up hotels and other forms of accommodations</a>.\n    " ;
        rdfs:label    "Resort" .

sdo:includedRiskFactor
        rdfs:comment  "A modifiable or non-modifiable risk factor included in the calculation, e.g. age, coexisting condition." ;
        rdfs:label    "included riskFactor" .

sdo:EvidenceLevelC  rdfs:comment  "Only consensus opinion of experts, case studies, or standard-of-care." ;
        rdfs:label    "EvidenceLevelC" .

sdo:availableChannel  rdfs:comment  "A means of accessing the service (e.g. a phone bank, a web site, a location, etc.)." ;
        rdfs:label    "available channel" .

sdo:Campground  rdfs:comment  "A camping site, campsite, or [[Campground]] is a place used for overnight stay in the outdoors, typically containing individual [[CampingPitch]] locations. \\n\\n\nIn British English a campsite is an area, usually divided into a number of pitches, where people can camp overnight using tents or camper vans or caravans; this British English use of the word is synonymous with the American English expression campground. In American English the term campsite generally means an area where an individual, family, group, or military unit can pitch a tent or park a camper; a campground may contain many campsites (Source: Wikipedia see [https://en.wikipedia.org/wiki/Campsite](https://en.wikipedia.org/wiki/Campsite)).\\n\\n\n\nSee also the dedicated [document on the use of schema.org for marking up hotels and other forms of accommodations](/docs/hotels.html).\n" ;
        rdfs:label    "Campground" .

sdo:sourceOrganization
        rdfs:comment  "The Organization on whose behalf the creator was working." ;
        rdfs:label    "source organization" .

sdo:Attorney  rdfs:comment  "Professional service: Attorney. \\n\\nThis type is deprecated - [[LegalService]] is more inclusive and less ambiguous." ;
        rdfs:label    "Attorney" .

sdo:yearlyRevenue  rdfs:comment  "The size of the business in annual revenue." ;
        rdfs:label    "yearly revenue" .

sdo:broadcastChannelId
        rdfs:comment  "The unique address by which the BroadcastService can be identified in a provider lineup. In US, this is typically a number." ;
        rdfs:label    "broadcast channelId" .

sdo:APIReference  rdfs:comment  "Reference documentation for application programming interfaces (APIs)." ;
        rdfs:label    "APIReference" .

sdo:cvdCollectionDate
        rdfs:comment  "collectiondate - Date for which patient counts are reported." ;
        rdfs:label    "cvd collectionDate" .

sdo:calories  rdfs:comment  "The number of calories." ;
        rdfs:label    "calories" .

sdo:disambiguatingDescription
        rdfs:comment  "A sub property of description. A short description of the item used to disambiguate from other, similar items. Information from other properties (in particular, name) may be necessary for the description to be useful for disambiguation." ;
        rdfs:label    "disambiguating description" .

sdo:3DModel  rdfs:comment  "A 3D model represents some kind of 3D content, which may have [[encoding]]s in one or more [[MediaObject]]s. Many 3D formats are available (e.g. see [Wikipedia](https://en.wikipedia.org/wiki/Category:3D_graphics_file_formats)); specific encoding formats can be represented using the [[encodingFormat]] property applied to the relevant [[MediaObject]]. For the\ncase of a single file published after Zip compression, the convention of appending '+zip' to the [[encodingFormat]] can be used. Geospatial, AR/VR, artistic/animation, gaming, engineering and scientific content can all be represented using [[3DModel]]." ;
        rdfs:label    "3DModel" .

sdo:HowToSection  rdfs:comment  "A sub-grouping of steps in the instructions for how to achieve a result (e.g. steps for making a pie crust within a pie recipe)." ;
        rdfs:label    "HowToSection" .

sdo:liveBlogUpdate  rdfs:comment  "An update to the LiveBlog." ;
        rdfs:label    "live blogUpdate" .

sdo:isBasedOn  rdfs:comment  "A resource from which this work is derived or from which it is a modification or adaption." ;
        rdfs:label    "is basedOn" .

sdo:playMode  rdfs:comment  "Indicates whether this game is multi-player, co-op or single-player.  The game can be marked as multi-player, co-op and single-player at the same time." ;
        rdfs:label    "play mode" .

sdo:inPlaylist  rdfs:comment  "The playlist to which this recording belongs." ;
        rdfs:label    "in playlist" .

sdo:QAPage  rdfs:comment  "A QAPage is a WebPage focussed on a specific Question and its Answer(s), e.g. in a question answering site or documenting Frequently Asked Questions (FAQs)." ;
        rdfs:label    "QAPage" .

sdo:Quiz  rdfs:comment  "Quiz: A test of knowledge, skills and abilities." ;
        rdfs:label    "Quiz" .

sdo:actionOption  rdfs:comment  "A sub property of object. The options subject to this action." ;
        rdfs:label    "action option" .

sdo:TaxiVehicleUsage  rdfs:comment  "Indicates the usage of the car as a taxi." ;
        rdfs:label    "TaxiVehicleUsage" .

sdo:accountOverdraftLimit
        rdfs:comment  "An overdraft is an extension of credit from a lending institution when an account reaches zero. An overdraft allows the individual to continue withdrawing money even if the account has no funds in it. Basically the bank allows people to borrow a set amount of money." ;
        rdfs:label    "account overdraftLimit" .

sdo:MusicGroup  rdfs:comment  "A musical group, such as a band, an orchestra, or a choir. Can also be a solo musician." ;
        rdfs:label    "MusicGroup" .

sdo:fuelType  rdfs:comment  "The type of fuel suitable for the engine or engines of the vehicle. If the vehicle has only one engine, this property can be attached directly to the vehicle." ;
        rdfs:label    "fuel type" .

sdo:ProfessionalService
        rdfs:comment  "Original definition: \"provider of professional services.\"\\n\\nThe general [[ProfessionalService]] type for local businesses was deprecated due to confusion with [[Service]]. For reference, the types that it included were: [[Dentist]],\n        [[AccountingService]], [[Attorney]], [[Notary]], as well as types for several kinds of [[HomeAndConstructionBusiness]]: [[Electrician]], [[GeneralContractor]],\n        [[HousePainter]], [[Locksmith]], [[Plumber]], [[RoofingContractor]]. [[LegalService]] was introduced as a more inclusive supertype of [[Attorney]]." ;
        rdfs:label    "ProfessionalService" .

sdo:geoMidpoint  rdfs:comment  "Indicates the GeoCoordinates at the centre of a GeoShape e.g. GeoCircle." ;
        rdfs:label    "geo midpoint" .

sdo:AuthorizeAction  rdfs:comment  "The act of granting permission to an object." ;
        rdfs:label    "AuthorizeAction" .

sdo:agent  rdfs:comment  "The direct performer or driver of the action (animate or inanimate). e.g. *John* wrote a book." ;
        rdfs:label    "agent" .

sdo:assesses  rdfs:comment  "The item being described is intended to assess the competency or learning outcome defined by the referenced term." ;
        rdfs:label    "assesses" .

sdo:estimatesRiskOf  rdfs:comment  "The condition, complication, or symptom whose risk is being estimated." ;
        rdfs:label    "estimates riskOf" .

sdo:honorificPrefix  rdfs:comment  "An honorific prefix preceding a Person's name such as Dr/Mrs/Mr." ;
        rdfs:label    "honorific prefix" .

sdo:employmentUnit  rdfs:comment  "Indicates the department, unit and/or facility where the employee reports and/or in which the job is to be performed." ;
        rdfs:label    "employment unit" .

sdo:Movie  rdfs:comment  "A movie." ;
        rdfs:label    "Movie" .

sdo:repeatCount  rdfs:comment  "Defines the number of times a recurring [[Event]] will take place" ;
        rdfs:label    "repeat count" .

sdo:MonetaryGrant  rdfs:comment  "A monetary grant." ;
        rdfs:label    "MonetaryGrant" .

sdo:LoanOrCredit  rdfs:comment  "A financial product for the loaning of an amount of money, or line of credit, under agreed terms and charges." ;
        rdfs:label    "LoanOrCredit" .

sdo:energyEfficiencyScaleMin
        rdfs:comment  "Specifies the least energy efficient class on the regulated EU energy consumption scale for the product category a product belongs to. For example, energy consumption for televisions placed on the market after January 1, 2020 is scaled from D to A+++." ;
        rdfs:label    "energy efficiencyScaleMin" .

sdo:CaseSeries  rdfs:comment  "A case series (also known as a clinical series) is a medical research study that tracks patients with a known exposure given similar treatment or examines their medical records for exposure and outcome. A case series can be retrospective or prospective and usually involves a smaller number of patients than the more powerful case-control studies or randomized controlled trials. Case series may be consecutive or non-consecutive, depending on whether all cases presenting to the reporting authors over a period of time were included, or only a selection." ;
        rdfs:label    "CaseSeries" .

sdo:performTime  rdfs:comment  "The length of time it takes to perform instructions or a direction (not including time to prepare the supplies), in [ISO 8601 duration format](http://en.wikipedia.org/wiki/ISO_8601)." ;
        rdfs:label    "perform time" .

sdo:ratingValue  rdfs:comment  "The rating for the content.\\n\\nUsage guidelines:\\n\\n* Use values from 0123456789 (Unicode 'DIGIT ZERO' (U+0030) to 'DIGIT NINE' (U+0039)) rather than superficially similiar Unicode symbols.\\n* Use '.' (Unicode 'FULL STOP' (U+002E)) rather than ',' to indicate a decimal point. Avoid using these symbols as a readability separator." ;
        rdfs:label    "rating value" .

sdo:releaseNotes  rdfs:comment  "Description of what changed in this version." ;
        rdfs:label    "release notes" .

sdo:recipeInstructions
        rdfs:comment  "A step in making the recipe, in the form of a single item (document, video, etc.) or an ordered list with HowToStep and/or HowToSection items." ;
        rdfs:label    "recipe instructions" .

sdo:PriceTypeEnumeration
        rdfs:comment  "Enumerates different price types, for example list price, invoice price, and sale price." ;
        rdfs:label    "PriceTypeEnumeration" .

sdo:CDCPMDRecord  rdfs:comment  "A CDCPMDRecord is a data structure representing a record in a CDC tabular data format\n      used for hospital data reporting. See [documentation](/docs/cdc-covid.html) for details, and the linked CDC materials for authoritative\n      definitions used as the source here.\n      " ;
        rdfs:label    "CDCPMDRecord" .

sdo:Airline  rdfs:comment  "An organization that provides flights for passengers." ;
        rdfs:label    "Airline" .

sdo:LowSaltDiet  rdfs:comment  "A diet focused on reduced sodium intake." ;
        rdfs:label    "LowSaltDiet" .

sdo:DefinitiveLegalValue
        rdfs:comment  "Indicates a document for which the text is conclusively what the law says and is legally binding. (e.g. The digitally signed version of an Official Journal.)\n  Something \"Definitive\" is considered to be also [[AuthoritativeLegalValue]]." ;
        rdfs:label    "DefinitiveLegalValue" .

sdo:additionalVariable
        rdfs:comment  "Any additional component of the exercise prescription that may need to be articulated to the patient. This may include the order of exercises, the number of repetitions of movement, quantitative distance, progressions over time, etc." ;
        rdfs:label    "additional variable" .

sdo:Observational  rdfs:comment  "An observational study design." ;
        rdfs:label    "Observational" .

sdo:Clinician  rdfs:comment  "Medical clinicians, including practicing physicians and other medical professionals involved in clinical practice." ;
        rdfs:label    "Clinician" .

sdo:partOfTVSeries  rdfs:comment  "The TV series to which this episode or season belongs." ;
        rdfs:label    "part ofTVSeries" .

sdo:contactPoint  rdfs:comment  "A contact point for a person or organization." ;
        rdfs:label    "contact point" .

sdo:reservationStatus
        rdfs:comment  "The current status of the reservation." ;
        rdfs:label    "reservation status" .

sdo:MedicalGuidelineRecommendation
        rdfs:comment  "A guideline recommendation that is regarded as efficacious and where quality of the data supporting the recommendation is sound." ;
        rdfs:label    "MedicalGuidelineRecommendation" .

sdo:FMRadioChannel  rdfs:comment  "A radio channel that uses FM." ;
        rdfs:label    "FMRadioChannel" .

sdo:Observation  rdfs:comment  "Instances of the class [[Observation]] are used to specify observations about an entity (which may or may not be an instance of a [[StatisticalPopulation]]), at a particular time. The principal properties of an [[Observation]] are [[observedNode]], [[measuredProperty]], [[measuredValue]] (or [[median]], etc.) and [[observationDate]] ([[measuredProperty]] properties can, but need not always, be W3C RDF Data Cube \"measure properties\", as in the [lifeExpectancy example](https://www.w3.org/TR/vocab-data-cube/#dsd-example)).\nSee also [[StatisticalPopulation]], and the [data and datasets](/docs/data-and-datasets.html) overview for more details.\n  " ;
        rdfs:label    "Observation" .

sdo:sodiumContent  rdfs:comment  "The number of milligrams of sodium." ;
        rdfs:label    "sodium content" .

sdo:durationOfWarranty
        rdfs:comment  "The duration of the warranty promise. Common unitCode values are ANN for year, MON for months, or DAY for days." ;
        rdfs:label    "duration ofWarranty" .

sdo:WearableSizeSystemBR
        rdfs:comment  "Brazilian size system for wearables." ;
        rdfs:label    "WearableSizeSystemBR" .

sdo:DemoAlbum  rdfs:comment  "DemoAlbum." ;
        rdfs:label    "DemoAlbum" .

sdo:trackingNumber  rdfs:comment  "Shipper tracking number." ;
        rdfs:label    "tracking number" .

sdo:RiverBodyOfWater  rdfs:comment  "A river (for example, the broad majestic Shannon)." ;
        rdfs:label    "RiverBodyOfWater" .

sdo:Claim  rdfs:comment  "A [[Claim]] in Schema.org represents a specific, factually-oriented claim that could be the [[itemReviewed]] in a [[ClaimReview]]. The content of a claim can be summarized with the [[text]] property. Variations on well known claims can have their common identity indicated via [[sameAs]] links, and summarized with a [[name]]. Ideally, a [[Claim]] description includes enough contextual information to minimize the risk of ambiguity or inclarity. In practice, many claims are better understood in the context in which they appear or the interpretations provided by claim reviews.\n\n  Beyond [[ClaimReview]], the Claim type can be associated with related creative works - for example a [[ScholarlyArticle]] or [[Question]] might be [[about]] some [[Claim]].\n\n  At this time, Schema.org does not define any types of relationship between claims. This is a natural area for future exploration.\n  " ;
        rdfs:label    "Claim" .

sdo:CoOp  rdfs:comment  "Play mode: CoOp. Co-operative games, where you play on the same team with friends." ;
        rdfs:label    "CoOp" .

sdo:typicalCreditsPerTerm
        rdfs:comment  "The number of credits or units a full-time student would be expected to take in 1 term however 'term' is defined by the institution." ;
        rdfs:label    "typical creditsPerTerm" .

sdo:orderDelivery  rdfs:comment  "The delivery of the parcel related to this order or order item." ;
        rdfs:label    "order delivery" .

sdo:BoatTrip  rdfs:comment  "A trip on a commercial ferry line." ;
        rdfs:label    "BoatTrip" .

sdo:RestockingFees  rdfs:comment  "Specifies that the customer must pay a restocking fee when returning a product" ;
        rdfs:label    "RestockingFees" .

sdo:activityDuration  rdfs:comment  "Length of time to engage in the activity." ;
        rdfs:label    "activity duration" .

sdo:vehicleEngine  rdfs:comment  "Information about the engine or engines of the vehicle." ;
        rdfs:label    "vehicle engine" .

sdo:floorLimit  rdfs:comment  "A floor limit is the amount of money above which credit card transactions must be authorized." ;
        rdfs:label    "floor limit" .

sdo:ArriveAction  rdfs:comment  "The act of arriving at a place. An agent arrives at a destination from a fromLocation, optionally with participants." ;
        rdfs:label    "ArriveAction" .

sdo:Rheumatologic  rdfs:comment  "A specific branch of medical science that deals with the study and treatment of rheumatic, autoimmune or joint diseases." ;
        rdfs:label    "Rheumatologic" .

sdo:SeatingMap  rdfs:comment  "A seating map." ;
        rdfs:label    "SeatingMap" .

sdo:SoftwareSourceCode
        rdfs:comment  "Computer programming source code. Example: Full (compile ready) solutions, code snippet samples, scripts, templates." ;
        rdfs:label    "SoftwareSourceCode" .

sdo:legislationApplies
        rdfs:comment  "Indicates that this legislation (or part of a legislation) somehow transfers another legislation in a different legislative context. This is an informative link, and it has no legal value. For legally-binding links of transposition, use the <a href=\"/legislationTransposes\">legislationTransposes</a> property. For example an informative consolidated law of a European Union's member state \"applies\" the consolidated version of the European Directive implemented in it." ;
        rdfs:label    "legislation applies" .

sdo:learningResourceType
        rdfs:comment  "The predominant type or kind characterizing the learning resource. For example, 'presentation', 'handout'." ;
        rdfs:label    "learning resourceType" .

sdo:inCodeSet  rdfs:comment  "A [[CategoryCodeSet]] that contains this category code." ;
        rdfs:label    "in codeSet" .

sdo:programmingLanguage
        rdfs:comment  "The computer programming language." ;
        rdfs:label    "programming language" .

sdo:creditedTo  rdfs:comment  "The group the release is credited to if different than the byArtist. For example, Red and Blue is credited to \"Stefani Germanotta Band\", but by Lady Gaga." ;
        rdfs:label    "credited to" .

sdo:providesBroadcastService
        rdfs:comment  "The BroadcastService offered on this channel." ;
        rdfs:label    "provides broadcastService" .

sdo:LiveBlogPosting  rdfs:comment  "A [[LiveBlogPosting]] is a [[BlogPosting]] intended to provide a rolling textual coverage of an ongoing event through continuous updates." ;
        rdfs:label    "LiveBlogPosting" .

sdo:isEncodedByBioChemEntity
        rdfs:comment  "Another BioChemEntity encoding by this one." ;
        rdfs:label    "is encodedByBioChemEntity" .

sdo:ApplyAction  rdfs:comment  "The act of registering to an organization/service without the guarantee to receive it.\\n\\nRelated actions:\\n\\n* [[RegisterAction]]: Unlike RegisterAction, ApplyAction has no guarantees that the application will be accepted." ;
        rdfs:label    "ApplyAction" .

sdo:missionCoveragePrioritiesPolicy
        rdfs:comment  "For a [[NewsMediaOrganization]], a statement on coverage priorities, including any public agenda or stance on issues." ;
        rdfs:label    "mission coveragePrioritiesPolicy" .

sdo:EBook  rdfs:comment  "Book format: Ebook." ;
        rdfs:label    "EBook" .

sdo:BodyMeasurementHeight
        rdfs:comment  "Body height (measured between crown of head and soles of feet). Used, for example, to fit jackets." ;
        rdfs:label    "BodyMeasurementHeight" .

sdo:fileSize  rdfs:comment  "Size of the application / package (e.g. 18MB). In the absence of a unit (MB, KB etc.), KB will be assumed." ;
        rdfs:label    "file size" .

sdo:RightHandDriving  rdfs:comment  "The steering position is on the right side of the vehicle (viewed from the main direction of driving)." ;
        rdfs:label    "RightHandDriving" .

sdo:vendor  rdfs:comment  "'vendor' is an earlier term for 'seller'." ;
        rdfs:label    "vendor" .

sdo:MathSolver  rdfs:comment  "A math solver which is capable of solving a subset of mathematical problems." ;
        rdfs:label    "MathSolver" .

sdo:deliveryLeadTime  rdfs:comment  "The typical delay between the receipt of the order and the goods either leaving the warehouse or being prepared for pickup, in case the delivery method is on site pickup." ;
        rdfs:label    "delivery leadTime" .

sdo:restPeriods  rdfs:comment  "How often one should break from the activity." ;
        rdfs:label    "rest periods" .

sdo:annualPercentageRate
        rdfs:comment  "The annual rate that is charged for borrowing (or made by investing), expressed as a single percentage number that represents the actual yearly cost of funds over the term of a loan. This includes any fees or additional costs associated with the transaction." ;
        rdfs:label    "annual percentageRate" .

sdo:TrainReservation  rdfs:comment  "A reservation for train travel.\\n\\nNote: This type is for information about actual reservations, e.g. in confirmation emails or HTML pages with individual confirmations of reservations. For offers of tickets, use [[Offer]]." ;
        rdfs:label    "TrainReservation" .

sdo:WearableSizeGroupEnumeration
        rdfs:comment  "Enumerates common size groups (also known as \"size types\") for wearable products." ;
        rdfs:label    "WearableSizeGroupEnumeration" .

sdo:VideoObject  rdfs:comment  "A video file." ;
        rdfs:label    "VideoObject" .

sdo:Embassy  rdfs:comment  "An embassy." ;
        rdfs:label    "Embassy" .

sdo:Renal  rdfs:comment  "A specific branch of medical science that pertains to the study of the kidneys and its respective disease states." ;
        rdfs:label    "Renal" .

sdo:Neuro  rdfs:comment  "Neurological system clinical examination." ;
        rdfs:label    "Neuro" .

sdo:MedicalTrialDesign
        rdfs:comment  "Design models for medical trials. Enumerated type." ;
        rdfs:label    "MedicalTrialDesign" .

sdo:Collection  rdfs:comment  "A collection of items e.g. creative works or products." ;
        rdfs:label    "Collection" .

sdo:DefinedTerm  rdfs:comment  "A word, name, acronym, phrase, etc. with a formal definition. Often used in the context of category or subject classification, glossaries or dictionaries, product or creative work types, etc. Use the name property for the term being defined, use termCode if the term has an alpha-numeric code allocated, use description to provide the definition of the term." ;
        rdfs:label    "DefinedTerm" .

sdo:MovieClip  rdfs:comment  "A short segment/part of a movie." ;
        rdfs:label    "MovieClip" .

sdo:paymentDue  rdfs:comment  "The date that payment is due." ;
        rdfs:label    "payment due" .

sdo:inverseOf  rdfs:comment  "Relates a property to a property that is its inverse. Inverse properties relate the same pairs of items to each other, but in reversed direction. For example, the 'alumni' and 'alumniOf' properties are inverseOf each other. Some properties don't have explicit inverses; in these situations RDFa and JSON-LD syntax for reverse properties can be used." ;
        rdfs:label    "inverse of" .

sdo:eventSchedule  rdfs:comment  "Associates an [[Event]] with a [[Schedule]]. There are circumstances where it is preferable to share a schedule for a series of\n      repeating events rather than data on the individual events themselves. For example, a website or application might prefer to publish a schedule for a weekly\n      gym class rather than provide data on every event. A schedule could be processed by applications to add forthcoming events to a calendar. An [[Event]] that\n      is associated with a [[Schedule]] using this property should not have [[startDate]] or [[endDate]] properties. These are instead defined within the associated\n      [[Schedule]], this avoids any ambiguity for clients using the data. The property might have repeated values to specify different schedules, e.g. for different months\n      or seasons." ;
        rdfs:label    "event schedule" .

sdo:percentile25  rdfs:comment  "The 25th percentile value." ;
        rdfs:label    "percentile25" .

sdo:naturalProgression
        rdfs:comment  "The expected progression of the condition if it is not treated and allowed to progress naturally." ;
        rdfs:label    "natural progression" .

sdo:AlignmentObject  rdfs:comment  "An intangible item that describes an alignment between a learning resource and a node in an educational framework.\n\nShould not be used where the nature of the alignment can be described using a simple property, for example to express that a resource [[teaches]] or [[assesses]] a competency." ;
        rdfs:label    "AlignmentObject" .

sdo:IgnoreAction  rdfs:comment  "The act of intentionally disregarding the object. An agent ignores an object." ;
        rdfs:label    "IgnoreAction" .

sdo:Protozoa  rdfs:comment  "Single-celled organism that causes an infection." ;
        rdfs:label    "Protozoa" .

sdo:RsvpResponseType  rdfs:comment  "RsvpResponseType is an enumeration type whose instances represent responding to an RSVP request." ;
        rdfs:label    "RsvpResponseType" .

sdo:Vessel  rdfs:comment  "A component of the human body circulatory system comprised of an intricate network of hollow tubes that transport blood throughout the entire body." ;
        rdfs:label    "Vessel" .

sdo:educationalProgramMode
        rdfs:comment  "Similar to courseMode, The medium or means of delivery of the program as a whole. The value may either be a text label (e.g. \"online\", \"onsite\" or \"blended\"; \"synchronous\" or \"asynchronous\"; \"full-time\" or \"part-time\") or a URL reference to a term from a controlled vocabulary (e.g. https://ceds.ed.gov/element/001311#Asynchronous )." ;
        rdfs:label    "educational programMode" .

sdo:CreativeWork  rdfs:comment  "The most generic kind of creative work, including books, movies, photographs, software programs, etc." ;
        rdfs:label    "CreativeWork" .

sdo:directApply  rdfs:comment  "Indicates whether an [[url]] that is associated with a [[JobPosting]] enables direct application for the job, via the posting website. A job posting is considered to have directApply of [[True]] if an application process for the specified job can be directly initiated via the url(s) given (noting that e.g. multiple internet domains might nevertheless be involved at an implementation level). A value of [[False]] is appropriate if there is no clear path to applying directly online for the specified job, navigating directly from the JobPosting url(s) supplied." ;
        rdfs:label    "direct apply" .

sdo:Continent  rdfs:comment  "One of the continents (for example, Europe or Africa)." ;
        rdfs:label    "Continent" .

sdo:publisherImprint  rdfs:comment  "The publishing division which published the comic." ;
        rdfs:label    "publisher imprint" .

sdo:exchangeRateSpread
        rdfs:comment  "The difference between the price at which a broker or other intermediary buys and sells foreign currency." ;
        rdfs:label    "exchange rateSpread" .

sdo:WearableSizeSystemEnumeration
        rdfs:comment  "Enumerates common size systems specific for wearable products" ;
        rdfs:label    "WearableSizeSystemEnumeration" .

sdo:Notary  rdfs:comment  "A notary." ;
        rdfs:label    "Notary" .

sdo:SellAction  rdfs:comment  "The act of taking money from a buyer in exchange for goods or services rendered. An agent sells an object, product, or service to a buyer for a price. Reciprocal of BuyAction." ;
        rdfs:label    "SellAction" .

sdo:GovernmentBuilding
        rdfs:comment  "A government building." ;
        rdfs:label    "GovernmentBuilding" .

sdo:inventoryLevel  rdfs:comment  "The current approximate inventory level for the item or items." ;
        rdfs:label    "inventory level" .

sdo:providesService  rdfs:comment  "The service provided by this channel." ;
        rdfs:label    "provides service" .

sdo:additionalProperty
        rdfs:comment  "A property-value pair representing an additional characteristics of the entitity, e.g. a product feature or another characteristic for which there is no matching property in schema.org.\\n\\nNote: Publishers should be aware that applications designed to use specific schema.org properties (e.g. https://schema.org/width, https://schema.org/color, https://schema.org/gtin13, ...) will typically expect such data to be provided using those properties, rather than using the generic property/value mechanism.\n" ;
        rdfs:label    "additional property" .

sdo:Quantity  rdfs:comment  "Quantities such as distance, time, mass, weight, etc. Particular instances of say Mass are entities like '3 Kg' or '4 milligrams'." ;
        rdfs:label    "Quantity" .

sdo:occupationalCredentialAwarded
        rdfs:comment  "A description of the qualification, award, certificate, diploma or other occupational credential awarded as a consequence of successful completion of this course or program." ;
        rdfs:label    "occupational credentialAwarded" .

sdo:Courthouse  rdfs:comment  "A courthouse." ;
        rdfs:label    "Courthouse" .

sdo:areaServed  rdfs:comment  "The geographic area where a service or offered item is provided." ;
        rdfs:label    "area served" .

sdo:ConsumeAction  rdfs:comment  "The act of ingesting information/resources/food." ;
        rdfs:label    "ConsumeAction" .

sdo:relevantSpecialty
        rdfs:comment  "If applicable, a medical specialty in which this entity is relevant." ;
        rdfs:label    "relevant specialty" .

sdo:HowToItem  rdfs:comment  "An item used as either a tool or supply when performing the instructions for how to to achieve a result." ;
        rdfs:label    "HowToItem" .

sdo:icaoCode  rdfs:comment  "ICAO identifier for an airport." ;
        rdfs:label    "icao code" .

sdo:LifestyleModification
        rdfs:comment  "A process of care involving exercise, changes to diet, fitness routines, and other lifestyle changes aimed at improving a health condition." ;
        rdfs:label    "LifestyleModification" .

sdo:MerchantReturnFiniteReturnWindow
        rdfs:comment  "Specifies that there is a finite window for product returns." ;
        rdfs:label    "MerchantReturnFiniteReturnWindow" .

sdo:familyName  rdfs:comment  "Family name. In the U.S., the last name of a Person." ;
        rdfs:label    "family name" .

sdo:isAvailableGenerically
        rdfs:comment  "True if the drug is available in a generic form (regardless of name)." ;
        rdfs:label    "is availableGenerically" .

sdo:Text  rdfs:comment  "Data type: Text." ;
        rdfs:label    "Text" .

sdo:BodyMeasurementHips
        rdfs:comment  "Girth of hips (measured around the buttocks). Used, for example, to fit skirts." ;
        rdfs:label    "BodyMeasurementHips" .

sdo:numberOfEpisodes  rdfs:comment  "The number of episodes in this season or series." ;
        rdfs:label    "number ofEpisodes" .

sdo:Nonprofit501c18  rdfs:comment  "Nonprofit501c18: Non-profit type referring to Employee Funded Pension Trust (created before 25 June 1959)." ;
        rdfs:label    "Nonprofit501c18" .

sdo:EducationalOccupationalProgram
        rdfs:comment  "A program offered by an institution which determines the learning progress to achieve an outcome, usually a credential like a degree or certificate. This would define a discrete set of opportunities (e.g., job, courses) that together constitute a program with a clear start, end, set of requirements, and transition to a new occupational opportunity (e.g., a job), or sometimes a higher educational opportunity (e.g., an advanced degree)." ;
        rdfs:label    "EducationalOccupationalProgram" .

sdo:ReturnLabelInBox  rdfs:comment  "Specifies that a return label will be provided by the seller in the shipping box." ;
        rdfs:label    "ReturnLabelInBox" .

sdo:mpn  rdfs:comment  "The Manufacturer Part Number (MPN) of the product, or the product to which the offer refers." ;
        rdfs:label    "mpn" .

sdo:Permit  rdfs:comment  "A permit issued by an organization, e.g. a parking pass." ;
        rdfs:label    "Permit" .

sdo:FreeReturn  rdfs:comment  "Specifies that product returns are free of charge for the customer." ;
        rdfs:label    "FreeReturn" .

sdo:City  rdfs:comment  "A city or town." ;
        rdfs:label    "City" .

sdo:Duration  rdfs:comment  "Quantity: Duration (use [ISO 8601 duration format](http://en.wikipedia.org/wiki/ISO_8601))." ;
        rdfs:label    "Duration" .

sdo:SpeakableSpecification
        rdfs:comment  "A SpeakableSpecification indicates (typically via [[xpath]] or [[cssSelector]]) sections of a document that are highlighted as particularly [[speakable]]. Instances of this type are expected to be used primarily as values of the [[speakable]] property." ;
        rdfs:label    "SpeakableSpecification" .

sdo:WearableMeasurementWidth
        rdfs:comment  "Measurement of the width, for example of shoes" ;
        rdfs:label    "WearableMeasurementWidth" .

sdo:FastFoodRestaurant
        rdfs:comment  "A fast-food restaurant." ;
        rdfs:label    "FastFoodRestaurant" .

sdo:LiteraryEvent  rdfs:comment  "Event type: Literary event." ;
        rdfs:label    "LiteraryEvent" .

sdo:InstallAction  rdfs:comment  "The act of installing an application." ;
        rdfs:label    "InstallAction" .

sdo:MedicineSystem  rdfs:comment  "Systems of medical practice." ;
        rdfs:label    "MedicineSystem" .

sdo:PriceSpecification
        rdfs:comment  "A structured value representing a price or price range. Typically, only the subclasses of this type are used for markup. It is recommended to use [[MonetaryAmount]] to describe independent amounts of money such as a salary, credit card limits, etc." ;
        rdfs:label    "PriceSpecification" .

sdo:availableOnDevice
        rdfs:comment  "Device required to run the application. Used in cases where a specific make/model is required to run the application." ;
        rdfs:label    "available onDevice" .

sdo:vehicleConfiguration
        rdfs:comment  "A short text indicating the configuration of the vehicle, e.g. '5dr hatchback ST 2.5 MT 225 hp' or 'limited edition'." ;
        rdfs:label    "vehicle configuration" .

sdo:seriousAdverseOutcome
        rdfs:comment  "A possible serious complication and/or serious side effect of this therapy. Serious adverse outcomes include those that are life-threatening; result in death, disability, or permanent damage; require hospitalization or prolong existing hospitalization; cause congenital anomalies or birth defects; or jeopardize the patient and may require medical or surgical intervention to prevent one of the outcomes in this definition." ;
        rdfs:label    "serious adverseOutcome" .

sdo:conditionsOfAccess
        rdfs:comment  "Conditions that affect the availability of, or method(s) of access to, an item. Typically used for real world items such as an [[ArchiveComponent]] held by an [[ArchiveOrganization]]. This property is not suitable for use as a general Web access control mechanism. It is expressed only in natural language.\\n\\nFor example \"Available by appointment from the Reading Room\" or \"Accessible only from logged-in accounts \". " ;
        rdfs:label    "conditions ofAccess" .

sdo:eligibleDuration  rdfs:comment  "The duration for which the given offer is valid." ;
        rdfs:label    "eligible duration" .

sdo:answerExplanation
        rdfs:comment  "A step-by-step or full explanation about Answer. Can outline how this Answer was achieved or contain more broad clarification or statement about it. " ;
        rdfs:label    "answer explanation" .

sdo:CassetteFormat  rdfs:comment  "CassetteFormat." ;
        rdfs:label    "CassetteFormat" .

sdo:OpinionNewsArticle
        rdfs:comment  "An [[OpinionNewsArticle]] is a [[NewsArticle]] that primarily expresses opinions rather than journalistic reporting of news and events. For example, a [[NewsArticle]] consisting of a column or [[Blog]]/[[BlogPosting]] entry in the Opinions section of a news publication. " ;
        rdfs:label    "OpinionNewsArticle" .

sdo:cholesterolContent
        rdfs:comment  "The number of milligrams of cholesterol." ;
        rdfs:label    "cholesterol content" .

sdo:ChooseAction  rdfs:comment  "The act of expressing a preference from a set of options or a large or unbounded set of choices/options." ;
        rdfs:label    "ChooseAction" .

sdo:SingleCenterTrial
        rdfs:comment  "A trial that takes place at a single center." ;
        rdfs:label    "SingleCenterTrial" .

sdo:hasMerchantReturnPolicy
        rdfs:comment  "Specifies a MerchantReturnPolicy that may be applicable." ;
        rdfs:label    "has merchantReturnPolicy" .

sdo:measuredValue  rdfs:comment  "The measuredValue of an [[Observation]]." ;
        rdfs:label    "measured value" .

sdo:ingredients  rdfs:comment  "A single ingredient used in the recipe, e.g. sugar, flour or garlic." ;
        rdfs:label    "ingredients" .

sdo:PerformingArtsTheater
        rdfs:comment  "A theater or other performing art center." ;
        rdfs:label    "PerformingArtsTheater" .

sdo:geoWithin  rdfs:comment  "Represents a relationship between two geometries (or the places they represent), relating a geometry to one that contains it, i.e. it is inside (i.e. within) its interior. As defined in [DE-9IM](https://en.wikipedia.org/wiki/DE-9IM)." ;
        rdfs:label    "geo within" .

sdo:Offer  rdfs:comment  "An offer to transfer some rights to an item or to provide a service — for example, an offer to sell tickets to an event, to rent the DVD of a movie, to stream a TV show over the internet, to repair a motorcycle, or to loan a book.\\n\\nNote: As the [[businessFunction]] property, which identifies the form of offer (e.g. sell, lease, repair, dispose), defaults to http://purl.org/goodrelations/v1#Sell; an Offer without a defined businessFunction value can be assumed to be an offer to sell.\\n\\nFor [GTIN](http://www.gs1.org/barcodes/technical/idkeys/gtin)-related fields, see [Check Digit calculator](http://www.gs1.org/barcodes/support/check_digit_calculator) and [validation guide](http://www.gs1us.org/resources/standards/gtin-validation-guide) from [GS1](http://www.gs1.org/)." ;
        rdfs:label    "Offer" .

sdo:TieAction  rdfs:comment  "The act of reaching a draw in a competitive activity." ;
        rdfs:label    "TieAction" .

sdo:TheaterEvent  rdfs:comment  "Event type: Theater performance." ;
        rdfs:label    "TheaterEvent" .

sdo:BookmarkAction  rdfs:comment  "An agent bookmarks/flags/labels/tags/marks an object." ;
        rdfs:label    "BookmarkAction" .

sdo:ExerciseGym  rdfs:comment  "A gym." ;
        rdfs:label    "ExerciseGym" .

sdo:runtime  rdfs:comment  "Runtime platform or script interpreter dependencies (Example - Java v1, Python2.3, .Net Framework 3.0)." ;
        rdfs:label    "runtime" .

sdo:MusicAlbum  rdfs:comment  "A collection of music tracks." ;
        rdfs:label    "MusicAlbum" .

sdo:object  rdfs:comment  "The object upon which the action is carried out, whose state is kept intact or changed. Also known as the semantic roles patient, affected or undergoer (which change their state) or theme (which doesn't). e.g. John read *a book*." ;
        rdfs:label    "object" .

sdo:menuAddOn  rdfs:comment  "Additional menu item(s) such as a side dish of salad or side order of fries that can be added to this menu item. Additionally it can be a menu section containing allowed add-on menu items for this menu item." ;
        rdfs:label    "menu addOn" .

sdo:CovidTestingFacility
        rdfs:comment  "A CovidTestingFacility is a [[MedicalClinic]] where testing for the COVID-19 Coronavirus\n      disease is available. If the facility is being made available from an established [[Pharmacy]], [[Hotel]], or other\n      non-medical organization, multiple types can be listed. This makes it easier to re-use existing schema.org information\n      about that place e.g. contact info, address, opening hours. Note that in an emergency, such information may not always be reliable.\n      " ;
        rdfs:label    "CovidTestingFacility" .

sdo:MerchantReturnUnlimitedWindow
        rdfs:comment  "Specifies that there is an unlimited window for product returns." ;
        rdfs:label    "MerchantReturnUnlimitedWindow" .

sdo:discussionUrl  rdfs:comment  "A link to the page containing the comments of the CreativeWork." ;
        rdfs:label    "discussion url" .

sdo:educationalFramework
        rdfs:comment  "The framework to which the resource being described is aligned." ;
        rdfs:label    "educational framework" .

sdo:maximumIntake  rdfs:comment  "Recommended intake of this supplement for a given population as defined by a specific recommending authority." ;
        rdfs:label    "maximum intake" .

sdo:MedicalSymptom  rdfs:comment  "Any complaint sensed and expressed by the patient (therefore defined as subjective)  like stomachache, lower-back pain, or fatigue." ;
        rdfs:label    "MedicalSymptom" .

sdo:TaxiReservation  rdfs:comment  "A reservation for a taxi.\\n\\nNote: This type is for information about actual reservations, e.g. in confirmation emails or HTML pages with individual confirmations of reservations. For offers of tickets, use [[Offer]]." ;
        rdfs:label    "TaxiReservation" .

sdo:NGO  rdfs:comment  "Organization: Non-governmental Organization." ;
        rdfs:label    "NGO" .

sdo:WearableSizeGroupWomens
        rdfs:comment  "Size group \"Womens\" for wearables." ;
        rdfs:label    "WearableSizeGroupWomens" .

sdo:legislationDate  rdfs:comment  "The date of adoption or signature of the legislation. This is the date at which the text is officially aknowledged to be a legislation, even though it might not even be published or in force." ;
        rdfs:label    "legislation date" .

sdo:doorTime  rdfs:comment  "The time admission will commence." ;
        rdfs:label    "door time" .

sdo:ListItem  rdfs:comment  "An list item, e.g. a step in a checklist or how-to description." ;
        rdfs:label    "ListItem" .

sdo:NailSalon  rdfs:comment  "A nail salon." ;
        rdfs:label    "NailSalon" .

sdo:CrossSectional  rdfs:comment  "Studies carried out on pre-existing data (usually from 'snapshot' surveys), such as that collected by the Census Bureau. Sometimes called Prevalence Studies." ;
        rdfs:label    "CrossSectional" .

sdo:muscleAction  rdfs:comment  "The movement the muscle generates." ;
        rdfs:label    "muscle action" .

sdo:ViewAction  rdfs:comment  "The act of consuming static visual content." ;
        rdfs:label    "ViewAction" .

sdo:deathPlace  rdfs:comment  "The place where the person died." ;
        rdfs:label    "death place" .

sdo:geoIntersects  rdfs:comment  "Represents spatial relations in which two geometries (or the places they represent) have at least one point in common. As defined in [DE-9IM](https://en.wikipedia.org/wiki/DE-9IM)." ;
        rdfs:label    "geo intersects" .

sdo:hasDefinedTerm  rdfs:comment  "A Defined Term contained in this term set." ;
        rdfs:label    "has definedTerm" .

sdo:returnMethod  rdfs:comment  "The type of return method offered, specified from an enumeration." ;
        rdfs:label    "return method" .

sdo:Surgical  rdfs:comment  "A specific branch of medical science that pertains to treating diseases, injuries and deformities by manual and instrumental means." ;
        rdfs:label    "Surgical" .

sdo:bankAccountType  rdfs:comment  "The type of a bank account." ;
        rdfs:label    "bank accountType" .

sdo:ReservationCancelled
        rdfs:comment  "The status for a previously confirmed reservation that is now cancelled." ;
        rdfs:label    "ReservationCancelled" .

sdo:LeaveAction  rdfs:comment  "An agent leaves an event / group with participants/friends at a location.\\n\\nRelated actions:\\n\\n* [[JoinAction]]: The antonym of LeaveAction.\\n* [[UnRegisterAction]]: Unlike UnRegisterAction, LeaveAction implies leaving a group/team of people rather than a service." ;
        rdfs:label    "LeaveAction" .

sdo:actionAccessibilityRequirement
        rdfs:comment  "A set of requirements that a must be fulfilled in order to perform an Action. If more than one value is specied, fulfilling one set of requirements will allow the Action to be performed." ;
        rdfs:label    "action accessibilityRequirement" .

sdo:isProprietary  rdfs:comment  "True if this item's name is a proprietary/brand name (vs. generic name)." ;
        rdfs:label    "is proprietary" .

sdo:SocialEvent  rdfs:comment  "Event type: Social event." ;
        rdfs:label    "SocialEvent" .

sdo:MedicalClinic  rdfs:comment  "A facility, often associated with a hospital or medical school, that is devoted to the specific diagnosis and/or healthcare. Previously limited to outpatients but with evolution it may be open to inpatients as well." ;
        rdfs:label    "MedicalClinic" .

sdo:hasEnergyConsumptionDetails
        rdfs:comment  "Defines the energy efficiency Category (also known as \"class\" or \"rating\") for a product according to an international energy efficiency standard." ;
        rdfs:label    "has energyConsumptionDetails" .

sdo:PublicToilet  rdfs:comment  "A public toilet is a room or small building containing one or more toilets (and possibly also urinals) which is available for use by the general public, or by customers or employees of certain businesses." ;
        rdfs:label    "PublicToilet" .

sdo:BroadcastRelease  rdfs:comment  "BroadcastRelease." ;
        rdfs:label    "BroadcastRelease" .

sdo:TouristTrip  rdfs:comment  "A tourist trip. A created itinerary of visits to one or more places of interest ([[TouristAttraction]]/[[TouristDestination]]) often linked by a similar theme, geographic area, or interest to a particular [[touristType]]. The [UNWTO](http://www2.unwto.org/) defines tourism trip as the Trip taken by visitors.\n  (See examples below)." ;
        rdfs:label    "TouristTrip" .

sdo:EvidenceLevelA  rdfs:comment  "Data derived from multiple randomized clinical trials or meta-analyses." ;
        rdfs:label    "EvidenceLevelA" .

sdo:SubwayStation  rdfs:comment  "A subway station." ;
        rdfs:label    "SubwayStation" .

sdo:hasBroadcastChannel
        rdfs:comment  "A broadcast channel of a broadcast service." ;
        rdfs:label    "has broadcastChannel" .

sdo:hasMenuSection  rdfs:comment  "A subgrouping of the menu (by dishes, course, serving time period, etc.)." ;
        rdfs:label    "has menuSection" .

sdo:programName  rdfs:comment  "The program providing the membership." ;
        rdfs:label    "program name" .

sdo:ItemListUnordered
        rdfs:comment  "An ItemList ordered with no explicit order." ;
        rdfs:label    "ItemListUnordered" .

sdo:Play  rdfs:comment  "A play is a form of literature, usually consisting of dialogue between characters, intended for theatrical performance rather than just reading. Note: A performance of a Play would be a [[TheaterEvent]] or [[BroadcastEvent]] - the *Play* being the [[workPerformed]]." ;
        rdfs:label    "Play" .

sdo:CreativeWorkSeries
        rdfs:comment  "A CreativeWorkSeries in schema.org is a group of related items, typically but not necessarily of the same kind. CreativeWorkSeries are usually organized into some order, often chronological. Unlike [[ItemList]] which is a general purpose data structure for lists of things, the emphasis with CreativeWorkSeries is on published materials (written e.g. books and periodicals, or media such as tv, radio and games).\\n\\nSpecific subtypes are available for describing [[TVSeries]], [[RadioSeries]], [[MovieSeries]], [[BookSeries]], [[Periodical]] and [[VideoGameSeries]]. In each case, the [[hasPart]] / [[isPartOf]] properties can be used to relate the CreativeWorkSeries to its parts. The general CreativeWorkSeries type serves largely just to organize these more specific and practical subtypes.\\n\\nIt is common for properties applicable to an item from the series to be usefully applied to the containing group. Schema.org attempts to anticipate some of these cases, but publishers should be free to apply properties of the series parts to the series as a whole wherever they seem appropriate.\n\t  " ;
        rdfs:label    "CreativeWorkSeries" .

sdo:BookSeries  rdfs:comment  "A series of books. Included books can be indicated with the hasPart property." ;
        rdfs:label    "BookSeries" .

sdo:subtitleLanguage  rdfs:comment  "Languages in which subtitles/captions are available, in [IETF BCP 47 standard format](http://tools.ietf.org/html/bcp47)." ;
        rdfs:label    "subtitle language" .

sdo:greater  rdfs:comment  "This ordering relation for qualitative values indicates that the subject is greater than the object." ;
        rdfs:label    "greater" .

sdo:pagination  rdfs:comment  "Any description of pages that is not separated into pageStart and pageEnd; for example, \"1-6, 9, 55\" or \"10-12, 46-49\"." ;
        rdfs:label    "pagination" .

sdo:StrengthTraining  rdfs:comment  "Physical activity that is engaged in to improve muscle and bone strength. Also referred to as resistance training." ;
        rdfs:label    "StrengthTraining" .

sdo:numberOfPlayers  rdfs:comment  "Indicate how many people can play this game (minimum, maximum, or range)." ;
        rdfs:label    "number ofPlayers" .

sdo:amount  rdfs:comment  "The amount of money." ;
        rdfs:label    "amount" .

sdo:noBylinesPolicy  rdfs:comment  "For a [[NewsMediaOrganization]] or other news-related [[Organization]], a statement explaining when authors of articles are not named in bylines." ;
        rdfs:label    "no bylinesPolicy" .

sdo:nonEqual  rdfs:comment  "This ordering relation for qualitative values indicates that the subject is not equal to the object." ;
        rdfs:label    "non equal" .

sdo:IceCreamShop  rdfs:comment  "An ice cream shop." ;
        rdfs:label    "IceCreamShop" .

sdo:variantCover  rdfs:comment  "A description of the variant cover\n    \tfor the issue, if the issue is a variant printing. For example, \"Bryan Hitch\n    \tVariant Cover\" or \"2nd Printing Variant\"." ;
        rdfs:label    "variant cover" .

sdo:audience  rdfs:comment  "An intended audience, i.e. a group for whom something was created." ;
        rdfs:label    "audience" .

sdo:mediaItemAppearance
        rdfs:comment  "In the context of a [[MediaReview]], indicates specific media item(s) that are grouped using a [[MediaReviewItem]]." ;
        rdfs:label    "media itemAppearance" .

sdo:MayTreatHealthAspect
        rdfs:comment  "Related topics may be treated by a Topic." ;
        rdfs:label    "MayTreatHealthAspect" .

sdo:blogPost  rdfs:comment  "A posting that is part of this blog." ;
        rdfs:label    "blog post" .

sdo:cvdFacilityCounty
        rdfs:comment  "Name of the County of the NHSN facility that this data record applies to. Use [[cvdFacilityId]] to identify the facility. To provide other details, [[healthcareReportingData]] can be used on a [[Hospital]] entry." ;
        rdfs:label    "cvd facilityCounty" .

sdo:Nonprofit501c25  rdfs:comment  "Nonprofit501c25: Non-profit type referring to Real Property Title-Holding Corporations or Trusts with Multiple Parents." ;
        rdfs:label    "Nonprofit501c25" .

sdo:DamagedCondition  rdfs:comment  "Indicates that the item is damaged." ;
        rdfs:label    "DamagedCondition" .

sdo:LivingWithHealthAspect
        rdfs:comment  "Information about coping or life related to the topic." ;
        rdfs:label    "LivingWithHealthAspect" .

sdo:Bridge  rdfs:comment  "A bridge." ;
        rdfs:label    "Bridge" .

sdo:inChI  rdfs:comment  "Non-proprietary identifier for molecular entity that can be used in printed and electronic data sources thus enabling easier linking of diverse data compilations." ;
        rdfs:label    "in chI" .

sdo:Nerve  rdfs:comment  "A common pathway for the electrochemical nerve impulses that are transmitted along each of the axons." ;
        rdfs:label    "Nerve" .

sdo:MenuSection  rdfs:comment  "A sub-grouping of food or drink items in a menu. E.g. courses (such as 'Dinner', 'Breakfast', etc.), specific type of dishes (such as 'Meat', 'Vegan', 'Drinks', etc.), or some other classification made by the menu provider." ;
        rdfs:label    "MenuSection" .

sdo:geo  rdfs:comment  "The geo coordinates of the place." ;
        rdfs:label    "geo" .

sdo:albumRelease  rdfs:comment  "A release of this album." ;
        rdfs:label    "album release" .

sdo:speakable  rdfs:comment  "Indicates sections of a Web page that are particularly 'speakable' in the sense of being highlighted as being especially appropriate for text-to-speech conversion. Other sections of a page may also be usefully spoken in particular circumstances; the 'speakable' property serves to indicate the parts most likely to be generally useful for speech.\n\nThe *speakable* property can be repeated an arbitrary number of times, with three kinds of possible 'content-locator' values:\n\n1.) *id-value* URL references - uses *id-value* of an element in the page being annotated. The simplest use of *speakable* has (potentially relative) URL values, referencing identified sections of the document concerned.\n\n2.) CSS Selectors - addresses content in the annotated page, eg. via class attribute. Use the [[cssSelector]] property.\n\n3.)  XPaths - addresses content via XPaths (assuming an XML view of the content). Use the [[xpath]] property.\n\n\nFor more sophisticated markup of speakable sections beyond simple ID references, either CSS selectors or XPath expressions to pick out document section(s) as speakable. For this\nwe define a supporting type, [[SpeakableSpecification]]  which is defined to be a possible value of the *speakable* property.\n         " ;
        rdfs:label    "speakable" .

sdo:doseSchedule  rdfs:comment  "A dosing schedule for the drug for a given population, either observed, recommended, or maximum dose based on the type used." ;
        rdfs:label    "dose schedule" .

sdo:honorificSuffix  rdfs:comment  "An honorific suffix following a Person's name such as M.D. /PhD/MSCSW." ;
        rdfs:label    "honorific suffix" .

sdo:Gene  rdfs:comment  "A discrete unit of inheritance which affects one or more biological traits (Source: [https://en.wikipedia.org/wiki/Gene](https://en.wikipedia.org/wiki/Gene)). Examples include FOXP2 (Forkhead box protein P2), SCARNA21 (small Cajal body-specific RNA 21), A- (agouti genotype)." ;
        rdfs:label    "Gene" .

sdo:OfferForLease  rdfs:comment  "An [[OfferForLease]] in Schema.org represents an [[Offer]] to lease out something, i.e. an [[Offer]] whose\n  [[businessFunction]] is [lease out](http://purl.org/goodrelations/v1#LeaseOut.). See [Good Relations](https://en.wikipedia.org/wiki/GoodRelations) for\n  background on the underlying concepts.\n  " ;
        rdfs:label    "OfferForLease" .

sdo:ReviewNewsArticle
        rdfs:comment  "A [[NewsArticle]] and [[CriticReview]] providing a professional critic's assessment of a service, product, performance, or artistic or literary work." ;
        rdfs:label    "ReviewNewsArticle" .

sdo:softwareAddOn  rdfs:comment  "Additional content for a software application." ;
        rdfs:label    "software addOn" .

sdo:Service  rdfs:comment  "A service provided by an organization, e.g. delivery service, print services, etc." ;
        rdfs:label    "Service" .

sdo:rsvpResponse  rdfs:comment  "The response (yes, no, maybe) to the RSVP." ;
        rdfs:label    "rsvp response" .

sdo:ResultsAvailable  rdfs:comment  "Results are available." ;
        rdfs:label    "ResultsAvailable" .

sdo:billingStart  rdfs:comment  "Specifies after how much time this price (or price component) becomes valid and billing starts. Can be used, for example, to model a price increase after the first year of a subscription. The unit of measurement is specified by the unitCode property." ;
        rdfs:label    "billing start" .

sdo:imagingTechnique  rdfs:comment  "Imaging technique used." ;
        rdfs:label    "imaging technique" .

sdo:PronounceableText
        rdfs:comment  "Data type: PronounceableText." ;
        rdfs:label    "PronounceableText" .

sdo:ShippingRateSettings
        rdfs:comment  "A ShippingRateSettings represents re-usable pieces of shipping information. It is designed for publication on an URL that may be referenced via the [[shippingSettingsLink]] property of an [[OfferShippingDetails]]. Several occurrences can be published, distinguished and matched (i.e. identified/referenced) by their different values for [[shippingLabel]]." ;
        rdfs:label    "ShippingRateSettings" .

sdo:Lung  rdfs:comment  "Lung and respiratory system clinical examination." ;
        rdfs:label    "Lung" .

sdo:increasesRiskOf  rdfs:comment  "The condition, complication, etc. influenced by this factor." ;
        rdfs:label    "increases riskOf" .

sdo:PreventionIndication
        rdfs:comment  "An indication for preventing an underlying condition, symptom, etc." ;
        rdfs:label    "PreventionIndication" .

sdo:BenefitsHealthAspect
        rdfs:comment  "Content about the benefits and advantages of usage or utilization of topic." ;
        rdfs:label    "BenefitsHealthAspect" .

sdo:code  rdfs:comment  "A medical code for the entity, taken from a controlled vocabulary or ontology such as ICD-9, DiseasesDB, MeSH, SNOMED-CT, RxNorm, etc." ;
        rdfs:label    "code" .

sdo:Nonprofit501c17  rdfs:comment  "Nonprofit501c17: Non-profit type referring to Supplemental Unemployment Benefit Trusts." ;
        rdfs:label    "Nonprofit501c17" .

sdo:ShortStory  rdfs:comment  "Short story or tale. A brief work of literature, usually written in narrative prose." ;
        rdfs:label    "ShortStory" .

sdo:eligibleRegion  rdfs:comment  "The ISO 3166-1 (ISO 3166-1 alpha-2) or ISO 3166-2 code, the place, or the GeoShape for the geo-political region(s) for which the offer or delivery charge specification is valid.\\n\\nSee also [[ineligibleRegion]].\n    " ;
        rdfs:label    "eligible region" .

sdo:CreativeWorkSeason
        rdfs:comment  "A media season e.g. tv, radio, video game etc." ;
        rdfs:label    "CreativeWorkSeason" .

sdo:GroupBoardingPolicy
        rdfs:comment  "The airline boards by groups based on check-in time, priority, etc." ;
        rdfs:label    "GroupBoardingPolicy" .

sdo:OrderDelivered  rdfs:comment  "OrderStatus representing successful delivery of an order." ;
        rdfs:label    "OrderDelivered" .

sdo:MenuItem  rdfs:comment  "A food or drink item listed in a menu or menu section." ;
        rdfs:label    "MenuItem" .

sdo:spouse  rdfs:comment  "The person's spouse." ;
        rdfs:label    "spouse" .

sdo:WearableSizeGroupBoys
        rdfs:comment  "Size group \"Boys\" for wearables." ;
        rdfs:label    "WearableSizeGroupBoys" .

sdo:givenName  rdfs:comment  "Given name. In the U.S., the first name of a Person." ;
        rdfs:label    "given name" .

sdo:MedicalOrganization
        rdfs:comment  "A medical organization (physical or not), such as hospital, institution or clinic." ;
        rdfs:label    "MedicalOrganization" .

sdo:appearance  rdfs:comment  "Indicates an occurence of a [[Claim]] in some [[CreativeWork]]." ;
        rdfs:label    "appearance" .

sdo:InfectiousAgentClass
        rdfs:comment  "Classes of agents or pathogens that transmit infectious diseases. Enumerated type." ;
        rdfs:label    "InfectiousAgentClass" .

sdo:typicalTest  rdfs:comment  "A medical test typically performed given this condition." ;
        rdfs:label    "typical test" .

sdo:relatedDrug  rdfs:comment  "Any other drug related to this one, for example commonly-prescribed alternatives." ;
        rdfs:label    "related drug" .

sdo:CivicStructure  rdfs:comment  "A public structure, such as a town hall or concert hall." ;
        rdfs:label    "CivicStructure" .

sdo:measurementTechnique
        rdfs:comment  "A technique or technology used in a [[Dataset]] (or [[DataDownload]], [[DataCatalog]]),\ncorresponding to the method used for measuring the corresponding variable(s) (described using [[variableMeasured]]). This is oriented towards scientific and scholarly dataset publication but may have broader applicability; it is not intended as a full representation of measurement, but rather as a high level summary for dataset discovery.\n\nFor example, if [[variableMeasured]] is: molecule concentration, [[measurementTechnique]] could be: \"mass spectrometry\" or \"nmr spectroscopy\" or \"colorimetry\" or \"immunofluorescence\".\n\nIf the [[variableMeasured]] is \"depression rating\", the [[measurementTechnique]] could be \"Zung Scale\" or \"HAM-D\" or \"Beck Depression Inventory\".\n\nIf there are several [[variableMeasured]] properties recorded for some given data object, use a [[PropertyValue]] for each [[variableMeasured]] and attach the corresponding [[measurementTechnique]].\n      " ;
        rdfs:label    "measurement technique" .

sdo:Diet  rdfs:comment  "A strategy of regulating the intake of food to achieve or maintain a specific health-related goal." ;
        rdfs:label    "Diet" .

sdo:jobLocationType  rdfs:comment  "A description of the job location (e.g TELECOMMUTE for telecommute jobs)." ;
        rdfs:label    "job locationType" .

sdo:OrderProcessing  rdfs:comment  "OrderStatus representing that an order is being processed." ;
        rdfs:label    "OrderProcessing" .

sdo:EventStatusType  rdfs:comment  "EventStatusType is an enumeration type whose instances represent several states that an Event may be in." ;
        rdfs:label    "EventStatusType" .

sdo:valueAddedTaxIncluded
        rdfs:comment  "Specifies whether the applicable value-added tax (VAT) is included in the price specification or not." ;
        rdfs:label    "value addedTaxIncluded" .

sdo:ReplyAction  rdfs:comment  "The act of responding to a question/message asked/sent by the object. Related to [[AskAction]]\\n\\nRelated actions:\\n\\n* [[AskAction]]: Appears generally as an origin of a ReplyAction." ;
        rdfs:label    "ReplyAction" .

sdo:lyricist  rdfs:comment  "The person who wrote the words." ;
        rdfs:label    "lyricist" .

sdo:FAQPage  rdfs:comment  "A [[FAQPage]] is a [[WebPage]] presenting one or more \"[Frequently asked questions](https://en.wikipedia.org/wiki/FAQ)\" (see also [[QAPage]])." ;
        rdfs:label    "FAQPage" .

sdo:SuperficialAnatomy
        rdfs:comment  "Anatomical features that can be observed by sight (without dissection), including the form and proportions of the human body as well as surface landmarks that correspond to deeper subcutaneous structures. Superficial anatomy plays an important role in sports medicine, phlebotomy, and other medical specialties as underlying anatomical structures can be identified through surface palpation. For example, during back surgery, superficial anatomy can be used to palpate and count vertebrae to find the site of incision. Or in phlebotomy, superficial anatomy can be used to locate an underlying vein; for example, the median cubital vein can be located by palpating the borders of the cubital fossa (such as the epicondyles of the humerus) and then looking for the superficial signs of the vein, such as size, prominence, ability to refill after depression, and feel of surrounding tissue support. As another example, in a subluxation (dislocation) of the glenohumeral joint, the bony structure becomes pronounced with the deltoid muscle failing to cover the glenohumeral joint allowing the edges of the scapula to be superficially visible. Here, the superficial anatomy is the visible edges of the scapula, implying the underlying dislocation of the joint (the related anatomical structure)." ;
        rdfs:label    "SuperficialAnatomy" .

sdo:legalName  rdfs:comment  "The official name of the organization, e.g. the registered company name." ;
        rdfs:label    "legal name" .

sdo:MusicVenue  rdfs:comment  "A music venue." ;
        rdfs:label    "MusicVenue" .

sdo:Neck  rdfs:comment  "Neck assessment with clinical examination." ;
        rdfs:label    "Neck" .

sdo:EUEnergyEfficiencyCategoryA2Plus
        rdfs:comment  "Represents EU Energy Efficiency Class A++ as defined in EU energy labeling regulations." ;
        rdfs:label    "EUEnergyEfficiencyCategoryA2Plus" .

sdo:UserPlusOnes  rdfs:comment  "UserInteraction and its subtypes is an old way of talking about users interacting with pages. It is generally better to use [[Action]]-based vocabulary, alongside types such as [[Comment]]." ;
        rdfs:label    "UserPlusOnes" .

sdo:variesBy  rdfs:comment  "Indicates the property or properties by which the variants in a [[ProductGroup]] vary, e.g. their size, color etc. Schema.org properties can be referenced by their short name e.g. \"color\"; terms defined elsewhere can be referenced with their URIs." ;
        rdfs:label    "varies by" .

sdo:LeftHandDriving  rdfs:comment  "The steering position is on the left side of the vehicle (viewed from the main direction of driving)." ;
        rdfs:label    "LeftHandDriving" .

sdo:healthPlanDrugTier
        rdfs:comment  "The tier(s) of drugs offered by this formulary or insurance plan." ;
        rdfs:label    "health planDrugTier" .

sdo:photos  rdfs:comment  "Photographs of this place." ;
        rdfs:label    "photos" .

sdo:AutoRental  rdfs:comment  "A car rental business." ;
        rdfs:label    "AutoRental" .

sdo:educationalUse  rdfs:comment  "The purpose of a work in the context of education; for example, 'assignment', 'group work'." ;
        rdfs:label    "educational use" .

sdo:typicalAgeRange  rdfs:comment  "The typical expected age range, e.g. '7-9', '11-'." ;
        rdfs:label    "typical ageRange" .

sdo:toRecipient  rdfs:comment  "A sub property of recipient. The recipient who was directly sent the message." ;
        rdfs:label    "to recipient" .

sdo:WearableMeasurementLength
        rdfs:comment  "Represents the length, for example of a dress" ;
        rdfs:label    "WearableMeasurementLength" .

sdo:HinduTemple  rdfs:comment  "A Hindu temple." ;
        rdfs:label    "HinduTemple" .

sdo:SafetyHealthAspect
        rdfs:comment  "Content about the safety-related aspects of a health topic." ;
        rdfs:label    "SafetyHealthAspect" .

sdo:paymentMethod  rdfs:comment  "The name of the credit card or other method of payment for the order." ;
        rdfs:label    "payment method" .

sdo:RadioChannel  rdfs:comment  "A unique instance of a radio BroadcastService on a CableOrSatelliteService lineup." ;
        rdfs:label    "RadioChannel" .

sdo:hospitalAffiliation
        rdfs:comment  "A hospital with which the physician or office is affiliated." ;
        rdfs:label    "hospital affiliation" .

sdo:iataCode  rdfs:comment  "IATA identifier for an airline or airport." ;
        rdfs:label    "iata code" .

sdo:Time  rdfs:comment  "A point in time recurring on multiple days in the form hh:mm:ss[Z|(+|-)hh:mm] (see [XML schema for details](http://www.w3.org/TR/xmlschema-2/#time))." ;
        rdfs:label    "Time" .

sdo:broker  rdfs:comment  "An entity that arranges for an exchange between a buyer and a seller.  In most cases a broker never acquires or releases ownership of a product or service involved in an exchange.  If it is not clear whether an entity is a broker, seller, or buyer, the latter two terms are preferred." ;
        rdfs:label    "broker" .

sdo:query  rdfs:comment  "A sub property of instrument. The query used on this action." ;
        rdfs:label    "query" .

sdo:AerobicActivity  rdfs:comment  "Physical activity of relatively low intensity that depends primarily on the aerobic energy-generating process; during activity, the aerobic metabolism uses oxygen to adequately meet energy demands during exercise." ;
        rdfs:label    "AerobicActivity" .

sdo:typeOfBed  rdfs:comment  "The type of bed to which the BedDetail refers, i.e. the type of bed available in the quantity indicated by quantity." ;
        rdfs:label    "type ofBed" .

sdo:TouristDestination
        rdfs:comment  "A tourist destination. In principle any [[Place]] can be a [[TouristDestination]] from a [[City]], Region or [[Country]] to an [[AmusementPark]] or [[Hotel]]. This Type can be used on its own to describe a general [[TouristDestination]], or be used as an [[additionalType]] to add tourist relevant properties to any other [[Place]].  A [[TouristDestination]] is defined as a [[Place]] that contains, or is colocated with, one or more [[TouristAttraction]]s, often linked by a similar theme or interest to a particular [[touristType]]. The [UNWTO](http://www2.unwto.org/) defines Destination (main destination of a tourism trip) as the place visited that is central to the decision to take the trip.\n  (See examples below)." ;
        rdfs:label    "TouristDestination" .

sdo:inAlbum  rdfs:comment  "The album to which this recording belongs." ;
        rdfs:label    "in album" .

sdo:recipient  rdfs:comment  "A sub property of participant. The participant who is at the receiving end of the action." ;
        rdfs:label    "recipient" .

sdo:studyDesign  rdfs:comment  "Specifics about the observational study design (enumerated)." ;
        rdfs:label    "study design" .

sdo:LocationFeatureSpecification
        rdfs:comment  "Specifies a location feature by providing a structured value representing a feature of an accommodation as a property-value pair of varying degrees of formality." ;
        rdfs:label    "LocationFeatureSpecification" .

sdo:EducationalOrganization
        rdfs:comment  "An educational organization." ;
        rdfs:label    "EducationalOrganization" .

sdo:VinylFormat  rdfs:comment  "VinylFormat." ;
        rdfs:label    "VinylFormat" .

sdo:specialOpeningHoursSpecification
        rdfs:comment  "The special opening hours of a certain place.\\n\\nUse this to explicitly override general opening hours brought in scope by [[openingHoursSpecification]] or [[openingHours]].\n      " ;
        rdfs:label    "special openingHoursSpecification" .

sdo:CafeOrCoffeeShop  rdfs:comment  "A cafe or coffee shop." ;
        rdfs:label    "CafeOrCoffeeShop" .

sdo:producer  rdfs:comment  "The person or organization who produced the work (e.g. music album, movie, tv/radio series etc.)." ;
        rdfs:label    "producer" .

sdo:totalPaymentDue  rdfs:comment  "The total amount due." ;
        rdfs:label    "total paymentDue" .

sdo:courseWorkload  rdfs:comment  "The amount of work expected of students taking the course, often provided as a figure per week or per month, and may be broken down by type. For example, \"2 hours of lectures, 1 hour of lab work and 3 hours of independent study per week\"." ;
        rdfs:label    "course workload" .

sdo:percentile75  rdfs:comment  "The 75th percentile value." ;
        rdfs:label    "percentile75" .

sdo:LendAction  rdfs:comment  "The act of providing an object under an agreement that it will be returned at a later date. Reciprocal of BorrowAction.\\n\\nRelated actions:\\n\\n* [[BorrowAction]]: Reciprocal of LendAction." ;
        rdfs:label    "LendAction" .

sdo:ShoppingCenter  rdfs:comment  "A shopping center or mall." ;
        rdfs:label    "ShoppingCenter" .

sdo:ScreeningEvent  rdfs:comment  "A screening of a movie or other video." ;
        rdfs:label    "ScreeningEvent" .

sdo:BodyMeasurementArm
        rdfs:comment  "Arm length (measured between arms/shoulder line intersection and the prominent wrist bone). Used, for example, to fit shirts." ;
        rdfs:label    "BodyMeasurementArm" .

sdo:timeRequired  rdfs:comment  "Approximate or typical time it takes to work with or through this learning resource for the typical intended target audience, e.g. 'PT30M', 'PT1H25M'." ;
        rdfs:label    "time required" .

sdo:ActionStatusType  rdfs:comment  "The status of an Action." ;
        rdfs:label    "ActionStatusType" .

sdo:requiredQuantity  rdfs:comment  "The required quantity of the item(s)." ;
        rdfs:label    "required quantity" .

sdo:steps  rdfs:comment  "A single step item (as HowToStep, text, document, video, etc.) or a HowToSection (originally misnamed 'steps'; 'step' is preferred)." ;
        rdfs:label    "steps" .

sdo:WearableSizeGroupShort
        rdfs:comment  "Size group \"Short\" for wearables." ;
        rdfs:label    "WearableSizeGroupShort" .

sdo:UseAction  rdfs:comment  "The act of applying an object to its intended purpose." ;
        rdfs:label    "UseAction" .

sdo:ShippingDeliveryTime
        rdfs:comment  "ShippingDeliveryTime provides various pieces of information about delivery times for shipping." ;
        rdfs:label    "ShippingDeliveryTime" .

sdo:FundingAgency  rdfs:comment  "A FundingAgency is an organization that implements one or more [[FundingScheme]]s and manages\n    the granting process (via [[Grant]]s, typically [[MonetaryGrant]]s).\n    A funding agency is not always required for grant funding, e.g. philanthropic giving, corporate sponsorship etc.\n    \nExamples of funding agencies include ERC, REA, NIH, Bill and Melinda Gates Foundation...\n    " ;
        rdfs:label    "FundingAgency" .

sdo:checkoutTime  rdfs:comment  "The latest someone may check out of a lodging establishment." ;
        rdfs:label    "checkout time" .

sdo:transcript  rdfs:comment  "If this MediaObject is an AudioObject or VideoObject, the transcript of that object." ;
        rdfs:label    "transcript" .

sdo:loanMortgageMandateAmount
        rdfs:comment  "Amount of mortgage mandate that can be converted into a proper mortgage at a later stage." ;
        rdfs:label    "loan mortgageMandateAmount" .

sdo:alignmentType  rdfs:comment  "A category of alignment between the learning resource and the framework node. Recommended values include: 'requires', 'textComplexity', 'readingLevel', and 'educationalSubject'." ;
        rdfs:label    "alignment type" .

sdo:WearableMeasurementHeight
        rdfs:comment  "Measurement of the height, for example the heel height of a shoe" ;
        rdfs:label    "WearableMeasurementHeight" .

sdo:executableLibraryName
        rdfs:comment  "Library file name e.g., mscorlib.dll, system.web.dll." ;
        rdfs:label    "executable libraryName" .

sdo:DiagnosticLab  rdfs:comment  "A medical laboratory that offers on-site or off-site diagnostic services." ;
        rdfs:label    "DiagnosticLab" .

sdo:HealthClub  rdfs:comment  "A health club." ;
        rdfs:label    "HealthClub" .

sdo:CityHall  rdfs:comment  "A city hall." ;
        rdfs:label    "CityHall" .

sdo:softwareHelp  rdfs:comment  "Software application help." ;
        rdfs:label    "software help" .

sdo:availableAtOrFrom
        rdfs:comment  "The place(s) from which the offer can be obtained (e.g. store locations)." ;
        rdfs:label    "available atOrFrom" .

sdo:dateModified  rdfs:comment  "The date on which the CreativeWork was most recently modified or when the item's entry was modified within a DataFeed." ;
        rdfs:label    "date modified" .

sdo:AccountingService
        rdfs:comment  "Accountancy business.\\n\\nAs a [[LocalBusiness]] it can be described as a [[provider]] of one or more [[Service]]\\(s).\n      " ;
        rdfs:label    "AccountingService" .

sdo:Festival  rdfs:comment  "Event type: Festival." ;
        rdfs:label    "Festival" .

sdo:includesHealthPlanFormulary
        rdfs:comment  "Formularies covered by this plan." ;
        rdfs:label    "includes healthPlanFormulary" .

sdo:members  rdfs:comment  "A member of this organization." ;
        rdfs:label    "members" .

sdo:OnDemandEvent  rdfs:comment  "A publication event e.g. catch-up TV or radio podcast, during which a program is available on-demand." ;
        rdfs:label    "OnDemandEvent" .

sdo:SeaBodyOfWater  rdfs:comment  "A sea (for example, the Caspian sea)." ;
        rdfs:label    "SeaBodyOfWater" .

sdo:Waterfall  rdfs:comment  "A waterfall, like Niagara." ;
        rdfs:label    "Waterfall" .

sdo:numChildren  rdfs:comment  "The number of children staying in the unit." ;
        rdfs:label    "num children" .

sdo:FinancialService  rdfs:comment  "Financial services business." ;
        rdfs:label    "FinancialService" .

sdo:box  rdfs:comment  "A box is the area enclosed by the rectangle formed by two points. The first point is the lower corner, the second point is the upper corner. A box is expressed as two points separated by a space character." ;
        rdfs:label    "box" .

sdo:repeatFrequency  rdfs:comment  "Defines the frequency at which [[Event]]s will occur according to a schedule [[Schedule]]. The intervals between\n      events should be defined as a [[Duration]] of time." ;
        rdfs:label    "repeat frequency" .

sdo:proteinContent  rdfs:comment  "The number of grams of protein." ;
        rdfs:label    "protein content" .

sdo:risks  rdfs:comment  "Specific physiologic risks associated to the diet plan." ;
        rdfs:label    "risks" .

sdo:WearAction  rdfs:comment  "The act of dressing oneself in clothing." ;
        rdfs:label    "WearAction" .

sdo:accessModeSufficient
        rdfs:comment  "A list of single or combined accessModes that are sufficient to understand all the intellectual content of a resource. Expected values include:  auditory, tactile, textual, visual.\n      " ;
        rdfs:label    "access modeSufficient" .

sdo:ownershipFundingInfo
        rdfs:comment  "For an [[Organization]] (often but not necessarily a [[NewsMediaOrganization]]), a description of organizational ownership structure; funding and grants. In a news/media setting, this is with particular reference to editorial independence.   Note that the [[funder]] is also available and can be used to make basic funder information machine-readable." ;
        rdfs:label    "ownership fundingInfo" .

sdo:acceptsReservations
        rdfs:comment  "Indicates whether a FoodEstablishment accepts reservations. Values can be Boolean, an URL at which reservations can be made or (for backwards compatibility) the strings ```Yes``` or ```No```." ;
        rdfs:label    "accepts reservations" .

sdo:procedure  rdfs:comment  "A description of the procedure involved in setting up, using, and/or installing the device." ;
        rdfs:label    "procedure" .

sdo:SheetMusic  rdfs:comment  "Printed music, as opposed to performed or recorded music." ;
        rdfs:label    "SheetMusic" .

sdo:WearableMeasurementTypeEnumeration
        rdfs:comment  "Enumerates common types of measurement for wearables products." ;
        rdfs:label    "WearableMeasurementTypeEnumeration" .

sdo:printColumn  rdfs:comment  "The number of the column in which the NewsArticle appears in the print edition." ;
        rdfs:label    "print column" .

sdo:offeredBy  rdfs:comment  "A pointer to the organization or person making the offer." ;
        rdfs:label    "offered by" .

sdo:productID  rdfs:comment  "The product identifier, such as ISBN. For example: ``` meta itemprop=\"productID\" content=\"isbn:123-456-789\" ```." ;
        rdfs:label    "product id" .

sdo:responsibilities  rdfs:comment  "Responsibilities associated with this role or Occupation." ;
        rdfs:label    "responsibilities" .

sdo:nextItem  rdfs:comment  "A link to the ListItem that follows the current one." ;
        rdfs:label    "next item" .

sdo:eligibleQuantity  rdfs:comment  "The interval and unit of measurement of ordering quantities for which the offer or price specification is valid. This allows e.g. specifying that a certain freight charge is valid only for a certain quantity." ;
        rdfs:label    "eligible quantity" .

sdo:bookEdition  rdfs:comment  "The edition of the book." ;
        rdfs:label    "book edition" .

sdo:resultReview  rdfs:comment  "A sub property of result. The review that resulted in the performing of the action." ;
        rdfs:label    "result review" .

sdo:UserLikes  rdfs:comment  "UserInteraction and its subtypes is an old way of talking about users interacting with pages. It is generally better to use [[Action]]-based vocabulary, alongside types such as [[Comment]]." ;
        rdfs:label    "UserLikes" .

sdo:usageInfo  rdfs:comment  "The schema.org [[usageInfo]] property indicates further information about a [[CreativeWork]]. This property is applicable both to works that are freely available and to those that require payment or other transactions. It can reference additional information e.g. community expectations on preferred linking and citation conventions, as well as purchasing details. For something that can be commercially licensed, usageInfo can provide detailed, resource-specific information about licensing options.\n\nThis property can be used alongside the license property which indicates license(s) applicable to some piece of content. The usageInfo property can provide information about other licensing options, e.g. acquiring commercial usage rights for an image that is also available under non-commercial creative commons licenses." ;
        rdfs:label    "usage info" .

sdo:videoFrameSize  rdfs:comment  "The frame size of the video." ;
        rdfs:label    "video frameSize" .

sdo:Nonprofit501c3  rdfs:comment  "Nonprofit501c3: Non-profit type referring to Religious, Educational, Charitable, Scientific, Literary, Testing for Public Safety, to Foster National or International Amateur Sports Competition, or Prevention of Cruelty to Children or Animals Organizations." ;
        rdfs:label    "Nonprofit501c3" .

sdo:appliesToDeliveryMethod
        rdfs:comment  "The delivery method(s) to which the delivery charge or payment charge specification applies." ;
        rdfs:label    "applies toDeliveryMethod" .

sdo:Motorcycle  rdfs:comment  "A motorcycle or motorbike is a single-track, two-wheeled motor vehicle." ;
        rdfs:label    "Motorcycle" .

sdo:Cardiovascular  rdfs:comment  "A specific branch of medical science that pertains to diagnosis and treatment of disorders of heart and vasculature." ;
        rdfs:label    "Cardiovascular" .

sdo:numberOfCredits  rdfs:comment  "The number of credits or units awarded by a Course or required to complete an EducationalOccupationalProgram." ;
        rdfs:label    "number ofCredits" .

sdo:howPerformed  rdfs:comment  "How the procedure is performed." ;
        rdfs:label    "how performed" .

sdo:RejectAction  rdfs:comment  "The act of rejecting to/adopting an object.\\n\\nRelated actions:\\n\\n* [[AcceptAction]]: The antonym of RejectAction." ;
        rdfs:label    "RejectAction" .

sdo:Nonprofit501c26  rdfs:comment  "Nonprofit501c26: Non-profit type referring to State-Sponsored Organizations Providing Health Coverage for High-Risk Individuals." ;
        rdfs:label    "Nonprofit501c26" .

sdo:departureTerminal
        rdfs:comment  "Identifier of the flight's departure terminal." ;
        rdfs:label    "departure terminal" .

sdo:prescriptionStatus
        rdfs:comment  "Indicates the status of drug prescription eg. local catalogs classifications or whether the drug is available by prescription or over-the-counter, etc." ;
        rdfs:label    "prescription status" .

sdo:gtin  rdfs:comment  "A Global Trade Item Number ([GTIN](https://www.gs1.org/standards/id-keys/gtin)). GTINs identify trade items, including products and services, using numeric identification codes. The [[gtin]] property generalizes the earlier [[gtin8]], [[gtin12]], [[gtin13]], and [[gtin14]] properties. The GS1 [digital link specifications](https://www.gs1.org/standards/Digital-Link/) express GTINs as URLs. A correct [[gtin]] value should be a valid GTIN, which means that it should be an all-numeric string of either 8, 12, 13 or 14 digits, or a \"GS1 Digital Link\" URL based on such a string. The numeric component should also have a [valid GS1 check digit](https://www.gs1.org/services/check-digit-calculator) and meet the other rules for valid GTINs. See also [GS1's GTIN Summary](http://www.gs1.org/barcodes/technical/idkeys/gtin) and [Wikipedia](https://en.wikipedia.org/wiki/Global_Trade_Item_Number) for more details. Left-padding of the gtin values is not required or encouraged.\n   " ;
        rdfs:label    "gtin" .

sdo:AuthoritativeLegalValue
        rdfs:comment  "Indicates that the publisher gives some special status to the publication of the document. (\"The Queens Printer\" version of a UK Act of Parliament, or the PDF version of a Directive published by the EU Office of Publications). Something \"Authoritative\" is considered to be also [[OfficialLegalValue]]\"." ;
        rdfs:label    "AuthoritativeLegalValue" .

sdo:currenciesAccepted
        rdfs:comment  "The currency accepted.\\n\\nUse standard formats: [ISO 4217 currency format](http://en.wikipedia.org/wiki/ISO_4217) e.g. \"USD\"; [Ticker symbol](https://en.wikipedia.org/wiki/List_of_cryptocurrencies) for cryptocurrencies e.g. \"BTC\"; well known names for [Local Exchange Tradings Systems](https://en.wikipedia.org/wiki/Local_exchange_trading_system) (LETS) and other currency types e.g. \"Ithaca HOUR\"." ;
        rdfs:label    "currencies accepted" .

sdo:athlete  rdfs:comment  "A person that acts as performing member of a sports team; a player as opposed to a coach." ;
        rdfs:label    "athlete" .

sdo:NonprofitSBBI  rdfs:comment  "NonprofitSBBI: Non-profit type referring to a Social Interest Promoting Institution (NL)." ;
        rdfs:label    "NonprofitSBBI" .

sdo:sdDatePublished  rdfs:comment  "Indicates the date on which the current structured data was generated / published. Typically used alongside [[sdPublisher]]" ;
        rdfs:label    "sd datePublished" .

sdo:interactionCount  rdfs:comment  "This property is deprecated, alongside the UserInteraction types on which it depended." ;
        rdfs:label    "interaction count" .

sdo:healthPlanDrugOption
        rdfs:comment  "" ;
        rdfs:label    "health planDrugOption" .

sdo:EmailMessage  rdfs:comment  "An email message." ;
        rdfs:label    "EmailMessage" .

sdo:priceComponent  rdfs:comment  "This property links to all [[UnitPriceSpecification]] nodes that apply in parallel for the [[CompoundPriceSpecification]] node." ;
        rdfs:label    "price component" .

sdo:commentText  rdfs:comment  "The text of the UserComment." ;
        rdfs:label    "comment text" .

sdo:arrivalBusStop  rdfs:comment  "The stop or station from which the bus arrives." ;
        rdfs:label    "arrival busStop" .

sdo:Subscription  rdfs:comment  "Represents the subscription pricing component of the total price for an offered product." ;
        rdfs:label    "Subscription" .

sdo:unsaturatedFatContent
        rdfs:comment  "The number of grams of unsaturated fat." ;
        rdfs:label    "unsaturated fatContent" .

sdo:PaymentCard  rdfs:comment  "A payment method using a credit, debit, store or other card to associate the payment with an account." ;
        rdfs:label    "PaymentCard" .

sdo:telephone  rdfs:comment  "The telephone number." ;
        rdfs:label    "telephone" .

sdo:musicCompositionForm
        rdfs:comment  "The type of composition (e.g. overture, sonata, symphony, etc.)." ;
        rdfs:label    "music compositionForm" .

sdo:workPerformed  rdfs:comment  "A work performed in some event, for example a play performed in a TheaterEvent." ;
        rdfs:label    "work performed" .

sdo:ReviewAction  rdfs:comment  "The act of producing a balanced opinion about the object for an audience. An agent reviews an object with participants resulting in a review." ;
        rdfs:label    "ReviewAction" .

sdo:regionsAllowed  rdfs:comment  "The regions where the media is allowed. If not specified, then it's assumed to be allowed everywhere. Specify the countries in [ISO 3166 format](http://en.wikipedia.org/wiki/ISO_3166)." ;
        rdfs:label    "regions allowed" .

sdo:sizeSystem  rdfs:comment  "The size system used to identify a product's size. Typically either a standard (for example, \"GS1\" or \"ISO-EN13402\"), country code (for example \"US\" or \"JP\"), or a measuring system (for example \"Metric\" or \"Imperial\")." ;
        rdfs:label    "size system" .

sdo:Patient  rdfs:comment  "A patient is any person recipient of health care services." ;
        rdfs:label    "Patient" .

sdo:BookFormatType  rdfs:comment  "The publication format of the book." ;
        rdfs:label    "BookFormatType" .

sdo:MobileApplication
        rdfs:comment  "A software application designed specifically to work well on a mobile device such as a telephone." ;
        rdfs:label    "MobileApplication" .

sdo:department  rdfs:comment  "A relationship between an organization and a department of that organization, also described as an organization (allowing different urls, logos, opening hours). For example: a store with a pharmacy, or a bakery with a cafe." ;
        rdfs:label    "department" .

sdo:PreOrder  rdfs:comment  "Indicates that the item is available for pre-order." ;
        rdfs:label    "PreOrder" .

sdo:additionalName  rdfs:comment  "An additional name for a Person, can be used for a middle name." ;
        rdfs:label    "additional name" .

sdo:browserRequirements
        rdfs:comment  "Specifies browser requirements in human-readable text. For example, 'requires HTML5 support'." ;
        rdfs:label    "browser requirements" .

sdo:SearchResultsPage
        rdfs:comment  "Web page type: Search results page." ;
        rdfs:label    "SearchResultsPage" .

sdo:OutOfStock  rdfs:comment  "Indicates that the item is out of stock." ;
        rdfs:label    "OutOfStock" .

sdo:PublicHolidays  rdfs:comment  "This stands for any day that is a public holiday; it is a placeholder for all official public holidays in some particular location. While not technically a \"day of the week\", it can be used with [[OpeningHoursSpecification]]. In the context of an opening hours specification it can be used to indicate opening hours on public holidays, overriding general opening hours for the day of the week on which a public holiday occurs." ;
        rdfs:label    "PublicHolidays" .

sdo:DiagnosticProcedure
        rdfs:comment  "A medical procedure intended primarily for diagnostic, as opposed to therapeutic, purposes." ;
        rdfs:label    "DiagnosticProcedure" .

sdo:MensClothingStore
        rdfs:comment  "A men's clothing store." ;
        rdfs:label    "MensClothingStore" .

sdo:UKTrust  rdfs:comment  "UKTrust: Non-profit type referring to a UK trust." ;
        rdfs:label    "UKTrust" .

sdo:successorOf  rdfs:comment  "A pointer from a newer variant of a product  to its previous, often discontinued predecessor." ;
        rdfs:label    "successor of" .

sdo:RandomizedTrial  rdfs:comment  "A randomized trial design." ;
        rdfs:label    "RandomizedTrial" .

sdo:guidelineSubject  rdfs:comment  "The medical conditions, treatments, etc. that are the subject of the guideline." ;
        rdfs:label    "guideline subject" .

sdo:broadcastFrequencyValue
        rdfs:comment  "The frequency in MHz for a particular broadcast." ;
        rdfs:label    "broadcast frequencyValue" .

sdo:multipleValues  rdfs:comment  "Whether multiple values are allowed for the property.  Default is false." ;
        rdfs:label    "multiple values" .

sdo:seatingCapacity  rdfs:comment  "The number of persons that can be seated (e.g. in a vehicle), both in terms of the physical space available, and in terms of limitations set by law.\\n\\nTypical unit code(s): C62 for persons " ;
        rdfs:label    "seating capacity" .

sdo:contactType  rdfs:comment  "A person or organization can have different contact points, for different purposes. For example, a sales contact point, a PR contact point and so on. This property is used to specify the kind of contact point." ;
        rdfs:label    "contact type" .

sdo:numberOfLoanPayments
        rdfs:comment  "The number of payments contractually required at origination to repay the loan. For monthly paying loans this is the number of months from the contractual first payment date to the maturity date." ;
        rdfs:label    "number ofLoanPayments" .

sdo:UnitPriceSpecification
        rdfs:comment  "The price asked for a given offer by the respective organization or person." ;
        rdfs:label    "UnitPriceSpecification" .

sdo:bodyType  rdfs:comment  "Indicates the design and body style of the vehicle (e.g. station wagon, hatchback, etc.)." ;
        rdfs:label    "body type" .

sdo:MedicalStudy  rdfs:comment  "A medical study is an umbrella type covering all kinds of research studies relating to human medicine or health, including observational studies and interventional trials and registries, randomized, controlled or not. When the specific type of study is known, use one of the extensions of this type, such as MedicalTrial or MedicalObservationalStudy. Also, note that this type should be used to mark up data that describes the study itself; to tag an article that publishes the results of a study, use MedicalScholarlyArticle. Note: use the code property of MedicalEntity to store study IDs, e.g. clinicaltrials.gov ID." ;
        rdfs:label    "MedicalStudy" .

sdo:mainContentOfPage
        rdfs:comment  "Indicates if this web page element is the main subject of the page." ;
        rdfs:label    "main contentOfPage" .

sdo:logo  rdfs:comment  "An associated logo." ;
        rdfs:label    "logo" .

sdo:AllocateAction  rdfs:comment  "The act of organizing tasks/objects/events by associating resources to it." ;
        rdfs:label    "AllocateAction" .

sdo:driveWheelConfiguration
        rdfs:comment  "The drive wheel configuration, i.e. which roadwheels will receive torque from the vehicle's engine via the drivetrain." ;
        rdfs:label    "drive wheelConfiguration" .

sdo:associatedMedia  rdfs:comment  "A media object that encodes this CreativeWork. This property is a synonym for encoding." ;
        rdfs:label    "associated media" .

sdo:trainingSalary  rdfs:comment  "The estimated salary earned while in the program." ;
        rdfs:label    "training salary" .

sdo:WritePermission  rdfs:comment  "Permission to write or edit the document." ;
        rdfs:label    "WritePermission" .

sdo:MobilePhoneStore  rdfs:comment  "A store that sells mobile phones and related accessories." ;
        rdfs:label    "MobilePhoneStore" .

sdo:DrugClass  rdfs:comment  "A class of medical drugs, e.g., statins. Classes can represent general pharmacological class, common mechanisms of action, common physiological effects, etc." ;
        rdfs:label    "DrugClass" .

sdo:depth  rdfs:comment  "The depth of the item." ;
        rdfs:label    "depth" .

sdo:ToyStore  rdfs:comment  "A toy store." ;
        rdfs:label    "ToyStore" .

sdo:PalliativeProcedure
        rdfs:comment  "A medical procedure intended primarily for palliative purposes, aimed at relieving the symptoms of an underlying health condition." ;
        rdfs:label    "PalliativeProcedure" .

sdo:healthPlanCoinsuranceRate
        rdfs:comment  "Whether The rate of coinsurance expressed as a number between 0.0 and 1.0." ;
        rdfs:label    "health planCoinsuranceRate" .

sdo:hasCategoryCode  rdfs:comment  "A Category code contained in this code set." ;
        rdfs:label    "has categoryCode" .

sdo:BodyMeasurementTypeEnumeration
        rdfs:comment  "Enumerates types (or dimensions) of a person's body measurements, for example for fitting of clothes." ;
        rdfs:label    "BodyMeasurementTypeEnumeration" .

sdo:loanPaymentAmount
        rdfs:comment  "The amount of money to pay in a single payment." ;
        rdfs:label    "loan paymentAmount" .

sdo:valuePattern  rdfs:comment  "Specifies a regular expression for testing literal values according to the HTML spec." ;
        rdfs:label    "value pattern" .

sdo:organizer  rdfs:comment  "An organizer of an Event." ;
        rdfs:label    "organizer" .

sdo:ParcelDelivery  rdfs:comment  "The delivery of a parcel either via the postal service or a commercial service." ;
        rdfs:label    "ParcelDelivery" .

sdo:skills  rdfs:comment  "A statement of knowledge, skill, ability, task or any other assertion expressing a competency that is desired or required to fulfill this role or to work in this occupation." ;
        rdfs:label    "skills" .

sdo:Specialty  rdfs:comment  "Any branch of a field in which people typically develop specific expertise, usually after significant study, time, and effort." ;
        rdfs:label    "Specialty" .

sdo:discount  rdfs:comment  "Any discount applied (to an Order)." ;
        rdfs:label    "discount" .

sdo:chemicalComposition
        rdfs:comment  "The chemical composition describes the identity and relative ratio of the chemical elements that make up the substance." ;
        rdfs:label    "chemical composition" .

sdo:CategoryCode  rdfs:comment  "A Category Code." ;
        rdfs:label    "CategoryCode" .

sdo:Reservation  rdfs:comment  "Describes a reservation for travel, dining or an event. Some reservations require tickets. \\n\\nNote: This type is for information about actual reservations, e.g. in confirmation emails or HTML pages with individual confirmations of reservations. For offers of tickets, restaurant reservations, flights, or rental cars, use [[Offer]]." ;
        rdfs:label    "Reservation" .

sdo:includesHealthPlanNetwork
        rdfs:comment  "Networks covered by this plan." ;
        rdfs:label    "includes healthPlanNetwork" .

sdo:CampingPitch  rdfs:comment  "A [[CampingPitch]] is an individual place for overnight stay in the outdoors, typically being part of a larger camping site, or [[Campground]].\\n\\n\nIn British English a campsite, or campground, is an area, usually divided into a number of pitches, where people can camp overnight using tents or camper vans or caravans; this British English use of the word is synonymous with the American English expression campground. In American English the term campsite generally means an area where an individual, family, group, or military unit can pitch a tent or park a camper; a campground may contain many campsites.\n(Source: Wikipedia see [https://en.wikipedia.org/wiki/Campsite](https://en.wikipedia.org/wiki/Campsite)).\\n\\n\nSee also the dedicated [document on the use of schema.org for marking up hotels and other forms of accommodations](/docs/hotels.html).\n" ;
        rdfs:label    "CampingPitch" .

sdo:bed  rdfs:comment  "The type of bed or beds included in the accommodation. For the single case of just one bed of a certain type, you use bed directly with a text.\n      If you want to indicate the quantity of a certain kind of bed, use an instance of BedDetails. For more detailed information, use the amenityFeature property." ;
        rdfs:label    "bed" .

sdo:fromLocation  rdfs:comment  "A sub property of location. The original location of the object or the agent before the action." ;
        rdfs:label    "from location" .

sdo:OfferCatalog  rdfs:comment  "An OfferCatalog is an ItemList that contains related Offers and/or further OfferCatalogs that are offeredBy the same provider." ;
        rdfs:label    "OfferCatalog" .

sdo:LockerDelivery  rdfs:comment  "A DeliveryMethod in which an item is made available via locker." ;
        rdfs:label    "LockerDelivery" .

sdo:applicationCategory
        rdfs:comment  "Type of software application, e.g. 'Game, Multimedia'." ;
        rdfs:label    "application category" .

sdo:TennisComplex  rdfs:comment  "A tennis complex." ;
        rdfs:label    "TennisComplex" .

sdo:QuantitativeValueDistribution
        rdfs:comment  "A statistical distribution of values." ;
        rdfs:label    "QuantitativeValueDistribution" .

sdo:warning  rdfs:comment  "Any FDA or other warnings about the drug (text or URL)." ;
        rdfs:label    "warning" .

sdo:reviewBody  rdfs:comment  "The actual body of the review." ;
        rdfs:label    "review body" .

sdo:targetPopulation  rdfs:comment  "Characteristics of the population for which this is intended, or which typically uses it, e.g. 'adults'." ;
        rdfs:label    "target population" .

sdo:parentService  rdfs:comment  "A broadcast service to which the broadcast service may belong to such as regional variations of a national channel." ;
        rdfs:label    "parent service" .

sdo:albumProductionType
        rdfs:comment  "Classification of the album by it's type of content: soundtrack, live album, studio album, etc." ;
        rdfs:label    "album productionType" .

sdo:monthsOfExperience
        rdfs:comment  "Indicates the minimal number of months of experience required for a position." ;
        rdfs:label    "months ofExperience" .

sdo:Occupation  rdfs:comment  "A profession, may involve prolonged training and/or a formal qualification." ;
        rdfs:label    "Occupation" .

sdo:guideline  rdfs:comment  "A medical guideline related to this entity." ;
        rdfs:label    "guideline" .

sdo:PaintAction  rdfs:comment  "The act of producing a painting, typically with paint and canvas as instruments." ;
        rdfs:label    "PaintAction" .

sdo:nerveMotor  rdfs:comment  "The neurological pathway extension that involves muscle control." ;
        rdfs:label    "nerve motor" .

sdo:maxPrice  rdfs:comment  "The highest price if the price is a range." ;
        rdfs:label    "max price" .

sdo:handlingTime  rdfs:comment  "The typical delay between the receipt of the order and the goods either leaving the warehouse or being prepared for pickup, in case the delivery method is on site pickup. Typical properties: minValue, maxValue, unitCode (d for DAY).  This is by common convention assumed to mean business days (if a unitCode is used, coded as \"d\"), i.e. only counting days when the business normally operates." ;
        rdfs:label    "handling time" .

sdo:molecularWeight  rdfs:comment  "This is the molecular weight of the entity being described, not of the parent. Units should be included in the form '&lt;Number&gt; &lt;unit&gt;', for example '12 amu' or as '&lt;QuantitativeValue&gt;." ;
        rdfs:label    "molecular weight" .

sdo:validIn  rdfs:comment  "The geographic area where a permit or similar thing is valid." ;
        rdfs:label    "valid in" .

sdo:thumbnailUrl  rdfs:comment  "A thumbnail image relevant to the Thing." ;
        rdfs:label    "thumbnail url" .

sdo:musicBy  rdfs:comment  "The composer of the soundtrack." ;
        rdfs:label    "music by" .

sdo:numberOfRooms  rdfs:comment  "The number of rooms (excluding bathrooms and closets) of the accommodation or lodging business.\nTypical unit code(s): ROM for room or C62 for no unit. The type of room can be put in the unitText property of the QuantitativeValue." ;
        rdfs:label    "number ofRooms" .

sdo:TouristInformationCenter
        rdfs:comment  "A tourist information center." ;
        rdfs:label    "TouristInformationCenter" .

sdo:DanceEvent  rdfs:comment  "Event type: A social dance." ;
        rdfs:label    "DanceEvent" .

sdo:SizeGroupEnumeration
        rdfs:comment  "Enumerates common size groups for various product categories." ;
        rdfs:label    "SizeGroupEnumeration" .

sdo:incentives  rdfs:comment  "Description of bonus and commission compensation aspects of the job." ;
        rdfs:label    "incentives" .

sdo:EventRescheduled  rdfs:comment  "The event has been rescheduled. The event's previousStartDate should be set to the old date and the startDate should be set to the event's new date. (If the event has been rescheduled multiple times, the previousStartDate property may be repeated)." ;
        rdfs:label    "EventRescheduled" .

sdo:ListPrice  rdfs:comment  "Represents the list price (the price a product is actually advertised for) of an offered product." ;
        rdfs:label    "ListPrice" .

sdo:Friday  rdfs:comment  "The day of the week between Thursday and Saturday." ;
        rdfs:label    "Friday" .

sdo:ProgramMembership
        rdfs:comment  "Used to describe membership in a loyalty programs (e.g. \"StarAliance\"), traveler clubs (e.g. \"AAA\"), purchase clubs (\"Safeway Club\"), etc." ;
        rdfs:label    "ProgramMembership" .

sdo:floorLevel  rdfs:comment  "The floor level for an [[Accommodation]] in a multi-storey building. Since counting\n  systems [vary internationally](https://en.wikipedia.org/wiki/Storey#Consecutive_number_floor_designations), the local system should be used where possible." ;
        rdfs:label    "floor level" .

sdo:latitude  rdfs:comment  "The latitude of a location. For example ```37.42242``` ([WGS 84](https://en.wikipedia.org/wiki/World_Geodetic_System))." ;
        rdfs:label    "latitude" .

sdo:RsvpResponseNo  rdfs:comment  "The invitee will not attend." ;
        rdfs:label    "RsvpResponseNo" .

sdo:applicationSubCategory
        rdfs:comment  "Subcategory of the application, e.g. 'Arcade Game'." ;
        rdfs:label    "application subCategory" .

sdo:totalJobOpenings  rdfs:comment  "The number of positions open for this job posting. Use a positive integer. Do not use if the number of positions is unclear or not known." ;
        rdfs:label    "total jobOpenings" .

sdo:primaryPrevention
        rdfs:comment  "A preventative therapy used to prevent an initial occurrence of the medical condition, such as vaccination." ;
        rdfs:label    "primary prevention" .

sdo:WearableSizeSystemAU
        rdfs:comment  "Australian size system for wearables." ;
        rdfs:label    "WearableSizeSystemAU" .

sdo:InStock  rdfs:comment  "Indicates that the item is in stock." ;
        rdfs:label    "InStock" .

sdo:MulticellularParasite
        rdfs:comment  "Multicellular parasite that causes an infection." ;
        rdfs:label    "MulticellularParasite" .

sdo:suggestedAnswer  rdfs:comment  "An answer (possibly one of several, possibly incorrect) to a Question, e.g. on a Question/Answer site." ;
        rdfs:label    "suggested answer" .

sdo:billingIncrement  rdfs:comment  "This property specifies the minimal quantity and rounding increment that will be the basis for the billing. The unit of measurement is specified by the unitCode property." ;
        rdfs:label    "billing increment" .

sdo:AutomatedTeller  rdfs:comment  "ATM/cash machine." ;
        rdfs:label    "AutomatedTeller" .

sdo:EUEnergyEfficiencyCategoryF
        rdfs:comment  "Represents EU Energy Efficiency Class F as defined in EU energy labeling regulations." ;
        rdfs:label    "EUEnergyEfficiencyCategoryF" .

sdo:BodyMeasurementFoot
        rdfs:comment  "Foot length (measured between end of the most prominent toe and the most prominent part of the heel). Used, for example, to measure socks." ;
        rdfs:label    "BodyMeasurementFoot" .

sdo:Recruiting  rdfs:comment  "Recruiting participants." ;
        rdfs:label    "Recruiting" .

sdo:numberOfDoors  rdfs:comment  "The number of doors.\\n\\nTypical unit code(s): C62" ;
        rdfs:label    "number ofDoors" .

sdo:dropoffTime  rdfs:comment  "When a rental car can be dropped off." ;
        rdfs:label    "dropoff time" .

sdo:caption  rdfs:comment  "The caption for this object. For downloadable machine formats (closed caption, subtitles etc.) use MediaObject and indicate the [[encodingFormat]]." ;
        rdfs:label    "caption" .

sdo:AcceptAction  rdfs:comment  "The act of committing to/adopting an object.\\n\\nRelated actions:\\n\\n* [[RejectAction]]: The antonym of AcceptAction." ;
        rdfs:label    "AcceptAction" .

sdo:relatedTo  rdfs:comment  "The most generic familial relation." ;
        rdfs:label    "related to" .

sdo:associatedMediaReview
        rdfs:comment  "An associated [[MediaReview]], related by specific common content, topic or claim. The expectation is that this property would be most typically used in cases where a single activity is conducting both claim reviews and media reviews, in which case [[relatedMediaReview]] would commonly be used on a [[ClaimReview]], while [[relatedClaimReview]] would be used on [[MediaReview]]." ;
        rdfs:label    "associated mediaReview" .

sdo:CharitableIncorporatedOrganization
        rdfs:comment  "CharitableIncorporatedOrganization: Non-profit type referring to a Charitable Incorporated Organization (UK)." ;
        rdfs:label    "CharitableIncorporatedOrganization" .

sdo:WarrantyScope  rdfs:comment  "A range of of services that will be provided to a customer free of charge in case of a defect or malfunction of a product.\\n\\nCommonly used values:\\n\\n* http://purl.org/goodrelations/v1#Labor-BringIn\\n* http://purl.org/goodrelations/v1#PartsAndLabor-BringIn\\n* http://purl.org/goodrelations/v1#PartsAndLabor-PickUp\n      " ;
        rdfs:label    "WarrantyScope" .

sdo:sampleType  rdfs:comment  "What type of code sample: full (compile ready) solution, code snippet, inline code, scripts, template." ;
        rdfs:label    "sample type" .

sdo:VenueMap  rdfs:comment  "A venue map (e.g. for malls, auditoriums, museums, etc.)." ;
        rdfs:label    "VenueMap" .

sdo:unnamedSourcesPolicy
        rdfs:comment  "For an [[Organization]] (typically a [[NewsMediaOrganization]]), a statement about policy on use of unnamed sources and the decision process required." ;
        rdfs:label    "unnamed sourcesPolicy" .

sdo:exerciseCourse  rdfs:comment  "A sub property of location. The course where this action was taken." ;
        rdfs:label    "exercise course" .

sdo:landlord  rdfs:comment  "A sub property of participant. The owner of the real estate property." ;
        rdfs:label    "landlord" .

sdo:correctionsPolicy
        rdfs:comment  "For an [[Organization]] (e.g. [[NewsMediaOrganization]]), a statement describing (in news media, the newsroom’s) disclosure and correction policy for errors." ;
        rdfs:label    "corrections policy" .

sdo:RadioEpisode  rdfs:comment  "A radio episode which can be part of a series or season." ;
        rdfs:label    "RadioEpisode" .

sdo:workFeatured  rdfs:comment  "A work featured in some event, e.g. exhibited in an ExhibitionEvent.\n       Specific subproperties are available for workPerformed (e.g. a play), or a workPresented (a Movie at a ScreeningEvent)." ;
        rdfs:label    "work featured" .

sdo:ReturnInStore  rdfs:comment  "Specifies that product returns must be made in a store." ;
        rdfs:label    "ReturnInStore" .

sdo:DepartAction  rdfs:comment  "The act of  departing from a place. An agent departs from an fromLocation for a destination, optionally with participants." ;
        rdfs:label    "DepartAction" .

sdo:EventVenue  rdfs:comment  "An event venue." ;
        rdfs:label    "EventVenue" .

sdo:dropoffLocation  rdfs:comment  "Where a rental car can be dropped off." ;
        rdfs:label    "dropoff location" .

sdo:WearableSizeSystemJP
        rdfs:comment  "Japanese size system for wearables." ;
        rdfs:label    "WearableSizeSystemJP" .

sdo:permittedUsage  rdfs:comment  "Indications regarding the permitted usage of the accommodation." ;
        rdfs:label    "permitted usage" .

sdo:offersPrescriptionByMail
        rdfs:comment  "Whether prescriptions can be delivered by mail." ;
        rdfs:label    "offers prescriptionByMail" .

sdo:broadcastAffiliateOf
        rdfs:comment  "The media network(s) whose content is broadcast on this station." ;
        rdfs:label    "broadcast affiliateOf" .

sdo:diversityStaffingReport
        rdfs:comment  "For an [[Organization]] (often but not necessarily a [[NewsMediaOrganization]]), a report on staffing diversity issues. In a news context this might be for example ASNE or RTDNA (US) reports, or self-reported." ;
        rdfs:label    "diversity staffingReport" .

sdo:OceanBodyOfWater  rdfs:comment  "An ocean (for example, the Pacific)." ;
        rdfs:label    "OceanBodyOfWater" .

sdo:incentiveCompensation
        rdfs:comment  "Description of bonus and commission compensation aspects of the job." ;
        rdfs:label    "incentive compensation" .

sdo:expressedIn  rdfs:comment  "Tissue, organ, biological sample, etc in which activity of this gene has been observed experimentally. For example brain, digestive system." ;
        rdfs:label    "expressed in" .

sdo:ExchangeRefund  rdfs:comment  "Specifies that a refund can be done as an exchange for the same product." ;
        rdfs:label    "ExchangeRefund" .

sdo:Series  rdfs:comment  "A Series in schema.org is a group of related items, typically but not necessarily of the same kind. See also [[CreativeWorkSeries]], [[EventSeries]]." ;
        rdfs:label    "Series" .

sdo:ContactPointOption
        rdfs:comment  "Enumerated options related to a ContactPoint." ;
        rdfs:label    "ContactPointOption" .

sdo:CheckAction  rdfs:comment  "An agent inspects, determines, investigates, inquires, or examines an object's accuracy, quality, condition, or state." ;
        rdfs:label    "CheckAction" .

sdo:WebApplication  rdfs:comment  "Web applications." ;
        rdfs:label    "WebApplication" .

sdo:mealService  rdfs:comment  "Description of the meals that will be provided or available for purchase." ;
        rdfs:label    "meal service" .

sdo:numberOfEmployees
        rdfs:comment  "The number of employees in an organization e.g. business." ;
        rdfs:label    "number ofEmployees" .

sdo:AlbumRelease  rdfs:comment  "AlbumRelease." ;
        rdfs:label    "AlbumRelease" .

sdo:Drawing  rdfs:comment  "A picture or diagram made with a pencil, pen, or crayon rather than paint." ;
        rdfs:label    "Drawing" .

sdo:geoOverlaps  rdfs:comment  "Represents a relationship between two geometries (or the places they represent), relating a geometry to another that geospatially overlaps it, i.e. they have some but not all points in common. As defined in [DE-9IM](https://en.wikipedia.org/wiki/DE-9IM)." ;
        rdfs:label    "geo overlaps" .

sdo:doesNotShip  rdfs:comment  "Indicates when shipping to a particular [[shippingDestination]] is not available." ;
        rdfs:label    "does notShip" .

sdo:dateCreated  rdfs:comment  "The date on which the CreativeWork was created or the item was added to a DataFeed." ;
        rdfs:label    "date created" .

sdo:PerformingGroup  rdfs:comment  "A performance group, such as a band, an orchestra, or a circus." ;
        rdfs:label    "PerformingGroup" .

sdo:LakeBodyOfWater  rdfs:comment  "A lake (for example, Lake Pontrachain)." ;
        rdfs:label    "LakeBodyOfWater" .

sdo:educationalCredentialAwarded
        rdfs:comment  "A description of the qualification, award, certificate, diploma or other educational credential awarded as a consequence of successful completion of this course or program." ;
        rdfs:label    "educational credentialAwarded" .

sdo:teaches  rdfs:comment  "The item being described is intended to help a person learn the competency or learning outcome defined by the referenced term." ;
        rdfs:label    "teaches" .

sdo:geographicArea  rdfs:comment  "The geographic area associated with the audience." ;
        rdfs:label    "geographic area" .

sdo:EventMovedOnline  rdfs:comment  "Indicates that the event was changed to allow online participation. See [[eventAttendanceMode]] for specifics of whether it is now fully or partially online." ;
        rdfs:label    "EventMovedOnline" .

sdo:hasPOS  rdfs:comment  "Points-of-Sales operated by the organization or person." ;
        rdfs:label    "has pos" .

sdo:BrainStructure  rdfs:comment  "Any anatomical structure which pertains to the soft nervous tissue functioning as the coordinating center of sensation and intellectual and nervous activity." ;
        rdfs:label    "BrainStructure" .

sdo:SaleEvent  rdfs:comment  "Event type: Sales event." ;
        rdfs:label    "SaleEvent" .

sdo:signDetected  rdfs:comment  "A sign detected by the test." ;
        rdfs:label    "sign detected" .

sdo:Nonprofit501d  rdfs:comment  "Nonprofit501d: Non-profit type referring to Religious and Apostolic Associations." ;
        rdfs:label    "Nonprofit501d" .

sdo:Property  rdfs:comment  "A property, used to indicate attributes and relationships of some Thing; equivalent to rdf:Property." ;
        rdfs:label    "Property" .

sdo:supply  rdfs:comment  "A sub-property of instrument. A supply consumed when performing instructions or a direction." ;
        rdfs:label    "supply" .

sdo:HVACBusiness  rdfs:comment  "A business that provide Heating, Ventilation and Air Conditioning services." ;
        rdfs:label    "HVACBusiness" .

sdo:CommunicateAction
        rdfs:comment  "The act of conveying information to another person via a communication medium (instrument) such as speech, email, or telephone conversation." ;
        rdfs:label    "CommunicateAction" .

sdo:serviceAudience  rdfs:comment  "The audience eligible for this service." ;
        rdfs:label    "service audience" .

sdo:ParcelService  rdfs:comment  "A private parcel service as the delivery mode available for a certain offer.\\n\\nCommonly used values:\\n\\n* http://purl.org/goodrelations/v1#DHL\\n* http://purl.org/goodrelations/v1#FederalExpress\\n* http://purl.org/goodrelations/v1#UPS\n      " ;
        rdfs:label    "ParcelService" .

sdo:subTrip  rdfs:comment  "Identifies a [[Trip]] that is a subTrip of this Trip.  For example Day 1, Day 2, etc. of a multi-day trip." ;
        rdfs:label    "sub trip" .

sdo:cvdNumBedsOcc  rdfs:comment  "numbedsocc - HOSPITAL INPATIENT BED OCCUPANCY: Total number of staffed inpatient beds that are occupied." ;
        rdfs:label    "cvd numBedsOcc" .

sdo:emissionsCO2  rdfs:comment  "The CO2 emissions in g/km. When used in combination with a QuantitativeValue, put \"g/km\" into the unitText property of that value, since there is no UN/CEFACT Common Code for \"g/km\"." ;
        rdfs:label    "emissions co2" .

sdo:departureBoatTerminal
        rdfs:comment  "The terminal or port from which the boat departs." ;
        rdfs:label    "departure boatTerminal" .

sdo:PerformanceRole  rdfs:comment  "A PerformanceRole is a Role that some entity places with regard to a theatrical performance, e.g. in a Movie, TVSeries etc." ;
        rdfs:label    "PerformanceRole" .

sdo:OnlineOnly  rdfs:comment  "Indicates that the item is available only online." ;
        rdfs:label    "OnlineOnly" .

sdo:downPayment  rdfs:comment  "a type of payment made in cash during the onset of the purchase of an expensive good/service. The payment typically represents only a percentage of the full purchase price." ;
        rdfs:label    "down payment" .

sdo:masthead  rdfs:comment  "For a [[NewsMediaOrganization]], a link to the masthead page or a page listing top editorial management." ;
        rdfs:label    "masthead" .

sdo:BankAccount  rdfs:comment  "A product or service offered by a bank whereby one may deposit, withdraw or transfer money and in some cases be paid interest." ;
        rdfs:label    "BankAccount" .

sdo:AutoWash  rdfs:comment  "A car wash business." ;
        rdfs:label    "AutoWash" .

sdo:associatedClaimReview
        rdfs:comment  "An associated [[ClaimReview]], related by specific common content, topic or claim. The expectation is that this property would be most typically used in cases where a single activity is conducting both claim reviews and media reviews, in which case [[relatedMediaReview]] would commonly be used on a [[ClaimReview]], while [[relatedClaimReview]] would be used on [[MediaReview]]." ;
        rdfs:label    "associated claimReview" .

sdo:HyperTocEntry  rdfs:comment  "A HyperToEntry is an item within a [[HyperToc]], which represents a hypertext table of contents for complex media objects, such as [[VideoObject]], [[AudioObject]]. The media object itself is indicated using [[associatedMedia]]. Each section of interest within that content can be described with a [[HyperTocEntry]], with associated [[startOffset]] and [[endOffset]]. When several entries are all from the same file, [[associatedMedia]] is used on the overarching [[HyperTocEntry]]; if the content has been split into multiple files, they can be referenced using [[associatedMedia]] on each [[HyperTocEntry]]." ;
        rdfs:label    "HyperTocEntry" .

sdo:BreadcrumbList  rdfs:comment  "A BreadcrumbList is an ItemList consisting of a chain of linked Web pages, typically described using at least their URL and their name, and typically ending with the current page.\\n\\nThe [[position]] property is used to reconstruct the order of the items in a BreadcrumbList The convention is that a breadcrumb list has an [[itemListOrder]] of [[ItemListOrderAscending]] (lower values listed first), and that the first items in this list correspond to the \"top\" or beginning of the breadcrumb trail, e.g. with a site or section homepage. The specific values of 'position' are not assigned meaning for a BreadcrumbList, but they should be integers, e.g. beginning with '1' for the first item in the list.\n      " ;
        rdfs:label    "BreadcrumbList" .

sdo:WPHeader  rdfs:comment  "The header section of the page." ;
        rdfs:label    "WPHeader" .

sdo:ratingCount  rdfs:comment  "The count of total number of ratings." ;
        rdfs:label    "rating count" .

sdo:startOffset  rdfs:comment  "The start time of the clip expressed as the number of seconds from the beginning of the work." ;
        rdfs:label    "start offset" .

sdo:VoteAction  rdfs:comment  "The act of expressing a preference from a fixed/finite/structured set of choices/options." ;
        rdfs:label    "VoteAction" .

sdo:artMedium  rdfs:comment  "The material used. (e.g. Oil, Watercolour, Acrylic, Linoprint, Marble, Cyanotype, Digital, Lithograph, DryPoint, Intaglio, Pastel, Woodcut, Pencil, Mixed Media, etc.)" ;
        rdfs:label    "art medium" .

sdo:mainEntity  rdfs:comment  "Indicates the primary entity described in some page or other CreativeWork." ;
        rdfs:label    "main entity" .

sdo:maximumAttendeeCapacity
        rdfs:comment  "The total number of individuals that may attend an event or venue." ;
        rdfs:label    "maximum attendeeCapacity" .

sdo:storageRequirements
        rdfs:comment  "Storage requirements (free space required)." ;
        rdfs:label    "storage requirements" .

sdo:MedicalRiskEstimator
        rdfs:comment  "Any rule set or interactive tool for estimating the risk of developing a complication or condition." ;
        rdfs:label    "MedicalRiskEstimator" .

sdo:UserReview  rdfs:comment  "A review created by an end-user (e.g. consumer, purchaser, attendee etc.), in contrast with [[CriticReview]]." ;
        rdfs:label    "UserReview" .

sdo:publicationType  rdfs:comment  "The type of the medical article, taken from the US NLM MeSH publication type catalog. See also [MeSH documentation](http://www.nlm.nih.gov/mesh/pubtypes.html)." ;
        rdfs:label    "publication type" .

sdo:text  rdfs:comment  "The textual content of this CreativeWork." ;
        rdfs:label    "text" .

sdo:OriginalMediaContent
        rdfs:comment  "Content coded 'as original media content' in a [[MediaReview]], considered in the context of how it was published or shared.\n\nFor a [[VideoObject]] to be 'original': No evidence the footage has been misleadingly altered or manipulated, though it may contain false or misleading claims.\n\nFor an [[ImageObject]] to be 'original': No evidence the image has been misleadingly altered or manipulated, though it may still contain false or misleading claims.\n\nFor an [[ImageObject]] with embedded text to be 'original': No evidence the image has been misleadingly altered or manipulated, though it may still contain false or misleading claims.\n\nFor an [[AudioObject]] to be 'original': No evidence the audio has been misleadingly altered or manipulated, though it may contain false or misleading claims.\n" ;
        rdfs:label    "OriginalMediaContent" .

sdo:billingAddress  rdfs:comment  "The billing address for the order." ;
        rdfs:label    "billing address" .

sdo:Sculpture  rdfs:comment  "A piece of sculpture." ;
        rdfs:label    "Sculpture" .

sdo:addOn  rdfs:comment  "An additional offer that can only be obtained in combination with the first base offer (e.g. supplements and extensions that are available for a surcharge)." ;
        rdfs:label    "add on" .

sdo:WearableSizeGroupMens
        rdfs:comment  "Size group \"Mens\" for wearables." ;
        rdfs:label    "WearableSizeGroupMens" .

sdo:instrument  rdfs:comment  "The object that helped the agent perform the action. e.g. John wrote a book with *a pen*." ;
        rdfs:label    "instrument" .

sdo:DJMixAlbum  rdfs:comment  "DJMixAlbum." ;
        rdfs:label    "DJMixAlbum" .

sdo:MedicalGuidelineContraindication
        rdfs:comment  "A guideline contraindication that designates a process as harmful and where quality of the data supporting the contraindication is sound." ;
        rdfs:label    "MedicalGuidelineContraindication" .

sdo:cvdNumC19Died  rdfs:comment  "numc19died - DEATHS: Patients with suspected or confirmed COVID-19 who died in the hospital, ED, or any overflow location." ;
        rdfs:label    "cvd numC19Died" .

sdo:greaterOrEqual  rdfs:comment  "This ordering relation for qualitative values indicates that the subject is greater than or equal to the object." ;
        rdfs:label    "greater orEqual" .

sdo:yield  rdfs:comment  "The quantity that results by performing instructions. For example, a paper airplane, 10 personalized candles." ;
        rdfs:label    "yield" .

sdo:BorrowAction  rdfs:comment  "The act of obtaining an object under an agreement to return it at a later date. Reciprocal of LendAction.\\n\\nRelated actions:\\n\\n* [[LendAction]]: Reciprocal of BorrowAction." ;
        rdfs:label    "BorrowAction" .

sdo:PatientExperienceHealthAspect
        rdfs:comment  "Content about the real life experience of patients or people that have lived a similar experience about the topic. May be forums, topics, Q-and-A and related material." ;
        rdfs:label    "PatientExperienceHealthAspect" .

sdo:distinguishingSign
        rdfs:comment  "One of a set of signs and symptoms that can be used to distinguish this diagnosis from others in the differential diagnosis." ;
        rdfs:label    "distinguishing sign" .

sdo:trackingUrl  rdfs:comment  "Tracking url for the parcel delivery." ;
        rdfs:label    "tracking url" .

sdo:warranty  rdfs:comment  "The warranty promise(s) included in the offer." ;
        rdfs:label    "warranty" .

sdo:populationType  rdfs:comment  "Indicates the populationType common to all members of a [[StatisticalPopulation]]." ;
        rdfs:label    "population type" .

sdo:WearableMeasurementSleeve
        rdfs:comment  "Measurement of the sleeve length, for example of a shirt" ;
        rdfs:label    "WearableMeasurementSleeve" .

sdo:RsvpResponseYes  rdfs:comment  "The invitee will attend." ;
        rdfs:label    "RsvpResponseYes" .

sdo:dayOfWeek  rdfs:comment  "The day of the week for which these opening hours are valid." ;
        rdfs:label    "day ofWeek" .

sdo:LodgingBusiness  rdfs:comment  "A lodging business, such as a motel, hotel, or inn." ;
        rdfs:label    "LodgingBusiness" .

sdo:departureBusStop  rdfs:comment  "The stop or station from which the bus departs." ;
        rdfs:label    "departure busStop" .

sdo:gamePlatform  rdfs:comment  "The electronic systems used to play <a href=\"http://en.wikipedia.org/wiki/Category:Video_game_platforms\">video games</a>." ;
        rdfs:label    "game platform" .

sdo:ItemAvailability  rdfs:comment  "A list of possible product availability options." ;
        rdfs:label    "ItemAvailability" .

sdo:membershipNumber  rdfs:comment  "A unique identifier for the membership." ;
        rdfs:label    "membership number" .

sdo:DatedMoneySpecification
        rdfs:comment  "A DatedMoneySpecification represents monetary values with optional start and end dates. For example, this could represent an employee's salary over a specific period of time. __Note:__ This type has been superseded by [[MonetaryAmount]] use of that type is recommended" ;
        rdfs:label    "DatedMoneySpecification" .

sdo:legislationResponsible
        rdfs:comment  "An individual or organization that has some kind of responsibility for the legislation. Typically the ministry who is/was in charge of elaborating the legislation, or the adressee for potential questions about the legislation once it is published." ;
        rdfs:label    "legislation responsible" .

sdo:BusTrip  rdfs:comment  "A trip on a commercial bus line." ;
        rdfs:label    "BusTrip" .

sdo:ComputerStore  rdfs:comment  "A computer store." ;
        rdfs:label    "ComputerStore" .

sdo:Country  rdfs:comment  "A country." ;
        rdfs:label    "Country" .

sdo:vehicleModelDate  rdfs:comment  "The release date of a vehicle model (often used to differentiate versions of the same make and model)." ;
        rdfs:label    "vehicle modelDate" .

sdo:Skin  rdfs:comment  "Skin assessment with clinical examination." ;
        rdfs:label    "Skin" .

sdo:serviceLocation  rdfs:comment  "The location (e.g. civic structure, local business, etc.) where a person can go to access the service." ;
        rdfs:label    "service location" .

sdo:eventAttendanceMode
        rdfs:comment  "The eventAttendanceMode of an event indicates whether it occurs online, offline, or a mix." ;
        rdfs:label    "event attendanceMode" .

sdo:RadiationTherapy  rdfs:comment  "A process of care using radiation aimed at improving a health condition." ;
        rdfs:label    "RadiationTherapy" .

sdo:geoCoveredBy  rdfs:comment  "Represents a relationship between two geometries (or the places they represent), relating a geometry to another that covers it. As defined in [DE-9IM](https://en.wikipedia.org/wiki/DE-9IM)." ;
        rdfs:label    "geo coveredBy" .

sdo:endorsers  rdfs:comment  "People or organizations that endorse the plan." ;
        rdfs:label    "endorsers" .

sdo:recourseLoan  rdfs:comment  "The only way you get the money back in the event of default is the security. Recourse is where you still have the opportunity to go back to the borrower for the rest of the money." ;
        rdfs:label    "recourse loan" .

sdo:arrivalAirport  rdfs:comment  "The airport where the flight terminates." ;
        rdfs:label    "arrival airport" .

sdo:StructuredValue  rdfs:comment  "Structured values are used when the value of a property has a more complex structure than simply being a textual value or a reference to another thing." ;
        rdfs:label    "StructuredValue" .

sdo:MedicalRiskFactor
        rdfs:comment  "A risk factor is anything that increases a person's likelihood of developing or contracting a disease, medical condition, or complication." ;
        rdfs:label    "MedicalRiskFactor" .

sdo:broadcastFrequency
        rdfs:comment  "The frequency used for over-the-air broadcasts. Numeric values or simple ranges e.g. 87-99. In addition a shortcut idiom is supported for frequences of AM and FM radio channels, e.g. \"87 FM\"." ;
        rdfs:label    "broadcast frequency" .

sdo:Church  rdfs:comment  "A church." ;
        rdfs:label    "Church" .

sdo:screenshot  rdfs:comment  "A link to a screenshot image of the app." ;
        rdfs:label    "screenshot" .

sdo:remainingAttendeeCapacity
        rdfs:comment  "The number of attendee places for an event that remain unallocated." ;
        rdfs:label    "remaining attendeeCapacity" .

sdo:email  rdfs:comment  "Email address." ;
        rdfs:label    "email" .

sdo:applicantLocationRequirements
        rdfs:comment  "The location(s) applicants can apply from. This is usually used for telecommuting jobs where the applicant does not need to be in a physical office. Note: This should not be used for citizenship or work visa requirements." ;
        rdfs:label    "applicant locationRequirements" .

sdo:AskPublicNewsArticle
        rdfs:comment  "A [[NewsArticle]] expressing an open call by a [[NewsMediaOrganization]] asking the public for input, insights, clarifications, anecdotes, documentation, etc., on an issue, for reporting purposes." ;
        rdfs:label    "AskPublicNewsArticle" .

sdo:PaidLeave  rdfs:comment  "PaidLeave: this is a benefit for paid leave." ;
        rdfs:label    "PaidLeave" .

sdo:CssSelectorType  rdfs:comment  "Text representing a CSS selector." ;
        rdfs:label    "CssSelectorType" .

sdo:itemShipped  rdfs:comment  "Item(s) being shipped." ;
        rdfs:label    "item shipped" .

sdo:Nonprofit501n  rdfs:comment  "Nonprofit501n: Non-profit type referring to Charitable Risk Pools." ;
        rdfs:label    "Nonprofit501n" .

sdo:associatedDisease
        rdfs:comment  "Disease associated to this BioChemEntity. Such disease can be a MedicalCondition or a URL. If you want to add an evidence supporting the association, please use PropertyValue." ;
        rdfs:label    "associated disease" .

sdo:countryOfAssembly
        rdfs:comment  "The place where the product was assembled." ;
        rdfs:label    "country ofAssembly" .

sdo:deliveryTime  rdfs:comment  "The total delay between the receipt of the order and the goods reaching the final customer." ;
        rdfs:label    "delivery time" .

sdo:TrackAction  rdfs:comment  "An agent tracks an object for updates.\\n\\nRelated actions:\\n\\n* [[FollowAction]]: Unlike FollowAction, TrackAction refers to the interest on the location of innanimates objects.\\n* [[SubscribeAction]]: Unlike SubscribeAction, TrackAction refers to  the interest on the location of innanimate objects." ;
        rdfs:label    "TrackAction" .

sdo:characterAttribute
        rdfs:comment  "A piece of data that represents a particular aspect of a fictional character (skill, power, character points, advantage, disadvantage)." ;
        rdfs:label    "character attribute" .

sdo:observedNode  rdfs:comment  "The observedNode of an [[Observation]], often a [[StatisticalPopulation]]." ;
        rdfs:label    "observed node" .

sdo:contactOption  rdfs:comment  "An option available on this contact point (e.g. a toll-free number or support for hearing-impaired callers)." ;
        rdfs:label    "contact option" .

sdo:SideEffectsHealthAspect
        rdfs:comment  "Side effects that can be observed from the usage of the topic." ;
        rdfs:label    "SideEffectsHealthAspect" .

sdo:HealthPlanCostSharingSpecification
        rdfs:comment  "A description of costs to the patient under a given network or formulary." ;
        rdfs:label    "HealthPlanCostSharingSpecification" .

sdo:hasBioChemEntityPart
        rdfs:comment  "Indicates a BioChemEntity that (in some sense) has this BioChemEntity as a part. " ;
        rdfs:label    "has bioChemEntityPart" .

sdo:BusinessEntityType
        rdfs:comment  "A business entity type is a conceptual entity representing the legal form, the size, the main line of business, the position in the value chain, or any combination thereof, of an organization or business person.\\n\\nCommonly used values:\\n\\n* http://purl.org/goodrelations/v1#Business\\n* http://purl.org/goodrelations/v1#Enduser\\n* http://purl.org/goodrelations/v1#PublicInstitution\\n* http://purl.org/goodrelations/v1#Reseller\n\t  " ;
        rdfs:label    "BusinessEntityType" .

sdo:ReturnFeesCustomerResponsibility
        rdfs:comment  "Specifies that product returns must be paid for, and are the responsibility of, the customer." ;
        rdfs:label    "ReturnFeesCustomerResponsibility" .

sdo:Midwifery  rdfs:comment  "A nurse-like health profession that deals with pregnancy, childbirth, and the postpartum period (including care of the newborn), besides sexual and reproductive health of women throughout their lives." ;
        rdfs:label    "Midwifery" .

sdo:OrderPaymentDue  rdfs:comment  "OrderStatus representing that payment is due on an order." ;
        rdfs:label    "OrderPaymentDue" .

sdo:ReportedDoseSchedule
        rdfs:comment  "A patient-reported or observed dosing schedule for a drug or supplement." ;
        rdfs:label    "ReportedDoseSchedule" .

sdo:PoliceStation  rdfs:comment  "A police station." ;
        rdfs:label    "PoliceStation" .

sdo:estimatedFlightDuration
        rdfs:comment  "The estimated time the flight will take." ;
        rdfs:label    "estimated flightDuration" .

sdo:Male  rdfs:comment  "The male gender." ;
        rdfs:label    "Male" .

sdo:NewsMediaOrganization
        rdfs:comment  "A News/Media organization such as a newspaper or TV station." ;
        rdfs:label    "NewsMediaOrganization" .

sdo:AllergiesHealthAspect
        rdfs:comment  "Content about the allergy-related aspects of a health topic." ;
        rdfs:label    "AllergiesHealthAspect" .

sdo:DiabeticDiet  rdfs:comment  "A diet appropriate for people with diabetes." ;
        rdfs:label    "DiabeticDiet" .

sdo:SingleFamilyResidence
        rdfs:comment  "Residence type: Single-family home." ;
        rdfs:label    "SingleFamilyResidence" .

sdo:Nonprofit501c16  rdfs:comment  "Nonprofit501c16: Non-profit type referring to Cooperative Organizations to Finance Crop Operations." ;
        rdfs:label    "Nonprofit501c16" .

sdo:playerType  rdfs:comment  "Player type required&#x2014;for example, Flash or Silverlight." ;
        rdfs:label    "player type" .

sdo:playersOnline  rdfs:comment  "Number of players on the server." ;
        rdfs:label    "players online" .

sdo:produces  rdfs:comment  "The tangible thing generated by the service, e.g. a passport, permit, etc." ;
        rdfs:label    "produces" .

sdo:steeringPosition  rdfs:comment  "The position of the steering wheel or similar device (mostly for cars)." ;
        rdfs:label    "steering position" .

sdo:ChildCare  rdfs:comment  "A Childcare center." ;
        rdfs:label    "ChildCare" .

sdo:AudioObjectSnapshot
        rdfs:comment  "A specific and exact (byte-for-byte) version of an [[AudioObject]]. Two byte-for-byte identical files, for the purposes of this type, considered identical. If they have different embedded metadata the files will differ. Different external facts about the files, e.g. creator or dateCreated that aren't represented in their actual content, do not affect this notion of identity." ;
        rdfs:label    "AudioObjectSnapshot" .

sdo:pickupLocation  rdfs:comment  "Where a taxi will pick up a passenger or a rental car can be picked up." ;
        rdfs:label    "pickup location" .

sdo:MultiCenterTrial  rdfs:comment  "A trial that takes place at multiple centers." ;
        rdfs:label    "MultiCenterTrial" .

sdo:AskAction  rdfs:comment  "The act of posing a question / favor to someone.\\n\\nRelated actions:\\n\\n* [[ReplyAction]]: Appears generally as a response to AskAction." ;
        rdfs:label    "AskAction" .

sdo:Cemetery  rdfs:comment  "A graveyard." ;
        rdfs:label    "Cemetery" .

sdo:GatedResidenceCommunity
        rdfs:comment  "Residence type: Gated community." ;
        rdfs:label    "GatedResidenceCommunity" .

sdo:TouristAttraction
        rdfs:comment  "A tourist attraction.  In principle any Thing can be a [[TouristAttraction]], from a [[Mountain]] and [[LandmarksOrHistoricalBuildings]] to a [[LocalBusiness]].  This Type can be used on its own to describe a general [[TouristAttraction]], or be used as an [[additionalType]] to add tourist attraction properties to any other type.  (See examples below)" ;
        rdfs:label    "TouristAttraction" .

sdo:FDAcategoryX  rdfs:comment  "A designation by the US FDA signifying that studies in animals or humans have demonstrated fetal abnormalities and/or there is positive evidence of human fetal risk based on adverse reaction data from investigational or marketing experience, and the risks involved in use of the drug in pregnant women clearly outweigh potential benefits." ;
        rdfs:label    "FDAcategoryX" .

sdo:diseasePreventionInfo
        rdfs:comment  "Information about disease prevention." ;
        rdfs:label    "disease preventionInfo" .

sdo:illustrator  rdfs:comment  "The illustrator of the book." ;
        rdfs:label    "illustrator" .

sdo:WPAdBlock  rdfs:comment  "An advertising section of the page." ;
        rdfs:label    "WPAdBlock" .

sdo:returnPolicyCountry
        rdfs:comment  "The country where the product has to be sent to for returns, for example \"Ireland\" using the [[name]] property of [[Country]]. You can also provide the two-letter [ISO 3166-1 alpha-2 country code](http://en.wikipedia.org/wiki/ISO_3166-1). Note that this can be different from the country where the product was originally shipped from or sent too." ;
        rdfs:label    "return policyCountry" .

sdo:payload  rdfs:comment  "The permitted weight of passengers and cargo, EXCLUDING the weight of the empty vehicle.\\n\\nTypical unit code(s): KGM for kilogram, LBR for pound\\n\\n* Note 1: Many databases specify the permitted TOTAL weight instead, which is the sum of [[weight]] and [[payload]]\\n* Note 2: You can indicate additional information in the [[name]] of the [[QuantitativeValue]] node.\\n* Note 3: You may also link to a [[QualitativeValue]] node that provides additional information using [[valueReference]].\\n* Note 4: Note that you can use [[minValue]] and [[maxValue]] to indicate ranges." ;
        rdfs:label    "payload" .

sdo:EventAttendanceModeEnumeration
        rdfs:comment  "An EventAttendanceModeEnumeration value is one of potentially several modes of organising an event, relating to whether it is online or offline." ;
        rdfs:label    "EventAttendanceModeEnumeration" .

sdo:WearableSizeGroupExtraShort
        rdfs:comment  "Size group \"Extra Short\" for wearables." ;
        rdfs:label    "WearableSizeGroupExtraShort" .

sdo:accessibilityControl
        rdfs:comment  "Identifies input methods that are sufficient to fully control the described resource ([WebSchemas wiki lists possible values](http://www.w3.org/wiki/WebSchemas/Accessibility))." ;
        rdfs:label    "accessibility control" .

sdo:category  rdfs:comment  "A category for the item. Greater signs or slashes can be used to informally indicate a category hierarchy." ;
        rdfs:label    "category" .

sdo:duns  rdfs:comment  "The Dun & Bradstreet DUNS number for identifying an organization or business person." ;
        rdfs:label    "duns" .

sdo:geoTouches  rdfs:comment  "Represents spatial relations in which two geometries (or the places they represent) touch: they have at least one boundary point in common, but no interior points.\" (a symmetric relationship, as defined in [DE-9IM](https://en.wikipedia.org/wiki/DE-9IM) )" ;
        rdfs:label    "geo touches" .

sdo:hasOfferCatalog  rdfs:comment  "Indicates an OfferCatalog listing for this Organization, Person, or Service." ;
        rdfs:label    "has offerCatalog" .

sdo:SpreadsheetDigitalDocument
        rdfs:comment  "A spreadsheet file." ;
        rdfs:label    "SpreadsheetDigitalDocument" .

sdo:codingSystem  rdfs:comment  "The coding system, e.g. 'ICD-10'." ;
        rdfs:label    "coding system" .

sdo:employmentType  rdfs:comment  "Type of employment (e.g. full-time, part-time, contract, temporary, seasonal, internship)." ;
        rdfs:label    "employment type" .

sdo:MovieTheater  rdfs:comment  "A movie theater." ;
        rdfs:label    "MovieTheater" .

sdo:DrinkAction  rdfs:comment  "The act of swallowing liquids." ;
        rdfs:label    "DrinkAction" .

sdo:Locksmith  rdfs:comment  "A locksmith." ;
        rdfs:label    "Locksmith" .

sdo:recordedIn  rdfs:comment  "The CreativeWork that captured all or part of this Event." ;
        rdfs:label    "recorded in" .

sdo:serialNumber  rdfs:comment  "The serial number or any alphanumeric identifier of a particular product. When attached to an offer, it is a shortcut for the serial number of the product included in the offer." ;
        rdfs:label    "serial number" .

sdo:audienceType  rdfs:comment  "The target group associated with a given audience (e.g. veterans, car owners, musicians, etc.)." ;
        rdfs:label    "audience type" .

sdo:relatedCondition  rdfs:comment  "A medical condition associated with this anatomy." ;
        rdfs:label    "related condition" .

sdo:SomeProducts  rdfs:comment  "A placeholder for multiple similar products of the same kind." ;
        rdfs:label    "SomeProducts" .

sdo:StadiumOrArena  rdfs:comment  "A stadium." ;
        rdfs:label    "StadiumOrArena" .

sdo:Vehicle  rdfs:comment  "A vehicle is a device that is designed or used to transport people or cargo over land, water, air, or through space." ;
        rdfs:label    "Vehicle" .

sdo:ShareAction  rdfs:comment  "The act of distributing content to people for their amusement or edification." ;
        rdfs:label    "ShareAction" .

sdo:SelfCareHealthAspect
        rdfs:comment  "Self care actions or measures that can be taken to sooth, health or avoid a topic. This may be carried at home and can be carried/managed by the person itself." ;
        rdfs:label    "SelfCareHealthAspect" .

sdo:Registry  rdfs:comment  "A registry-based study design." ;
        rdfs:label    "Registry" .

sdo:Newspaper  rdfs:comment  "A publication containing information about varied topics that are pertinent to general information, a geographic area, or a specific subject matter (i.e. business, culture, education). Often published daily." ;
        rdfs:label    "Newspaper" .

sdo:assembly  rdfs:comment  "Library file name e.g., mscorlib.dll, system.web.dll." ;
        rdfs:label    "assembly" .

sdo:applicationSuite  rdfs:comment  "The name of the application suite to which the application belongs (e.g. Excel belongs to Office)." ;
        rdfs:label    "application suite" .

sdo:cashBack  rdfs:comment  "A cardholder benefit that pays the cardholder a small percentage of their net expenditures." ;
        rdfs:label    "cash back" .

sdo:Park  rdfs:comment  "A park." ;
        rdfs:label    "Park" .

sdo:postalCodeRange  rdfs:comment  "A defined range of postal codes." ;
        rdfs:label    "postal codeRange" .

sdo:CollectionPage  rdfs:comment  "Web page type: Collection page." ;
        rdfs:label    "CollectionPage" .

sdo:FDAnotEvaluated  rdfs:comment  "A designation that the drug in question has not been assigned a pregnancy category designation by the US FDA." ;
        rdfs:label    "FDAnotEvaluated" .

sdo:ReturnMethodEnumeration
        rdfs:comment  "Enumerates several types of product return methods." ;
        rdfs:label    "ReturnMethodEnumeration" .

sdo:IngredientsHealthAspect
        rdfs:comment  "Content discussing ingredients-related aspects of a health topic." ;
        rdfs:label    "IngredientsHealthAspect" .

sdo:pageStart  rdfs:comment  "The page on which the work starts; for example \"135\" or \"xiii\"." ;
        rdfs:label    "page start" .

sdo:RespiratoryTherapy
        rdfs:comment  "The therapy that is concerned with the maintenance or improvement of respiratory function (as in patients with pulmonary disease)." ;
        rdfs:label    "RespiratoryTherapy" .

sdo:ExerciseAction  rdfs:comment  "The act of participating in exertive activity for the purposes of improving health and fitness." ;
        rdfs:label    "ExerciseAction" .

sdo:funder  rdfs:comment  "A person or organization that supports (sponsors) something through some kind of financial contribution." ;
        rdfs:label    "funder" .

sdo:recognizedBy  rdfs:comment  "An organization that acknowledges the validity, value or utility of a credential. Note: recognition may include a process of quality assurance or accreditation." ;
        rdfs:label    "recognized by" .

sdo:estimatedCost  rdfs:comment  "The estimated cost of the supply or supplies consumed when performing instructions." ;
        rdfs:label    "estimated cost" .

sdo:interactionService
        rdfs:comment  "The WebSite or SoftwareApplication where the interactions took place." ;
        rdfs:label    "interaction service" .

sdo:Nonprofit501c20  rdfs:comment  "Nonprofit501c20: Non-profit type referring to Group Legal Services Plan Organizations." ;
        rdfs:label    "Nonprofit501c20" .

sdo:appliesToPaymentMethod
        rdfs:comment  "The payment method(s) to which the payment charge specification applies." ;
        rdfs:label    "applies toPaymentMethod" .

sdo:Nonprofit527  rdfs:comment  "Nonprofit527: Non-profit type referring to Political organizations." ;
        rdfs:label    "Nonprofit527" .

sdo:LegalValueLevel  rdfs:comment  "A list of possible levels for the legal validity of a legislation." ;
        rdfs:label    "LegalValueLevel" .

sdo:cookTime  rdfs:comment  "The time it takes to actually cook the dish, in [ISO 8601 duration format](http://en.wikipedia.org/wiki/ISO_8601)." ;
        rdfs:label    "cook time" .

sdo:abstract  rdfs:comment  "An abstract is a short description that summarizes a [[CreativeWork]]." ;
        rdfs:label    "abstract" .

sdo:orderQuantity  rdfs:comment  "The number of the item ordered. If the property is not set, assume the quantity is one." ;
        rdfs:label    "order quantity" .

sdo:BodyMeasurementChest
        rdfs:comment  "Maximum girth of chest. Used, for example, to fit men's suits." ;
        rdfs:label    "BodyMeasurementChest" .

sdo:SpokenWordAlbum  rdfs:comment  "SpokenWordAlbum." ;
        rdfs:label    "SpokenWordAlbum" .

sdo:identifier  rdfs:comment  "The identifier property represents any kind of identifier for any kind of [[Thing]], such as ISBNs, GTIN codes, UUIDs etc. Schema.org provides dedicated properties for representing many of these, either as textual strings or as URL (URI) links. See [background notes](/docs/datamodel.html#identifierBg) for more details.\n        " ;
        rdfs:label    "identifier" .

sdo:gtin14  rdfs:comment  "The GTIN-14 code of the product, or the product to which the offer refers. See [GS1 GTIN Summary](http://www.gs1.org/barcodes/technical/idkeys/gtin) for more details." ;
        rdfs:label    "gtin14" .

sdo:releasedEvent  rdfs:comment  "The place and time the release was issued, expressed as a PublicationEvent." ;
        rdfs:label    "released event" .

sdo:titleEIDR  rdfs:comment  "An [EIDR](https://eidr.org/) (Entertainment Identifier Registry) [[identifier]] representing at the most general/abstract level, a work of film or television.\n\nFor example, the motion picture known as \"Ghostbusters\" has a titleEIDR of  \"10.5240/7EC7-228A-510A-053E-CBB8-J\". This title (or work) may have several variants, which EIDR calls \"edits\". See [[editEIDR]].\n\nSince schema.org types like [[Movie]] and [[TVEpisode]] can be used for both works and their multiple expressions, it is possible to use [[titleEIDR]] alone (for a general description), or alongside [[editEIDR]] for a more edit-specific description.\n" ;
        rdfs:label    "title eidr" .

sdo:broadcastSignalModulation
        rdfs:comment  "The modulation (e.g. FM, AM, etc) used by a particular broadcast service." ;
        rdfs:label    "broadcast signalModulation" .

sdo:legislationDateVersion
        rdfs:comment  "The point-in-time at which the provided description of the legislation is valid (e.g. : when looking at the law on the 2016-04-07 (= dateVersion), I get the consolidation of 2015-04-12 of the \"National Insurance Contributions Act 2015\")" ;
        rdfs:label    "legislation dateVersion" .

sdo:WearableSizeGroupExtraTall
        rdfs:comment  "Size group \"Extra Tall\" for wearables." ;
        rdfs:label    "WearableSizeGroupExtraTall" .

sdo:MedicalAudience  rdfs:comment  "Target audiences for medical web pages." ;
        rdfs:label    "MedicalAudience" .

sdo:measuredProperty  rdfs:comment  "The measuredProperty of an [[Observation]], either a schema.org property, a property from other RDF-compatible systems e.g. W3C RDF Data Cube, or schema.org extensions such as [GS1's](https://www.gs1.org/voc/?show=properties)." ;
        rdfs:label    "measured property" .

sdo:LibrarySystem  rdfs:comment  "A [[LibrarySystem]] is a collaborative system amongst several libraries." ;
        rdfs:label    "LibrarySystem" .

sdo:OrganizeAction  rdfs:comment  "The act of manipulating/administering/supervising/controlling one or more objects." ;
        rdfs:label    "OrganizeAction" .

sdo:reviewRating  rdfs:comment  "The rating given in this review. Note that reviews can themselves be rated. The ```reviewRating``` applies to rating given by the review. The [[aggregateRating]] property applies to the review itself, as a creative work." ;
        rdfs:label    "review rating" .

sdo:episode  rdfs:comment  "An episode of a tv, radio or game media within a series or season." ;
        rdfs:label    "episode" .

sdo:sameAs  rdfs:comment  "URL of a reference Web page that unambiguously indicates the item's identity. E.g. the URL of the item's Wikipedia page, Wikidata entry, or official website." ;
        rdfs:label    "same as" .

sdo:originalMediaContextDescription
        rdfs:comment  "Describes, in a [[MediaReview]] when dealing with [[DecontextualizedContent]], background information that can contribute to better interpretation of the [[MediaObject]]." ;
        rdfs:label    "original mediaContextDescription" .

sdo:MisconceptionsHealthAspect
        rdfs:comment  "Content about common misconceptions and myths that are related to a topic." ;
        rdfs:label    "MisconceptionsHealthAspect" .

sdo:isLocatedInSubcellularLocation
        rdfs:comment  "Subcellular location where this BioChemEntity is located; please use PropertyValue if you want to include any evidence." ;
        rdfs:label    "is locatedInSubcellularLocation" .

sdo:inBroadcastLineup
        rdfs:comment  "The CableOrSatelliteService offering the channel." ;
        rdfs:label    "in broadcastLineup" .

sdo:Pathology  rdfs:comment  "A specific branch of medical science that is concerned with the study of the cause, origin and nature of a disease state, including its consequences as a result of manifestation of the disease. In clinical care, the term is used to designate a branch of medicine using laboratory tests to diagnose and determine the prognostic significance of illness." ;
        rdfs:label    "Pathology" .

sdo:amountOfThisGood  rdfs:comment  "The quantity of the goods included in the offer." ;
        rdfs:label    "amount ofThisGood" .

sdo:shippingSettingsLink
        rdfs:comment  "Link to a page containing [[ShippingRateSettings]] and [[DeliveryTimeSettings]] details." ;
        rdfs:label    "shipping settingsLink" .

sdo:BowlingAlley  rdfs:comment  "A bowling alley." ;
        rdfs:label    "BowlingAlley" .

sdo:numberOfBathroomsTotal
        rdfs:comment  "The total integer number of bathrooms in a some [[Accommodation]], following real estate conventions as [documented in RESO](https://ddwiki.reso.org/display/DDW17/BathroomsTotalInteger+Field): \"The simple sum of the number of bathrooms. For example for a property with two Full Bathrooms and one Half Bathroom, the Bathrooms Total Integer will be 3.\". See also [[numberOfRooms]]." ;
        rdfs:label    "number ofBathroomsTotal" .

sdo:False  rdfs:comment  "The boolean value false." ;
        rdfs:label    "False" .

sdo:Musculoskeletal  rdfs:comment  "A specific branch of medical science that pertains to diagnosis and treatment of disorders of muscles, ligaments and skeletal system." ;
        rdfs:label    "Musculoskeletal" .

sdo:warrantyScope  rdfs:comment  "The scope of the warranty promise." ;
        rdfs:label    "warranty scope" .

sdo:issuedBy  rdfs:comment  "The organization issuing the ticket or permit." ;
        rdfs:label    "issued by" .

sdo:returnFees  rdfs:comment  "The type of return fees for purchased products (for any return reason)" ;
        rdfs:label    "return fees" .

sdo:occupationalCategory
        rdfs:comment  "A category describing the job, preferably using a term from a taxonomy such as [BLS O*NET-SOC](http://www.onetcenter.org/taxonomy.html), [ISCO-08](https://www.ilo.org/public/english/bureau/stat/isco/isco08/) or similar, with the property repeated for each applicable value. Ideally the taxonomy should be identified, and both the textual label and formal code for the category should be provided.\\n\nNote: for historical reasons, any textual label and formal code provided as a literal may be assumed to be from O*NET-SOC." ;
        rdfs:label    "occupational category" .

sdo:median  rdfs:comment  "The median value." ;
        rdfs:label    "median" .

sdo:startTime  rdfs:comment  "The startTime of something. For a reserved event or service (e.g. FoodEstablishmentReservation), the time that it is expected to start. For actions that span a period of time, when the action was performed. e.g. John wrote a book from *January* to December. For media, including audio and video, it's the time offset of the start of a clip within a larger file.\\n\\nNote that Event uses startDate/endDate instead of startTime/endTime, even when describing dates with times. This situation may be clarified in future revisions." ;
        rdfs:label    "start time" .

sdo:Ticket  rdfs:comment  "Used to describe a ticket to an event, a flight, a bus ride, etc." ;
        rdfs:label    "Ticket" .

sdo:HowItWorksHealthAspect
        rdfs:comment  "Content that discusses and explains how a particular health-related topic works, e.g. in terms of mechanisms and underlying science." ;
        rdfs:label    "HowItWorksHealthAspect" .

sdo:cargoVolume  rdfs:comment  "The available volume for cargo or luggage. For automobiles, this is usually the trunk volume.\\n\\nTypical unit code(s): LTR for liters, FTQ for cubic foot/feet\\n\\nNote: You can use [[minValue]] and [[maxValue]] to indicate ranges." ;
        rdfs:label    "cargo volume" .

sdo:publication  rdfs:comment  "A publication event associated with the item." ;
        rdfs:label    "publication" .

sdo:repetitions  rdfs:comment  "Number of times one should repeat the activity." ;
        rdfs:label    "repetitions" .

sdo:CancelAction  rdfs:comment  "The act of asserting that a future event/action is no longer going to happen.\\n\\nRelated actions:\\n\\n* [[ConfirmAction]]: The antonym of CancelAction." ;
        rdfs:label    "CancelAction" .

sdo:addressRegion  rdfs:comment  "The region in which the locality is, and which is in the country. For example, California or another appropriate first-level [Administrative division](https://en.wikipedia.org/wiki/List_of_administrative_divisions_by_country) " ;
        rdfs:label    "address region" .

sdo:EUEnergyEfficiencyEnumeration
        rdfs:comment  "Enumerates the EU energy efficiency classes A-G as well as A+, A++, and A+++ as defined in EU directive 2017/1369." ;
        rdfs:label    "EUEnergyEfficiencyEnumeration" .

sdo:TransferAction  rdfs:comment  "The act of transferring/moving (abstract or concrete) animate or inanimate objects from one place to another." ;
        rdfs:label    "TransferAction" .

sdo:LowLactoseDiet  rdfs:comment  "A diet appropriate for people with lactose intolerance." ;
        rdfs:label    "LowLactoseDiet" .

sdo:datasetTimeInterval
        rdfs:comment  "The range of temporal applicability of a dataset, e.g. for a 2011 census dataset, the year 2011 (in ISO 8601 time interval format)." ;
        rdfs:label    "dataset timeInterval" .

sdo:adverseOutcome  rdfs:comment  "A possible complication and/or side effect of this therapy. If it is known that an adverse outcome is serious (resulting in death, disability, or permanent damage; requiring hospitalization; or is otherwise life-threatening or requires immediate medical attention), tag it as a seriouseAdverseOutcome instead." ;
        rdfs:label    "adverse outcome" .

sdo:Flexibility  rdfs:comment  "Physical activity that is engaged in to improve joint and muscle flexibility." ;
        rdfs:label    "Flexibility" .

sdo:MediaManipulationRatingEnumeration
        rdfs:comment  " Codes for use with the [[mediaAuthenticityCategory]] property, indicating the authenticity of a media object (in the context of how it was published or shared). In general these codes are not mutually exclusive, although some combinations (such as 'original' versus 'transformed', 'edited' and 'staged') would be contradictory if applied in the same [[MediaReview]]. Note that the application of these codes is with regard to a piece of media shared or published in a particular context." ;
        rdfs:label    "MediaManipulationRatingEnumeration" .

sdo:RentalCarReservation
        rdfs:comment  "A reservation for a rental car.\\n\\nNote: This type is for information about actual reservations, e.g. in confirmation emails or HTML pages with individual confirmations of reservations." ;
        rdfs:label    "RentalCarReservation" .

sdo:MerchantReturnPolicy
        rdfs:comment  "A MerchantReturnPolicy provides information about product return policies associated with an [[Organization]], [[Product]], or [[Offer]]." ;
        rdfs:label    "MerchantReturnPolicy" .

sdo:speechToTextMarkup
        rdfs:comment  "Form of markup used. eg. [SSML](https://www.w3.org/TR/speech-synthesis11) or [IPA](https://www.wikidata.org/wiki/Property:P898)." ;
        rdfs:label    "speech toTextMarkup" .

sdo:relatedStructure  rdfs:comment  "Related anatomical structure(s) that are not part of the system but relate or connect to it, such as vascular bundles associated with an organ system." ;
        rdfs:label    "related structure" .

sdo:WearableSizeSystemIT
        rdfs:comment  "Italian size system for wearables." ;
        rdfs:label    "WearableSizeSystemIT" .

sdo:ProductCollection
        rdfs:comment  "A set of products (either [[ProductGroup]]s or specific variants) that are listed together e.g. in an [[Offer]]." ;
        rdfs:label    "ProductCollection" .

sdo:Nonprofit501c14  rdfs:comment  "Nonprofit501c14: Non-profit type referring to State-Chartered Credit Unions, Mutual Reserve Funds." ;
        rdfs:label    "Nonprofit501c14" .

sdo:childMaxAge  rdfs:comment  "Maximal age of the child." ;
        rdfs:label    "child maxAge" .

sdo:PaymentDeclined  rdfs:comment  "The payee received the payment, but it was declined for some reason." ;
        rdfs:label    "PaymentDeclined" .

sdo:OrderReturned  rdfs:comment  "OrderStatus representing that an order has been returned." ;
        rdfs:label    "OrderReturned" .

sdo:underName  rdfs:comment  "The person or organization the reservation or ticket is for." ;
        rdfs:label    "under name" .

sdo:isAccessibleForFree
        rdfs:comment  "A flag to signal that the item, event, or place is accessible for free." ;
        rdfs:label    "is accessibleForFree" .

sdo:ItemListOrderType
        rdfs:comment  "Enumerated for values for itemListOrder for indicating how an ordered ItemList is organized." ;
        rdfs:label    "ItemListOrderType" .

sdo:Painting  rdfs:comment  "A painting." ;
        rdfs:label    "Painting" .

sdo:CorrectionComment
        rdfs:comment  "A [[comment]] that corrects [[CreativeWork]]." ;
        rdfs:label    "CorrectionComment" .

sdo:DislikeAction  rdfs:comment  "The act of expressing a negative sentiment about the object. An agent dislikes an object (a proposition, topic or theme) with participants." ;
        rdfs:label    "DislikeAction" .

sdo:clipNumber  rdfs:comment  "Position of the clip within an ordered group of clips." ;
        rdfs:label    "clip number" .

sdo:loanRepaymentForm
        rdfs:comment  "A form of paying back money previously borrowed from a lender. Repayment usually takes the form of periodic payments that normally include part principal plus interest in each payment." ;
        rdfs:label    "loan repaymentForm" .

sdo:orderedItem  rdfs:comment  "The item ordered." ;
        rdfs:label    "ordered item" .

sdo:boardingGroup  rdfs:comment  "The airline-specific indicator of boarding order / preference." ;
        rdfs:label    "boarding group" .

sdo:applicationDeadline
        rdfs:comment  "The date at which the program stops collecting applications for the next enrollment cycle." ;
        rdfs:label    "application deadline" .

sdo:applicationStartDate
        rdfs:comment  "The date at which the program begins collecting applications for the next enrollment cycle." ;
        rdfs:label    "application startDate" .

sdo:legislationIdentifier
        rdfs:comment  "An identifier for the legislation. This can be either a string-based identifier, like the CELEX at EU level or the NOR in France, or a web-based, URL/URI identifier, like an ELI (European Legislation Identifier) or an URN-Lex." ;
        rdfs:label    "legislation identifier" .

sdo:collectionSize  rdfs:comment  "The number of items in the [[Collection]]."@en ;
        rdfs:label    "collection size"@en .

sdo:GovernmentService
        rdfs:comment  "A service provided by a government organization, e.g. food stamps, veterans benefits, etc." ;
        rdfs:label    "GovernmentService" .

sdo:salaryUponCompletion
        rdfs:comment  "The expected salary upon completing the training." ;
        rdfs:label    "salary uponCompletion" .

sdo:exceptDate  rdfs:comment  "Defines a [[Date]] or [[DateTime]] during which a scheduled [[Event]] will not take place. The property allows exceptions to\n      a [[Schedule]] to be specified. If an exception is specified as a [[DateTime]] then only the event that would have started at that specific date and time\n      should be excluded from the schedule. If an exception is specified as a [[Date]] then any event that is scheduled for that 24 hour period should be\n      excluded from the schedule. This allows a whole day to be excluded from the schedule without having to itemise every scheduled event." ;
        rdfs:label    "except date" .

sdo:flightDistance  rdfs:comment  "The distance of the flight." ;
        rdfs:label    "flight distance" .

sdo:chemicalRole  rdfs:comment  "A role played by the BioChemEntity within a chemical context." ;
        rdfs:label    "chemical role" .

sdo:VitalSign  rdfs:comment  "Vital signs are measures of various physiological functions in order to assess the most basic body functions." ;
        rdfs:label    "VitalSign" .

sdo:servicePhone  rdfs:comment  "The phone number to use to access the service." ;
        rdfs:label    "service phone" .

sdo:CheckoutPage  rdfs:comment  "Web page type: Checkout page." ;
        rdfs:label    "CheckoutPage" .

sdo:Completed  rdfs:comment  "Completed." ;
        rdfs:label    "Completed" .

sdo:Ligament  rdfs:comment  "A short band of tough, flexible, fibrous connective tissue that functions to connect multiple bones, cartilages, and structurally support joints." ;
        rdfs:label    "Ligament" .

sdo:isAccessoryOrSparePartFor
        rdfs:comment  "A pointer to another product (or multiple products) for which this product is an accessory or spare part." ;
        rdfs:label    "is accessoryOrSparePartFor" .

sdo:numConstraints  rdfs:comment  "Indicates the number of constraints (not counting [[populationType]]) defined for a particular [[StatisticalPopulation]]. This helps applications understand if they have access to a sufficiently complete description of a [[StatisticalPopulation]]." ;
        rdfs:label    "num constraints" .

sdo:seatingType  rdfs:comment  "The type/class of the seat." ;
        rdfs:label    "seating type" .

sdo:safetyConsideration
        rdfs:comment  "Any potential safety concern associated with the supplement. May include interactions with other drugs and foods, pregnancy, breastfeeding, known adverse reactions, and documented efficacy of the supplement." ;
        rdfs:label    "safety consideration" .

sdo:FourWheelDriveConfiguration
        rdfs:comment  "Four-wheel drive is a transmission layout where the engine primarily drives two wheels with a part-time four-wheel drive capability." ;
        rdfs:label    "FourWheelDriveConfiguration" .

sdo:fatContent  rdfs:comment  "The number of grams of fat." ;
        rdfs:label    "fat content" .

sdo:Infectious  rdfs:comment  "Something in medical science that pertains to infectious diseases i.e caused by bacterial, viral, fungal or parasitic infections." ;
        rdfs:label    "Infectious" .

sdo:RentalVehicleUsage
        rdfs:comment  "Indicates the usage of the vehicle as a rental car." ;
        rdfs:label    "RentalVehicleUsage" .

sdo:VideoGame  rdfs:comment  "A video game is an electronic game that involves human interaction with a user interface to generate visual feedback on a video device." ;
        rdfs:label    "VideoGame" .

sdo:servesCuisine  rdfs:comment  "The cuisine of the restaurant." ;
        rdfs:label    "serves cuisine" .

sdo:diagram  rdfs:comment  "An image containing a diagram that illustrates the structure and/or its component substructures and/or connections with other structures." ;
        rdfs:label    "diagram" .

sdo:domiciledMortgage
        rdfs:comment  "Whether borrower is a resident of the jurisdiction where the property is located." ;
        rdfs:label    "domiciled mortgage" .

sdo:Nonprofit501c13  rdfs:comment  "Nonprofit501c13: Non-profit type referring to Cemetery Companies." ;
        rdfs:label    "Nonprofit501c13" .

sdo:offers  rdfs:comment  "An offer to provide this item&#x2014;for example, an offer to sell a product, rent the DVD of a movie, perform a service, or give away tickets to an event. Use [[businessFunction]] to indicate the kind of transaction offered, i.e. sell, lease, etc. This property can also be used to describe a [[Demand]]. While this property is listed as expected on a number of common types, it can be used in others. In that case, using a second type, such as Product or a subtype of Product, can clarify the nature of the offer.\n      " ;
        rdfs:label    "offers" .

sdo:exifData  rdfs:comment  "exif data for this object." ;
        rdfs:label    "exif data" .

sdo:mainEntityOfPage  rdfs:comment  "Indicates a page (or other CreativeWork) for which this thing is the main entity being described. See [background notes](/docs/datamodel.html#mainEntityBackground) for details." ;
        rdfs:label    "main entityOfPage" .

sdo:PostOffice  rdfs:comment  "A post office." ;
        rdfs:label    "PostOffice" .

sdo:percentile90  rdfs:comment  "The 90th percentile value." ;
        rdfs:label    "percentile90" .

sdo:numberOfForwardGears
        rdfs:comment  "The total number of forward gears available for the transmission system of the vehicle.\\n\\nTypical unit code(s): C62" ;
        rdfs:label    "number ofForwardGears" .

sdo:hasBioPolymerSequence
        rdfs:comment  "A symbolic representation of a BioChemEnity. For example, a nucleotide sequence of a Gene or an amino acid sequence of a Protein." ;
        rdfs:label    "has bioPolymerSequence" .

sdo:EUEnergyEfficiencyCategoryE
        rdfs:comment  "Represents EU Energy Efficiency Class E as defined in EU energy labeling regulations." ;
        rdfs:label    "EUEnergyEfficiencyCategoryE" .

sdo:HousePainter  rdfs:comment  "A house painting service." ;
        rdfs:label    "HousePainter" .

sdo:attendees  rdfs:comment  "A person attending the event." ;
        rdfs:label    "attendees" .

sdo:Nonprofit501c5  rdfs:comment  "Nonprofit501c5: Non-profit type referring to Labor, Agricultural and Horticultural Organizations." ;
        rdfs:label    "Nonprofit501c5" .

sdo:deliveryMethod  rdfs:comment  "A sub property of instrument. The method of delivery." ;
        rdfs:label    "delivery method" .

sdo:reviewAspect  rdfs:comment  "This Review or Rating is relevant to this part or facet of the itemReviewed." ;
        rdfs:label    "review aspect" .

sdo:Order  rdfs:comment  "An order is a confirmation of a transaction (a receipt), which can contain multiple line items, each represented by an Offer that has been accepted by the customer." ;
        rdfs:label    "Order" .

sdo:countriesSupported
        rdfs:comment  "Countries for which the application is supported. You can also provide the two-letter ISO 3166-1 alpha-2 country code." ;
        rdfs:label    "countries supported" .

sdo:aggregateRating  rdfs:comment  "The overall rating, based on a collection of reviews or ratings, of the item." ;
        rdfs:label    "aggregate rating" .

sdo:interactionType  rdfs:comment  "The Action representing the type of interaction. For up votes, +1s, etc. use [[LikeAction]]. For down votes use [[DislikeAction]]. Otherwise, use the most specific Action." ;
        rdfs:label    "interaction type" .

sdo:fuelConsumption  rdfs:comment  "The amount of fuel consumed for traveling a particular distance or temporal duration with the given vehicle (e.g. liters per 100 km).\\n\\n* Note 1: There are unfortunately no standard unit codes for liters per 100 km.  Use [[unitText]] to indicate the unit of measurement, e.g. L/100 km.\\n* Note 2: There are two ways of indicating the fuel consumption, [[fuelConsumption]] (e.g. 8 liters per 100 km) and [[fuelEfficiency]] (e.g. 30 miles per gallon). They are reciprocal.\\n* Note 3: Often, the absolute value is useful only when related to driving speed (\"at 80 km/h\") or usage pattern (\"city traffic\"). You can use [[valueReference]] to link the value for the fuel consumption to another value." ;
        rdfs:label    "fuel consumption" .

sdo:interactivityType
        rdfs:comment  "The predominant mode of learning supported by the learning resource. Acceptable values are 'active', 'expositive', or 'mixed'." ;
        rdfs:label    "interactivity type" .

sdo:composer  rdfs:comment  "The person or organization who wrote a composition, or who is the composer of a work performed at some event." ;
        rdfs:label    "composer" .

sdo:gameServer  rdfs:comment  "The server on which  it is possible to play the game." ;
        rdfs:label    "game server" .

sdo:arrivalTime  rdfs:comment  "The expected arrival time." ;
        rdfs:label    "arrival time" .

sdo:causeOf  rdfs:comment  "The condition, complication, symptom, sign, etc. caused." ;
        rdfs:label    "cause of" .

sdo:significantLink  rdfs:comment  "One of the more significant URLs on the page. Typically, these are the non-navigation links that are clicked on the most." ;
        rdfs:label    "significant link" .

sdo:DefenceEstablishment
        rdfs:comment  "A defence establishment, such as an army or navy base." ;
        rdfs:label    "DefenceEstablishment" .

sdo:EUEnergyEfficiencyCategoryA
        rdfs:comment  "Represents EU Energy Efficiency Class A as defined in EU energy labeling regulations." ;
        rdfs:label    "EUEnergyEfficiencyCategoryA" .

sdo:Terminated  rdfs:comment  "Terminated." ;
        rdfs:label    "Terminated" .

sdo:freeShippingThreshold
        rdfs:comment  "A monetary value above which (or equal to) the shipping rate becomes free. Intended to be used via an [[OfferShippingDetails]] with [[shippingSettingsLink]] matching this [[ShippingRateSettings]]." ;
        rdfs:label    "free shippingThreshold" .

sdo:DeleteAction  rdfs:comment  "The act of editing a recipient by removing one of its objects." ;
        rdfs:label    "DeleteAction" .

sdo:Periodical  rdfs:comment  "A publication in any medium issued in successive parts bearing numerical or chronological designations and intended, such as a magazine, scholarly journal, or newspaper to continue indefinitely.\\n\\nSee also [blog post](http://blog.schema.org/2014/09/schemaorg-support-for-bibliographic_2.html)." ;
        rdfs:label    "Periodical" .

sdo:MusicStore  rdfs:comment  "A music store." ;
        rdfs:label    "MusicStore" .

sdo:Nonprofit501c24  rdfs:comment  "Nonprofit501c24: Non-profit type referring to Section 4049 ERISA Trusts." ;
        rdfs:label    "Nonprofit501c24" .

sdo:targetUrl  rdfs:comment  "The URL of a node in an established educational framework." ;
        rdfs:label    "target url" .

sdo:medicineSystem  rdfs:comment  "The system of medicine that includes this MedicalEntity, for example 'evidence-based', 'homeopathic', 'chiropractic', etc." ;
        rdfs:label    "medicine system" .

sdo:geoCrosses  rdfs:comment  "Represents a relationship between two geometries (or the places they represent), relating a geometry to another that crosses it: \"a crosses b: they have some but not all interior points in common, and the dimension of the intersection is less than that of at least one of them\". As defined in [DE-9IM](https://en.wikipedia.org/wiki/DE-9IM)." ;
        rdfs:label    "geo crosses" .

sdo:PhysicalExam  rdfs:comment  "A type of physical examination of a patient performed by a physician. " ;
        rdfs:label    "PhysicalExam" .

sdo:DoubleBlindedTrial
        rdfs:comment  "A trial design in which neither the researcher nor the patient knows the details of the treatment the patient was randomly assigned to." ;
        rdfs:label    "DoubleBlindedTrial" .

sdo:DepositAccount  rdfs:comment  "A type of Bank Account with a main purpose of depositing funds to gain interest or other benefits." ;
        rdfs:label    "DepositAccount" .

sdo:primaryImageOfPage
        rdfs:comment  "Indicates the main image on the page." ;
        rdfs:label    "primary imageOfPage" .

sdo:Homeopathic  rdfs:comment  "A system of medicine based on the principle that a disease can be cured by a substance that produces similar symptoms in healthy people." ;
        rdfs:label    "Homeopathic" .

sdo:hasCourse  rdfs:comment  "A course or class that is one of the learning opportunities that constitute an educational / occupational program. No information is implied about whether the course is mandatory or optional; no guarantee is implied about whether the course will be available to everyone on the program." ;
        rdfs:label    "has course" .

sdo:interactingDrug  rdfs:comment  "Another drug that is known to interact with this drug in a way that impacts the effect of this drug or causes a risk to the patient. Note: disease interactions are typically captured as contraindications." ;
        rdfs:label    "interacting drug" .

sdo:Article  rdfs:comment  "An article, such as a news article or piece of investigative report. Newspapers and magazines have articles of many different types and this is intended to cover them all.\\n\\nSee also [blog post](http://blog.schema.org/2014/09/schemaorg-support-for-bibliographic_2.html)." ;
        rdfs:label    "Article" .

sdo:UpdateAction  rdfs:comment  "The act of managing by changing/editing the state of the object." ;
        rdfs:label    "UpdateAction" .

sdo:OrganizationRole  rdfs:comment  "A subclass of Role used to describe roles within organizations." ;
        rdfs:label    "OrganizationRole" .

sdo:LikeAction  rdfs:comment  "The act of expressing a positive sentiment about the object. An agent likes an object (a proposition, topic or theme) with participants." ;
        rdfs:label    "LikeAction" .

sdo:DriveWheelConfigurationValue
        rdfs:comment  "A value indicating which roadwheels will receive torque." ;
        rdfs:label    "DriveWheelConfigurationValue" .

sdo:byMonth  rdfs:comment  "Defines the month(s) of the year on which a recurring [[Event]] takes place. Specified as an [[Integer]] between 1-12. January is 1." ;
        rdfs:label    "by month" .

sdo:foodEvent  rdfs:comment  "A sub property of location. The specific food event where the action occurred." ;
        rdfs:label    "food event" .

sdo:fuelCapacity  rdfs:comment  "The capacity of the fuel tank or in the case of electric cars, the battery. If there are multiple components for storage, this should indicate the total of all storage of the same type.\\n\\nTypical unit code(s): LTR for liters, GLL of US gallons, GLI for UK / imperial gallons, AMH for ampere-hours (for electrical vehicles)." ;
        rdfs:label    "fuel capacity" .

sdo:serviceType  rdfs:comment  "The type of service being offered, e.g. veterans' benefits, emergency relief, etc." ;
        rdfs:label    "service type" .

sdo:memoryRequirements
        rdfs:comment  "Minimum memory requirements." ;
        rdfs:label    "memory requirements" .

sdo:EnergyStarEnergyEfficiencyEnumeration
        rdfs:comment  "Used to indicate whether a product is EnergyStar certified." ;
        rdfs:label    "EnergyStarEnergyEfficiencyEnumeration" .

sdo:stageAsNumber  rdfs:comment  "The stage represented as a number, e.g. 3." ;
        rdfs:label    "stage asNumber" .

sdo:MedicalImagingTechnique
        rdfs:comment  "Any medical imaging modality typically used for diagnostic purposes. Enumerated type." ;
        rdfs:label    "MedicalImagingTechnique" .

sdo:geoDisjoint  rdfs:comment  "Represents spatial relations in which two geometries (or the places they represent) are topologically disjoint: they have no point in common. They form a set of disconnected geometries.\" (a symmetric relationship, as defined in [DE-9IM](https://en.wikipedia.org/wiki/DE-9IM))" ;
        rdfs:label    "geo disjoint" .

sdo:Nonprofit501q  rdfs:comment  "Nonprofit501q: Non-profit type referring to Credit Counseling Organizations." ;
        rdfs:label    "Nonprofit501q" .

sdo:PeopleAudience  rdfs:comment  "A set of characteristics belonging to people, e.g. who compose an item's target audience." ;
        rdfs:label    "PeopleAudience" .

sdo:children  rdfs:comment  "A child of the person." ;
        rdfs:label    "children" .

sdo:BroadcastChannel  rdfs:comment  "A unique instance of a BroadcastService on a CableOrSatelliteService lineup." ;
        rdfs:label    "BroadcastChannel" .

sdo:ComicCoverArt  rdfs:comment  "The artwork on the cover of a comic." ;
        rdfs:label    "ComicCoverArt" .

sdo:FloorPlan  rdfs:comment  "A FloorPlan is an explicit representation of a collection of similar accommodations, allowing the provision of common information (room counts, sizes, layout diagrams) and offers for rental or sale. In typical use, some [[ApartmentComplex]] has an [[accommodationFloorPlan]] which is a [[FloorPlan]].  A FloorPlan is always in the context of a particular place, either a larger [[ApartmentComplex]] or a single [[Apartment]]. The visual/spatial aspects of a floor plan (i.e. room layout, [see wikipedia](https://en.wikipedia.org/wiki/Floor_plan)) can be indicated using [[image]]. " ;
        rdfs:label    "FloorPlan" .

sdo:birthPlace  rdfs:comment  "The place where the person was born." ;
        rdfs:label    "birth place" .

sdo:PregnancyHealthAspect
        rdfs:comment  "Content discussing pregnancy-related aspects of a health topic." ;
        rdfs:label    "PregnancyHealthAspect" .

sdo:employees  rdfs:comment  "People working for this organization." ;
        rdfs:label    "employees" .

sdo:arterialBranch  rdfs:comment  "The branches that comprise the arterial structure." ;
        rdfs:label    "arterial branch" .

sdo:MedicalGuideline  rdfs:comment  "Any recommendation made by a standard society (e.g. ACC/AHA) or consensus statement that denotes how to diagnose and treat a particular condition. Note: this type should be used to tag the actual guideline recommendation; if the guideline recommendation occurs in a larger scholarly article, use MedicalScholarlyArticle to tag the overall article, not this type. Note also: the organization making the recommendation should be captured in the recognizingAuthority base property of MedicalEntity." ;
        rdfs:label    "MedicalGuideline" .

sdo:VideoGameSeries  rdfs:comment  "A video game series." ;
        rdfs:label    "VideoGameSeries" .

sdo:MSRP  rdfs:comment  "Represents the manufacturer suggested retail price (\"MSRP\") of an offered product." ;
        rdfs:label    "MSRP" .

sdo:MedicalSign  rdfs:comment  "Any physical manifestation of a person's medical condition discoverable by objective diagnostic tests or physical examination." ;
        rdfs:label    "MedicalSign" .

sdo:subEvent  rdfs:comment  "An Event that is part of this event. For example, a conference event includes many presentations, each of which is a subEvent of the conference." ;
        rdfs:label    "sub event" .

sdo:preparation  rdfs:comment  "Typical preparation that a patient must undergo before having the procedure performed." ;
        rdfs:label    "preparation" .

sdo:ContactPage  rdfs:comment  "Web page type: Contact page." ;
        rdfs:label    "ContactPage" .

sdo:numberOfAvailableAccommodationUnits
        rdfs:comment  "Indicates the number of available accommodation units in an [[ApartmentComplex]], or the number of accommodation units for a specific [[FloorPlan]] (within its specific [[ApartmentComplex]]). See also [[numberOfAccommodationUnits]]." ;
        rdfs:label    "number ofAvailableAccommodationUnits" .

sdo:ineligibleRegion  rdfs:comment  "The ISO 3166-1 (ISO 3166-1 alpha-2) or ISO 3166-2 code, the place, or the GeoShape for the geo-political region(s) for which the offer or delivery charge specification is not valid, e.g. a region where the transaction is not allowed.\\n\\nSee also [[eligibleRegion]].\n      " ;
        rdfs:label    "ineligible region" .

sdo:postalCode  rdfs:comment  "The postal code. For example, 94043." ;
        rdfs:label    "postal code" .

sdo:vehicleTransmission
        rdfs:comment  "The type of component used for transmitting the power from a rotating power source to the wheels or other relevant component(s) (\"gearbox\" for cars)." ;
        rdfs:label    "vehicle transmission" .

sdo:breastfeedingWarning
        rdfs:comment  "Any precaution, guidance, contraindication, etc. related to this drug's use by breastfeeding mothers." ;
        rdfs:label    "breastfeeding warning" .

sdo:CohortStudy  rdfs:comment  "Also known as a panel study. A cohort study is a form of longitudinal study used in medicine and social science. It is one type of study design and should be compared with a cross-sectional study.  A cohort is a group of people who share a common characteristic or experience within a defined period (e.g., are born, leave school, lose their job, are exposed to a drug or a vaccine, etc.). The comparison group may be the general population from which the cohort is drawn, or it may be another cohort of persons thought to have had little or no exposure to the substance under investigation, but otherwise similar. Alternatively, subgroups within the cohort may be compared with each other." ;
        rdfs:label    "CohortStudy" .

sdo:InvoicePrice  rdfs:comment  "Represents the invoice price of an offered product." ;
        rdfs:label    "InvoicePrice" .

sdo:proficiencyLevel  rdfs:comment  "Proficiency needed for this content; expected values: 'Beginner', 'Expert'." ;
        rdfs:label    "proficiency level" .

sdo:alumni  rdfs:comment  "Alumni of an organization." ;
        rdfs:label    "alumni" .

sdo:issn  rdfs:comment  "The International Standard Serial Number (ISSN) that identifies this serial publication. You can repeat this property to identify different formats of, or the linking ISSN (ISSN-L) for, this serial publication." ;
        rdfs:label    "issn" .

sdo:FDAcategoryB  rdfs:comment  "A designation by the US FDA signifying that animal reproduction studies have failed to demonstrate a risk to the fetus and there are no adequate and well-controlled studies in pregnant women." ;
        rdfs:label    "FDAcategoryB" .

sdo:MedicalSignOrSymptom
        rdfs:comment  "Any feature associated or not with a medical condition. In medicine a symptom is generally subjective while a sign is objective." ;
        rdfs:label    "MedicalSignOrSymptom" .

sdo:Prion  rdfs:comment  "A prion is an infectious agent composed of protein in a misfolded form." ;
        rdfs:label    "Prion" .

sdo:Audience  rdfs:comment  "Intended audience for an item, i.e. the group for whom the item was created." ;
        rdfs:label    "Audience" .

sdo:vehicleIdentificationNumber
        rdfs:comment  "The Vehicle Identification Number (VIN) is a unique serial number used by the automotive industry to identify individual motor vehicles." ;
        rdfs:label    "vehicle identificationNumber" .

sdo:qualifications  rdfs:comment  "Specific qualifications required for this role or Occupation." ;
        rdfs:label    "qualifications" .

sdo:urlTemplate  rdfs:comment  "An url template (RFC6570) that will be used to construct the target of the execution of the action." ;
        rdfs:label    "url template" .

sdo:AmusementPark  rdfs:comment  "An amusement park." ;
        rdfs:label    "AmusementPark" .

sdo:LymphaticVessel  rdfs:comment  "A type of blood vessel that specifically carries lymph fluid unidirectionally toward the heart." ;
        rdfs:label    "LymphaticVessel" .

sdo:itemListElement  rdfs:comment  "For itemListElement values, you can use simple strings (e.g. \"Peter\", \"Paul\", \"Mary\"), existing entities, or use ListItem.\\n\\nText values are best if the elements in the list are plain strings. Existing entities are best for a simple, unordered list of existing things in your data. ListItem is used with ordered lists when you want to provide additional context about the element in that list or when the same item might be in different places in different lists.\\n\\nNote: The order of elements in your mark-up is not sufficient for indicating the order or elements.  Use ListItem with a 'position' property in such cases." ;
        rdfs:label    "item listElement" .

sdo:Motel  rdfs:comment  "A motel.\n<br /><br />\nSee also the <a href=\"/docs/hotels.html\">dedicated document on the use of schema.org for marking up hotels and other forms of accommodations</a>.\n" ;
        rdfs:label    "Motel" .

sdo:downloadUrl  rdfs:comment  "If the file can be downloaded, URL to download the binary." ;
        rdfs:label    "download url" .

sdo:Nonprofit501c22  rdfs:comment  "Nonprofit501c22: Non-profit type referring to Withdrawal Liability Payment Funds." ;
        rdfs:label    "Nonprofit501c22" .

sdo:value  rdfs:comment  "The value of the quantitative value or property value node.\\n\\n* For [[QuantitativeValue]] and [[MonetaryAmount]], the recommended type for values is 'Number'.\\n* For [[PropertyValue]], it can be 'Text;', 'Number', 'Boolean', or 'StructuredValue'.\\n* Use values from 0123456789 (Unicode 'DIGIT ZERO' (U+0030) to 'DIGIT NINE' (U+0039)) rather than superficially similiar Unicode symbols.\\n* Use '.' (Unicode 'FULL STOP' (U+002E)) rather than ',' to indicate a decimal point. Avoid using these symbols as a readability separator." ;
        rdfs:label    "value" .

sdo:CommunityHealth  rdfs:comment  "A field of public health focusing on improving health characteristics of a defined population in relation with their geographical or environment areas." ;
        rdfs:label    "CommunityHealth" .

sdo:MediaGallery  rdfs:comment  "Web page type: Media gallery page. A mixed-media page that can contains media such as images, videos, and other multimedia." ;
        rdfs:label    "MediaGallery" .

sdo:WearableMeasurementWaist
        rdfs:comment  "Measurement of the waist section, for example of pants" ;
        rdfs:label    "WearableMeasurementWaist" .

sdo:propertyID  rdfs:comment  "A commonly used identifier for the characteristic represented by the property, e.g. a manufacturer or a standard code for a property. propertyID can be\n(1) a prefixed string, mainly meant to be used with standards for product properties; (2) a site-specific, non-prefixed string (e.g. the primary key of the property or the vendor-specific id of the property), or (3)\na URL indicating the type of the property, either pointing to an external vocabulary, or a Web resource that describes the property (e.g. a glossary entry).\nStandards bodies should promote a standard prefix for the identifiers of properties from their standards." ;
        rdfs:label    "property id" .

sdo:colleague  rdfs:comment  "A colleague of the person." ;
        rdfs:label    "colleague" .

sdo:creditText  rdfs:comment  "Text that can be used to credit person(s) and/or organization(s) associated with a published Creative Work." ;
        rdfs:label    "credit text" .

sdo:BusReservation  rdfs:comment  "A reservation for bus travel. \\n\\nNote: This type is for information about actual reservations, e.g. in confirmation emails or HTML pages with individual confirmations of reservations. For offers of tickets, use [[Offer]]." ;
        rdfs:label    "BusReservation" .

sdo:isFamilyFriendly  rdfs:comment  "Indicates whether this content is family friendly." ;
        rdfs:label    "is familyFriendly" .

sdo:legalStatus  rdfs:comment  "The drug or supplement's legal status, including any controlled substance schedules that apply." ;
        rdfs:label    "legal status" .

sdo:contentLocation  rdfs:comment  "The location depicted or described in the content. For example, the location in a photograph or painting." ;
        rdfs:label    "content location" .

sdo:AnatomicalSystem  rdfs:comment  "An anatomical system is a group of anatomical structures that work together to perform a certain task. Anatomical systems, such as organ systems, are one organizing principle of anatomy, and can includes circulatory, digestive, endocrine, integumentary, immune, lymphatic, muscular, nervous, reproductive, respiratory, skeletal, urinary, vestibular, and other systems." ;
        rdfs:label    "AnatomicalSystem" .

sdo:resultComment  rdfs:comment  "A sub property of result. The Comment created or sent as a result of this action." ;
        rdfs:label    "result comment" .

sdo:CourseInstance  rdfs:comment  "An instance of a [[Course]] which is distinct from other instances because it is offered at a different time or location or through different media or modes of study or to a specific section of students." ;
        rdfs:label    "CourseInstance" .

sdo:diet  rdfs:comment  "A sub property of instrument. The diet used in this action." ;
        rdfs:label    "diet" .

sdo:license  rdfs:comment  "A license document that applies to this content, typically indicated by URL." ;
        rdfs:label    "license" .

sdo:priceType  rdfs:comment  "Defines the type of a price specified for an offered product, for example a list price, a (temporary) sale price or a manufacturer suggested retail price. If multiple prices are specified for an offer the [[priceType]] property can be used to identify the type of each such specified price. The value of priceType can be specified as a value from enumeration PriceTypeEnumeration or as a free form text string for price types that are not already predefined in PriceTypeEnumeration." ;
        rdfs:label    "price type" .

sdo:device  rdfs:comment  "Device required to run the application. Used in cases where a specific make/model is required to run the application." ;
        rdfs:label    "device" .

sdo:CompilationAlbum  rdfs:comment  "CompilationAlbum." ;
        rdfs:label    "CompilationAlbum" .

sdo:MedicalTest  rdfs:comment  "Any medical test, typically performed for diagnostic purposes." ;
        rdfs:label    "MedicalTest" .

sdo:arrivalPlatform  rdfs:comment  "The platform where the train arrives." ;
        rdfs:label    "arrival platform" .

sdo:customerRemorseReturnFees
        rdfs:comment  "The type of return fees if the product is returned due to customer remorse." ;
        rdfs:label    "customer remorseReturnFees" .

sdo:MedicalAudienceType
        rdfs:comment  "Target audiences types for medical web pages. Enumerated type." ;
        rdfs:label    "MedicalAudienceType" .

sdo:carrierRequirements
        rdfs:comment  "Specifies specific carrier(s) requirements for the application (e.g. an application may only work on a specific carrier network)." ;
        rdfs:label    "carrier requirements" .

sdo:siblings  rdfs:comment  "A sibling of the person." ;
        rdfs:label    "siblings" .

sdo:lastReviewed  rdfs:comment  "Date on which the content on this web page was last reviewed for accuracy and/or completeness." ;
        rdfs:label    "last reviewed" .

sdo:Library  rdfs:comment  "A library." ;
        rdfs:label    "Library" .

sdo:DayOfWeek  rdfs:comment  "The day of the week, e.g. used to specify to which day the opening hours of an OpeningHoursSpecification refer.\n\nOriginally, URLs from [GoodRelations](http://purl.org/goodrelations/v1) were used (for [[Monday]], [[Tuesday]], [[Wednesday]], [[Thursday]], [[Friday]], [[Saturday]], [[Sunday]] plus a special entry for [[PublicHolidays]]); these have now been integrated directly into schema.org.\n      " ;
        rdfs:label    "DayOfWeek" .

sdo:applicableLocation
        rdfs:comment  "The location in which the status applies." ;
        rdfs:label    "applicable location" .

sdo:CompleteDataFeed  rdfs:comment  "A [[CompleteDataFeed]] is a [[DataFeed]] whose standard representation includes content for every item currently in the feed.\n\nThis is the equivalent of Atom's element as defined in Feed Paging and Archiving [RFC 5005](https://tools.ietf.org/html/rfc5005), For example (and as defined for Atom), when using data from a feed that represents a collection of items that varies over time (e.g. \"Top Twenty Records\") there is no need to have newer entries mixed in alongside older, obsolete entries. By marking this feed as a CompleteDataFeed, old entries can be safely discarded when the feed is refreshed, since we can assume the feed has provided descriptions for all current items." ;
        rdfs:label    "CompleteDataFeed" .

sdo:recipeYield  rdfs:comment  "The quantity produced by the recipe (for example, number of people served, number of servings, etc)." ;
        rdfs:label    "recipe yield" .

sdo:WearableSizeGroupJuniors
        rdfs:comment  "Size group \"Juniors\" for wearables." ;
        rdfs:label    "WearableSizeGroupJuniors" .

sdo:verificationFactCheckingPolicy
        rdfs:comment  "Disclosure about verification and fact-checking processes for a [[NewsMediaOrganization]] or other fact-checking [[Organization]]." ;
        rdfs:label    "verification factCheckingPolicy" .

sdo:paymentAccepted  rdfs:comment  "Cash, Credit Card, Cryptocurrency, Local Exchange Tradings System, etc." ;
        rdfs:label    "payment accepted" .

sdo:DDxElement  rdfs:comment  "An alternative, closely-related condition typically considered later in the differential diagnosis process along with the signs that are used to distinguish it." ;
        rdfs:label    "DDxElement" .

sdo:variableMeasured  rdfs:comment  "The variableMeasured property can indicate (repeated as necessary) the  variables that are measured in some dataset, either described as text or as pairs of identifier and description using PropertyValue." ;
        rdfs:label    "variable measured" .

sdo:SeeDoctorHealthAspect
        rdfs:comment  "Information about questions that may be asked, when to see a professional, measures before seeing a doctor or content about the first consultation." ;
        rdfs:label    "SeeDoctorHealthAspect" .

sdo:MedicalResearcher
        rdfs:comment  "Medical researchers." ;
        rdfs:label    "MedicalResearcher" .

sdo:video  rdfs:comment  "An embedded video object." ;
        rdfs:label    "video" .

sdo:Playground  rdfs:comment  "A playground." ;
        rdfs:label    "Playground" .

sdo:TakeAction  rdfs:comment  "The act of gaining ownership of an object from an origin. Reciprocal of GiveAction.\\n\\nRelated actions:\\n\\n* [[GiveAction]]: The reciprocal of TakeAction.\\n* [[ReceiveAction]]: Unlike ReceiveAction, TakeAction implies that ownership has been transfered." ;
        rdfs:label    "TakeAction" .

sdo:LandmarksOrHistoricalBuildings
        rdfs:comment  "An historical landmark or building." ;
        rdfs:label    "LandmarksOrHistoricalBuildings" .

sdo:EndorseAction  rdfs:comment  "An agent approves/certifies/likes/supports/sanction an object." ;
        rdfs:label    "EndorseAction" .

sdo:carbohydrateContent
        rdfs:comment  "The number of grams of carbohydrates." ;
        rdfs:label    "carbohydrate content" .

sdo:FDAcategoryD  rdfs:comment  "A designation by the US FDA signifying that there is positive evidence of human fetal risk based on adverse reaction data from investigational or marketing experience or studies in humans, but potential benefits may warrant use of the drug in pregnant women despite potential risks." ;
        rdfs:label    "FDAcategoryD" .

sdo:Substance  rdfs:comment  "Any matter of defined composition that has discrete existence, whose origin may be biological, mineral or chemical." ;
        rdfs:label    "Substance" .

sdo:MixtapeAlbum  rdfs:comment  "MixtapeAlbum." ;
        rdfs:label    "MixtapeAlbum" .

sdo:affectedBy  rdfs:comment  "Drugs that affect the test's results." ;
        rdfs:label    "affected by" .

sdo:releaseDate  rdfs:comment  "The release date of a product or product model. This can be used to distinguish the exact variant of a product." ;
        rdfs:label    "release date" .

sdo:numberOfAxles  rdfs:comment  "The number of axles.\\n\\nTypical unit code(s): C62" ;
        rdfs:label    "number ofAxles" .

sdo:hostingOrganization
        rdfs:comment  "The organization (airline, travelers' club, etc.) the membership is made with." ;
        rdfs:label    "hosting organization" .

sdo:procedureType  rdfs:comment  "The type of procedure, for example Surgical, Noninvasive, or Percutaneous." ;
        rdfs:label    "procedure type" .

sdo:UserBlocks  rdfs:comment  "UserInteraction and its subtypes is an old way of talking about users interacting with pages. It is generally better to use [[Action]]-based vocabulary, alongside types such as [[Comment]]." ;
        rdfs:label    "UserBlocks" .

sdo:cvdNumVentUse  rdfs:comment  "numventuse - MECHANICAL VENTILATORS IN USE: Total number of ventilators in use." ;
        rdfs:label    "cvd numVentUse" .

sdo:deliveryStatus  rdfs:comment  "New entry added as the package passes through each leg of its journey (from shipment to final delivery)." ;
        rdfs:label    "delivery status" .

sdo:exercisePlan  rdfs:comment  "A sub property of instrument. The exercise plan used on this action." ;
        rdfs:label    "exercise plan" .

sdo:availableDeliveryMethod
        rdfs:comment  "The delivery method(s) available for this offer." ;
        rdfs:label    "available deliveryMethod" .

sdo:MedicalProcedure  rdfs:comment  "A process of care used in either a diagnostic, therapeutic, preventive or palliative capacity that relies on invasive (surgical), non-invasive, or other techniques." ;
        rdfs:label    "MedicalProcedure" .

sdo:feesAndCommissionsSpecification
        rdfs:comment  "Description of fees, commissions, and other terms applied either to a class of financial product, or by a financial service organization." ;
        rdfs:label    "fees andCommissionsSpecification" .

sdo:unitCode  rdfs:comment  "The unit of measurement given using the UN/CEFACT Common Code (3 characters) or a URL. Other codes than the UN/CEFACT Common Code may be used with a prefix followed by a colon." ;
        rdfs:label    "unit code" .

sdo:Photograph  rdfs:comment  "A photograph." ;
        rdfs:label    "Photograph" .

sdo:study  rdfs:comment  "A medical study or trial related to this entity." ;
        rdfs:label    "study" .

sdo:printSection  rdfs:comment  "If this NewsArticle appears in print, this field indicates the print section in which the article appeared." ;
        rdfs:label    "print section" .

sdo:CommentPermission
        rdfs:comment  "Permission to add comments to the document." ;
        rdfs:label    "CommentPermission" .

sdo:discountCurrency  rdfs:comment  "The currency of the discount.\\n\\nUse standard formats: [ISO 4217 currency format](http://en.wikipedia.org/wiki/ISO_4217) e.g. \"USD\"; [Ticker symbol](https://en.wikipedia.org/wiki/List_of_cryptocurrencies) for cryptocurrencies e.g. \"BTC\"; well known names for [Local Exchange Tradings Systems](https://en.wikipedia.org/wiki/Local_exchange_trading_system) (LETS) and other currency types e.g. \"Ithaca HOUR\"." ;
        rdfs:label    "discount currency" .

sdo:partOfEpisode  rdfs:comment  "The episode to which this clip belongs." ;
        rdfs:label    "part ofEpisode" .

sdo:character  rdfs:comment  "Fictional person connected with a creative work." ;
        rdfs:label    "character" .

sdo:dataFeedElement  rdfs:comment  "An item within in a data feed. Data feeds may have many elements." ;
        rdfs:label    "data feedElement" .

sdo:SportsClub  rdfs:comment  "A sports club." ;
        rdfs:label    "SportsClub" .

sdo:MeasurementTypeEnumeration
        rdfs:comment  "Enumeration of common measurement types (or dimensions), for example \"chest\" for a person, \"inseam\" for pants, \"gauge\" for screws, or \"wheel\" for bicycles." ;
        rdfs:label    "MeasurementTypeEnumeration" .

sdo:BodyMeasurementHand
        rdfs:comment  "Maximum hand girth (measured over the knuckles of the open right hand excluding thumb, fingers together). Used, for example, to fit gloves." ;
        rdfs:label    "BodyMeasurementHand" .

sdo:busNumber  rdfs:comment  "The unique identifier for the bus." ;
        rdfs:label    "bus number" .

sdo:actionPlatform  rdfs:comment  "The high level platform(s) where the Action can be performed for the given URL. To specify a specific application or operating system instance, use actionApplication." ;
        rdfs:label    "action platform" .

sdo:actors  rdfs:comment  "An actor, e.g. in tv, radio, movie, video games etc. Actors can be associated with individual items or with a series, episode, clip." ;
        rdfs:label    "actors" .

sdo:BodyMeasurementBust
        rdfs:comment  "Maximum girth of bust. Used, for example, to fit women's suits." ;
        rdfs:label    "BodyMeasurementBust" .

sdo:provider  rdfs:comment  "The service provider, service operator, or service performer; the goods producer. Another party (a seller) may offer those services or goods on behalf of the provider. A provider may also serve as the seller." ;
        rdfs:label    "provider" .

sdo:OrderPickupAvailable
        rdfs:comment  "OrderStatus representing availability of an order for pickup." ;
        rdfs:label    "OrderPickupAvailable" .

sdo:MusicPlaylist  rdfs:comment  "A collection of music tracks in playlist form." ;
        rdfs:label    "MusicPlaylist" .

sdo:LegislativeBuilding
        rdfs:comment  "A legislative building&#x2014;for example, the state capitol." ;
        rdfs:label    "LegislativeBuilding" .

sdo:orderDate  rdfs:comment  "Date order was placed." ;
        rdfs:label    "order date" .

sdo:MusicRelease  rdfs:comment  "A MusicRelease is a specific release of a music album." ;
        rdfs:label    "MusicRelease" .

sdo:distance  rdfs:comment  "The distance travelled, e.g. exercising or travelling." ;
        rdfs:label    "distance" .

sdo:CheckInAction  rdfs:comment  "The act of an agent communicating (service provider, social media, etc) their arrival by registering/confirming for a previously reserved service (e.g. flight check in) or at a place (e.g. hotel), possibly resulting in a result (boarding pass, etc).\\n\\nRelated actions:\\n\\n* [[CheckOutAction]]: The antonym of CheckInAction.\\n* [[ArriveAction]]: Unlike ArriveAction, CheckInAction implies that the agent is informing/confirming the start of a previously reserved service.\\n* [[ConfirmAction]]: Unlike ConfirmAction, CheckInAction implies that the agent is informing/confirming the *start* of a previously reserved service rather than its validity/existence." ;
        rdfs:label    "CheckInAction" .

sdo:LowCalorieDiet  rdfs:comment  "A diet focused on reduced calorie intake." ;
        rdfs:label    "LowCalorieDiet" .

sdo:numberOfAccommodationUnits
        rdfs:comment  "Indicates the total (available plus unavailable) number of accommodation units in an [[ApartmentComplex]], or the number of accommodation units for a specific [[FloorPlan]] (within its specific [[ApartmentComplex]]). See also [[numberOfAvailableAccommodationUnits]]." ;
        rdfs:label    "number ofAccommodationUnits" .

sdo:Nonprofit501c23  rdfs:comment  "Nonprofit501c23: Non-profit type referring to Veterans Organizations." ;
        rdfs:label    "Nonprofit501c23" .

sdo:Joint  rdfs:comment  "The anatomical location at which two or more bones make contact." ;
        rdfs:label    "Joint" .

sdo:ReservationPending
        rdfs:comment  "The status of a reservation when a request has been sent, but not confirmed." ;
        rdfs:label    "ReservationPending" .

sdo:GeospatialGeometry
        rdfs:comment  "(Eventually to be defined as) a supertype of GeoShape designed to accommodate definitions from Geo-Spatial best practices." ;
        rdfs:label    "GeospatialGeometry" .

sdo:vatID  rdfs:comment  "The Value-added Tax ID of the organization or person." ;
        rdfs:label    "vat id" .

sdo:recordingOf  rdfs:comment  "The composition this track is a recording of." ;
        rdfs:label    "recording of" .

sdo:worstRating  rdfs:comment  "The lowest value allowed in this rating system. If worstRating is omitted, 1 is assumed." ;
        rdfs:label    "worst rating" .

sdo:Recommendation  rdfs:comment  "[[Recommendation]] is a type of [[Review]] that suggests or proposes something as the best option or best course of action. Recommendations may be for products or services, or other concrete things, as in the case of a ranked list or product guide. A [[Guide]] may list multiple recommendations for different categories. For example, in a [[Guide]] about which TVs to buy, the author may have several [[Recommendation]]s." ;
        rdfs:label    "Recommendation" .

sdo:eduQuestionType  rdfs:comment  "For questions that are part of learning resources (e.g. Quiz), eduQuestionType indicates the format of question being given. Example: \"Multiple choice\", \"Open ended\", \"Flashcard\"." ;
        rdfs:label    "edu questionType" .

sdo:AssessAction  rdfs:comment  "The act of forming one's opinion, reaction or sentiment." ;
        rdfs:label    "AssessAction" .

sdo:broadcastOfEvent  rdfs:comment  "The event being broadcast such as a sporting event or awards ceremony." ;
        rdfs:label    "broadcast ofEvent" .

sdo:partOfOrder  rdfs:comment  "The overall order the items in this delivery were included in." ;
        rdfs:label    "part ofOrder" .

sdo:ProductModel  rdfs:comment  "A datasheet or vendor specification of a product (in the sense of a prototypical description)." ;
        rdfs:label    "ProductModel" .

sdo:processingTime  rdfs:comment  "Estimated processing time for the service using this channel." ;
        rdfs:label    "processing time" .

sdo:hasRepresentation
        rdfs:comment  "A common representation such as a protein sequence or chemical structure for this entity. For images use schema.org/image." ;
        rdfs:label    "has representation" .

sdo:legislationConsolidates
        rdfs:comment  "Indicates another legislation taken into account in this consolidated legislation (which is usually the product of an editorial process that revises the legislation). This property should be used multiple times to refer to both the original version or the previous consolidated version, and to the legislations making the change." ;
        rdfs:label    "legislation consolidates" .

sdo:gameItem  rdfs:comment  "An item is an object within the game world that can be collected by a player or, occasionally, a non-player character." ;
        rdfs:label    "game item" .

sdo:HealthAspectEnumeration
        rdfs:comment  "HealthAspectEnumeration enumerates several aspects of health content online, each of which might be described using [[hasHealthAspect]] and [[HealthTopicContent]]." ;
        rdfs:label    "HealthAspectEnumeration" .

sdo:RadioStation  rdfs:comment  "A radio station." ;
        rdfs:label    "RadioStation" .

sdo:Aquarium  rdfs:comment  "Aquarium." ;
        rdfs:label    "Aquarium" .

sdo:OfficialLegalValue
        rdfs:comment  "All the documents published by an official publisher should have at least the legal value level \"OfficialLegalValue\". This indicates that the document was published by an organisation with the public task of making it available (e.g. a consolidated version of a EU directive published by the EU Office of Publications)." ;
        rdfs:label    "OfficialLegalValue" .

sdo:originatesFrom  rdfs:comment  "The vasculature the lymphatic structure originates, or afferents, from." ;
        rdfs:label    "originates from" .

sdo:TollFree  rdfs:comment  "The associated telephone number is toll free." ;
        rdfs:label    "TollFree" .

sdo:follows  rdfs:comment  "The most generic uni-directional social relation." ;
        rdfs:label    "follows" .

sdo:albums  rdfs:comment  "A collection of music albums." ;
        rdfs:label    "albums" .

sdo:position  rdfs:comment  "The position of an item in a series or sequence of items." ;
        rdfs:label    "position" .

sdo:Pharmacy  rdfs:comment  "A pharmacy or drugstore." ;
        rdfs:label    "Pharmacy" .

sdo:branch  rdfs:comment  "The branches that delineate from the nerve bundle. Not to be confused with [[branchOf]]." ;
        rdfs:label    "branch" .

sdo:DefinedTermSet  rdfs:comment  "A set of defined terms for example a set of categories or a classification scheme, a glossary, dictionary or enumeration." ;
        rdfs:label    "DefinedTermSet" .

sdo:renegotiableLoan  rdfs:comment  "Whether the terms for payment of interest can be renegotiated during the life of the loan." ;
        rdfs:label    "renegotiable loan" .

sdo:Nursing  rdfs:comment  "A health profession of a person formally educated and trained in the care of the sick or infirm person." ;
        rdfs:label    "Nursing" .

sdo:includedComposition
        rdfs:comment  "Smaller compositions included in this work (e.g. a movement in a symphony)." ;
        rdfs:label    "included composition" .

sdo:comprisedOf  rdfs:comment  "Specifying something physically contained by something else. Typically used here for the underlying anatomical structures, such as organs, that comprise the anatomical system." ;
        rdfs:label    "comprised of" .

sdo:MedicalIndication
        rdfs:comment  "A condition or factor that indicates use of a medical therapy, including signs, symptoms, risk factors, anatomical states, etc." ;
        rdfs:label    "MedicalIndication" .

sdo:BloodTest  rdfs:comment  "A medical test performed on a sample of a patient's blood." ;
        rdfs:label    "BloodTest" .

sdo:AnimalShelter  rdfs:comment  "Animal shelter." ;
        rdfs:label    "AnimalShelter" .

sdo:molecularFormula  rdfs:comment  "The empirical formula is the simplest whole number ratio of all the atoms in a molecule." ;
        rdfs:label    "molecular formula" .

sdo:option  rdfs:comment  "A sub property of object. The options subject to this action." ;
        rdfs:label    "option" .

sdo:equal  rdfs:comment  "This ordering relation for qualitative values indicates that the subject is equal to the object." ;
        rdfs:label    "equal" .

sdo:bitrate  rdfs:comment  "The bitrate of the media object." ;
        rdfs:label    "bitrate" .

sdo:version  rdfs:comment  "The version of the CreativeWork embodied by a specified resource." ;
        rdfs:label    "version" .

sdo:Sunday  rdfs:comment  "The day of the week between Saturday and Monday." ;
        rdfs:label    "Sunday" .

sdo:Head  rdfs:comment  "Head assessment with clinical examination." ;
        rdfs:label    "Head" .

sdo:Store  rdfs:comment  "A retail good store." ;
        rdfs:label    "Store" .

sdo:volumeNumber  rdfs:comment  "Identifies the volume of publication or multi-part work; for example, \"iii\" or \"2\"." ;
        rdfs:label    "volume number" .

sdo:additionalNumberOfGuests
        rdfs:comment  "If responding yes, the number of guests who will attend in addition to the invitee." ;
        rdfs:label    "additional numberOfGuests" .

sdo:Answer  rdfs:comment  "An answer offered to a question; perhaps correct, perhaps opinionated or wrong." ;
        rdfs:label    "Answer" .

sdo:employerOverview  rdfs:comment  "A description of the employer, career opportunities and work environment for this position." ;
        rdfs:label    "employer overview" .

sdo:entertainmentBusiness
        rdfs:comment  "A sub property of location. The entertainment business where the action occurred." ;
        rdfs:label    "entertainment business" .

sdo:commentTime  rdfs:comment  "The time at which the UserComment was made." ;
        rdfs:label    "comment time" .

sdo:Museum  rdfs:comment  "A museum." ;
        rdfs:label    "Museum" .

sdo:ccRecipient  rdfs:comment  "A sub property of recipient. The recipient copied on a message." ;
        rdfs:label    "cc recipient" .

sdo:FDAcategoryA  rdfs:comment  "A designation by the US FDA signifying that adequate and well-controlled studies have failed to demonstrate a risk to the fetus in the first trimester of pregnancy (and there is no evidence of risk in later trimesters)." ;
        rdfs:label    "FDAcategoryA" .

sdo:MovieSeries  rdfs:comment  "A series of movies. Included movies can be indicated with the hasPart property." ;
        rdfs:label    "MovieSeries" .

sdo:actionApplication
        rdfs:comment  "An application that can complete the request." ;
        rdfs:label    "action application" .

sdo:trainNumber  rdfs:comment  "The unique identifier for the train." ;
        rdfs:label    "train number" .

sdo:diversityPolicy  rdfs:comment  "Statement on diversity policy by an [[Organization]] e.g. a [[NewsMediaOrganization]]. For a [[NewsMediaOrganization]], a statement describing the newsroom’s diversity policy on both staffing and sources, typically providing staffing data." ;
        rdfs:label    "diversity policy" .

sdo:True  rdfs:comment  "The boolean value true." ;
        rdfs:label    "True" .

sdo:tongueWeight  rdfs:comment  "The permitted vertical load (TWR) of a trailer attached to the vehicle. Also referred to as Tongue Load Rating (TLR) or Vertical Load Rating (VLR)\\n\\nTypical unit code(s): KGM for kilogram, LBR for pound\\n\\n* Note 1: You can indicate additional information in the [[name]] of the [[QuantitativeValue]] node.\\n* Note 2: You may also link to a [[QualitativeValue]] node that provides additional information using [[valueReference]].\\n* Note 3: Note that you can use [[minValue]] and [[maxValue]] to indicate ranges." ;
        rdfs:label    "tongue weight" .

sdo:SymptomsHealthAspect
        rdfs:comment  "Symptoms or related symptoms of a Topic." ;
        rdfs:label    "SymptomsHealthAspect" .

sdo:recommendedIntake
        rdfs:comment  "Recommended intake of this supplement for a given population as defined by a specific recommending authority." ;
        rdfs:label    "recommended intake" .

sdo:ResearchOrganization
        rdfs:comment  "A Research Organization (e.g. scientific institute, research company)." ;
        rdfs:label    "ResearchOrganization" .

sdo:BodyMeasurementWeight
        rdfs:comment  "Body weight. Used, for example, to measure pantyhose." ;
        rdfs:label    "BodyMeasurementWeight" .

sdo:trialDesign  rdfs:comment  "Specifics about the trial design (enumerated)." ;
        rdfs:label    "trial design" .

sdo:MedicalRiskCalculator
        rdfs:comment  "A complex mathematical calculation requiring an online calculator, used to assess prognosis. Note: use the url property of Thing to record any URLs for online calculators." ;
        rdfs:label    "MedicalRiskCalculator" .

sdo:currentExchangeRate
        rdfs:comment  "The current price of a currency." ;
        rdfs:label    "current exchangeRate" .

sdo:temporal  rdfs:comment  "The \"temporal\" property can be used in cases where more specific properties\n(e.g. [[temporalCoverage]], [[dateCreated]], [[dateModified]], [[datePublished]]) are not known to be appropriate." ;
        rdfs:label    "temporal" .

sdo:WearableSizeSystemFR
        rdfs:comment  "French size system for wearables." ;
        rdfs:label    "WearableSizeSystemFR" .

sdo:RecommendedDoseSchedule
        rdfs:comment  "A recommended dosing schedule for a drug or supplement as prescribed or recommended by an authority or by the drug/supplement's manufacturer. Capture the recommending authority in the recognizingAuthority property of MedicalEntity." ;
        rdfs:label    "RecommendedDoseSchedule" .

sdo:AggregateRating  rdfs:comment  "The average rating based on multiple ratings or reviews." ;
        rdfs:label    "AggregateRating" .

sdo:exerciseRelatedDiet
        rdfs:comment  "A sub property of instrument. The diet used in this action." ;
        rdfs:label    "exercise relatedDiet" .

sdo:Psychiatric  rdfs:comment  "A specific branch of medical science that is concerned with the study, treatment, and prevention of mental illness, using both medical and psychological therapies." ;
        rdfs:label    "Psychiatric" .

sdo:travelBans  rdfs:comment  "Information about travel bans, e.g. in the context of a pandemic." ;
        rdfs:label    "travel bans" .

sdo:modelDate  rdfs:comment  "The release date of a vehicle model (often used to differentiate versions of the same make and model)." ;
        rdfs:label    "model date" .

sdo:numberedPosition  rdfs:comment  "A number associated with a role in an organization, for example, the number on an athlete's jersey." ;
        rdfs:label    "numbered position" .

sdo:productionDate  rdfs:comment  "The date of production of the item, e.g. vehicle." ;
        rdfs:label    "production date" .

sdo:yearsInOperation  rdfs:comment  "The age of the business." ;
        rdfs:label    "years inOperation" .

sdo:albumReleaseType  rdfs:comment  "The kind of release which this album is: single, EP or album." ;
        rdfs:label    "album releaseType" .

sdo:smokingAllowed  rdfs:comment  "Indicates whether it is allowed to smoke in the place, e.g. in the restaurant, hotel or hotel room." ;
        rdfs:label    "smoking allowed" .

sdo:offerCount  rdfs:comment  "The number of offers for the product." ;
        rdfs:label    "offer count" .

sdo:PaymentMethod  rdfs:comment  "A payment method is a standardized procedure for transferring the monetary amount for a purchase. Payment methods are characterized by the legal and technical structures used, and by the organization or group carrying out the transaction.\\n\\nCommonly used values:\\n\\n* http://purl.org/goodrelations/v1#ByBankTransferInAdvance\\n* http://purl.org/goodrelations/v1#ByInvoice\\n* http://purl.org/goodrelations/v1#Cash\\n* http://purl.org/goodrelations/v1#CheckInAdvance\\n* http://purl.org/goodrelations/v1#COD\\n* http://purl.org/goodrelations/v1#DirectDebit\\n* http://purl.org/goodrelations/v1#GoogleCheckout\\n* http://purl.org/goodrelations/v1#PayPal\\n* http://purl.org/goodrelations/v1#PaySwarm\n        " ;
        rdfs:label    "PaymentMethod" .

sdo:foundingLocation  rdfs:comment  "The place where the Organization was founded." ;
        rdfs:label    "founding location" .

sdo:bestRating  rdfs:comment  "The highest value allowed in this rating system. If bestRating is omitted, 5 is assumed." ;
        rdfs:label    "best rating" .

sdo:isVariantOf  rdfs:comment  "Indicates the kind of product that this is a variant of. In the case of [[ProductModel]], this is a pointer (from a ProductModel) to a base product from which this product is a variant. It is safe to infer that the variant inherits all product features from the base model, unless defined locally. This is not transitive. In the case of a [[ProductGroup]], the group description also serves as a template, representing a set of Products that vary on explicitly defined, specific dimensions only (so it defines both a set of variants, as well as which values distinguish amongst those variants). When used with [[ProductGroup]], this property can apply to any [[Product]] included in the group." ;
        rdfs:label    "is variantOf" .

sdo:isicV4  rdfs:comment  "The International Standard of Industrial Classification of All Economic Activities (ISIC), Revision 4 code for a particular organization, business person, or place." ;
        rdfs:label    "isic v4" .

sdo:recordedAs  rdfs:comment  "An audio recording of the work." ;
        rdfs:label    "recorded as" .

sdo:epidemiology  rdfs:comment  "The characteristics of associated patients, such as age, gender, race etc." ;
        rdfs:label    "epidemiology" .

sdo:documentation  rdfs:comment  "Further documentation describing the Web API in more detail." ;
        rdfs:label    "documentation" .

sdo:USNonprofitType  rdfs:comment  "USNonprofitType: Non-profit organization type originating from the United States." ;
        rdfs:label    "USNonprofitType" .

sdo:RsvpAction  rdfs:comment  "The act of notifying an event organizer as to whether you expect to attend the event." ;
        rdfs:label    "RsvpAction" .

sdo:OrderInTransit  rdfs:comment  "OrderStatus representing that an order is in transit." ;
        rdfs:label    "OrderInTransit" .

sdo:SizeSystemMetric  rdfs:comment  "Metric size system." ;
        rdfs:label    "SizeSystemMetric" .

sdo:GovernmentPermit  rdfs:comment  "A permit issued by a government agency." ;
        rdfs:label    "GovernmentPermit" .

sdo:numberOfItems  rdfs:comment  "The number of items in an ItemList. Note that some descriptions might not fully describe all items in a list (e.g., multi-page pagination); in such cases, the numberOfItems would be for the entire list." ;
        rdfs:label    "number ofItems" .

sdo:ComedyEvent  rdfs:comment  "Event type: Comedy event." ;
        rdfs:label    "ComedyEvent" .

sdo:addressLocality  rdfs:comment  "The locality in which the street address is, and which is in the region. For example, Mountain View." ;
        rdfs:label    "address locality" .

sdo:ExhibitionEvent  rdfs:comment  "Event type: Exhibition event, e.g. at a museum, library, archive, tradeshow, ..." ;
        rdfs:label    "ExhibitionEvent" .

sdo:HomeGoodsStore  rdfs:comment  "A home goods store." ;
        rdfs:label    "HomeGoodsStore" .

sdo:PlayAction  rdfs:comment  "The act of playing/exercising/training/performing for enjoyment, leisure, recreation, Competition or exercise.\\n\\nRelated actions:\\n\\n* [[ListenAction]]: Unlike ListenAction (which is under ConsumeAction), PlayAction refers to performing for an audience or at an event, rather than consuming music.\\n* [[WatchAction]]: Unlike WatchAction (which is under ConsumeAction), PlayAction refers to showing/displaying for an audience or at an event, rather than consuming visual content." ;
        rdfs:label    "PlayAction" .

sdo:legislationJurisdiction
        rdfs:comment  "The jurisdiction from which the legislation originates." ;
        rdfs:label    "legislation jurisdiction" .

sdo:VideoObjectSnapshot
        rdfs:comment  "A specific and exact (byte-for-byte) version of a [[VideoObject]]. Two byte-for-byte identical files, for the purposes of this type, considered identical. If they have different embedded metadata the files will differ. Different external facts about the files, e.g. creator or dateCreated that aren't represented in their actual content, do not affect this notion of identity." ;
        rdfs:label    "VideoObjectSnapshot" .

sdo:EnergyEfficiencyEnumeration
        rdfs:comment  "Enumerates energy efficiency levels (also known as \"classes\" or \"ratings\") and certifications that are part of several international energy efficiency standards." ;
        rdfs:label    "EnergyEfficiencyEnumeration" .

sdo:ImagingTest  rdfs:comment  "Any medical imaging modality typically used for diagnostic purposes." ;
        rdfs:label    "ImagingTest" .

sdo:Monday  rdfs:comment  "The day of the week between Sunday and Tuesday." ;
        rdfs:label    "Monday" .

sdo:maximumVirtualAttendeeCapacity
        rdfs:comment  "The maximum physical attendee capacity of an [[Event]] whose [[eventAttendanceMode]] is [[OnlineEventAttendanceMode]] (or the online aspects, in the case of a [[MixedEventAttendanceMode]]). " ;
        rdfs:label    "maximum virtualAttendeeCapacity" .

sdo:Mountain  rdfs:comment  "A mountain, like Mount Whitney or Mount Everest." ;
        rdfs:label    "Mountain" .

sdo:DisabilitySupport
        rdfs:comment  "DisabilitySupport: this is a benefit for disability support." ;
        rdfs:label    "DisabilitySupport" .

sdo:HyperToc  rdfs:comment  "A HyperToc represents a hypertext table of contents for complex media objects, such as [[VideoObject]], [[AudioObject]]. Items in the table of contents are indicated using the [[tocEntry]] property, and typed [[HyperTocEntry]]. For cases where the same larger work is split into multiple files, [[associatedMedia]] can be used on individual [[HyperTocEntry]] items." ;
        rdfs:label    "HyperToc" .

sdo:BusinessSupport  rdfs:comment  "BusinessSupport: this is a benefit for supporting businesses." ;
        rdfs:label    "BusinessSupport" .

sdo:PsychologicalTreatment
        rdfs:comment  "A process of care relying upon counseling, dialogue and communication  aimed at improving a mental health condition without use of drugs." ;
        rdfs:label    "PsychologicalTreatment" .

sdo:cssSelector  rdfs:comment  "A CSS selector, e.g. of a [[SpeakableSpecification]] or [[WebPageElement]]. In the latter case, multiple matches within a page can constitute a single conceptual \"Web page element\"." ;
        rdfs:label    "css selector" .

sdo:CookAction  rdfs:comment  "The act of producing/preparing food." ;
        rdfs:label    "CookAction" .

sdo:area  rdfs:comment  "The area within which users can expect to reach the broadcast service." ;
        rdfs:label    "area" .

sdo:parentTaxon  rdfs:comment  "Closest parent taxon of the taxon in question." ;
        rdfs:label    "parent taxon" .

sdo:GameServerStatus  rdfs:comment  "Status of a game server." ;
        rdfs:label    "GameServerStatus" .

sdo:sensoryRequirement
        rdfs:comment  "A description of any sensory requirements and levels necessary to function on the job, including hearing and vision. Defined terms such as those in O*net may be used, but note that there is no way to specify the level of ability as well as its nature when using a defined term." ;
        rdfs:label    "sensory requirement" .

sdo:taxonRank  rdfs:comment  "The taxonomic rank of this taxon given preferably as a URI from a controlled vocabulary – (typically the ranks from TDWG TaxonRank ontology or equivalent Wikidata URIs)." ;
        rdfs:label    "taxon rank" .

sdo:abridged  rdfs:comment  "Indicates whether the book is an abridged edition." ;
        rdfs:label    "abridged" .

sdo:Nonprofit501c1  rdfs:comment  "Nonprofit501c1: Non-profit type referring to Corporations Organized Under Act of Congress, including Federal Credit Unions and National Farm Loan Associations." ;
        rdfs:label    "Nonprofit501c1" .

sdo:OrderCancelled  rdfs:comment  "OrderStatus representing cancellation of an order." ;
        rdfs:label    "OrderCancelled" .

sdo:Clip  rdfs:comment  "A short TV or radio program or a segment/part of a program." ;
        rdfs:label    "Clip" .

sdo:replacer  rdfs:comment  "A sub property of object. The object that replaces." ;
        rdfs:label    "replacer" .

sdo:HealthTopicContent
        rdfs:comment  "[[HealthTopicContent]] is [[WebContent]] that is about some aspect of a health topic, e.g. a condition, its symptoms or treatments. Such content may be comprised of several parts or sections and use different types of media. Multiple instances of [[WebContent]] (and hence [[HealthTopicContent]]) can be related using [[hasPart]] / [[isPartOf]] where there is some kind of content hierarchy, and their content described with [[about]] and [[mentions]] e.g. building upon the existing [[MedicalCondition]] vocabulary.\n  " ;
        rdfs:label    "HealthTopicContent" .

sdo:tool  rdfs:comment  "A sub property of instrument. An object used (but not consumed) when performing instructions or a direction." ;
        rdfs:label    "tool" .

sdo:MortgageLoan  rdfs:comment  "A loan in which property or real estate is used as collateral. (A loan securitized against some real estate)." ;
        rdfs:label    "MortgageLoan" .

sdo:jobImmediateStart
        rdfs:comment  "An indicator as to whether a position is available for an immediate start." ;
        rdfs:label    "job immediateStart" .

sdo:RentAction  rdfs:comment  "The act of giving money in return for temporary use, but not ownership, of an object such as a vehicle or property. For example, an agent rents a property from a landlord in exchange for a periodic payment." ;
        rdfs:label    "RentAction" .

sdo:programMembershipUsed
        rdfs:comment  "Any membership in a frequent flyer, hotel loyalty program, etc. being applied to the reservation." ;
        rdfs:label    "program membershipUsed" .

sdo:workLocation  rdfs:comment  "A contact location for a person's place of work." ;
        rdfs:label    "work location" .

sdo:WarrantyPromise  rdfs:comment  "A structured value representing the duration and scope of services that will be provided to a customer free of charge in case of a defect or malfunction of a product." ;
        rdfs:label    "WarrantyPromise" .

sdo:ParentalSupport  rdfs:comment  "ParentalSupport: this is a benefit for parental support." ;
        rdfs:label    "ParentalSupport" .

sdo:leaseLength  rdfs:comment  "Length of the lease for some [[Accommodation]], either particular to some [[Offer]] or in some cases intrinsic to the property." ;
        rdfs:label    "lease length" .

sdo:specialty  rdfs:comment  "One of the domain specialities to which this web page's content applies." ;
        rdfs:label    "specialty" .

sdo:cvdNumC19OFMechVentPats
        rdfs:comment  "numc19ofmechventpats - ED/OVERFLOW and VENTILATED: Patients with suspected or confirmed COVID-19 who are in the ED or any overflow location awaiting an inpatient bed and on a mechanical ventilator." ;
        rdfs:label    "cvd numC19OFMechVentPats" .

sdo:diseaseSpreadStatistics
        rdfs:comment  "Statistical information about the spread of a disease, either as [[WebContent]], or\n  described directly as a [[Dataset]], or the specific [[Observation]]s in the dataset. When a [[WebContent]] URL is\n  provided, the page indicated might also contain more such markup." ;
        rdfs:label    "disease spreadStatistics" .

sdo:AutoBodyShop  rdfs:comment  "Auto body shop." ;
        rdfs:label    "AutoBodyShop" .

sdo:originAddress  rdfs:comment  "Shipper's address." ;
        rdfs:label    "origin address" .

sdo:PharmacySpecialty
        rdfs:comment  "The practice or art and science of preparing and dispensing drugs and medicines." ;
        rdfs:label    "PharmacySpecialty" .

sdo:drugClass  rdfs:comment  "The class of drug this belongs to (e.g., statins)." ;
        rdfs:label    "drug class" .

sdo:highPrice  rdfs:comment  "The highest price of all offers available.\\n\\nUsage guidelines:\\n\\n* Use values from 0123456789 (Unicode 'DIGIT ZERO' (U+0030) to 'DIGIT NINE' (U+0039)) rather than superficially similiar Unicode symbols.\\n* Use '.' (Unicode 'FULL STOP' (U+002E)) rather than ',' to indicate a decimal point. Avoid using these symbols as a readability separator." ;
        rdfs:label    "high price" .

sdo:cvdFacilityId  rdfs:comment  "Identifier of the NHSN facility that this data record applies to. Use [[cvdFacilityCounty]] to indicate the county. To provide other details, [[healthcareReportingData]] can be used on a [[Hospital]] entry." ;
        rdfs:label    "cvd facilityId" .

sdo:MusicReleaseFormatType
        rdfs:comment  "Format of this release (the type of recording media used, ie. compact disc, digital media, LP, etc.)." ;
        rdfs:label    "MusicReleaseFormatType" .

sdo:DepartmentStore  rdfs:comment  "A department store." ;
        rdfs:label    "DepartmentStore" .

sdo:supplyTo  rdfs:comment  "The area to which the artery supplies blood." ;
        rdfs:label    "supply to" .

sdo:itemDefectReturnFees
        rdfs:comment  "The type of return fees for returns of defect products." ;
        rdfs:label    "item defectReturnFees" .

sdo:CollegeOrUniversity
        rdfs:comment  "A college, university, or other third-level educational institution." ;
        rdfs:label    "CollegeOrUniversity" .

sdo:passengerPriorityStatus
        rdfs:comment  "The priority status assigned to a passenger for security or boarding (e.g. FastTrack or Priority)." ;
        rdfs:label    "passenger priorityStatus" .

sdo:coach  rdfs:comment  "A person that acts in a coaching role for a sports team." ;
        rdfs:label    "coach" .

sdo:speed  rdfs:comment  "The speed range of the vehicle. If the vehicle is powered by an engine, the upper limit of the speed range (indicated by [[maxValue]] should be the maximum speed achievable under regular conditions.\\n\\nTypical unit code(s): KMH for km/h, HM for mile per hour (0.447 04 m/s), KNT for knot\\n\\n*Note 1: Use [[minValue]] and [[maxValue]] to indicate the range. Typically, the minimal value is zero.\\n* Note 2: There are many different ways of measuring the speed range. You can link to information about how the given value has been determined using the [[valueReference]] property." ;
        rdfs:label    "speed" .

sdo:educationRequirements
        rdfs:comment  "Educational background needed for the position or Occupation." ;
        rdfs:label    "education requirements" .

sdo:membershipPointsEarned
        rdfs:comment  "The number of membership points earned by the member. If necessary, the unitText can be used to express the units the points are issued in. (e.g. stars, miles, etc.)" ;
        rdfs:label    "membership pointsEarned" .

sdo:PreOrderAction  rdfs:comment  "An agent orders a (not yet released) object/product/service to be delivered/sent." ;
        rdfs:label    "PreOrderAction" .

sdo:scheduledTime  rdfs:comment  "The time the object is scheduled to." ;
        rdfs:label    "scheduled time" .

sdo:shippingRate  rdfs:comment  "The shipping rate is the cost of shipping to the specified destination. Typically, the maxValue and currency values (of the [[MonetaryAmount]]) are most appropriate." ;
        rdfs:label    "shipping rate" .

sdo:BusinessFunction  rdfs:comment  "The business function specifies the type of activity or access (i.e., the bundle of rights) offered by the organization or business person through the offer. Typical are sell, rental or lease, maintenance or repair, manufacture / produce, recycle / dispose, engineering / construction, or installation. Proprietary specifications of access rights are also instances of this class.\\n\\nCommonly used values:\\n\\n* http://purl.org/goodrelations/v1#ConstructionInstallation\\n* http://purl.org/goodrelations/v1#Dispose\\n* http://purl.org/goodrelations/v1#LeaseOut\\n* http://purl.org/goodrelations/v1#Maintain\\n* http://purl.org/goodrelations/v1#ProvideService\\n* http://purl.org/goodrelations/v1#Repair\\n* http://purl.org/goodrelations/v1#Sell\\n* http://purl.org/goodrelations/v1#Buy\n        " ;
        rdfs:label    "BusinessFunction" .

sdo:termCode  rdfs:comment  "A code that identifies this [[DefinedTerm]] within a [[DefinedTermSet]]" ;
        rdfs:label    "term code" .

sdo:dissolutionDate  rdfs:comment  "The date that this organization was dissolved." ;
        rdfs:label    "dissolution date" .

sdo:ownedFrom  rdfs:comment  "The date and time of obtaining the product." ;
        rdfs:label    "owned from" .

sdo:HowToDirection  rdfs:comment  "A direction indicating a single action to do in the instructions for how to achieve a result." ;
        rdfs:label    "HowToDirection" .

sdo:DrugCost  rdfs:comment  "The cost per unit of a medical drug. Note that this type is not meant to represent the price in an offer of a drug for sale; see the Offer type for that. This type will typically be used to tag wholesale or average retail cost of a drug, or maximum reimbursable cost. Costs of medical drugs vary widely depending on how and where they are paid for, so while this type captures some of the variables, costs should be used with caution by consumers of this schema's markup." ;
        rdfs:label    "DrugCost" .

sdo:Physiotherapy  rdfs:comment  "The practice of treatment of disease, injury, or deformity by physical methods such as massage, heat treatment, and exercise rather than by drugs or surgery.." ;
        rdfs:label    "Physiotherapy" .

sdo:Wholesale  rdfs:comment  "The drug's cost represents the wholesale acquisition cost of the drug." ;
        rdfs:label    "Wholesale" .

sdo:intensity  rdfs:comment  "Quantitative measure gauging the degree of force involved in the exercise, for example, heartbeats per minute. May include the velocity of the movement." ;
        rdfs:label    "intensity" .

sdo:AllWheelDriveConfiguration
        rdfs:comment  "All-wheel Drive is a transmission layout where the engine drives all four wheels." ;
        rdfs:label    "AllWheelDriveConfiguration" .

sdo:arrivalTerminal  rdfs:comment  "Identifier of the flight's arrival terminal." ;
        rdfs:label    "arrival terminal" .

sdo:MedicalCondition  rdfs:comment  "Any condition of the human body that affects the normal functioning of a person, whether physically or mentally. Includes diseases, injuries, disabilities, disorders, syndromes, etc." ;
        rdfs:label    "MedicalCondition" .

sdo:encodesCreativeWork
        rdfs:comment  "The CreativeWork encoded by this media object." ;
        rdfs:label    "encodes creativeWork" .

sdo:suggestedMeasurement
        rdfs:comment  "A suggested range of body measurements for the intended audience or person, for example inseam between 32 and 34 inches or height between 170 and 190 cm. Typically found on a size chart for wearable products." ;
        rdfs:label    "suggested measurement" .

sdo:PathologyTest  rdfs:comment  "A medical test performed by a laboratory that typically involves examination of a tissue sample by a pathologist." ;
        rdfs:label    "PathologyTest" .

sdo:MapCategoryType  rdfs:comment  "An enumeration of several kinds of Map." ;
        rdfs:label    "MapCategoryType" .

sdo:translationOfWork
        rdfs:comment  "The work that this work has been translated from. e.g. 物种起源 is a translationOf “On the Origin of Species”" ;
        rdfs:label    "translation ofWork" .

sdo:SizeSystemImperial
        rdfs:comment  "Imperial size system." ;
        rdfs:label    "SizeSystemImperial" .

sdo:blogPosts  rdfs:comment  "Indicates a post that is part of a [[Blog]]. Note that historically, what we term a \"Blog\" was once known as a \"weblog\", and that what we term a \"BlogPosting\" is now often colloquially referred to as a \"blog\"." ;
        rdfs:label    "blog posts" .

sdo:Game  rdfs:comment  "The Game type represents things which are games. These are typically rule-governed recreational activities, e.g. role-playing games in which players assume the role of characters in a fictional setting." ;
        rdfs:label    "Game" .

sdo:Schedule  rdfs:comment  "A schedule defines a repeating time period used to describe a regularly occurring [[Event]]. At a minimum a schedule will specify [[repeatFrequency]] which describes the interval between occurences of the event. Additional information can be provided to specify the schedule more precisely.\n      This includes identifying the day(s) of the week or month when the recurring event will take place, in addition to its start and end time. Schedules may also\n      have start and end dates to indicate when they are active, e.g. to define a limited calendar of events." ;
        rdfs:label    "Schedule" .

sdo:WearableSizeGroupGirls
        rdfs:comment  "Size group \"Girls\" for wearables." ;
        rdfs:label    "WearableSizeGroupGirls" .

sdo:GameServer  rdfs:comment  "Server that provides game interaction in a multiplayer game." ;
        rdfs:label    "GameServer" .

sdo:answerCount  rdfs:comment  "The number of answers this question has received." ;
        rdfs:label    "answer count" .

sdo:headline  rdfs:comment  "Headline of the article." ;
        rdfs:label    "headline" .

sdo:SingleBlindedTrial
        rdfs:comment  "A trial design in which the researcher knows which treatment the patient was randomly assigned to but the patient does not." ;
        rdfs:label    "SingleBlindedTrial" .

sdo:dietFeatures  rdfs:comment  "Nutritional information specific to the dietary plan. May include dietary recommendations on what foods to avoid, what foods to consume, and specific alterations/deviations from the USDA or other regulatory body's approved dietary guidelines." ;
        rdfs:label    "diet features" .

sdo:bookingAgent  rdfs:comment  "'bookingAgent' is an out-dated term indicating a 'broker' that serves as a booking agent." ;
        rdfs:label    "booking agent" .

sdo:catalogNumber  rdfs:comment  "The catalog number for the release." ;
        rdfs:label    "catalog number" .

sdo:TransitMap  rdfs:comment  "A transit map." ;
        rdfs:label    "TransitMap" .

sdo:SoldOut  rdfs:comment  "Indicates that the item has sold out." ;
        rdfs:label    "SoldOut" .

sdo:MotorizedBicycle  rdfs:comment  "A motorized bicycle is a bicycle with an attached motor used to power the vehicle, or to assist with pedaling." ;
        rdfs:label    "MotorizedBicycle" .

sdo:jobLocation  rdfs:comment  "A (typically single) geographic location associated with the job position." ;
        rdfs:label    "job location" .

sdo:season  rdfs:comment  "A season in a media series." ;
        rdfs:label    "season" .

sdo:sport  rdfs:comment  "A type of sport (e.g. Baseball)." ;
        rdfs:label    "sport" .

sdo:UnemploymentSupport
        rdfs:comment  "UnemploymentSupport: this is a benefit for unemployment support." ;
        rdfs:label    "UnemploymentSupport" .

sdo:MedicalProcedureType
        rdfs:comment  "An enumeration that describes different types of medical procedures." ;
        rdfs:label    "MedicalProcedureType" .

sdo:physiologicalBenefits
        rdfs:comment  "Specific physiologic benefits associated to the plan." ;
        rdfs:label    "physiological benefits" .

sdo:postalCodeEnd  rdfs:comment  "Last postal code in the range (included). Needs to be after [[postalCodeBegin]]." ;
        rdfs:label    "postal codeEnd" .

sdo:numberOfFullBathrooms
        rdfs:comment  "Number of full bathrooms - The total number of full and ¾ bathrooms in an [[Accommodation]]. This corresponds to the [BathroomsFull field in RESO](https://ddwiki.reso.org/display/DDW17/BathroomsFull+Field)." ;
        rdfs:label    "number ofFullBathrooms" .

sdo:Online  rdfs:comment  "Game server status: Online. Server is available." ;
        rdfs:label    "Online" .

sdo:WearableMeasurementCollar
        rdfs:comment  "Measurement of the collar, for example of a shirt" ;
        rdfs:label    "WearableMeasurementCollar" .

sdo:InsertAction  rdfs:comment  "The act of adding at a specific location in an ordered collection." ;
        rdfs:label    "InsertAction" .

sdo:ReserveAction  rdfs:comment  "Reserving a concrete object.\\n\\nRelated actions:\\n\\n* [[ScheduleAction]]: Unlike ScheduleAction, ReserveAction reserves concrete objects (e.g. a table, a hotel) towards a time slot / spatial allocation." ;
        rdfs:label    "ReserveAction" .

sdo:hasOccupation  rdfs:comment  "The Person's occupation. For past professions, use Role for expressing dates." ;
        rdfs:label    "has occupation" .

sdo:roleName  rdfs:comment  "A role played, performed or filled by a person or organization. For example, the team of creators for a comic book might fill the roles named 'inker', 'penciller', and 'letterer'; or an athlete in a SportsTeam might play in the position named 'Quarterback'." ;
        rdfs:label    "role name" .

sdo:normalRange  rdfs:comment  "Range of acceptable values for a typical patient, when applicable." ;
        rdfs:label    "normal range" .

sdo:contactlessPayment
        rdfs:comment  "A secure method for consumers to purchase products or services via debit, credit or smartcards by using RFID or NFC technology." ;
        rdfs:label    "contactless payment" .

sdo:sdLicense  rdfs:comment  "A license document that applies to this structured data, typically indicated by URL." ;
        rdfs:label    "sd license" .

sdo:customer  rdfs:comment  "Party placing the order or paying the invoice." ;
        rdfs:label    "customer" .

sdo:gettingTestedInfo
        rdfs:comment  "Information about getting tested (for a [[MedicalCondition]]), e.g. in the context of a pandemic." ;
        rdfs:label    "getting testedInfo" .

sdo:billingDuration  rdfs:comment  "Specifies for how long this price (or price component) will be billed. Can be used, for example, to model the contractual duration of a subscription or payment plan. Type can be either a Duration or a Number (in which case the unit of measurement, for example month, is specified by the unitCode property)." ;
        rdfs:label    "billing duration" .

sdo:loser  rdfs:comment  "A sub property of participant. The loser of the action." ;
        rdfs:label    "loser" .

sdo:embedUrl  rdfs:comment  "A URL pointing to a player for a specific video. In general, this is the information in the ```src``` element of an ```embed``` tag and should not be the same as the content of the ```loc``` tag." ;
        rdfs:label    "embed url" .

sdo:bloodSupply  rdfs:comment  "The blood vessel that carries blood from the heart to the muscle." ;
        rdfs:label    "blood supply" .

sdo:lyrics  rdfs:comment  "The words in the song." ;
        rdfs:label    "lyrics" .

sdo:EffectivenessHealthAspect
        rdfs:comment  "Content about the effectiveness-related aspects of a health topic." ;
        rdfs:label    "EffectivenessHealthAspect" .

sdo:readonlyValue  rdfs:comment  "Whether or not a property is mutable.  Default is false. Specifying this for a property that also has a value makes it act similar to a \"hidden\" input in an HTML form." ;
        rdfs:label    "readonly value" .

sdo:previousItem  rdfs:comment  "A link to the ListItem that preceeds the current one." ;
        rdfs:label    "previous item" .

sdo:Appearance  rdfs:comment  "Appearance assessment with clinical examination." ;
        rdfs:label    "Appearance" .

sdo:Hematologic  rdfs:comment  "A specific branch of medical science that pertains to diagnosis and treatment of disorders of blood and blood producing organs." ;
        rdfs:label    "Hematologic" .

sdo:Nonprofit501c27  rdfs:comment  "Nonprofit501c27: Non-profit type referring to State-Sponsored Workers' Compensation Reinsurance Organizations." ;
        rdfs:label    "Nonprofit501c27" .

sdo:shippingLabel  rdfs:comment  "Label to match an [[OfferShippingDetails]] with a [[ShippingRateSettings]] (within the context of a [[shippingSettingsLink]] cross-reference)." ;
        rdfs:label    "shipping label" .

sdo:map  rdfs:comment  "A URL to a map of the place." ;
        rdfs:label    "map" .

sdo:ethicsPolicy  rdfs:comment  "Statement about ethics policy, e.g. of a [[NewsMediaOrganization]] regarding journalistic and publishing practices, or of a [[Restaurant]], a page describing food source policies. In the case of a [[NewsMediaOrganization]], an ethicsPolicy is typically a statement describing the personal, organizational, and corporate standards of behavior expected by the organization." ;
        rdfs:label    "ethics policy" .

sdo:subjectOf  rdfs:comment  "A CreativeWork or Event about this Thing." ;
        rdfs:label    "subject of" .

sdo:OfflinePermanently
        rdfs:comment  "Game server status: OfflinePermanently. Server is offline and not available." ;
        rdfs:label    "OfflinePermanently" .

sdo:sourcedFrom  rdfs:comment  "The neurological pathway that originates the neurons." ;
        rdfs:label    "sourced from" .

sdo:MedicalContraindication
        rdfs:comment  "A condition or factor that serves as a reason to withhold a certain medical therapy. Contraindications can be absolute (there are no reasonable circumstances for undertaking a course of action) or relative (the patient is at higher risk of complications, but that these risks may be outweighed by other considerations or mitigated by other measures)." ;
        rdfs:label    "MedicalContraindication" .

sdo:percentile10  rdfs:comment  "The 10th percentile value." ;
        rdfs:label    "percentile10" .

sdo:CableOrSatelliteService
        rdfs:comment  "A service which provides access to media programming like TV or radio. Access may be via cable or satellite." ;
        rdfs:label    "CableOrSatelliteService" .

sdo:accountMinimumInflow
        rdfs:comment  "A minimum amount that has to be paid in every month." ;
        rdfs:label    "account minimumInflow" .

sdo:description  rdfs:comment  "A description of the item." ;
        rdfs:label    "description" .

sdo:SpeechPathology  rdfs:comment  "The scientific study and treatment of defects, disorders, and malfunctions of speech and voice, as stuttering, lisping, or lalling, and of language disturbances, as aphasia or delayed language acquisition." ;
        rdfs:label    "SpeechPathology" .

sdo:LowFatDiet  rdfs:comment  "A diet focused on reduced fat and cholesterol intake." ;
        rdfs:label    "LowFatDiet" .

sdo:PreSale  rdfs:comment  "Indicates that the item is available for ordering and delivery before general availability." ;
        rdfs:label    "PreSale" .

sdo:AssignAction  rdfs:comment  "The act of allocating an action/event/task to some destination (someone or something)." ;
        rdfs:label    "AssignAction" .

sdo:ticketNumber  rdfs:comment  "The unique identifier for the ticket." ;
        rdfs:label    "ticket number" .

sdo:audio  rdfs:comment  "An embedded audio object." ;
        rdfs:label    "audio" .

sdo:WearableMeasurementInseam
        rdfs:comment  "Measurement of the inseam, for example of pants" ;
        rdfs:label    "WearableMeasurementInseam" .

sdo:UserPageVisits  rdfs:comment  "UserInteraction and its subtypes is an old way of talking about users interacting with pages. It is generally better to use [[Action]]-based vocabulary, alongside types such as [[Comment]]." ;
        rdfs:label    "UserPageVisits" .

sdo:WearableSizeGroupPetite
        rdfs:comment  "Size group \"Petite\" for wearables." ;
        rdfs:label    "WearableSizeGroupPetite" .

sdo:programPrerequisites
        rdfs:comment  "Prerequisites for enrolling in the program." ;
        rdfs:label    "program prerequisites" .

sdo:cvdNumC19HOPats  rdfs:comment  "numc19hopats - HOSPITAL ONSET: Patients hospitalized in an NHSN inpatient care location with onset of suspected or confirmed COVID-19 14 or more days after hospitalization." ;
        rdfs:label    "cvd numC19HOPats" .

sdo:RelatedTopicsHealthAspect
        rdfs:comment  "Other prominent or relevant topics tied to the main topic." ;
        rdfs:label    "RelatedTopicsHealthAspect" .

sdo:passengerSequenceNumber
        rdfs:comment  "The passenger's sequence number as assigned by the airline." ;
        rdfs:label    "passenger sequenceNumber" .

sdo:Distance  rdfs:comment  "Properties that take Distances as values are of the form '&lt;Number&gt; &lt;Length unit of measure&gt;'. E.g., '7 ft'." ;
        rdfs:label    "Distance" .

sdo:cvdNumC19HospPats
        rdfs:comment  "numc19hosppats - HOSPITALIZED: Patients currently hospitalized in an inpatient care location who have suspected or confirmed COVID-19." ;
        rdfs:label    "cvd numC19HospPats" .

sdo:PayAction  rdfs:comment  "An agent pays a price to a participant." ;
        rdfs:label    "PayAction" .

sdo:childTaxon  rdfs:comment  "Closest child taxa of the taxon in question." ;
        rdfs:label    "child taxon" .

sdo:suggestedGender  rdfs:comment  "The suggested gender of the intended person or audience, for example \"male\", \"female\", or \"unisex\"." ;
        rdfs:label    "suggested gender" .

sdo:DisagreeAction  rdfs:comment  "The act of expressing a difference of opinion with the object. An agent disagrees to/about an object (a proposition, topic or theme) with participants." ;
        rdfs:label    "DisagreeAction" .

sdo:AutoPartsStore  rdfs:comment  "An auto parts store." ;
        rdfs:label    "AutoPartsStore" .

sdo:GeneralContractor
        rdfs:comment  "A general contractor." ;
        rdfs:label    "GeneralContractor" .

sdo:Dermatologic  rdfs:comment  "Something relating to or practicing dermatology." ;
        rdfs:label    "Dermatologic" .

sdo:reviewCount  rdfs:comment  "The count of total number of reviews." ;
        rdfs:label    "review count" .

sdo:performer  rdfs:comment  "A performer at the event&#x2014;for example, a presenter, musician, musical group or actor." ;
        rdfs:label    "performer" .

sdo:weight  rdfs:comment  "The weight of the product or person." ;
        rdfs:label    "weight" .

sdo:FDAcategoryC  rdfs:comment  "A designation by the US FDA signifying that animal reproduction studies have shown an adverse effect on the fetus and there are no adequate and well-controlled studies in humans, but potential benefits may warrant use of the drug in pregnant women despite potential risks." ;
        rdfs:label    "FDAcategoryC" .

sdo:Researcher  rdfs:comment  "Researchers." ;
        rdfs:label    "Researcher" .

sdo:FailedActionStatus
        rdfs:comment  "An action that failed to complete. The action's error property and the HTTP return code contain more information about the failure." ;
        rdfs:label    "FailedActionStatus" .

sdo:itemReviewed  rdfs:comment  "The item that is being reviewed/rated." ;
        rdfs:label    "item reviewed" .

sdo:Protein  rdfs:comment  "Protein is here used in its widest possible definition, as classes of amino acid based molecules. Amyloid-beta Protein in human (UniProt P05067), eukaryota (e.g. an OrthoDB group) or even a single molecule that one can point to are all of type schema:Protein. A protein can thus be a subclass of another protein, e.g. schema:Protein as a UniProt record can have multiple isoforms inside it which would also be schema:Protein. They can be imagined, synthetic, hypothetical or naturally occurring." ;
        rdfs:label    "Protein" .

sdo:correction  rdfs:comment  "Indicates a correction to a [[CreativeWork]], either via a [[CorrectionComment]], textually or in another document." ;
        rdfs:label    "correction" .

sdo:accelerationTime  rdfs:comment  "The time needed to accelerate the vehicle from a given start velocity to a given target velocity.\\n\\nTypical unit code(s): SEC for seconds\\n\\n* Note: There are unfortunately no standard unit codes for seconds/0..100 km/h or seconds/0..60 mph. Simply use \"SEC\" for seconds and indicate the velocities in the [[name]] of the [[QuantitativeValue]], or use [[valueReference]] with a [[QuantitativeValue]] of 0..60 mph or 0..100 km/h to specify the reference speeds." ;
        rdfs:label    "acceleration time" .

sdo:Balance  rdfs:comment  "Physical activity that is engaged to help maintain posture and balance." ;
        rdfs:label    "Balance" .

sdo:TradeAction  rdfs:comment  "The act of participating in an exchange of goods and services for monetary compensation. An agent trades an object, product or service with a participant in exchange for a one time or periodic payment." ;
        rdfs:label    "TradeAction" .

sdo:codeRepository  rdfs:comment  "Link to the repository where the un-compiled, human readable code and related code is located (SVN, github, CodePlex)." ;
        rdfs:label    "code repository" .

sdo:maximumPhysicalAttendeeCapacity
        rdfs:comment  "The maximum physical attendee capacity of an [[Event]] whose [[eventAttendanceMode]] is [[OfflineEventAttendanceMode]] (or the offline aspects, in the case of a [[MixedEventAttendanceMode]]). " ;
        rdfs:label    "maximum physicalAttendeeCapacity" .

sdo:biomechnicalClass
        rdfs:comment  "The biomechanical properties of the bone." ;
        rdfs:label    "biomechnical class" .

sdo:featureList  rdfs:comment  "Features or modules provided by this application (and possibly required by other applications)." ;
        rdfs:label    "feature list" .

sdo:Electrician  rdfs:comment  "An electrician." ;
        rdfs:label    "Electrician" .

sdo:referenceQuantity
        rdfs:comment  "The reference quantity for which a certain price applies, e.g. 1 EUR per 4 kWh of electricity. This property is a replacement for unitOfMeasurement for the advanced cases where the price does not relate to a standard unit." ;
        rdfs:label    "reference quantity" .

sdo:UserComments  rdfs:comment  "UserInteraction and its subtypes is an old way of talking about users interacting with pages. It is generally better to use [[Action]]-based vocabulary, alongside types such as [[Comment]]." ;
        rdfs:label    "UserComments" .

sdo:byDay  rdfs:comment  "Defines the day(s) of the week on which a recurring [[Event]] takes place. May be specified using either [[DayOfWeek]], or alternatively [[Text]] conforming to iCal's syntax for byDay recurrence rules." ;
        rdfs:label    "by day" .

sdo:SportsTeam  rdfs:comment  "Organization: Sports team." ;
        rdfs:label    "SportsTeam" .

sdo:AutoRepair  rdfs:comment  "Car repair business." ;
        rdfs:label    "AutoRepair" .

sdo:PresentationDigitalDocument
        rdfs:comment  "A file containing slides or used for a presentation." ;
        rdfs:label    "PresentationDigitalDocument" .

sdo:ActivateAction  rdfs:comment  "The act of starting or activating a device or application (e.g. starting a timer or turning on a flashlight)." ;
        rdfs:label    "ActivateAction" .

sdo:RecyclingCenter  rdfs:comment  "A recycling center." ;
        rdfs:label    "RecyclingCenter" .

sdo:CurrencyConversionService
        rdfs:comment  "A service to convert funds from one currency to another currency." ;
        rdfs:label    "CurrencyConversionService" .

sdo:RadioSeason  rdfs:comment  "Season dedicated to radio broadcast and associated online delivery." ;
        rdfs:label    "RadioSeason" .

sdo:WearableMeasurementBack
        rdfs:comment  "Measurement of the back section, for example of a jacket" ;
        rdfs:label    "WearableMeasurementBack" .

sdo:BedDetails  rdfs:comment  "An entity holding detailed information about the available bed types, e.g. the quantity of twin beds for a hotel room. For the single case of just one bed of a certain type, you can use bed directly with a text. See also [[BedType]] (under development)." ;
        rdfs:label    "BedDetails" .

sdo:Nonprofit501c4  rdfs:comment  "Nonprofit501c4: Non-profit type referring to Civic Leagues, Social Welfare Organizations, and Local Associations of Employees." ;
        rdfs:label    "Nonprofit501c4" .

sdo:MedicalTrial  rdfs:comment  "A medical trial is a type of medical study that uses scientific process used to compare the safety and efficacy of medical therapies or medical procedures. In general, medical trials are controlled and subjects are allocated at random to the different treatment and/or control groups." ;
        rdfs:label    "MedicalTrial" .

sdo:result  rdfs:comment  "The result produced in the action. e.g. John wrote *a book*." ;
        rdfs:label    "result" .

sdo:Integer  rdfs:comment  "Data type: Integer." ;
        rdfs:label    "Integer" .

sdo:ExchangeRateSpecification
        rdfs:comment  "A structured value representing exchange rate." ;
        rdfs:label    "ExchangeRateSpecification" .

sdo:Taxon  rdfs:comment  "A set of organisms asserted to represent a natural cohesive biological unit." ;
        rdfs:label    "Taxon" .

sdo:Canal  rdfs:comment  "A canal, like the Panama Canal." ;
        rdfs:label    "Canal" .

sdo:performers  rdfs:comment  "The main performer or performers of the event&#x2014;for example, a presenter, musician, or actor." ;
        rdfs:label    "performers" .

sdo:monoisotopicMolecularWeight
        rdfs:comment  "The monoisotopic mass is the sum of the masses of the atoms in a molecule using the unbound, ground-state, rest mass of the principal (most abundant) isotope for each element instead of the isotopic average mass. Please include the units the form '&lt;Number&gt; &lt;unit&gt;', for example '770.230488 g/mol' or as '&lt;QuantitativeValue&gt;." ;
        rdfs:label    "monoisotopic molecularWeight" .

sdo:Table  rdfs:comment  "A table on a Web page." ;
        rdfs:label    "Table" .

sdo:OverviewHealthAspect
        rdfs:comment  "Overview of the content. Contains a summarized view of the topic with the most relevant information for an introduction." ;
        rdfs:label    "OverviewHealthAspect" .

sdo:WebPageElement  rdfs:comment  "A web page element, like a table or an image." ;
        rdfs:label    "WebPageElement" .

sdo:jobBenefits  rdfs:comment  "Description of benefits associated with the job." ;
        rdfs:label    "job benefits" .

sdo:targetDescription
        rdfs:comment  "The description of a node in an established educational framework." ;
        rdfs:label    "target description" .

sdo:EUEnergyEfficiencyCategoryD
        rdfs:comment  "Represents EU Energy Efficiency Class D as defined in EU energy labeling regulations." ;
        rdfs:label    "EUEnergyEfficiencyCategoryD" .

sdo:estimatedSalary  rdfs:comment  "An estimated salary for a job posting or occupation, based on a variety of variables including, but not limited to industry, job title, and location. Estimated salaries  are often computed by outside organizations rather than the hiring organization, who may not have committed to the estimated value." ;
        rdfs:label    "estimated salary" .

sdo:MedicalObservationalStudy
        rdfs:comment  "An observational study is a type of medical study that attempts to infer the possible effect of a treatment through observation of a cohort of subjects over a period of time. In an observational study, the assignment of subjects into treatment groups versus control groups is outside the control of the investigator. This is in contrast with controlled studies, such as the randomized controlled trials represented by MedicalTrial, where each subject is randomly assigned to a treatment group or a control group before the start of the treatment." ;
        rdfs:label    "MedicalObservationalStudy" .

sdo:width  rdfs:comment  "The width of the item." ;
        rdfs:label    "width" .

sdo:iupacName  rdfs:comment  "Systematic method of naming chemical compounds as recommended by the International Union of Pure and Applied Chemistry (IUPAC)." ;
        rdfs:label    "iupac name" .

sdo:sponsor  rdfs:comment  "A person or organization that supports a thing through a pledge, promise, or financial contribution. e.g. a sponsor of a Medical Study or a corporate sponsor of an event." ;
        rdfs:label    "sponsor" .

sdo:reservationId  rdfs:comment  "A unique identifier for the reservation." ;
        rdfs:label    "reservation id" .

sdo:maintainer  rdfs:comment  "A maintainer of a [[Dataset]], software package ([[SoftwareApplication]]), or other [[Project]]. A maintainer is a [[Person]] or [[Organization]] that manages contributions to, and/or publication of, some (typically complex) artifact. It is common for distributions of software and data to be based on \"upstream\" sources. When [[maintainer]] is applied to a specific version of something e.g. a particular version or packaging of a [[Dataset]], it is always  possible that the upstream source has a different maintainer. The [[isBasedOn]] property can be used to indicate such relationships between datasets to make the different maintenance roles clear. Similarly in the case of software, a package may have dedicated maintainers working on integration into software distributions such as Ubuntu, as well as upstream maintainers of the underlying work.\n      " ;
        rdfs:label    "maintainer" .

sdo:publishedBy  rdfs:comment  "An agent associated with the publication event." ;
        rdfs:label    "published by" .

sdo:hasCredential  rdfs:comment  "A credential awarded to the Person or Organization." ;
        rdfs:label    "has credential" .

sdo:MaximumDoseSchedule
        rdfs:comment  "The maximum dosing schedule considered safe for a drug or supplement as recommended by an authority or by the drug/supplement's manufacturer. Capture the recommending authority in the recognizingAuthority property of MedicalEntity." ;
        rdfs:label    "MaximumDoseSchedule" .

sdo:RemixAlbum  rdfs:comment  "RemixAlbum." ;
        rdfs:label    "RemixAlbum" .

sdo:BodyMeasurementWaist
        rdfs:comment  "Girth of natural waistline (between hip bones and lower ribs). Used, for example, to fit pants." ;
        rdfs:label    "BodyMeasurementWaist" .

sdo:GolfCourse  rdfs:comment  "A golf course." ;
        rdfs:label    "GolfCourse" .

sdo:hasDigitalDocumentPermission
        rdfs:comment  "A permission related to the access to this document (e.g. permission to read or write an electronic document). For a public document, specify a grantee with an Audience with audienceType equal to \"public\"." ;
        rdfs:label    "has digitalDocumentPermission" .

sdo:maximumEnrollment
        rdfs:comment  "The maximum number of students who may be enrolled in the program." ;
        rdfs:label    "maximum enrollment" .

sdo:Reservoir  rdfs:comment  "A reservoir of water, typically an artificially created lake, like the Lake Kariba reservoir." ;
        rdfs:label    "Reservoir" .

sdo:discusses  rdfs:comment  "Specifies the CreativeWork associated with the UserComment." ;
        rdfs:label    "discusses" .

sdo:knowsLanguage  rdfs:comment  "Of a [[Person]], and less typically of an [[Organization]], to indicate a known language. We do not distinguish skill levels or reading/writing/speaking/signing here. Use language codes from the [IETF BCP 47 standard](http://tools.ietf.org/html/bcp47)." ;
        rdfs:label    "knows language" .

sdo:webFeed  rdfs:comment  "The URL for a feed, e.g. associated with a podcast series, blog, or series of date-stamped updates. This is usually RSS or Atom." ;
        rdfs:label    "web feed" .

sdo:vehicleInteriorType
        rdfs:comment  "The type or material of the interior of the vehicle (e.g. synthetic fabric, leather, wood, etc.). While most interior types are characterized by the material used, an interior type can also be based on vehicle usage or target audience." ;
        rdfs:label    "vehicle interiorType" .

sdo:healthcareReportingData
        rdfs:comment  "Indicates data describing a hospital, e.g. a CDC [[CDCPMDRecord]] or as some kind of [[Dataset]]." ;
        rdfs:label    "healthcare reportingData" .

sdo:ChemicalSubstance
        rdfs:comment  "A chemical substance is 'a portion of matter of constant composition, composed of molecular entities of the same type or of different types' (source: [ChEBI:59999](https://www.ebi.ac.uk/chebi/searchId.do?chebiId=59999))." ;
        rdfs:label    "ChemicalSubstance" .

sdo:EnergyConsumptionDetails
        rdfs:comment  "EnergyConsumptionDetails represents information related to the energy efficiency of a product that consumes energy. The information that can be provided is based on international regulations such as for example [EU directive 2017/1369](https://eur-lex.europa.eu/eli/reg/2017/1369/oj) for energy labeling and the [Energy labeling rule](https://www.ftc.gov/enforcement/rules/rulemaking-regulatory-reform-proceedings/energy-water-use-labeling-consumer) under the Energy Policy and Conservation Act (EPCA) in the US." ;
        rdfs:label    "EnergyConsumptionDetails" .

sdo:beneficiaryBank  rdfs:comment  "A bank or bank’s branch, financial institution or international financial institution operating the beneficiary’s bank account or releasing funds for the beneficiary." ;
        rdfs:label    "beneficiary bank" .

sdo:Course  rdfs:comment  "A description of an educational course which may be offered as distinct instances at which take place at different times or take place at different locations, or be offered through different media or modes of study. An educational course is a sequence of one or more educational events and/or creative works which aims to build knowledge, competence or ability of learners." ;
        rdfs:label    "Course" .

sdo:IndividualProduct
        rdfs:comment  "A single, identifiable product instance (e.g. a laptop with a particular serial number)." ;
        rdfs:label    "IndividualProduct" .

sdo:Season  rdfs:comment  "A media season e.g. tv, radio, video game etc." ;
        rdfs:label    "Season" .

sdo:warrantyPromise  rdfs:comment  "The warranty promise(s) included in the offer." ;
        rdfs:label    "warranty promise" .

sdo:trailerWeight  rdfs:comment  "The permitted weight of a trailer attached to the vehicle.\\n\\nTypical unit code(s): KGM for kilogram, LBR for pound\\n* Note 1: You can indicate additional information in the [[name]] of the [[QuantitativeValue]] node.\\n* Note 2: You may also link to a [[QualitativeValue]] node that provides additional information using [[valueReference]].\\n* Note 3: Note that you can use [[minValue]] and [[maxValue]] to indicate ranges." ;
        rdfs:label    "trailer weight" .

sdo:FilmAction  rdfs:comment  "The act of capturing sound and moving images on film, video, or digitally." ;
        rdfs:label    "FilmAction" .

sdo:eventStatus  rdfs:comment  "An eventStatus of an event represents its status; particularly useful when an event is cancelled or rescheduled." ;
        rdfs:label    "event status" .

sdo:serverStatus  rdfs:comment  "Status of a game server." ;
        rdfs:label    "server status" .

sdo:MusicRecording  rdfs:comment  "A music recording (track), usually a single song." ;
        rdfs:label    "MusicRecording" .

sdo:HalalDiet  rdfs:comment  "A diet conforming to Islamic dietary practices." ;
        rdfs:label    "HalalDiet" .

sdo:FundingScheme  rdfs:comment  "A FundingScheme combines organizational, project and policy aspects of grant-based funding\n    that sets guidelines, principles and mechanisms to support other kinds of projects and activities.\n    Funding is typically organized via [[Grant]] funding. Examples of funding schemes: Swiss Priority Programmes (SPPs); EU Framework 7 (FP7); Horizon 2020; the NIH-R01 Grant Program; Wellcome institutional strategic support fund. For large scale public sector funding, the management and administration of grant awards is often handled by other, dedicated, organizations - [[FundingAgency]]s such as ERC, REA, ..." ;
        rdfs:label    "FundingScheme" .

sdo:DeliveryEvent  rdfs:comment  "An event involving the delivery of an item." ;
        rdfs:label    "DeliveryEvent" .

sdo:Beach  rdfs:comment  "Beach." ;
        rdfs:label    "Beach" .

sdo:physicalRequirement
        rdfs:comment  "A description of the types of physical activity associated with the job. Defined terms such as those in O*net may be used, but note that there is no way to specify the level of ability as well as its nature when using a defined term." ;
        rdfs:label    "physical requirement" .

sdo:vehicleSpecialUsage
        rdfs:comment  "Indicates whether the vehicle has been used for special purposes, like commercial rental, driving school, or as a taxi. The legislation in many countries requires this information to be revealed when offering a car for sale." ;
        rdfs:label    "vehicle specialUsage" .

sdo:childMinAge  rdfs:comment  "Minimal age of the child." ;
        rdfs:label    "child minAge" .

sdo:DietarySupplement
        rdfs:comment  "A product taken by mouth that contains a dietary ingredient intended to supplement the diet. Dietary ingredients may include vitamins, minerals, herbs or other botanicals, amino acids, and substances such as enzymes, organ tissues, glandulars and metabolites." ;
        rdfs:label    "DietarySupplement" .

sdo:encodesBioChemEntity
        rdfs:comment  "Another BioChemEntity encoded by this one. " ;
        rdfs:label    "encodes bioChemEntity" .

sdo:sportsEvent  rdfs:comment  "A sub property of location. The sports event where this action occurred." ;
        rdfs:label    "sports event" .

sdo:subStructure  rdfs:comment  "Component (sub-)structure(s) that comprise this anatomical structure." ;
        rdfs:label    "sub structure" .

sdo:isbn  rdfs:comment  "The ISBN of the book." ;
        rdfs:label    "isbn" .

sdo:MiddleSchool  rdfs:comment  "A middle school (typically for children aged around 11-14, although this varies somewhat)." ;
        rdfs:label    "MiddleSchool" .

sdo:ItemListOrderDescending
        rdfs:comment  "An ItemList ordered with higher values listed first." ;
        rdfs:label    "ItemListOrderDescending" .

sdo:InForce  rdfs:comment  "Indicates that a legislation is in force." ;
        rdfs:label    "InForce" .

sdo:sibling  rdfs:comment  "A sibling of the person." ;
        rdfs:label    "sibling" .

sdo:availableIn  rdfs:comment  "The location in which the strength is available." ;
        rdfs:label    "available in" .

sdo:numberOfPreviousOwners
        rdfs:comment  "The number of owners of the vehicle, including the current one.\\n\\nTypical unit code(s): C62" ;
        rdfs:label    "number ofPreviousOwners" .

sdo:OriginalShippingFees
        rdfs:comment  "Specifies that the customer must pay the original shipping costs when returning a product." ;
        rdfs:label    "OriginalShippingFees" .

sdo:surface  rdfs:comment  "A material used as a surface in some artwork, e.g. Canvas, Paper, Wood, Board, etc." ;
        rdfs:label    "surface" .

sdo:associatedReview  rdfs:comment  "An associated [[Review]]." ;
        rdfs:label    "associated review" .

sdo:ReturnLabelCustomerResponsibility
        rdfs:comment  "Indicated that creating a return label is the responsibility of the customer." ;
        rdfs:label    "ReturnLabelCustomerResponsibility" .

sdo:MusicAlbumProductionType
        rdfs:comment  "Classification of the album by it's type of content: soundtrack, live album, studio album, etc." ;
        rdfs:label    "MusicAlbumProductionType" .

sdo:hasMolecularFunction
        rdfs:comment  "Molecular function performed by this BioChemEntity; please use PropertyValue if you want to include any evidence." ;
        rdfs:label    "has molecularFunction" .

sdo:loanType  rdfs:comment  "The type of a loan or credit." ;
        rdfs:label    "loan type" .

sdo:workPresented  rdfs:comment  "The movie presented during this event." ;
        rdfs:label    "work presented" .

sdo:MoneyTransfer  rdfs:comment  "The act of transferring money from one place to another place. This may occur electronically or physically." ;
        rdfs:label    "MoneyTransfer" .

sdo:WinAction  rdfs:comment  "The act of achieving victory in a competitive activity." ;
        rdfs:label    "WinAction" .

sdo:installUrl  rdfs:comment  "URL at which the app may be installed, if different from the URL of the item." ;
        rdfs:label    "install url" .

sdo:grantee  rdfs:comment  "The person, organization, contact point, or audience that has been granted this permission." ;
        rdfs:label    "grantee" .

sdo:ParkingMap  rdfs:comment  "A parking map." ;
        rdfs:label    "ParkingMap" .

sdo:member  rdfs:comment  "A member of an Organization or a ProgramMembership. Organizations can be members of organizations; ProgramMembership is typically for individuals." ;
        rdfs:label    "member" .

sdo:stepValue  rdfs:comment  "The stepValue attribute indicates the granularity that is expected (and required) of the value in a PropertyValueSpecification." ;
        rdfs:label    "step value" .

sdo:ReturnByMail  rdfs:comment  "Specifies that product returns must to be done by mail." ;
        rdfs:label    "ReturnByMail" .

sdo:runtimePlatform  rdfs:comment  "Runtime platform or script interpreter dependencies (Example - Java v1, Python2.3, .Net Framework 3.0)." ;
        rdfs:label    "runtime platform" .

sdo:priceRange  rdfs:comment  "The price range of the business, for example ```$$$```." ;
        rdfs:label    "price range" .

sdo:FrontWheelDriveConfiguration
        rdfs:comment  "Front-wheel drive is a transmission layout where the engine drives the front wheels." ;
        rdfs:label    "FrontWheelDriveConfiguration" .

sdo:ReplaceAction  rdfs:comment  "The act of editing a recipient by replacing an old object with a new object." ;
        rdfs:label    "ReplaceAction" .

sdo:FoodEstablishmentReservation
        rdfs:comment  "A reservation to dine at a food-related business.\\n\\nNote: This type is for information about actual reservations, e.g. in confirmation emails or HTML pages with individual confirmations of reservations." ;
        rdfs:label    "FoodEstablishmentReservation" .

sdo:DrugPrescriptionStatus
        rdfs:comment  "Indicates whether this drug is available by prescription or over-the-counter." ;
        rdfs:label    "DrugPrescriptionStatus" .

sdo:LimitedByGuaranteeCharity
        rdfs:comment  "LimitedByGuaranteeCharity: Non-profit type referring to a charitable company that is limited by guarantee (UK)." ;
        rdfs:label    "LimitedByGuaranteeCharity" .

sdo:HowToTip  rdfs:comment  "An explanation in the instructions for how to achieve a result. It provides supplementary information about a technique, supply, author's preference, etc. It can explain what could be done, or what should not be done, but doesn't specify what should be done (see HowToDirection)." ;
        rdfs:label    "HowToTip" .

sdo:PartiallyInForce  rdfs:comment  "Indicates that parts of the legislation are in force, and parts are not." ;
        rdfs:label    "PartiallyInForce" .

sdo:fundedItem  rdfs:comment  "Indicates an item funded or sponsored through a [[Grant]]." ;
        rdfs:label    "funded item" .

sdo:Room  rdfs:comment  "A room is a distinguishable space within a structure, usually separated from other spaces by interior walls. (Source: Wikipedia, the free encyclopedia, see <a href=\"http://en.wikipedia.org/wiki/Room\">http://en.wikipedia.org/wiki/Room</a>).\n<br /><br />\nSee also the <a href=\"/docs/hotels.html\">dedicated document on the use of schema.org for marking up hotels and other forms of accommodations</a>.\n" ;
        rdfs:label    "Room" .

sdo:Urologic  rdfs:comment  "A specific branch of medical science that is concerned with the diagnosis and treatment of diseases pertaining to the urinary tract and the urogenital system." ;
        rdfs:label    "Urologic" .

sdo:insertion  rdfs:comment  "The place of attachment of a muscle, or what the muscle moves." ;
        rdfs:label    "insertion" .

sdo:MRI  rdfs:comment  "Magnetic resonance imaging." ;
        rdfs:label    "MRI" .

sdo:Wednesday  rdfs:comment  "The day of the week between Tuesday and Thursday." ;
        rdfs:label    "Wednesday" .

sdo:Nonprofit501k  rdfs:comment  "Nonprofit501k: Non-profit type referring to Child Care Organizations." ;
        rdfs:label    "Nonprofit501k" .

sdo:HealthPlanFormulary
        rdfs:comment  "For a given health insurance plan, the specification for costs and coverage of prescription drugs. " ;
        rdfs:label    "HealthPlanFormulary" .

sdo:TireShop  rdfs:comment  "A tire shop." ;
        rdfs:label    "TireShop" .

sdo:distribution  rdfs:comment  "A downloadable form of this dataset, at a specific location, in a specific format." ;
        rdfs:label    "distribution" .

sdo:pregnancyWarning  rdfs:comment  "Any precaution, guidance, contraindication, etc. related to this drug's use during pregnancy." ;
        rdfs:label    "pregnancy warning" .

sdo:AudioObject  rdfs:comment  "An audio file." ;
        rdfs:label    "AudioObject" .

sdo:MedicalConditionStage
        rdfs:comment  "A stage of a medical condition, such as 'Stage IIIa'." ;
        rdfs:label    "MedicalConditionStage" .

sdo:merchant  rdfs:comment  "'merchant' is an out-dated term for 'seller'." ;
        rdfs:label    "merchant" .

sdo:MerchantReturnNotPermitted
        rdfs:comment  "Specifies that product returns are not permitted." ;
        rdfs:label    "MerchantReturnNotPermitted" .

sdo:legislationLegalValue
        rdfs:comment  "The legal value of this legislation file. The same legislation can be written in multiple files with different legal values. Typically a digitally signed PDF have a \"stronger\" legal value than the HTML file of the same act." ;
        rdfs:label    "legislation legalValue" .

sdo:videoFormat  rdfs:comment  "The type of screening or video broadcast used (e.g. IMAX, 3D, SD, HD, etc.)." ;
        rdfs:label    "video format" .

sdo:wheelbase  rdfs:comment  "The distance between the centers of the front and rear wheels.\\n\\nTypical unit code(s): CMT for centimeters, MTR for meters, INH for inches, FOT for foot/feet" ;
        rdfs:label    "wheelbase" .

sdo:Message  rdfs:comment  "A single message from a sender to one or more organizations or people." ;
        rdfs:label    "Message" .

sdo:isUnlabelledFallback
        rdfs:comment  "This can be marked 'true' to indicate that some published [[DeliveryTimeSettings]] or [[ShippingRateSettings]] are intended to apply to all [[OfferShippingDetails]] published by the same merchant, when referenced by a [[shippingSettingsLink]] in those settings. It is not meaningful to use a 'true' value for this property alongside a transitTimeLabel (for [[DeliveryTimeSettings]]) or shippingLabel (for [[ShippingRateSettings]]), since this property is for use with unlabelled settings." ;
        rdfs:label    "is unlabelledFallback" .

sdo:Nonprofit501c15  rdfs:comment  "Nonprofit501c15: Non-profit type referring to Mutual Insurance Companies or Associations." ;
        rdfs:label    "Nonprofit501c15" .

sdo:ownedThrough  rdfs:comment  "The date and time of giving up ownership on the product." ;
        rdfs:label    "owned through" .

sdo:departureAirport  rdfs:comment  "The airport where the flight originates." ;
        rdfs:label    "departure airport" .

sdo:customerRemorseReturnShippingFeesAmount
        rdfs:comment  "The amount of shipping costs if a product is returned due to customer remorse. Applicable when property [[customerRemorseReturnFees]] equals [[ReturnShippingFees]]." ;
        rdfs:label    "customer remorseReturnShippingFeesAmount" .

sdo:Retail  rdfs:comment  "The drug's cost represents the retail cost of the drug." ;
        rdfs:label    "Retail" .

sdo:lodgingUnitDescription
        rdfs:comment  "A full description of the lodging unit." ;
        rdfs:label    "lodging unitDescription" .

sdo:borrower  rdfs:comment  "A sub property of participant. The person that borrows the object being lent." ;
        rdfs:label    "borrower" .

sdo:Dataset  rdfs:comment  "A body of structured information describing some topic(s) of interest." ;
        rdfs:label    "Dataset" .

sdo:softwareRequirements
        rdfs:comment  "Component dependency requirements for application. This includes runtime environments and shared libraries that are not included in the application distribution package, but required to run the application (Examples: DirectX, Java or .NET runtime)." ;
        rdfs:label    "software requirements" .

sdo:servicePostalAddress
        rdfs:comment  "The address for accessing the service by mail." ;
        rdfs:label    "service postalAddress" .

sdo:Demand  rdfs:comment  "A demand entity represents the public, not necessarily binding, not necessarily exclusive, announcement by an organization or person to seek a certain type of goods or services. For describing demand using this type, the very same properties used for Offer apply." ;
        rdfs:label    "Demand" .

sdo:Toxicologic  rdfs:comment  "A specific branch of medical science that is concerned with poisons, their nature, effects and detection and involved in the treatment of poisoning." ;
        rdfs:label    "Toxicologic" .

sdo:Anesthesia  rdfs:comment  "A specific branch of medical science that pertains to study of anesthetics and their application." ;
        rdfs:label    "Anesthesia" .

sdo:ExercisePlan  rdfs:comment  "Fitness-related activity designed for a specific health-related purpose, including defined exercise routines as well as activity prescribed by a clinician." ;
        rdfs:label    "ExercisePlan" .

sdo:ActivationFee  rdfs:comment  "Represents the activation fee part of the total price for an offered product, for example a cellphone contract." ;
        rdfs:label    "ActivationFee" .

sdo:publishedOn  rdfs:comment  "A broadcast service associated with the publication event." ;
        rdfs:label    "published on" .

sdo:domainIncludes  rdfs:comment  "Relates a property to a class that is (one of) the type(s) the property is expected to be used on." ;
        rdfs:label    "domain includes" .

sdo:Nonprofit501c19  rdfs:comment  "Nonprofit501c19: Non-profit type referring to Post or Organization of Past or Present Members of the Armed Forces." ;
        rdfs:label    "Nonprofit501c19" .

sdo:securityScreening
        rdfs:comment  "The type of security screening the passenger is subject to." ;
        rdfs:label    "security screening" .

sdo:endOffset  rdfs:comment  "The end time of the clip expressed as the number of seconds from the beginning of the work." ;
        rdfs:label    "end offset" .

sdo:MovingCompany  rdfs:comment  "A moving company." ;
        rdfs:label    "MovingCompany" .

sdo:contentType  rdfs:comment  "The supported content type(s) for an EntryPoint response." ;
        rdfs:label    "content type" .

sdo:applicationContact
        rdfs:comment  "Contact details for further information relevant to this job posting." ;
        rdfs:label    "application contact" .

sdo:temporalCoverage  rdfs:comment  "The temporalCoverage of a CreativeWork indicates the period that the content applies to, i.e. that it describes, either as a DateTime or as a textual string indicating a time period in [ISO 8601 time interval format](https://en.wikipedia.org/wiki/ISO_8601#Time_intervals). In\n      the case of a Dataset it will typically indicate the relevant time period in a precise notation (e.g. for a 2011 census dataset, the year 2011 would be written \"2011/2012\"). Other forms of content e.g. ScholarlyArticle, Book, TVSeries or TVEpisode may indicate their temporalCoverage in broader terms - textually or via well-known URL.\n      Written works such as books may sometimes have precise temporal coverage too, e.g. a work set in 1939 - 1945 can be indicated in ISO 8601 interval format format via \"1939/1945\".\n\nOpen-ended date ranges can be written with \"..\" in place of the end date. For example, \"2015-11/..\" indicates a range beginning in November 2015 and with no specified final date. This is tentative and might be updated in future when ISO 8601 is officially updated." ;
        rdfs:label    "temporal coverage" .

sdo:polygon  rdfs:comment  "A polygon is the area enclosed by a point-to-point path for which the starting and ending points are the same. A polygon is expressed as a series of four or more space delimited points where the first and final points are identical." ;
        rdfs:label    "polygon" .

sdo:gtin8  rdfs:comment  "The GTIN-8 code of the product, or the product to which the offer refers. This code is also known as EAN/UCC-8 or 8-digit EAN. See [GS1 GTIN Summary](http://www.gs1.org/barcodes/technical/idkeys/gtin) for more details." ;
        rdfs:label    "gtin8" .

sdo:artform  rdfs:comment  "e.g. Painting, Drawing, Sculpture, Print, Photograph, Assemblage, Collage, etc." ;
        rdfs:label    "artform" .

sdo:numberOfSeasons  rdfs:comment  "The number of seasons in this series." ;
        rdfs:label    "number ofSeasons" .

sdo:educationalAlignment
        rdfs:comment  "An alignment to an established educational framework.\n\nThis property should not be used where the nature of the alignment can be described using a simple property, for example to express that a resource [[teaches]] or [[assesses]] a competency." ;
        rdfs:label    "educational alignment" .

sdo:MotorcycleDealer  rdfs:comment  "A motorcycle dealer." ;
        rdfs:label    "MotorcycleDealer" .

sdo:overdosage  rdfs:comment  "Any information related to overdose on a drug, including signs or symptoms, treatments, contact information for emergency response." ;
        rdfs:label    "overdosage" .

sdo:availabilityStarts
        rdfs:comment  "The beginning of the availability of the product or service included in the offer." ;
        rdfs:label    "availability starts" .

sdo:Synagogue  rdfs:comment  "A synagogue." ;
        rdfs:label    "Synagogue" .

sdo:FireStation  rdfs:comment  "A fire station. With firemen." ;
        rdfs:label    "FireStation" .

sdo:Bakery  rdfs:comment  "A bakery." ;
        rdfs:label    "Bakery" .

sdo:floorSize  rdfs:comment  "The size of the accommodation, e.g. in square meter or squarefoot.\nTypical unit code(s): MTK for square meter, FTK for square foot, or YDK for square yard " ;
        rdfs:label    "floor size" .

sdo:UnofficialLegalValue
        rdfs:comment  "Indicates that a document has no particular or special standing (e.g. a republication of a law by a private publisher)." ;
        rdfs:label    "UnofficialLegalValue" .

sdo:sdPublisher  rdfs:comment  "Indicates the party responsible for generating and publishing the current structured data markup, typically in cases where the structured data is derived automatically from existing published content but published on a different site. For example, student projects and open data initiatives often re-publish existing content with more explicitly structured metadata. The\n[[sdPublisher]] property helps make such practices more explicit." ;
        rdfs:label    "sd publisher" .

sdo:LimitedAvailability
        rdfs:comment  "Indicates that the item has limited availability." ;
        rdfs:label    "LimitedAvailability" .

sdo:LiquorStore  rdfs:comment  "A shop that sells alcoholic drinks such as wine, beer, whisky and other spirits." ;
        rdfs:label    "LiquorStore" .

sdo:PublicHealth  rdfs:comment  "Branch of medicine that pertains to the health services to improve and protect community health, especially epidemiology, sanitation, immunization, and preventive medicine." ;
        rdfs:label    "PublicHealth" .

sdo:availableLanguage
        rdfs:comment  "A language someone may use with or at the item, service or place. Please use one of the language codes from the [IETF BCP 47 standard](http://tools.ietf.org/html/bcp47). See also [[inLanguage]]" ;
        rdfs:label    "available language" .

sdo:actionableFeedbackPolicy
        rdfs:comment  "For a [[NewsMediaOrganization]] or other news-related [[Organization]], a statement about public engagement activities (for news media, the newsroom’s), including involving the public - digitally or otherwise -- in coverage decisions, reporting and activities after publication." ;
        rdfs:label    "actionable feedbackPolicy" .

sdo:openingHours  rdfs:comment  "The general opening hours for a business. Opening hours can be specified as a weekly time range, starting with days, then times per day. Multiple days can be listed with commas ',' separating each day. Day or time ranges are specified using a hyphen '-'.\\n\\n* Days are specified using the following two-letter combinations: ```Mo```, ```Tu```, ```We```, ```Th```, ```Fr```, ```Sa```, ```Su```.\\n* Times are specified using 24:00 format. For example, 3pm is specified as ```15:00```, 10am as ```10:00```. \\n* Here is an example: <code>&lt;time itemprop=\"openingHours\" datetime=&quot;Tu,Th 16:00-20:00&quot;&gt;Tuesdays and Thursdays 4-8pm&lt;/time&gt;</code>.\\n* If a business is open 7 days a week, then it can be specified as <code>&lt;time itemprop=&quot;openingHours&quot; datetime=&quot;Mo-Su&quot;&gt;Monday through Sunday, all day&lt;/time&gt;</code>." ;
        rdfs:label    "opening hours" .

sdo:creativeWorkStatus
        rdfs:comment  "The status of a creative work in terms of its stage in a lifecycle. Example terms include Incomplete, Draft, Published, Obsolete. Some organizations define a set of terms for the stages of their publication lifecycle." ;
        rdfs:label    "creative workStatus" .

sdo:governmentBenefitsInfo
        rdfs:comment  "governmentBenefitsInfo provides information about government benefits associated with a SpecialAnnouncement." ;
        rdfs:label    "government benefitsInfo" .

sdo:studyLocation  rdfs:comment  "The location in which the study is taking/took place." ;
        rdfs:label    "study location" .

sdo:upvoteCount  rdfs:comment  "The number of upvotes this question, answer or comment has received from the community." ;
        rdfs:label    "upvote count" .

sdo:dateline  rdfs:comment  "A [dateline](https://en.wikipedia.org/wiki/Dateline) is a brief piece of text included in news articles that describes where and when the story was written or filed though the date is often omitted. Sometimes only a placename is provided.\n\nStructured representations of dateline-related information can also be expressed more explicitly using [[locationCreated]] (which represents where a work was created e.g. where a news report was written).  For location depicted or described in the content, use [[contentLocation]].\n\nDateline summaries are oriented more towards human readers than towards automated processing, and can vary substantially. Some examples: \"BEIRUT, Lebanon, June 2.\", \"Paris, France\", \"December 19, 2017 11:43AM Reporting from Washington\", \"Beijing/Moscow\", \"QUEZON CITY, Philippines\".\n      " ;
        rdfs:label    "dateline" .

sdo:StudioAlbum  rdfs:comment  "StudioAlbum." ;
        rdfs:label    "StudioAlbum" .

sdo:Geriatric  rdfs:comment  "A specific branch of medical science that is concerned with the diagnosis and treatment of diseases, debilities and provision of care to the aged." ;
        rdfs:label    "Geriatric" .

sdo:TelevisionStation
        rdfs:comment  "A television station." ;
        rdfs:label    "TelevisionStation" .

sdo:Fungus  rdfs:comment  "Pathogenic fungus." ;
        rdfs:label    "Fungus" .

sdo:returnPolicyCategory
        rdfs:comment  "Specifies an applicable return policy (from an enumeration)." ;
        rdfs:label    "return policyCategory" .

sdo:doseValue  rdfs:comment  "The value of the dose, e.g. 500." ;
        rdfs:label    "dose value" .

sdo:followup  rdfs:comment  "Typical or recommended followup care after the procedure is performed." ;
        rdfs:label    "followup" .

sdo:dateVehicleFirstRegistered
        rdfs:comment  "The date of the first registration of the vehicle with the respective public authorities." ;
        rdfs:label    "date vehicleFirstRegistered" .

sdo:legislationChanges
        rdfs:comment  "Another legislation that this legislation changes. This encompasses the notions of amendment, replacement, correction, repeal, or other types of change. This may be a direct change (textual or non-textual amendment) or a consequential or indirect change. The property is to be used to express the existence of a change relationship between two acts rather than the existence of a consolidated version of the text that shows the result of the change. For consolidation relationships, use the <a href=\"/legislationConsolidates\">legislationConsolidates</a> property." ;
        rdfs:label    "legislation changes" .

sdo:ParentAudience  rdfs:comment  "A set of characteristics describing parents, who can be interested in viewing some content." ;
        rdfs:label    "ParentAudience" .

sdo:accommodationCategory
        rdfs:comment  "Category of an [[Accommodation]], following real estate conventions e.g. RESO (see [PropertySubType](https://ddwiki.reso.org/display/DDW17/PropertySubType+Field), and [PropertyType](https://ddwiki.reso.org/display/DDW17/PropertyType+Field) fields  for suggested values)." ;
        rdfs:label    "accommodation category" .

sdo:Consortium  rdfs:comment  "A Consortium is a membership [[Organization]] whose members are typically Organizations." ;
        rdfs:label    "Consortium" .

sdo:spokenByCharacter
        rdfs:comment  "The (e.g. fictional) character, Person or Organization to whom the quotation is attributed within the containing CreativeWork." ;
        rdfs:label    "spoken byCharacter" .

sdo:genre  rdfs:comment  "Genre of the creative work, broadcast channel or group." ;
        rdfs:label    "genre" .

sdo:SocialMediaPosting
        rdfs:comment  "A post to a social media platform, including blog posts, tweets, Facebook posts, etc." ;
        rdfs:label    "SocialMediaPosting" .

sdo:numberOfBeds  rdfs:comment  "The quantity of the given bed type available in the HotelRoom, Suite, House, or Apartment." ;
        rdfs:label    "number ofBeds" .

sdo:saturatedFatContent
        rdfs:comment  "The number of grams of saturated fat." ;
        rdfs:label    "saturated fatContent" .

sdo:Residence  rdfs:comment  "The place where a person lives." ;
        rdfs:label    "Residence" .

sdo:significance  rdfs:comment  "The significance associated with the superficial anatomy; as an example, how characteristics of the superficial anatomy can suggest underlying medical conditions or courses of treatment." ;
        rdfs:label    "significance" .

sdo:articleSection  rdfs:comment  "Articles may belong to one or more 'sections' in a magazine or newspaper, such as Sports, Lifestyle, etc." ;
        rdfs:label    "article section" .

sdo:Project  rdfs:comment  "An enterprise (potentially individual but typically collaborative), planned to achieve a particular aim.\nUse properties from [[Organization]], [[subOrganization]]/[[parentOrganization]] to indicate project sub-structures. \n   " ;
        rdfs:label    "Project" .

sdo:recipeIngredient  rdfs:comment  "A single ingredient used in the recipe, e.g. sugar, flour or garlic." ;
        rdfs:label    "recipe ingredient" .

sdo:reviewedBy  rdfs:comment  "People or organizations that have reviewed the content on this web page for accuracy and/or completeness." ;
        rdfs:label    "reviewed by" .

sdo:billingPeriod  rdfs:comment  "The time interval used to compute the invoice." ;
        rdfs:label    "billing period" .

sdo:isPartOfBioChemEntity
        rdfs:comment  "Indicates a BioChemEntity that is (in some sense) a part of this BioChemEntity. " ;
        rdfs:label    "is partOfBioChemEntity" .

sdo:Crematorium  rdfs:comment  "A crematorium." ;
        rdfs:label    "Crematorium" .

sdo:serviceSmsNumber  rdfs:comment  "The number to access the service by text message." ;
        rdfs:label    "service smsNumber" .

sdo:HowOrWhereHealthAspect
        rdfs:comment  "Information about how or where to find a topic. Also may contain location data that can be used for where to look for help if the topic is observed." ;
        rdfs:label    "HowOrWhereHealthAspect" .

sdo:maxValue  rdfs:comment  "The upper value of some characteristic or property." ;
        rdfs:label    "max value" .

sdo:Diagnostic  rdfs:comment  "A medical device used for diagnostic purposes." ;
        rdfs:label    "Diagnostic" .

sdo:claimInterpreter  rdfs:comment  "For a [[Claim]] interpreted from [[MediaObject]] content\n    sed to indicate a claim contained, implied or refined from the content of a [[MediaObject]]." ;
        rdfs:label    "claim interpreter" .

sdo:previousStartDate
        rdfs:comment  "Used in conjunction with eventStatus for rescheduled or cancelled events. This property contains the previously scheduled start date. For rescheduled events, the startDate property should be used for the newly scheduled start date. In the (rare) case of an event that has been postponed and rescheduled multiple times, this field may be repeated." ;
        rdfs:label    "previous startDate" .

sdo:readBy  rdfs:comment  "A person who reads (performs) the audiobook." ;
        rdfs:label    "read by" .

sdo:SizeSystemEnumeration
        rdfs:comment  "Enumerates common size systems for different categories of products, for example \"EN-13402\" or \"UK\" for wearables or \"Imperial\" for screws." ;
        rdfs:label    "SizeSystemEnumeration" .

sdo:productSupported  rdfs:comment  "The product or service this support contact point is related to (such as product support for a particular product line). This can be a specific product or product line (e.g. \"iPhone\") or a general category of products or services (e.g. \"smartphones\")." ;
        rdfs:label    "product supported" .

sdo:clincalPharmacology
        rdfs:comment  "Description of the absorption and elimination of drugs, including their concentration (pharmacokinetics, pK) and biological effects (pharmacodynamics, pD)." ;
        rdfs:label    "clincal pharmacology" .

sdo:mileageFromOdometer
        rdfs:comment  "The total distance travelled by the particular vehicle since its initial production, as read from its odometer.\\n\\nTypical unit code(s): KMT for kilometers, SMI for statute miles" ;
        rdfs:label    "mileage fromOdometer" .

sdo:bccRecipient  rdfs:comment  "A sub property of recipient. The recipient blind copied on a message." ;
        rdfs:label    "bcc recipient" .

sdo:MovieRentalStore  rdfs:comment  "A movie rental store." ;
        rdfs:label    "MovieRentalStore" .

sdo:dependencies  rdfs:comment  "Prerequisites needed to fulfill steps in article." ;
        rdfs:label    "dependencies" .

sdo:materialExtent  rdfs:comment  "The quantity of the materials being described or an expression of the physical space they occupy."@en ;
        rdfs:label    "material extent"@en .

sdo:countryOfOrigin  rdfs:comment  "The country of origin of something, including products as well as creative  works such as movie and TV content.\n\nIn the case of TV and movie, this would be the country of the principle offices of the production company or individual responsible for the movie. For other kinds of [[CreativeWork]] it is difficult to provide fully general guidance, and properties such as [[contentLocation]] and [[locationCreated]] may be more applicable.\n\nIn the case of products, the country of origin of the product. The exact interpretation of this may vary by context and product type, and cannot be fully enumerated here." ;
        rdfs:label    "country ofOrigin" .

sdo:TaxiService  rdfs:comment  "A service for a vehicle for hire with a driver for local travel. Fares are usually calculated based on distance traveled." ;
        rdfs:label    "TaxiService" .

sdo:AutoDealer  rdfs:comment  "An car dealership." ;
        rdfs:label    "AutoDealer" .

sdo:encodingType  rdfs:comment  "The supported encoding type(s) for an EntryPoint request." ;
        rdfs:label    "encoding type" .

sdo:EventCancelled  rdfs:comment  "The event has been cancelled. If the event has multiple startDate values, all are assumed to be cancelled. Either startDate or previousStartDate may be used to specify the event's cancelled date(s)." ;
        rdfs:label    "EventCancelled" .

sdo:Otolaryngologic  rdfs:comment  "A specific branch of medical science that is concerned with the ear, nose and throat and their respective disease states." ;
        rdfs:label    "Otolaryngologic" .

sdo:MerchantReturnPolicySeasonalOverride
        rdfs:comment  "A seasonal override of a return policy, for example used for holidays." ;
        rdfs:label    "MerchantReturnPolicySeasonalOverride" .

sdo:PostalCodeRangeSpecification
        rdfs:comment  "Indicates a range of postalcodes, usually defined as the set of valid codes between [[postalCodeBegin]] and [[postalCodeEnd]], inclusively." ;
        rdfs:label    "PostalCodeRangeSpecification" .

sdo:OfferForPurchase  rdfs:comment  "An [[OfferForPurchase]] in Schema.org represents an [[Offer]] to sell something, i.e. an [[Offer]] whose\n  [[businessFunction]] is [sell](http://purl.org/goodrelations/v1#Sell.). See [Good Relations](https://en.wikipedia.org/wiki/GoodRelations) for\n  background on the underlying concepts.\n  " ;
        rdfs:label    "OfferForPurchase" .

sdo:costCategory  rdfs:comment  "The category of cost, such as wholesale, retail, reimbursement cap, etc." ;
        rdfs:label    "cost category" .

sdo:screenCount  rdfs:comment  "The number of screens in the movie theater." ;
        rdfs:label    "screen count" .

sdo:BlogPosting  rdfs:comment  "A blog post." ;
        rdfs:label    "BlogPosting" .

sdo:CarUsageType  rdfs:comment  "A value indicating a special usage of a car, e.g. commercial rental, driving school, or as a taxi." ;
        rdfs:label    "CarUsageType" .

sdo:AudiobookFormat  rdfs:comment  "Book format: Audiobook. This is an enumerated value for use with the bookFormat property. There is also a type 'Audiobook' in the bib extension which includes Audiobook specific properties." ;
        rdfs:label    "AudiobookFormat" .

sdo:containedInPlace  rdfs:comment  "The basic containment relation between a place and one that contains it." ;
        rdfs:label    "contained inPlace" .

sdo:starRating  rdfs:comment  "An official rating for a lodging business or food establishment, e.g. from national associations or standards bodies. Use the author property to indicate the rating organization, e.g. as an Organization with name such as (e.g. HOTREC, DEHOGA, WHR, or Hotelstars)." ;
        rdfs:label    "star rating" .

sdo:permissionType  rdfs:comment  "The type of permission granted the person, organization, or audience." ;
        rdfs:label    "permission type" .

sdo:isLiveBroadcast  rdfs:comment  "True if the broadcast is of a live event." ;
        rdfs:label    "is liveBroadcast" .

sdo:Thesis  rdfs:comment  "A thesis or dissertation document submitted in support of candidature for an academic degree or professional qualification." ;
        rdfs:label    "Thesis" .

sdo:DeliveryMethod  rdfs:comment  "A delivery method is a standardized procedure for transferring the product or service to the destination of fulfillment chosen by the customer. Delivery methods are characterized by the means of transportation used, and by the organization or group that is the contracting party for the sending organization or person.\\n\\nCommonly used values:\\n\\n* http://purl.org/goodrelations/v1#DeliveryModeDirectDownload\\n* http://purl.org/goodrelations/v1#DeliveryModeFreight\\n* http://purl.org/goodrelations/v1#DeliveryModeMail\\n* http://purl.org/goodrelations/v1#DeliveryModeOwnFleet\\n* http://purl.org/goodrelations/v1#DeliveryModePickUp\\n* http://purl.org/goodrelations/v1#DHL\\n* http://purl.org/goodrelations/v1#FederalExpress\\n* http://purl.org/goodrelations/v1#UPS\n        " ;
        rdfs:label    "DeliveryMethod" .

sdo:drainsTo  rdfs:comment  "The vasculature that the vein drains into." ;
        rdfs:label    "drains to" .

sdo:nutrition  rdfs:comment  "Nutrition information about the recipe or menu item." ;
        rdfs:label    "nutrition" .

sdo:OneTimePayments  rdfs:comment  "OneTimePayments: this is a benefit for one-time payments for individuals." ;
        rdfs:label    "OneTimePayments" .

sdo:isConsumableFor  rdfs:comment  "A pointer to another product (or multiple products) for which this product is a consumable." ;
        rdfs:label    "is consumableFor" .

sdo:WorkBasedProgram  rdfs:comment  "A program with both an educational and employment component. Typically based at a workplace and structured around work-based learning, with the aim of instilling competencies related to an occupation. WorkBasedProgram is used to distinguish programs such as apprenticeships from school, college or other classroom based educational programs." ;
        rdfs:label    "WorkBasedProgram" .

sdo:xpath  rdfs:comment  "An XPath, e.g. of a [[SpeakableSpecification]] or [[WebPageElement]]. In the latter case, multiple matches within a page can constitute a single conceptual \"Web page element\"." ;
        rdfs:label    "xpath" .

sdo:competencyRequired
        rdfs:comment  "Knowledge, skill, ability or personal attribute that must be demonstrated by a person or other entity in order to do something such as earn an Educational Occupational Credential or understand a LearningResource." ;
        rdfs:label    "competency required" .

sdo:prescribingInfo  rdfs:comment  "Link to prescribing information for the drug." ;
        rdfs:label    "prescribing info" .

sdo:Throat  rdfs:comment  "Throat assessment with  clinical examination." ;
        rdfs:label    "Throat" .

sdo:WantAction  rdfs:comment  "The act of expressing a desire about the object. An agent wants an object." ;
        rdfs:label    "WantAction" .

sdo:monthlyMinimumRepaymentAmount
        rdfs:comment  "The minimum payment is the lowest amount of money that one is required to pay on a credit card statement each month." ;
        rdfs:label    "monthly minimumRepaymentAmount" .

sdo:MediaReviewItem  rdfs:comment  "Represents an item or group of closely related items treated as a unit for the sake of evaluation in a [[MediaReview]]. Authorship etc. apply to the items rather than to the curation/grouping or reviewing party." ;
        rdfs:label    "MediaReviewItem" .

sdo:DigitalDocumentPermission
        rdfs:comment  "A permission for a particular person or group to access a particular file." ;
        rdfs:label    "DigitalDocumentPermission" .

sdo:relatedAnatomy  rdfs:comment  "Anatomical systems or structures that relate to the superficial anatomy." ;
        rdfs:label    "related anatomy" .

sdo:requiresSubscription
        rdfs:comment  "Indicates if use of the media require a subscription  (either paid or free). Allowed values are ```true``` or ```false``` (note that an earlier version had 'yes', 'no')." ;
        rdfs:label    "requires subscription" .

sdo:TVSeries  rdfs:comment  "CreativeWorkSeries dedicated to TV broadcast and associated online delivery." ;
        rdfs:label    "TVSeries" .

sdo:Tuesday  rdfs:comment  "The day of the week between Monday and Wednesday." ;
        rdfs:label    "Tuesday" .

sdo:OfflineEventAttendanceMode
        rdfs:comment  "OfflineEventAttendanceMode - an event that is primarily conducted offline. " ;
        rdfs:label    "OfflineEventAttendanceMode" .

sdo:Paperback  rdfs:comment  "Book format: Paperback." ;
        rdfs:label    "Paperback" .

sdo:EPRelease  rdfs:comment  "EPRelease." ;
        rdfs:label    "EPRelease" .

sdo:EducationalAudience
        rdfs:comment  "An EducationalAudience." ;
        rdfs:label    "EducationalAudience" .

sdo:UnRegisterAction  rdfs:comment  "The act of un-registering from a service.\\n\\nRelated actions:\\n\\n* [[RegisterAction]]: antonym of UnRegisterAction.\\n* [[LeaveAction]]: Unlike LeaveAction, UnRegisterAction implies that you are unregistering from a service you werer previously registered, rather than leaving a team/group of people." ;
        rdfs:label    "UnRegisterAction" .

sdo:containsSeason  rdfs:comment  "A season that is part of the media series." ;
        rdfs:label    "contains season" .

sdo:archiveHeld  rdfs:comment  "Collection, [fonds](https://en.wikipedia.org/wiki/Fonds), or item held, kept or maintained by an [[ArchiveOrganization]]."@en ;
        rdfs:label    "archive held"@en .

sdo:PublicationIssue  rdfs:comment  "A part of a successively published publication such as a periodical or publication volume, often numbered, usually containing a grouping of works such as articles.\\n\\nSee also [blog post](http://blog.schema.org/2014/09/schemaorg-support-for-bibliographic_2.html)." ;
        rdfs:label    "PublicationIssue" .

sdo:alternativeHeadline
        rdfs:comment  "A secondary title of the CreativeWork." ;
        rdfs:label    "alternative headline" .

sdo:DrugPregnancyCategory
        rdfs:comment  "Categories that represent an assessment of the risk of fetal injury due to a drug or pharmaceutical used as directed by the mother during pregnancy." ;
        rdfs:label    "DrugPregnancyCategory" .

sdo:ServiceChannel  rdfs:comment  "A means for accessing a service, e.g. a government office location, web site, or phone number." ;
        rdfs:label    "ServiceChannel" .

sdo:DanceGroup  rdfs:comment  "A dance group&#x2014;for example, the Alvin Ailey Dance Theater or Riverdance." ;
        rdfs:label    "DanceGroup" .

sdo:color  rdfs:comment  "The color of the product." ;
        rdfs:label    "color" .

sdo:bodyLocation  rdfs:comment  "Location in the body of the anatomical structure." ;
        rdfs:label    "body location" .

sdo:cheatCode  rdfs:comment  "Cheat codes to the game." ;
        rdfs:label    "cheat code" .

sdo:language  rdfs:comment  "A sub property of instrument. The language used on this action." ;
        rdfs:label    "language" .

sdo:slogan  rdfs:comment  "A slogan or motto associated with the item." ;
        rdfs:label    "slogan" .

sdo:tocContinuation  rdfs:comment  "A [[HyperTocEntry]] can have a [[tocContinuation]] indicated, which is another [[HyperTocEntry]] that would be the default next item to play or render." ;
        rdfs:label    "toc continuation" .

sdo:ControlAction  rdfs:comment  "An agent controls a device or application." ;
        rdfs:label    "ControlAction" .

sdo:experienceRequirements
        rdfs:comment  "Description of skills and experience needed for the position or Occupation." ;
        rdfs:label    "experience requirements" .

sdo:Muscle  rdfs:comment  "A muscle is an anatomical structure consisting of a contractile form of tissue that animals use to effect movement." ;
        rdfs:label    "Muscle" .

sdo:DataDownload  rdfs:comment  "A dataset in downloadable form." ;
        rdfs:label    "DataDownload" .

sdo:LaboratoryScience
        rdfs:comment  "A medical science pertaining to chemical, hematological, immunologic, microscopic, or bacteriological diagnostic analyses or research." ;
        rdfs:label    "LaboratoryScience" .

sdo:fuelEfficiency  rdfs:comment  "The distance traveled per unit of fuel used; most commonly miles per gallon (mpg) or kilometers per liter (km/L).\\n\\n* Note 1: There are unfortunately no standard unit codes for miles per gallon or kilometers per liter. Use [[unitText]] to indicate the unit of measurement, e.g. mpg or km/L.\\n* Note 2: There are two ways of indicating the fuel consumption, [[fuelConsumption]] (e.g. 8 liters per 100 km) and [[fuelEfficiency]] (e.g. 30 miles per gallon). They are reciprocal.\\n* Note 3: Often, the absolute value is useful only when related to driving speed (\"at 80 km/h\") or usage pattern (\"city traffic\"). You can use [[valueReference]] to link the value for the fuel economy to another value." ;
        rdfs:label    "fuel efficiency" .

sdo:ChildrensEvent  rdfs:comment  "Event type: Children's event." ;
        rdfs:label    "ChildrensEvent" .

sdo:KosherDiet  rdfs:comment  "A diet conforming to Jewish dietary practices." ;
        rdfs:label    "KosherDiet" .

sdo:AdministrativeArea
        rdfs:comment  "A geographical region, typically under the jurisdiction of a particular government." ;
        rdfs:label    "AdministrativeArea" .

sdo:arrivalBoatTerminal
        rdfs:comment  "The terminal or port from which the boat arrives." ;
        rdfs:label    "arrival boatTerminal" .

sdo:departureTime  rdfs:comment  "The expected departure time." ;
        rdfs:label    "departure time" .

sdo:totalTime  rdfs:comment  "The total time required to perform instructions or a direction (including time to prepare the supplies), in [ISO 8601 duration format](http://en.wikipedia.org/wiki/ISO_8601)." ;
        rdfs:label    "total time" .

sdo:directors  rdfs:comment  "A director of e.g. tv, radio, movie, video games etc. content. Directors can be associated with individual items or with a series, episode, clip." ;
        rdfs:label    "directors" .

sdo:MedicalBusiness  rdfs:comment  "A particular physical or virtual business of an organization for medical purposes. Examples of MedicalBusiness include differents business run by health professionals." ;
        rdfs:label    "MedicalBusiness" .

sdo:BankOrCreditUnion
        rdfs:comment  "Bank or credit union." ;
        rdfs:label    "BankOrCreditUnion" .

sdo:LegislationObject
        rdfs:comment  "A specific object or file containing a Legislation. Note that the same Legislation can be published in multiple files. For example, a digitally signed PDF, a plain PDF and an HTML version." ;
        rdfs:label    "LegislationObject" .

sdo:isPartOf  rdfs:comment  "Indicates an item or CreativeWork that this item, or CreativeWork (in some sense), is part of." ;
        rdfs:label    "is partOf" .

sdo:Oncologic  rdfs:comment  "A specific branch of medical science that deals with benign and malignant tumors, including the study of their development, diagnosis, treatment and prevention." ;
        rdfs:label    "Oncologic" .

sdo:AchieveAction  rdfs:comment  "The act of accomplishing something via previous efforts. It is an instantaneous action rather than an ongoing process." ;
        rdfs:label    "AchieveAction" .

sdo:ReservationStatusType
        rdfs:comment  "Enumerated status values for Reservation." ;
        rdfs:label    "ReservationStatusType" .

sdo:ReturnLabelDownloadAndPrint
        rdfs:comment  "Indicated that a return label must be downloaded and printed by the customer." ;
        rdfs:label    "ReturnLabelDownloadAndPrint" .

sdo:sportsActivityLocation
        rdfs:comment  "A sub property of location. The sports activity location where this action occurred." ;
        rdfs:label    "sports activityLocation" .

sdo:HealthCare  rdfs:comment  "HealthCare: this is a benefit for health care." ;
        rdfs:label    "HealthCare" .

sdo:Dentistry  rdfs:comment  "A branch of medicine that is involved in the dental care." ;
        rdfs:label    "Dentistry" .

sdo:Date  rdfs:comment  "A date value in [ISO 8601 date format](http://en.wikipedia.org/wiki/ISO_8601)." ;
        rdfs:label    "Date" .

sdo:meetsEmissionStandard
        rdfs:comment  "Indicates that the vehicle meets the respective emission standard." ;
        rdfs:label    "meets emissionStandard" .

sdo:creator  rdfs:comment  "The creator/author of this CreativeWork. This is the same as the Author property for CreativeWork." ;
        rdfs:label    "creator" .

sdo:cvdNumC19MechVentPats
        rdfs:comment  "numc19mechventpats - HOSPITALIZED and VENTILATED: Patients hospitalized in an NHSN inpatient care location who have suspected or confirmed COVID-19 and are on a mechanical ventilator." ;
        rdfs:label    "cvd numC19MechVentPats" .

sdo:QualitativeValue  rdfs:comment  "A predefined value for a product characteristic, e.g. the power cord plug type 'US' or the garment sizes 'S', 'M', 'L', and 'XL'." ;
        rdfs:label    "QualitativeValue" .

sdo:Brand  rdfs:comment  "A brand is a name used by an organization or business person for labeling a product, product group, or similar." ;
        rdfs:label    "Brand" .

sdo:minPrice  rdfs:comment  "The lowest price if the price is a range." ;
        rdfs:label    "min price" .

sdo:Recipe  rdfs:comment  "A recipe. For dietary restrictions covered by the recipe, a few common restrictions are enumerated via [[suitableForDiet]]. The [[keywords]] property can also be used to add more detail." ;
        rdfs:label    "Recipe" .

sdo:MediaSubscription
        rdfs:comment  "A subscription which allows a user to access media including audio, video, books, etc." ;
        rdfs:label    "MediaSubscription" .

sdo:PodcastEpisode  rdfs:comment  "A single episode of a podcast series." ;
        rdfs:label    "PodcastEpisode" .

sdo:DefinedRegion  rdfs:comment  "A DefinedRegion is a geographic area defined by potentially arbitrary (rather than political, administrative or natural geographical) criteria. Properties are provided for defining a region by reference to sets of postal codes.\n\nExamples: a delivery destination when shopping. Region where regional pricing is configured.\n\nRequirement 1:\nCountry: US\nStates: \"NY\", \"CA\"\n\nRequirement 2:\nCountry: US\nPostalCode Set: { [94000-94585], [97000, 97999], [13000, 13599]}\n{ [12345, 12345], [78945, 78945], }\nRegion = state, canton, prefecture, autonomous community...\n" ;
        rdfs:label    "DefinedRegion" .

sdo:busName  rdfs:comment  "The name of the bus (e.g. Bolt Express)." ;
        rdfs:label    "bus name" .

sdo:broadcaster  rdfs:comment  "The organization owning or operating the broadcast service." ;
        rdfs:label    "broadcaster" .

sdo:model  rdfs:comment  "The model of the product. Use with the URL of a ProductModel or a textual representation of the model identifier. The URL of the ProductModel can be from an external source. It is recommended to additionally provide strong product identifiers via the gtin8/gtin13/gtin14 and mpn properties." ;
        rdfs:label    "model" .

sdo:broadcastSubChannel
        rdfs:comment  "The subchannel used for the broadcast." ;
        rdfs:label    "broadcast subChannel" .

sdo:LinkRole  rdfs:comment  "A Role that represents a Web link e.g. as expressed via the 'url' property. Its linkRelationship property can indicate URL-based and plain textual link types e.g. those in IANA link registry or others such as 'amphtml'. This structure provides a placeholder where details from HTML's link element can be represented outside of HTML, e.g. in JSON-LD feeds." ;
        rdfs:label    "LinkRole" .

sdo:UsedCondition  rdfs:comment  "Indicates that the item is used." ;
        rdfs:label    "UsedCondition" .

sdo:founders  rdfs:comment  "A person who founded this organization." ;
        rdfs:label    "founders" .

sdo:Map  rdfs:comment  "A map." ;
        rdfs:label    "Map" .

sdo:OrderProblem  rdfs:comment  "OrderStatus representing that there is a problem with the order." ;
        rdfs:label    "OrderProblem" .

sdo:spatialCoverage  rdfs:comment  "The spatialCoverage of a CreativeWork indicates the place(s) which are the focus of the content. It is a subproperty of\n      contentLocation intended primarily for more technical and detailed materials. For example with a Dataset, it indicates\n      areas that the dataset describes: a dataset of New York weather would have spatialCoverage which was the place: the state of New York." ;
        rdfs:label    "spatial coverage" .

sdo:UserInteraction  rdfs:comment  "UserInteraction and its subtypes is an old way of talking about users interacting with pages. It is generally better to use [[Action]]-based vocabulary, alongside types such as [[Comment]]." ;
        rdfs:label    "UserInteraction" .

sdo:Drug  rdfs:comment  "A chemical or biologic substance, used as a medical therapy, that has a physiological effect on an organism. Here the term drug is used interchangeably with the term medicine although clinical knowledge make a clear difference between them." ;
        rdfs:label    "Drug" .

sdo:recommendationStrength
        rdfs:comment  "Strength of the guideline's recommendation (e.g. 'class I')." ;
        rdfs:label    "recommendation strength" .

sdo:engineType  rdfs:comment  "The type of engine or engines powering the vehicle." ;
        rdfs:label    "engine type" .

sdo:DrugStrength  rdfs:comment  "A specific strength in which a medical drug is available in a specific country." ;
        rdfs:label    "DrugStrength" .

sdo:pickupTime  rdfs:comment  "When a taxi will pickup a passenger or a rental car can be picked up." ;
        rdfs:label    "pickup time" .

sdo:aircraft  rdfs:comment  "The kind of aircraft (e.g., \"Boeing 747\")." ;
        rdfs:label    "aircraft" .

sdo:Nonprofit501f  rdfs:comment  "Nonprofit501f: Non-profit type referring to Cooperative Service Organizations." ;
        rdfs:label    "Nonprofit501f" .

sdo:orderItemStatus  rdfs:comment  "The current status of the order item." ;
        rdfs:label    "order itemStatus" .

sdo:question  rdfs:comment  "A sub property of object. A question." ;
        rdfs:label    "question" .

sdo:embeddedTextCaption
        rdfs:comment  "Represents textual captioning from a [[MediaObject]], e.g. text of a 'meme'." ;
        rdfs:label    "embedded textCaption" .

sdo:Vein  rdfs:comment  "A type of blood vessel that specifically carries blood to the heart." ;
        rdfs:label    "Vein" .

sdo:associatedAnatomy
        rdfs:comment  "The anatomy of the underlying organ system or structures associated with this entity." ;
        rdfs:label    "associated anatomy" .

sdo:BusStation  rdfs:comment  "A bus station." ;
        rdfs:label    "BusStation" .

sdo:toLocation  rdfs:comment  "A sub property of location. The final location of the object or the agent after the action." ;
        rdfs:label    "to location" .

sdo:hasMenu  rdfs:comment  "Either the actual menu as a structured representation, as text, or a URL of the menu." ;
        rdfs:label    "has menu" .

sdo:HowTo  rdfs:comment  "Instructions that explain how to achieve a result by performing a sequence of steps." ;
        rdfs:label    "HowTo" .

sdo:expertConsiderations
        rdfs:comment  "Medical expert advice related to the plan." ;
        rdfs:label    "expert considerations" .

sdo:workTranslation  rdfs:comment  "A work that is a translation of the content of this work. e.g. 西遊記 has an English workTranslation “Journey to the West”,a German workTranslation “Monkeys Pilgerfahrt” and a Vietnamese  translation Tây du ký bình khảo." ;
        rdfs:label    "work translation" .

sdo:DrugLegalStatus  rdfs:comment  "The legal availability status of a medical drug." ;
        rdfs:label    "DrugLegalStatus" .

sdo:Ultrasound  rdfs:comment  "Ultrasound imaging." ;
        rdfs:label    "Ultrasound" .

sdo:Distillery  rdfs:comment  "A distillery." ;
        rdfs:label    "Distillery" .

sdo:episodes  rdfs:comment  "An episode of a TV/radio series or season." ;
        rdfs:label    "episodes" .

sdo:healthPlanMarketingUrl
        rdfs:comment  "The URL that goes directly to the plan brochure for the specific standard plan or plan variation." ;
        rdfs:label    "health planMarketingUrl" .

sdo:possibleComplication
        rdfs:comment  "A possible unexpected and unfavorable evolution of a medical condition. Complications may include worsening of the signs or symptoms of the disease, extension of the condition to other organ systems, etc." ;
        rdfs:label    "possible complication" .

sdo:catalog  rdfs:comment  "A data catalog which contains this dataset." ;
        rdfs:label    "catalog" .

sdo:maps  rdfs:comment  "A URL to a map of the place." ;
        rdfs:label    "maps" .

sdo:CardiovascularExam
        rdfs:comment  "Cardiovascular system assessment withclinical examination." ;
        rdfs:label    "CardiovascularExam" .

sdo:BodyMeasurementNeck
        rdfs:comment  "Girth of neck. Used, for example, to fit shirts." ;
        rdfs:label    "BodyMeasurementNeck" .

sdo:hiringOrganization
        rdfs:comment  "Organization offering the job position." ;
        rdfs:label    "hiring organization" .

sdo:serviceUrl  rdfs:comment  "The website to access the service." ;
        rdfs:label    "service url" .

sdo:antagonist  rdfs:comment  "The muscle whose action counteracts the specified muscle." ;
        rdfs:label    "antagonist" .

sdo:gameTip  rdfs:comment  "Links to tips, tactics, etc." ;
        rdfs:label    "game tip" .

sdo:includedInHealthInsurancePlan
        rdfs:comment  "The insurance plans that cover this drug." ;
        rdfs:label    "included inHealthInsurancePlan" .

sdo:flightNumber  rdfs:comment  "The unique identifier for a flight including the airline IATA code. For example, if describing United flight 110, where the IATA code for United is 'UA', the flightNumber is 'UA110'." ;
        rdfs:label    "flight number" .

sdo:numAdults  rdfs:comment  "The number of adults staying in the unit." ;
        rdfs:label    "num adults" .

sdo:WebAPI  rdfs:comment  "An application programming interface accessible over Web/Internet technologies." ;
        rdfs:label    "WebAPI" .

sdo:SeekToAction  rdfs:comment  "This is the [[Action]] of navigating to a specific [[startOffset]] timestamp within a [[VideoObject]], typically represented with a URL template structure." ;
        rdfs:label    "SeekToAction" .

sdo:TrainTrip  rdfs:comment  "A trip on a commercial train line." ;
        rdfs:label    "TrainTrip" .

sdo:EUEnergyEfficiencyCategoryG
        rdfs:comment  "Represents EU Energy Efficiency Class G as defined in EU energy labeling regulations." ;
        rdfs:label    "EUEnergyEfficiencyCategoryG" .

sdo:BroadcastEvent  rdfs:comment  "An over the air or online broadcast event." ;
        rdfs:label    "BroadcastEvent" .

sdo:releaseOf  rdfs:comment  "The album this is a release of." ;
        rdfs:label    "release of" .

sdo:HowToStep  rdfs:comment  "A step in the instructions for how to achieve a result. It is an ordered list with HowToDirection and/or HowToTip items." ;
        rdfs:label    "HowToStep" .

sdo:httpMethod  rdfs:comment  "An HTTP method that specifies the appropriate HTTP method for a request to an HTTP EntryPoint. Values are capitalized strings as used in HTTP." ;
        rdfs:label    "http method" .

sdo:PrependAction  rdfs:comment  "The act of inserting at the beginning if an ordered collection." ;
        rdfs:label    "PrependAction" .

sdo:postalCodeBegin  rdfs:comment  "First postal code in a range (included)." ;
        rdfs:label    "postal codeBegin" .

sdo:Suspended  rdfs:comment  "Suspended." ;
        rdfs:label    "Suspended" .

sdo:Rating  rdfs:comment  "A rating is an evaluation on a numeric scale, such as 1 to 5 stars." ;
        rdfs:label    "Rating" .

sdo:arrivalStation  rdfs:comment  "The station where the train trip ends." ;
        rdfs:label    "arrival station" .

sdo:spatial  rdfs:comment  "The \"spatial\" property can be used in cases when more specific properties\n(e.g. [[locationCreated]], [[spatialCoverage]], [[contentLocation]]) are not known to be appropriate." ;
        rdfs:label    "spatial" .

sdo:usesHealthPlanIdStandard
        rdfs:comment  "The standard for interpreting thePlan ID. The preferred is \"HIOS\". See the Centers for Medicare & Medicaid Services for more details." ;
        rdfs:label    "uses healthPlanIdStandard" .

sdo:StagesHealthAspect
        rdfs:comment  "Stages that can be observed from a topic." ;
        rdfs:label    "StagesHealthAspect" .

sdo:PodcastSeason  rdfs:comment  "A single season of a podcast. Many podcasts do not break down into separate seasons. In that case, PodcastSeries should be used." ;
        rdfs:label    "PodcastSeason" .

sdo:termsPerYear  rdfs:comment  "The number of times terms of study are offered per year. Semesters and quarters are common units for term. For example, if the student can only take 2 semesters for the program in one year, then termsPerYear should be 2." ;
        rdfs:label    "terms perYear" .

sdo:size  rdfs:comment  "A standardized size of a product or creative work, specified either through a simple textual string (for example 'XL', '32Wx34L'), a  QuantitativeValue with a unitCode, or a comprehensive and structured [[SizeSpecification]]; in other cases, the [[width]], [[height]], [[depth]] and [[weight]] properties may be more applicable. " ;
        rdfs:label    "size" .

sdo:Grant  rdfs:comment  "A grant, typically financial or otherwise quantifiable, of resources. Typically a [[funder]] sponsors some [[MonetaryAmount]] to an [[Organization]] or [[Person]],\n    sometimes not necessarily via a dedicated or long-lived [[Project]], resulting in one or more outputs, or [[fundedItem]]s. For financial sponsorship, indicate the [[funder]] of a [[MonetaryGrant]]. For non-financial support, indicate [[sponsor]] of [[Grant]]s of resources (e.g. office space).\n\nGrants support  activities directed towards some agreed collective goals, often but not always organized as [[Project]]s. Long-lived projects are sometimes sponsored by a variety of grants over time, but it is also common for a project to be associated with a single grant.\n\nThe amount of a [[Grant]] is represented using [[amount]] as a [[MonetaryAmount]].\n    " ;
        rdfs:label    "Grant" .

sdo:Atlas  rdfs:comment  "A collection or bound volume of maps, charts, plates or tables, physical or in media form illustrating any subject." ;
        rdfs:label    "Atlas" .

sdo:SendAction  rdfs:comment  "The act of physically/electronically dispatching an object for transfer from an origin to a destination.Related actions:\\n\\n* [[ReceiveAction]]: The reciprocal of SendAction.\\n* [[GiveAction]]: Unlike GiveAction, SendAction does not imply the transfer of ownership (e.g. I can send you my laptop, but I'm not necessarily giving it to you)." ;
        rdfs:label    "SendAction" .

sdo:MusicComposition  rdfs:comment  "A musical composition." ;
        rdfs:label    "MusicComposition" .

sdo:industry  rdfs:comment  "The industry associated with the job position." ;
        rdfs:label    "industry" .

sdo:PrognosisHealthAspect
        rdfs:comment  "Typical progression and happenings of life course of the topic." ;
        rdfs:label    "PrognosisHealthAspect" .

sdo:Float  rdfs:comment  "Data type: Floating number." ;
        rdfs:label    "Float" .

sdo:Restaurant  rdfs:comment  "A restaurant." ;
        rdfs:label    "Restaurant" .

sdo:LegalService  rdfs:comment  "A LegalService is a business that provides legally-oriented services, advice and representation, e.g. law firms.\\n\\nAs a [[LocalBusiness]] it can be described as a [[provider]] of one or more [[Service]]\\(s)." ;
        rdfs:label    "LegalService" .

sdo:AnalysisNewsArticle
        rdfs:comment  "An AnalysisNewsArticle is a [[NewsArticle]] that, while based on factual reporting, incorporates the expertise of the author/producer, offering interpretations and conclusions." ;
        rdfs:label    "AnalysisNewsArticle" .

sdo:ItemList  rdfs:comment  "A list of items of any sort&#x2014;for example, Top 10 Movies About Weathermen, or Top 100 Party Songs. Not to be confused with HTML lists, which are often used only for formatting." ;
        rdfs:label    "ItemList" .

sdo:ComicIssue  rdfs:comment  "Individual comic issues are serially published as\n    \tpart of a larger series. For the sake of consistency, even one-shot issues\n    \tbelong to a series comprised of a single issue. All comic issues can be\n    \tuniquely identified by: the combination of the name and volume number of the\n    \tseries to which the issue belongs; the issue number; and the variant\n    \tdescription of the issue (if any)." ;
        rdfs:label    "ComicIssue" .

sdo:geoContains  rdfs:comment  "Represents a relationship between two geometries (or the places they represent), relating a containing geometry to a contained geometry. \"a contains b iff no points of b lie in the exterior of a, and at least one point of the interior of b lies in the interior of a\". As defined in [DE-9IM](https://en.wikipedia.org/wiki/DE-9IM)." ;
        rdfs:label    "geo contains" .

sdo:OnlineEventAttendanceMode
        rdfs:comment  "OnlineEventAttendanceMode - an event that is primarily conducted online. " ;
        rdfs:label    "OnlineEventAttendanceMode" .

sdo:closes  rdfs:comment  "The closing hour of the place or service on the given day(s) of the week." ;
        rdfs:label    "closes" .

sdo:address  rdfs:comment  "Physical address of the item." ;
        rdfs:label    "address" .

sdo:ResultsNotAvailable
        rdfs:comment  "Results are not available." ;
        rdfs:label    "ResultsNotAvailable" .

sdo:authenticator  rdfs:comment  "The Organization responsible for authenticating the user's subscription. For example, many media apps require a cable/satellite provider to authenticate your subscription before playing media." ;
        rdfs:label    "authenticator" .

sdo:EnergyStarCertified
        rdfs:comment  "Represents EnergyStar certification." ;
        rdfs:label    "EnergyStarCertified" .

sdo:relatedTherapy  rdfs:comment  "A medical therapy related to this anatomy." ;
        rdfs:label    "related therapy" .

sdo:acceptedOffer  rdfs:comment  "The offer(s) -- e.g., product, quantity and price combinations -- included in the order." ;
        rdfs:label    "accepted offer" .

sdo:smiles  rdfs:comment  "A specification in form of a line notation for describing the structure of chemical species using short ASCII strings.  Double bond stereochemistry \\ indicators may need to be escaped in the string in formats where the backslash is an escape character." ;
        rdfs:label    "smiles" .

sdo:articleBody  rdfs:comment  "The actual body of the article." ;
        rdfs:label    "article body" .

sdo:partOfSeason  rdfs:comment  "The season to which this episode belongs." ;
        rdfs:label    "part ofSeason" .

sdo:LeisureTimeActivity
        rdfs:comment  "Any physical activity engaged in for recreational purposes. Examples may include ballroom dancing, roller skating, canoeing, fishing, etc." ;
        rdfs:label    "LeisureTimeActivity" .

sdo:Nose  rdfs:comment  "Nose function assessment with clinical examination." ;
        rdfs:label    "Nose" .

sdo:inChIKey  rdfs:comment  "InChIKey is a hashed version of the full InChI (using the SHA-256 algorithm)." ;
        rdfs:label    "in chIKey" .

sdo:Mass  rdfs:comment  "Properties that take Mass as values are of the form '&lt;Number&gt; &lt;Mass unit of measure&gt;'. E.g., '7 kg'." ;
        rdfs:label    "Mass" .

sdo:MedicalObservationalStudyDesign
        rdfs:comment  "Design models for observational medical studies. Enumerated type." ;
        rdfs:label    "MedicalObservationalStudyDesign" .

sdo:customerRemorseReturnLabelSource
        rdfs:comment  "The method (from an enumeration) by which the customer obtains a return shipping label for a product returned due to customer remorse." ;
        rdfs:label    "customer remorseReturnLabelSource" .

sdo:PublicationEvent  rdfs:comment  "A PublicationEvent corresponds indifferently to the event of publication for a CreativeWork of any type e.g. a broadcast event, an on-demand event, a book/journal publication via a variety of delivery media." ;
        rdfs:label    "PublicationEvent" .

sdo:Florist  rdfs:comment  "A florist." ;
        rdfs:label    "Florist" .

sdo:FindAction  rdfs:comment  "The act of finding an object.\\n\\nRelated actions:\\n\\n* [[SearchAction]]: FindAction is generally lead by a SearchAction, but not necessarily." ;
        rdfs:label    "FindAction" .

sdo:WearableSizeGroupMaternity
        rdfs:comment  "Size group \"Maternity\" for wearables." ;
        rdfs:label    "WearableSizeGroupMaternity" .

sdo:UsageOrScheduleHealthAspect
        rdfs:comment  "Content about how, when, frequency and dosage of a topic." ;
        rdfs:label    "UsageOrScheduleHealthAspect" .

sdo:SchoolDistrict  rdfs:comment  "A School District is an administrative area for the administration of schools." ;
        rdfs:label    "SchoolDistrict" .

sdo:pathophysiology  rdfs:comment  "Changes in the normal mechanical, physical, and biochemical functions that are associated with this activity or condition." ;
        rdfs:label    "pathophysiology" .

sdo:opponent  rdfs:comment  "A sub property of participant. The opponent on this action." ;
        rdfs:label    "opponent" .

sdo:faxNumber  rdfs:comment  "The fax number." ;
        rdfs:label    "fax number" .

sdo:RegisterAction  rdfs:comment  "The act of registering to be a user of a service, product or web page.\\n\\nRelated actions:\\n\\n* [[JoinAction]]: Unlike JoinAction, RegisterAction implies you are registering to be a user of a service, *not* a group/team of people.\\n* [FollowAction]]: Unlike FollowAction, RegisterAction doesn't imply that the agent is expecting to poll for updates from the object.\\n* [[SubscribeAction]]: Unlike SubscribeAction, RegisterAction doesn't imply that the agent is expecting updates from the object." ;
        rdfs:label    "RegisterAction" .

sdo:coverageEndTime  rdfs:comment  "The time when the live blog will stop covering the Event. Note that coverage may continue after the Event concludes." ;
        rdfs:label    "coverage endTime" .

sdo:XRay  rdfs:comment  "X-ray imaging." ;
        rdfs:label    "XRay" .

sdo:connectedTo  rdfs:comment  "Other anatomical structures to which this structure is connected." ;
        rdfs:label    "connected to" .

sdo:LearningResource  rdfs:comment  "The LearningResource type can be used to indicate [[CreativeWork]]s (whether physical or digital) that have a particular and explicit orientation towards learning, education, skill acquisition, and other educational purposes.\n\n[[LearningResource]] is expected to be used as an addition to a primary type such as [[Book]], [[VideoObject]], [[Product]] etc.\n\n[[EducationEvent]] serves a similar purpose for event-like things (e.g. a [[Trip]]). A [[LearningResource]] may be created as a result of an [[EducationEvent]], for example by recording one." ;
        rdfs:label    "LearningResource" .

sdo:dateIssued  rdfs:comment  "The date the ticket was issued." ;
        rdfs:label    "date issued" .

sdo:identifyingTest  rdfs:comment  "A diagnostic test that can identify this sign." ;
        rdfs:label    "identifying test" .

sdo:replyToUrl  rdfs:comment  "The URL at which a reply may be posted to the specified UserComment." ;
        rdfs:label    "reply toUrl" .

sdo:CT  rdfs:comment  "X-ray computed tomography imaging." ;
        rdfs:label    "CT" .

sdo:ClaimReview  rdfs:comment  "A fact-checking review of claims made (or reported) in some creative work (referenced via itemReviewed)." ;
        rdfs:label    "ClaimReview" .

sdo:printPage  rdfs:comment  "If this NewsArticle appears in print, this field indicates the name of the page on which the article is found. Please note that this field is intended for the exact page name (e.g. A5, B18)." ;
        rdfs:label    "print page" .

sdo:DataType  rdfs:comment  "The basic data types such as Integers, Strings, etc." ;
        rdfs:label    "DataType" .

sdo:BoatTerminal  rdfs:comment  "A terminal for boats, ships, and other water vessels." ;
        rdfs:label    "BoatTerminal" .

sdo:sensoryUnit  rdfs:comment  "The neurological pathway extension that inputs and sends information to the brain or spinal cord." ;
        rdfs:label    "sensory unit" .

sdo:pregnancyCategory
        rdfs:comment  "Pregnancy category of this drug." ;
        rdfs:label    "pregnancy category" .

sdo:seatNumber  rdfs:comment  "The location of the reserved seat (e.g., 27)." ;
        rdfs:label    "seat number" .

sdo:winner  rdfs:comment  "A sub property of participant. The winner of the action." ;
        rdfs:label    "winner" .

sdo:HealthPlanNetwork
        rdfs:comment  "A US-style health insurance plan network. " ;
        rdfs:label    "HealthPlanNetwork" .

sdo:Gynecologic  rdfs:comment  "A specific branch of medical science that pertains to the health care of women, particularly in the diagnosis and treatment of disorders affecting the female reproductive system." ;
        rdfs:label    "Gynecologic" .

sdo:Pulmonary  rdfs:comment  "A specific branch of medical science that pertains to the study of the respiratory system and its respective disease states." ;
        rdfs:label    "Pulmonary" .

sdo:numTracks  rdfs:comment  "The number of tracks in this album or playlist." ;
        rdfs:label    "num tracks" .

sdo:contentRating  rdfs:comment  "Official rating of a piece of content&#x2014;for example,'MPAA PG-13'." ;
        rdfs:label    "content rating" .

sdo:Genitourinary  rdfs:comment  "Genitourinary system function assessment with clinical examination." ;
        rdfs:label    "Genitourinary" .

sdo:Taxi  rdfs:comment  "A taxi." ;
        rdfs:label    "Taxi" .

sdo:byMonthWeek  rdfs:comment  "Defines the week(s) of the month on which a recurring Event takes place. Specified as an Integer between 1-5. For clarity, byMonthWeek is best used in conjunction with byDay to indicate concepts like the first and third Mondays of a month." ;
        rdfs:label    "by monthWeek" .

sdo:endDate  rdfs:comment  "The end date and time of the item (in [ISO 8601 date format](http://en.wikipedia.org/wiki/ISO_8601))." ;
        rdfs:label    "end date" .

sdo:buyer  rdfs:comment  "A sub property of participant. The participant/person/organization that bought the object." ;
        rdfs:label    "buyer" .

sdo:SurgicalProcedure
        rdfs:comment  "A medical procedure involving an incision with instruments; performed for diagnose, or therapeutic purposes." ;
        rdfs:label    "SurgicalProcedure" .

sdo:Winery  rdfs:comment  "A winery." ;
        rdfs:label    "Winery" .

sdo:Hotel  rdfs:comment  "A hotel is an establishment that provides lodging paid on a short-term basis (Source: Wikipedia, the free encyclopedia, see http://en.wikipedia.org/wiki/Hotel).\n<br /><br />\nSee also the <a href=\"/docs/hotels.html\">dedicated document on the use of schema.org for marking up hotels and other forms of accommodations</a>.\n" ;
        rdfs:label    "Hotel" .

sdo:bookFormat  rdfs:comment  "The format of the book." ;
        rdfs:label    "book format" .

sdo:usesDevice  rdfs:comment  "Device used to perform the test." ;
        rdfs:label    "uses device" .

sdo:itemDefectReturnShippingFeesAmount
        rdfs:comment  "Amount of shipping costs for defect product returns. Applicable when property [[itemDefectReturnFees]] equals [[ReturnShippingFees]]." ;
        rdfs:label    "item defectReturnShippingFeesAmount" .

sdo:Review  rdfs:comment  "A review of an item - for example, of a restaurant, movie, or store." ;
        rdfs:label    "Review" .

sdo:accountablePerson
        rdfs:comment  "Specifies the Person that is legally accountable for the CreativeWork." ;
        rdfs:label    "accountable person" .

sdo:replacee  rdfs:comment  "A sub property of object. The object that is being replaced." ;
        rdfs:label    "replacee" .

sdo:DryCleaningOrLaundry
        rdfs:comment  "A dry-cleaning business." ;
        rdfs:label    "DryCleaningOrLaundry" .

sdo:administrationRoute
        rdfs:comment  "A route by which this drug may be administered, e.g. 'oral'." ;
        rdfs:label    "administration route" .

sdo:courseCode  rdfs:comment  "The identifier for the [[Course]] used by the course [[provider]] (e.g. CS101 or 6.001)." ;
        rdfs:label    "course code" .

sdo:shippingDestination
        rdfs:comment  "indicates (possibly multiple) shipping destinations. These can be defined in several ways e.g. postalCode ranges." ;
        rdfs:label    "shipping destination" .

sdo:partOfInvoice  rdfs:comment  "The order is being paid as part of the referenced Invoice." ;
        rdfs:label    "part ofInvoice" .

sdo:TVClip  rdfs:comment  "A short TV program or a segment/part of a TV program." ;
        rdfs:label    "TVClip" .

sdo:Airport  rdfs:comment  "An airport." ;
        rdfs:label    "Airport" .

sdo:functionalClass  rdfs:comment  "The degree of mobility the joint allows." ;
        rdfs:label    "functional class" .

sdo:expectedArrivalUntil
        rdfs:comment  "The latest date the package may arrive." ;
        rdfs:label    "expected arrivalUntil" .

sdo:EmployerReview  rdfs:comment  "An [[EmployerReview]] is a review of an [[Organization]] regarding its role as an employer, written by a current or former employee of that organization." ;
        rdfs:label    "EmployerReview" .

sdo:ratingExplanation
        rdfs:comment  "A short explanation (e.g. one to two sentences) providing background context and other information that led to the conclusion expressed in the rating. This is particularly applicable to ratings associated with \"fact check\" markup using [[ClaimReview]]." ;
        rdfs:label    "rating explanation" .

sdo:DeliveryChargeSpecification
        rdfs:comment  "The price for the delivery of an offer using a particular delivery method." ;
        rdfs:label    "DeliveryChargeSpecification" .

sdo:numberOfBedrooms  rdfs:comment  "The total integer number of bedrooms in a some [[Accommodation]], [[ApartmentComplex]] or [[FloorPlan]]." ;
        rdfs:label    "number ofBedrooms" .

sdo:opens  rdfs:comment  "The opening hour of the place or service on the given day(s) of the week." ;
        rdfs:label    "opens" .

sdo:Nonprofit501a  rdfs:comment  "Nonprofit501a: Non-profit type referring to Farmers’ Cooperative Associations." ;
        rdfs:label    "Nonprofit501a" .

sdo:ReservationConfirmed
        rdfs:comment  "The status of a confirmed reservation." ;
        rdfs:label    "ReservationConfirmed" .

sdo:cvdNumICUBedsOcc  rdfs:comment  "numicubedsocc - ICU BED OCCUPANCY: Total number of staffed inpatient ICU beds that are occupied." ;
        rdfs:label    "cvd numICUBedsOcc" .

sdo:BarOrPub  rdfs:comment  "A bar or pub." ;
        rdfs:label    "BarOrPub" .

sdo:SiteNavigationElement
        rdfs:comment  "A navigation element of the page." ;
        rdfs:label    "SiteNavigationElement" .

sdo:algorithm  rdfs:comment  "The algorithm or rules to follow to compute the score." ;
        rdfs:label    "algorithm" .

sdo:knows  rdfs:comment  "The most generic bi-directional social/work relation." ;
        rdfs:label    "knows" .

sdo:amenityFeature  rdfs:comment  "An amenity feature (e.g. a characteristic or service) of the Accommodation. This generic property does not make a statement about whether the feature is included in an offer for the main accommodation or available at extra costs." ;
        rdfs:label    "amenity feature" .

sdo:MolecularEntity  rdfs:comment  "Any constitutionally or isotopically distinct atom, molecule, ion, ion pair, radical, radical ion, complex, conformer etc., identifiable as a separately distinguishable entity." ;
        rdfs:label    "MolecularEntity" .

sdo:serviceArea  rdfs:comment  "The geographic area where the service is provided." ;
        rdfs:label    "service area" .

sdo:DataCatalog  rdfs:comment  "A collection of datasets." ;
        rdfs:label    "DataCatalog" .

sdo:AboutPage  rdfs:comment  "Web page type: About page." ;
        rdfs:label    "AboutPage" .

sdo:worksFor  rdfs:comment  "Organizations that the person works for." ;
        rdfs:label    "works for" .

sdo:DrivingSchoolVehicleUsage
        rdfs:comment  "Indicates the usage of the vehicle for driving school." ;
        rdfs:label    "DrivingSchoolVehicleUsage" .

sdo:Enumeration  rdfs:comment  "Lists or enumerations—for example, a list of cuisines or music genres, etc." ;
        rdfs:label    "Enumeration" .

sdo:afterMedia  rdfs:comment  "A media object representing the circumstances after performing this direction." ;
        rdfs:label    "after media" .

sdo:branchCode  rdfs:comment  "A short textual code (also called \"store code\") that uniquely identifies a place of business. The code is typically assigned by the parentOrganization and used in structured URLs.\\n\\nFor example, in the URL http://www.starbucks.co.uk/store-locator/etc/detail/3047 the code \"3047\" is a branchCode for a particular branch.\n      " ;
        rdfs:label    "branch code" .

sdo:numberOfAirbags  rdfs:comment  "The number or type of airbags in the vehicle." ;
        rdfs:label    "number ofAirbags" .

sdo:departureStation  rdfs:comment  "The station from which the train departs." ;
        rdfs:label    "departure station" .

sdo:Brewery  rdfs:comment  "Brewery." ;
        rdfs:label    "Brewery" .

sdo:OfficeEquipmentStore
        rdfs:comment  "An office equipment store." ;
        rdfs:label    "OfficeEquipmentStore" .

sdo:hasHealthAspect  rdfs:comment  "Indicates the aspect or aspects specifically addressed in some [[HealthTopicContent]]. For example, that the content is an overview, or that it talks about treatment, self-care, treatments or their side-effects." ;
        rdfs:label    "has healthAspect" .

sdo:workload  rdfs:comment  "Quantitative measure of the physiologic output of the exercise; also referred to as energy expenditure." ;
        rdfs:label    "workload" .

sdo:relatedLink  rdfs:comment  "A link related to this web page, for example to other related web pages." ;
        rdfs:label    "related link" .

sdo:WPFooter  rdfs:comment  "The footer section of the page." ;
        rdfs:label    "WPFooter" .

sdo:NoninvasiveProcedure
        rdfs:comment  "A type of medical procedure that involves noninvasive techniques." ;
        rdfs:label    "NoninvasiveProcedure" .

sdo:requiredMinAge  rdfs:comment  "Audiences defined by a person's minimum age." ;
        rdfs:label    "required minAge" .

sdo:Bacteria  rdfs:comment  "Pathogenic bacteria that cause bacterial infection." ;
        rdfs:label    "Bacteria" .

sdo:item  rdfs:comment  "An entity represented by an entry in a list or data feed (e.g. an 'artist' in a list of 'artists')’." ;
        rdfs:label    "item" .

sdo:Downpayment  rdfs:comment  "Represents the downpayment (up-front payment) price component of the total price for an offered product that has additional installment payments." ;
        rdfs:label    "Downpayment" .

sdo:TVSeason  rdfs:comment  "Season dedicated to TV broadcast and associated online delivery." ;
        rdfs:label    "TVSeason" .

sdo:foodEstablishment
        rdfs:comment  "A sub property of location. The specific food establishment where the action occurred." ;
        rdfs:label    "food establishment" .

sdo:OwnershipInfo  rdfs:comment  "A structured value providing information about when a certain organization or person owned a certain product." ;
        rdfs:label    "OwnershipInfo" .

sdo:transmissionMethod
        rdfs:comment  "How the disease spreads, either as a route or vector, for example 'direct contact', 'Aedes aegypti', etc." ;
        rdfs:label    "transmission method" .

sdo:SuspendAction  rdfs:comment  "The act of momentarily pausing a device or application (e.g. pause music playback or pause a timer)." ;
        rdfs:label    "SuspendAction" .

sdo:FurnitureStore  rdfs:comment  "A furniture store." ;
        rdfs:label    "FurnitureStore" .

sdo:energyEfficiencyScaleMax
        rdfs:comment  "Specifies the most energy efficient class on the regulated EU energy consumption scale for the product category a product belongs to. For example, energy consumption for televisions placed on the market after January 1, 2020 is scaled from D to A+++." ;
        rdfs:label    "energy efficiencyScaleMax" .

sdo:EventScheduled  rdfs:comment  "The event is taking place or has taken place on the startDate as scheduled. Use of this value is optional, as it is assumed by default." ;
        rdfs:label    "EventScheduled" .

sdo:OpenTrial  rdfs:comment  "A trial design in which the researcher knows the full details of the treatment, and so does the patient." ;
        rdfs:label    "OpenTrial" .

sdo:editor  rdfs:comment  "Specifies the Person who edited the CreativeWork." ;
        rdfs:label    "editor" .

sdo:School  rdfs:comment  "A school." ;
        rdfs:label    "School" .

sdo:earlyPrepaymentPenalty
        rdfs:comment  "The amount to be paid as a penalty in the event of early payment of the loan." ;
        rdfs:label    "early prepaymentPenalty" .

sdo:cutoffTime  rdfs:comment  "Order cutoff time allows merchants to describe the time after which they will no longer process orders received on that day. For orders processed after cutoff time, one day gets added to the delivery time estimate. This property is expected to be most typically used via the [[ShippingRateSettings]] publication pattern. The time is indicated using the ISO-8601 Time format, e.g. \"23:30:00-05:00\" would represent 6:30 pm Eastern Standard Time (EST) which is 5 hours behind Coordinated Universal Time (UTC)." ;
        rdfs:label    "cutoff time" .

sdo:artworkSurface  rdfs:comment  "The supporting materials for the artwork, e.g. Canvas, Paper, Wood, Board, etc." ;
        rdfs:label    "artwork surface" .

sdo:ItemPage  rdfs:comment  "A page devoted to a single item, such as a particular product or hotel." ;
        rdfs:label    "ItemPage" .

sdo:CompletedActionStatus
        rdfs:comment  "An action that has already taken place." ;
        rdfs:label    "CompletedActionStatus" .

sdo:LegalForceStatus  rdfs:comment  "A list of possible statuses for the legal force of a legislation." ;
        rdfs:label    "LegalForceStatus" .

sdo:PaymentChargeSpecification
        rdfs:comment  "The costs of settling the payment using a particular payment method." ;
        rdfs:label    "PaymentChargeSpecification" .

sdo:callSign  rdfs:comment  "A [callsign](https://en.wikipedia.org/wiki/Call_sign), as used in broadcasting and radio communications to identify people, radio and TV stations, or vehicles." ;
        rdfs:label    "call sign" .

sdo:userInteractionCount
        rdfs:comment  "The number of interactions for the CreativeWork using the WebSite or SoftwareApplication." ;
        rdfs:label    "user interactionCount" .

sdo:LocalBusiness  rdfs:comment  "A particular physical business or branch of an organization. Examples of LocalBusiness include a restaurant, a particular branch of a restaurant chain, a branch of a bank, a medical practice, a club, a bowling alley, etc." ;
        rdfs:label    "LocalBusiness" .

sdo:publicAccess  rdfs:comment  "A flag to signal that the [[Place]] is open to public visitors.  If this property is omitted there is no assumed default boolean value" ;
        rdfs:label    "public access" .

sdo:priceCurrency  rdfs:comment  "The currency of the price, or a price component when attached to [[PriceSpecification]] and its subtypes.\\n\\nUse standard formats: [ISO 4217 currency format](http://en.wikipedia.org/wiki/ISO_4217) e.g. \"USD\"; [Ticker symbol](https://en.wikipedia.org/wiki/List_of_cryptocurrencies) for cryptocurrencies e.g. \"BTC\"; well known names for [Local Exchange Tradings Systems](https://en.wikipedia.org/wiki/Local_exchange_trading_system) (LETS) and other currency types e.g. \"Ithaca HOUR\"." ;
        rdfs:label    "price currency" .

sdo:OfferShippingDetails
        rdfs:comment  "OfferShippingDetails represents information about shipping destinations.\n\nMultiple of these entities can be used to represent different shipping rates for different destinations:\n\nOne entity for Alaska/Hawaii. A different one for continental US.A different one for all France.\n\nMultiple of these entities can be used to represent different shipping costs and delivery times.\n\nTwo entities that are identical but differ in rate and time:\n\ne.g. Cheaper and slower: $5 in 5-7days\nor Fast and expensive: $15 in 1-2 days." ;
        rdfs:label    "OfferShippingDetails" .

sdo:significantLinks  rdfs:comment  "The most significant URLs on the page. Typically, these are the non-navigation links that are clicked on the most." ;
        rdfs:label    "significant links" .

sdo:tocEntry  rdfs:comment  "Indicates a [[HyperTocEntry]] in a [[HyperToc]]." ;
        rdfs:label    "toc entry" .

sdo:byMonthDay  rdfs:comment  "Defines the day(s) of the month on which a recurring [[Event]] takes place. Specified as an [[Integer]] between 1-31." ;
        rdfs:label    "by monthDay" .

sdo:SalePrice  rdfs:comment  "Represents a sale price (usually active for a limited period) of an offered product." ;
        rdfs:label    "SalePrice" .

sdo:WriteAction  rdfs:comment  "The act of authoring written creative content." ;
        rdfs:label    "WriteAction" .

sdo:title  rdfs:comment  "The title of the job." ;
        rdfs:label    "title" .

sdo:bookingTime  rdfs:comment  "The date and time the reservation was booked." ;
        rdfs:label    "booking time" .

sdo:geoEquals  rdfs:comment  "Represents spatial relations in which two geometries (or the places they represent) are topologically equal, as defined in [DE-9IM](https://en.wikipedia.org/wiki/DE-9IM). \"Two geometries are topologically equal if their interiors intersect and no part of the interior or boundary of one geometry intersects the exterior of the other\" (a symmetric relationship)" ;
        rdfs:label    "geo equals" .

sdo:accessibilityAPI  rdfs:comment  "Indicates that the resource is compatible with the referenced accessibility API ([WebSchemas wiki lists possible values](http://www.w3.org/wiki/WebSchemas/Accessibility))." ;
        rdfs:label    "accessibility api" .

sdo:credentialCategory
        rdfs:comment  "The category or type of credential being described, for example \"degree”, “certificate”, “badge”, or more specific term." ;
        rdfs:label    "credential category" .

sdo:AnaerobicActivity
        rdfs:comment  "Physical activity that is of high-intensity which utilizes the anaerobic metabolism of the body." ;
        rdfs:label    "AnaerobicActivity" .

sdo:Preschool  rdfs:comment  "A preschool." ;
        rdfs:label    "Preschool" .

sdo:healthCondition  rdfs:comment  "Specifying the health condition(s) of a patient, medical study, or other target audience." ;
        rdfs:label    "health condition" .

sdo:Person  rdfs:comment  "A person (alive, dead, undead, or fictional)." ;
        rdfs:label    "Person" .

sdo:BedType  rdfs:comment  "A type of bed. This is used for indicating the bed or beds available in an accommodation." ;
        rdfs:label    "BedType" .

sdo:containedIn  rdfs:comment  "The basic containment relation between a place and one that contains it." ;
        rdfs:label    "contained in" .

sdo:ArtGallery  rdfs:comment  "An art gallery." ;
        rdfs:label    "ArtGallery" .

sdo:CatholicChurch  rdfs:comment  "A Catholic church." ;
        rdfs:label    "CatholicChurch" .

sdo:structuralClass  rdfs:comment  "The name given to how bone physically connects to each other." ;
        rdfs:label    "structural class" .

sdo:editEIDR  rdfs:comment  "An [EIDR](https://eidr.org/) (Entertainment Identifier Registry) [[identifier]] representing a specific edit / edition for a work of film or television.\n\nFor example, the motion picture known as \"Ghostbusters\" whose [[titleEIDR]] is \"10.5240/7EC7-228A-510A-053E-CBB8-J\", has several edits e.g. \"10.5240/1F2A-E1C5-680A-14C6-E76B-I\" and \"10.5240/8A35-3BEE-6497-5D12-9E4F-3\".\n\nSince schema.org types like [[Movie]] and [[TVEpisode]] can be used for both works and their multiple expressions, it is possible to use [[titleEIDR]] alone (for a general description), or alongside [[editEIDR]] for a more edit-specific description.\n" ;
        rdfs:label    "edit eidr" .

sdo:branchOf  rdfs:comment  "The larger organization that this local business is a branch of, if any. Not to be confused with (anatomical)[[branch]]." ;
        rdfs:label    "branch of" .

sdo:shippingDetails  rdfs:comment  "Indicates information about the shipping policies and options associated with an [[Offer]]." ;
        rdfs:label    "shipping details" .

sdo:SizeSpecification
        rdfs:comment  "Size related properties of a product, typically a size code ([[name]]) and optionally a [[sizeSystem]], [[sizeGroup]], and product measurements ([[hasMeasurement]]). In addition, the intended audience can be defined through [[suggestedAge]], [[suggestedGender]], and suggested body measurements ([[suggestedMeasurement]])." ;
        rdfs:label    "SizeSpecification" .

sdo:recordLabel  rdfs:comment  "The label that issued the release." ;
        rdfs:label    "record label" .

sdo:healthPlanCopayOption
        rdfs:comment  "Whether the copay is before or after deductible, etc." ;
        rdfs:label    "health planCopayOption" .

sdo:PublicSwimmingPool
        rdfs:comment  "A public swimming pool." ;
        rdfs:label    "PublicSwimmingPool" .

sdo:potentialAction  rdfs:comment  "Indicates a potential Action, which describes an idealized action in which this thing would play an 'object' role." ;
        rdfs:label    "potential action" .

sdo:expires  rdfs:comment  "Date the content expires and is no longer useful or available. For example a [[VideoObject]] or [[NewsArticle]] whose availability or relevance is time-limited, or a [[ClaimReview]] fact check whose publisher wants to indicate that it may no longer be relevant (or helpful to highlight) after some date." ;
        rdfs:label    "expires" .

sdo:timeOfDay  rdfs:comment  "The time of day the program normally runs. For example, \"evenings\"." ;
        rdfs:label    "time ofDay" .

sdo:Guide  rdfs:comment  "[[Guide]] is a page or article that recommend specific products or services, or aspects of a thing for a user to consider. A [[Guide]] may represent a Buying Guide and detail aspects of products or services for a user to consider. A [[Guide]] may represent a Product Guide and recommend specific products or services. A [[Guide]] may represent a Ranked List and recommend specific products or services with ranking." ;
        rdfs:label    "Guide" .

sdo:PaymentAutomaticallyApplied
        rdfs:comment  "An automatic payment system is in place and will be used." ;
        rdfs:label    "PaymentAutomaticallyApplied" .

sdo:Nonprofit501c11  rdfs:comment  "Nonprofit501c11: Non-profit type referring to Teachers' Retirement Fund Associations." ;
        rdfs:label    "Nonprofit501c11" .

sdo:datePublished  rdfs:comment  "Date of first broadcast/publication." ;
        rdfs:label    "date published" .

sdo:availabilityEnds  rdfs:comment  "The end of the availability of the product or service included in the offer." ;
        rdfs:label    "availability ends" .

sdo:cookingMethod  rdfs:comment  "The method of cooking, such as Frying, Steaming, ..." ;
        rdfs:label    "cooking method" .

sdo:GettingAccessHealthAspect
        rdfs:comment  "Content that discusses practical and policy aspects for getting access to specific kinds of healthcare (e.g. distribution mechanisms for vaccines)." ;
        rdfs:label    "GettingAccessHealthAspect" .

sdo:Conversation  rdfs:comment  "One or more messages between organizations or people on a particular topic. Individual messages can be linked to the conversation with isPartOf or hasPart properties." ;
        rdfs:label    "Conversation" .

sdo:RisksOrComplicationsHealthAspect
        rdfs:comment  "Information about the risk factors and possible complications that may follow a topic." ;
        rdfs:label    "RisksOrComplicationsHealthAspect" .

sdo:paymentUrl  rdfs:comment  "The URL for sending a payment." ;
        rdfs:label    "payment url" .

sdo:torque  rdfs:comment  "The torque (turning force) of the vehicle's engine.\\n\\nTypical unit code(s): NU for newton metre (N m), F17 for pound-force per foot, or F48 for pound-force per inch\\n\\n* Note 1: You can link to information about how the given value has been determined (e.g. reference RPM) using the [[valueReference]] property.\\n* Note 2: You can use [[minValue]] and [[maxValue]] to indicate ranges." ;
        rdfs:label    "torque" .

sdo:Barcode  rdfs:comment  "An image of a visual machine-readable code such as a barcode or QR code." ;
        rdfs:label    "Barcode" .

sdo:TaxiStand  rdfs:comment  "A taxi stand." ;
        rdfs:label    "TaxiStand" .

sdo:jurisdiction  rdfs:comment  "Indicates a legal jurisdiction, e.g. of some legislation, or where some government service is based." ;
        rdfs:label    "jurisdiction" .

sdo:VideoGallery  rdfs:comment  "Web page type: Video gallery page." ;
        rdfs:label    "VideoGallery" .

sdo:memberOf  rdfs:comment  "An Organization (or ProgramMembership) to which this Person or Organization belongs." ;
        rdfs:label    "member of" .

sdo:targetCollection  rdfs:comment  "A sub property of object. The collection target of the action." ;
        rdfs:label    "target collection" .

sdo:EUEnergyEfficiencyCategoryA1Plus
        rdfs:comment  "Represents EU Energy Efficiency Class A+ as defined in EU energy labeling regulations." ;
        rdfs:label    "EUEnergyEfficiencyCategoryA1Plus" .

sdo:inStoreReturnsOffered
        rdfs:comment  "Are in-store returns offered? (for more advanced return methods use the [[returnMethod]] property)" ;
        rdfs:label    "in storeReturnsOffered" .

sdo:Saturday  rdfs:comment  "The day of the week between Friday and Sunday." ;
        rdfs:label    "Saturday" .

sdo:subTest  rdfs:comment  "A component test of the panel." ;
        rdfs:label    "sub test" .

sdo:RadioSeries  rdfs:comment  "CreativeWorkSeries dedicated to radio broadcast and associated online delivery." ;
        rdfs:label    "RadioSeries" .

sdo:DrugCostCategory  rdfs:comment  "Enumerated categories of medical drug costs." ;
        rdfs:label    "DrugCostCategory" .

sdo:downvoteCount  rdfs:comment  "The number of downvotes this question, answer or comment has received from the community." ;
        rdfs:label    "downvote count" .

sdo:MedicalRiskScore  rdfs:comment  "A simple system that adds up the number of risk factors to yield a score that is associated with prognosis, e.g. CHAD score, TIMI risk score." ;
        rdfs:label    "MedicalRiskScore" .

sdo:suitableForDiet  rdfs:comment  "Indicates a dietary restriction or guideline for which this recipe or menu item is suitable, e.g. diabetic, halal etc." ;
        rdfs:label    "suitable forDiet" .

sdo:SubscribeAction  rdfs:comment  "The act of forming a personal connection with someone/something (object) unidirectionally/asymmetrically to get updates pushed to.\\n\\nRelated actions:\\n\\n* [[FollowAction]]: Unlike FollowAction, SubscribeAction implies that the subscriber acts as a passive agent being constantly/actively pushed for updates.\\n* [[RegisterAction]]: Unlike RegisterAction, SubscribeAction implies that the agent is interested in continuing receiving updates from the object.\\n* [[JoinAction]]: Unlike JoinAction, SubscribeAction implies that the agent is interested in continuing receiving updates from the object." ;
        rdfs:label    "SubscribeAction" .

sdo:PET  rdfs:comment  "Positron emission tomography imaging." ;
        rdfs:label    "PET" .

sdo:transitTime  rdfs:comment  "The typical delay the order has been sent for delivery and the goods reach the final customer. Typical properties: minValue, maxValue, unitCode (d for DAY)." ;
        rdfs:label    "transit time" .

sdo:ticketToken  rdfs:comment  "Reference to an asset (e.g., Barcode, QR code image or PDF) usable for entrance." ;
        rdfs:label    "ticket token" .

sdo:application  rdfs:comment  "An application that can complete the request." ;
        rdfs:label    "application" .

sdo:ComicSeries  rdfs:comment  "A sequential publication of comic stories under a\n    \tunifying title, for example \"The Amazing Spider-Man\" or \"Groo the\n    \tWanderer\"." ;
        rdfs:label    "ComicSeries" .

sdo:RVPark  rdfs:comment  "A place offering space for \"Recreational Vehicles\", Caravans, mobile homes and the like." ;
        rdfs:label    "RVPark" .

sdo:servingSize  rdfs:comment  "The serving size, in terms of the number of volume or mass." ;
        rdfs:label    "serving size" .

sdo:confirmationNumber
        rdfs:comment  "A number that confirms the given order or payment has been received." ;
        rdfs:label    "confirmation number" .

sdo:BackgroundNewsArticle
        rdfs:comment  "A [[NewsArticle]] providing historical context, definition and detail on a specific topic (aka \"explainer\" or \"backgrounder\"). For example, an in-depth article or frequently-asked-questions ([FAQ](https://en.wikipedia.org/wiki/FAQ)) document on topics such as Climate Change or the European Union. Other kinds of background material from a non-news setting are often described using [[Book]] or [[Article]], in particular [[ScholarlyArticle]]. See also [[NewsArticle]] for related vocabulary from a learning/education perspective." ;
        rdfs:label    "BackgroundNewsArticle" .

sdo:merchantReturnLink
        rdfs:comment  "Specifies a Web page or service by URL, for product returns." ;
        rdfs:label    "merchant returnLink" .

sdo:DietNutrition  rdfs:comment  "Dietetic and nutrition as a medical specialty." ;
        rdfs:label    "DietNutrition" .

sdo:WPSideBar  rdfs:comment  "A sidebar section of the page." ;
        rdfs:label    "WPSideBar" .

sdo:ResearchProject  rdfs:comment  "A Research project." ;
        rdfs:label    "ResearchProject" .

sdo:tissueSample  rdfs:comment  "The type of tissue sample required for the test." ;
        rdfs:label    "tissue sample" .

sdo:recognizingAuthority
        rdfs:comment  "If applicable, the organization that officially recognizes this entity as part of its endorsed system of medicine." ;
        rdfs:label    "recognizing authority" .

sdo:GovernmentBenefitsType
        rdfs:comment  "GovernmentBenefitsType enumerates several kinds of government benefits to support the COVID-19 situation. Note that this structure may not capture all benefits offered." ;
        rdfs:label    "GovernmentBenefitsType" .

sdo:WearableSizeSystemUK
        rdfs:comment  "United Kingdom size system for wearables." ;
        rdfs:label    "WearableSizeSystemUK" .

sdo:EmploymentAgency  rdfs:comment  "An employment agency." ;
        rdfs:label    "EmploymentAgency" .

sdo:TattooParlor  rdfs:comment  "A tattoo parlor." ;
        rdfs:label    "TattooParlor" .

sdo:contentSize  rdfs:comment  "File size in (mega/kilo) bytes." ;
        rdfs:label    "content size" .

sdo:Eye  rdfs:comment  "Eye or ophtalmological function assessment with clinical examination." ;
        rdfs:label    "Eye" .

sdo:isInvolvedInBiologicalProcess
        rdfs:comment  "Biological process this BioChemEntity is involved in; please use PropertyValue if you want to include any evidence." ;
        rdfs:label    "is involvedInBiologicalProcess" .

sdo:manufacturer  rdfs:comment  "The manufacturer of the product." ;
        rdfs:label    "manufacturer" .

sdo:Language  rdfs:comment  "Natural languages such as Spanish, Tamil, Hindi, English, etc. Formal language code tags expressed in [BCP 47](https://en.wikipedia.org/wiki/IETF_language_tag) can be used via the [[alternateName]] property. The Language type previously also covered programming languages such as Scheme and Lisp, which are now best represented using [[ComputerLanguage]]." ;
        rdfs:label    "Language" .

sdo:PublicationVolume
        rdfs:comment  "A part of a successively published publication such as a periodical or multi-volume work, often numbered. It may represent a time span, such as a year.\\n\\nSee also [blog post](http://blog.schema.org/2014/09/schemaorg-support-for-bibliographic_2.html)." ;
        rdfs:label    "PublicationVolume" .

sdo:UnincorporatedAssociationCharity
        rdfs:comment  "UnincorporatedAssociationCharity: Non-profit type referring to a charitable company that is not incorporated (UK)." ;
        rdfs:label    "UnincorporatedAssociationCharity" .

sdo:workExample  rdfs:comment  "Example/instance/realization/derivation of the concept of this creative work. eg. The paperback edition, first edition, or eBook." ;
        rdfs:label    "work example" .

sdo:strengthValue  rdfs:comment  "The value of an active ingredient's strength, e.g. 325." ;
        rdfs:label    "strength value" .

sdo:BrokerageAccount  rdfs:comment  "An account that allows an investor to deposit funds and place investment orders with a licensed broker or brokerage firm." ;
        rdfs:label    "BrokerageAccount" .

sdo:eligibleCustomerType
        rdfs:comment  "The type(s) of customers for which the given offer is valid." ;
        rdfs:label    "eligible customerType" .

sdo:BuddhistTemple  rdfs:comment  "A Buddhist temple." ;
        rdfs:label    "BuddhistTemple" .

sdo:BuyAction  rdfs:comment  "The act of giving money to a seller in exchange for goods or services rendered. An agent buys an object, product, or service from a seller for a price. Reciprocal of SellAction." ;
        rdfs:label    "BuyAction" .

sdo:drugUnit  rdfs:comment  "The unit in which the drug is measured, e.g. '5 mg tablet'." ;
        rdfs:label    "drug unit" .

sdo:activityFrequency
        rdfs:comment  "How often one should engage in the activity." ;
        rdfs:label    "activity frequency" .

sdo:knowsAbout  rdfs:comment  "Of a [[Person]], and less typically of an [[Organization]], to indicate a topic that is known about - suggesting possible expertise but not implying it. We do not distinguish skill levels here, or relate this to educational content, events, objectives or [[JobPosting]] descriptions." ;
        rdfs:label    "knows about" .

sdo:healthPlanCopay  rdfs:comment  "Whether The copay amount." ;
        rdfs:label    "health planCopay" .

sdo:subStageSuffix  rdfs:comment  "The substage, e.g. 'a' for Stage IIIa." ;
        rdfs:label    "sub stageSuffix" .

sdo:elevation  rdfs:comment  "The elevation of a location ([WGS 84](https://en.wikipedia.org/wiki/World_Geodetic_System)). Values may be of the form 'NUMBER UNIT_OF_MEASUREMENT' (e.g., '1,000 m', '3,200 ft') while numbers alone should be assumed to be a value in meters." ;
        rdfs:label    "elevation" .

sdo:NewCondition  rdfs:comment  "Indicates that the item is new." ;
        rdfs:label    "NewCondition" .

sdo:accessibilitySummary
        rdfs:comment  "A human-readable summary of specific accessibility features or deficiencies, consistent with the other accessibility metadata but expressing subtleties such as \"short descriptions are present but long descriptions will be needed for non-visual users\" or \"short descriptions are present and no long descriptions are needed.\"" ;
        rdfs:label    "accessibility summary" .

sdo:colorist  rdfs:comment  "The individual who adds color to inked drawings." ;
        rdfs:label    "colorist" .

sdo:PotentialActionStatus
        rdfs:comment  "A description of an action that is supported." ;
        rdfs:label    "PotentialActionStatus" .

sdo:pageEnd  rdfs:comment  "The page on which the work ends; for example \"138\" or \"xvi\"." ;
        rdfs:label    "page end" .

sdo:PaymentDue  rdfs:comment  "The payment is due, but still within an acceptable time to be received." ;
        rdfs:label    "PaymentDue" .

sdo:parentItem  rdfs:comment  "The parent of a question, answer or item in general." ;
        rdfs:label    "parent item" .

sdo:inSupportOf  rdfs:comment  "Qualification, candidature, degree, application that Thesis supports." ;
        rdfs:label    "in supportOf" .

sdo:ClothingStore  rdfs:comment  "A clothing store." ;
        rdfs:label    "ClothingStore" .

sdo:Emergency  rdfs:comment  "A specific branch of medical science that deals with the evaluation and initial treatment of medical conditions caused by trauma or sudden illness." ;
        rdfs:label    "Emergency" .

sdo:originalMediaLink
        rdfs:comment  "Link to the page containing an original version of the content, or directly to an online copy of the original [[MediaObject]] content, e.g. video file." ;
        rdfs:label    "original mediaLink" .

sdo:WearableSizeSystemUS
        rdfs:comment  "United States size system for wearables." ;
        rdfs:label    "WearableSizeSystemUS" .

sdo:MusicEvent  rdfs:comment  "Event type: Music event." ;
        rdfs:label    "MusicEvent" .

sdo:usedToDiagnose  rdfs:comment  "A condition the test is used to diagnose." ;
        rdfs:label    "used toDiagnose" .

sdo:Nonprofit501c8  rdfs:comment  "Nonprofit501c8: Non-profit type referring to Fraternal Beneficiary Societies and Associations." ;
        rdfs:label    "Nonprofit501c8" .

sdo:PlaceOfWorship  rdfs:comment  "Place of worship, such as a church, synagogue, or mosque." ;
        rdfs:label    "PlaceOfWorship" .

sdo:loanPaymentFrequency
        rdfs:comment  "Frequency of payments due, i.e. number of months between payments. This is defined as a frequency, i.e. the reciprocal of a period of time." ;
        rdfs:label    "loan paymentFrequency" .

sdo:labelDetails  rdfs:comment  "Link to the drug's label details." ;
        rdfs:label    "label details" .

sdo:mathExpression  rdfs:comment  "A mathematical expression (e.g. 'x^2-3x=0') that may be solved for a specific variable, simplified, or transformed. This can take many formats, e.g. LaTeX, Ascii-Math, or math as you would write with a keyboard." ;
        rdfs:label    "math expression" .

sdo:publicTransportClosuresInfo
        rdfs:comment  "Information about public transport closures." ;
        rdfs:label    "public transportClosuresInfo" .

sdo:inDefinedTermSet  rdfs:comment  "A [[DefinedTermSet]] that contains this term." ;
        rdfs:label    "in definedTermSet" .

sdo:geoCovers  rdfs:comment  "Represents a relationship between two geometries (or the places they represent), relating a covering geometry to a covered geometry. \"Every point of b is a point of (the interior or boundary of) a\". As defined in [DE-9IM](https://en.wikipedia.org/wiki/DE-9IM)." ;
        rdfs:label    "geo covers" .

sdo:fiberContent  rdfs:comment  "The number of grams of fiber." ;
        rdfs:label    "fiber content" .

sdo:URL  rdfs:comment  "Data type: URL." ;
        rdfs:label    "URL" .

sdo:Statement  rdfs:comment  "A statement about something, for example a fun or interesting fact. If known, the main entity this statement is about, can be indicated using mainEntity. For more formal claims (e.g. in Fact Checking), consider using [[Claim]] instead. Use the [[text]] property to capture the text of the statement." ;
        rdfs:label    "Statement" .

sdo:HardwareStore  rdfs:comment  "A hardware store." ;
        rdfs:label    "HardwareStore" .

sdo:holdingArchive  rdfs:comment  "[[ArchiveOrganization]] that holds, keeps or maintains the [[ArchiveComponent]]."@en ;
        rdfs:label    "holding archive"@en .

sdo:includedInDataCatalog
        rdfs:comment  "A data catalog which contains this dataset." ;
        rdfs:label    "included inDataCatalog" .

sdo:announcementLocation
        rdfs:comment  "Indicates a specific [[CivicStructure]] or [[LocalBusiness]] associated with the SpecialAnnouncement. For example, a specific testing facility or business with special opening hours. For a larger geographic region like a quarantine of an entire region, use [[spatialCoverage]]." ;
        rdfs:label    "announcement location" .

sdo:DataFeedItem  rdfs:comment  "A single item within a larger data feed." ;
        rdfs:label    "DataFeedItem" .

sdo:studySubject  rdfs:comment  "A subject of the study, i.e. one of the medical conditions, therapies, devices, drugs, etc. investigated by the study." ;
        rdfs:label    "study subject" .

sdo:FlightReservation
        rdfs:comment  "A reservation for air travel.\\n\\nNote: This type is for information about actual reservations, e.g. in confirmation emails or HTML pages with individual confirmations of reservations. For offers of tickets, use [[Offer]]." ;
        rdfs:label    "FlightReservation" .

sdo:cvdNumICUBeds  rdfs:comment  "numicubeds - ICU BEDS: Total number of staffed inpatient intensive care unit (ICU) beds." ;
        rdfs:label    "cvd numICUBeds" .

sdo:UKNonprofitType  rdfs:comment  "UKNonprofitType: Non-profit organization type originating from the United Kingdom." ;
        rdfs:label    "UKNonprofitType" .

sdo:CreateAction  rdfs:comment  "The act of deliberately creating/producing/generating/building a result out of the agent." ;
        rdfs:label    "CreateAction" .

sdo:SportsActivityLocation
        rdfs:comment  "A sports location, such as a playing field." ;
        rdfs:label    "SportsActivityLocation" .

sdo:review  rdfs:comment  "A review of the item." ;
        rdfs:label    "review" .

sdo:NonprofitANBI  rdfs:comment  "NonprofitANBI: Non-profit type referring to a Public Benefit Organization (NL)." ;
        rdfs:label    "NonprofitANBI" .

sdo:Hospital  rdfs:comment  "A hospital." ;
        rdfs:label    "Hospital" .

sdo:predecessorOf  rdfs:comment  "A pointer from a previous, often discontinued variant of the product to its newer variant." ;
        rdfs:label    "predecessor of" .

sdo:HotelRoom  rdfs:comment  "A hotel room is a single room in a hotel.\n<br /><br />\nSee also the <a href=\"/docs/hotels.html\">dedicated document on the use of schema.org for marking up hotels and other forms of accommodations</a>.\n" ;
        rdfs:label    "HotelRoom" .

sdo:ApartmentComplex  rdfs:comment  "Residence type: Apartment complex." ;
        rdfs:label    "ApartmentComplex" .

sdo:CoverArt  rdfs:comment  "The artwork on the outer surface of a CreativeWork." ;
        rdfs:label    "CoverArt" .

sdo:valueMinLength  rdfs:comment  "Specifies the minimum allowed range for number of characters in a literal value." ;
        rdfs:label    "value minLength" .

sdo:phoneticText  rdfs:comment  "Representation of a text [[textValue]] using the specified [[speechToTextMarkup]]. For example the city name of Houston in IPA: /ˈhjuːstən/." ;
        rdfs:label    "phonetic text" .

sdo:datePosted  rdfs:comment  "Publication date of an online listing." ;
        rdfs:label    "date posted" .

sdo:costPerUnit  rdfs:comment  "The cost per unit of the drug." ;
        rdfs:label    "cost perUnit" .

sdo:ImageObject  rdfs:comment  "An image file." ;
        rdfs:label    "ImageObject" .

sdo:targetName  rdfs:comment  "The name of a node in an established educational framework." ;
        rdfs:label    "target name" .

sdo:dateSent  rdfs:comment  "The date/time at which the message was sent." ;
        rdfs:label    "date sent" .

sdo:occupancy  rdfs:comment  "The allowed total occupancy for the accommodation in persons (including infants etc). For individual accommodations, this is not necessarily the legal maximum but defines the permitted usage as per the contractual agreement (e.g. a double room used by a single person).\nTypical unit code(s): C62 for person" ;
        rdfs:label    "occupancy" .

sdo:Therapeutic  rdfs:comment  "A medical device used for therapeutic purposes." ;
        rdfs:label    "Therapeutic" .

sdo:error  rdfs:comment  "For failed actions, more information on the cause of the failure." ;
        rdfs:label    "error" .

sdo:dateReceived  rdfs:comment  "The date/time the message was received if a single recipient exists." ;
        rdfs:label    "date received" .

sdo:DVDFormat  rdfs:comment  "DVDFormat." ;
        rdfs:label    "DVDFormat" .

sdo:thumbnail  rdfs:comment  "Thumbnail image for an image or video." ;
        rdfs:label    "thumbnail" .

sdo:stage  rdfs:comment  "The stage of the condition, if applicable." ;
        rdfs:label    "stage" .

sdo:validFor  rdfs:comment  "The duration of validity of a permit or similar thing." ;
        rdfs:label    "valid for" .

sdo:modifiedTime  rdfs:comment  "The date and time the reservation was modified." ;
        rdfs:label    "modified time" .

sdo:HowToSupply  rdfs:comment  "A supply consumed when performing the instructions for how to achieve a result." ;
        rdfs:label    "HowToSupply" .

sdo:DistanceFee  rdfs:comment  "Represents the distance fee (e.g., price per km or mile) part of the total price for an offered product, for example a car rental." ;
        rdfs:label    "DistanceFee" .

sdo:awayTeam  rdfs:comment  "The away team in a sports event." ;
        rdfs:label    "away team" .

sdo:tickerSymbol  rdfs:comment  "The exchange traded instrument associated with a Corporation object. The tickerSymbol is expressed as an exchange and an instrument name separated by a space character. For the exchange component of the tickerSymbol attribute, we recommend using the controlled vocabulary of Market Identifier Codes (MIC) specified in ISO15022." ;
        rdfs:label    "ticker symbol" .

sdo:InteractionCounter
        rdfs:comment  "A summary of how users have interacted with this CreativeWork. In most cases, authors will use a subtype to specify the specific type of interaction." ;
        rdfs:label    "InteractionCounter" .

sdo:trailer  rdfs:comment  "The trailer of a movie or tv/radio series, season, episode, etc." ;
        rdfs:label    "trailer" .

sdo:course  rdfs:comment  "A sub property of location. The course where this action was taken." ;
        rdfs:label    "course" .

sdo:ResumeAction  rdfs:comment  "The act of resuming a device or application which was formerly paused (e.g. resume music playback or resume a timer)." ;
        rdfs:label    "ResumeAction" .

sdo:VirtualLocation  rdfs:comment  "An online or virtual location for attending events. For example, one may attend an online seminar or educational event. While a virtual location may be used as the location of an event, virtual locations should not be confused with physical locations in the real world." ;
        rdfs:label    "VirtualLocation" .

sdo:sender  rdfs:comment  "A sub property of participant. The participant who is at the sending end of the action." ;
        rdfs:label    "sender" .

sdo:Corporation  rdfs:comment  "Organization: A business corporation." ;
        rdfs:label    "Corporation" .

sdo:mentions  rdfs:comment  "Indicates that the CreativeWork contains a reference to, but is not necessarily about a concept." ;
        rdfs:label    "mentions" .

sdo:mediaAuthenticityCategory
        rdfs:comment  "Indicates a MediaManipulationRatingEnumeration classification of a media object (in the context of how it was published or shared)." ;
        rdfs:label    "media authenticityCategory" .

sdo:DeliveryTimeSettings
        rdfs:comment  "A DeliveryTimeSettings represents re-usable pieces of shipping information, relating to timing. It is designed for publication on an URL that may be referenced via the [[shippingSettingsLink]] property of a [[OfferShippingDetails]]. Several occurrences can be published, distinguished (and identified/referenced) by their different values for [[transitTimeLabel]]." ;
        rdfs:label    "DeliveryTimeSettings" .

sdo:textValue  rdfs:comment  "Text value being annotated." ;
        rdfs:label    "text value" .

sdo:CheckOutAction  rdfs:comment  "The act of an agent communicating (service provider, social media, etc) their departure of a previously reserved service (e.g. flight check in) or place (e.g. hotel).\\n\\nRelated actions:\\n\\n* [[CheckInAction]]: The antonym of CheckOutAction.\\n* [[DepartAction]]: Unlike DepartAction, CheckOutAction implies that the agent is informing/confirming the end of a previously reserved service.\\n* [[CancelAction]]: Unlike CancelAction, CheckOutAction implies that the agent is informing/confirming the end of a previously reserved service." ;
        rdfs:label    "CheckOutAction" .

sdo:OnSitePickup  rdfs:comment  "A DeliveryMethod in which an item is collected on site, e.g. in a store or at a box office." ;
        rdfs:label    "OnSitePickup" .

sdo:PrescriptionOnly  rdfs:comment  "Available by prescription only." ;
        rdfs:label    "PrescriptionOnly" .

sdo:MedicalTestPanel  rdfs:comment  "Any collection of tests commonly ordered together." ;
        rdfs:label    "MedicalTestPanel" .

sdo:FollowAction  rdfs:comment  "The act of forming a personal connection with someone/something (object) unidirectionally/asymmetrically to get updates polled from.\\n\\nRelated actions:\\n\\n* [[BefriendAction]]: Unlike BefriendAction, FollowAction implies that the connection is *not* necessarily reciprocal.\\n* [[SubscribeAction]]: Unlike SubscribeAction, FollowAction implies that the follower acts as an active agent constantly/actively polling for updates.\\n* [[RegisterAction]]: Unlike RegisterAction, FollowAction implies that the agent is interested in continuing receiving updates from the object.\\n* [[JoinAction]]: Unlike JoinAction, FollowAction implies that the agent is interested in getting updates from the object.\\n* [[TrackAction]]: Unlike TrackAction, FollowAction refers to the polling of updates of all aspects of animate objects rather than the location of inanimate objects (e.g. you track a package, but you don't follow it)." ;
        rdfs:label    "FollowAction" .

sdo:SkiResort  rdfs:comment  "A ski resort." ;
        rdfs:label    "SkiResort" .

sdo:AnatomicalStructure
        rdfs:comment  "Any part of the human body, typically a component of an anatomical system. Organs, tissues, and cells are all anatomical structures." ;
        rdfs:label    "AnatomicalStructure" .

sdo:CategoryCodeSet  rdfs:comment  "A set of Category Code values." ;
        rdfs:label    "CategoryCodeSet" .

sdo:operatingSystem  rdfs:comment  "Operating systems supported (Windows 7, OSX 10.6, Android 1.6)." ;
        rdfs:label    "operating system" .

sdo:includesObject  rdfs:comment  "This links to a node or nodes indicating the exact quantity of the products included in  an [[Offer]] or [[ProductCollection]]." ;
        rdfs:label    "includes object" .

sdo:valueRequired  rdfs:comment  "Whether the property must be filled in to complete the action.  Default is false." ;
        rdfs:label    "value required" .

sdo:differentialDiagnosis
        rdfs:comment  "One of a set of differential diagnoses for the condition. Specifically, a closely-related or competing diagnosis typically considered later in the cognitive process whereby this medical condition is distinguished from others most likely responsible for a similar collection of signs and symptoms to reach the most parsimonious diagnosis or diagnoses in a patient." ;
        rdfs:label    "differential diagnosis" .

sdo:Episode  rdfs:comment  "A media episode (e.g. TV, radio, video game) which can be part of a series or season." ;
        rdfs:label    "Episode" .

sdo:valueName  rdfs:comment  "Indicates the name of the PropertyValueSpecification to be used in URL templates and form encoding in a manner analogous to HTML's input@name." ;
        rdfs:label    "value name" .

sdo:productionCompany
        rdfs:comment  "The production company or studio responsible for the item e.g. series, video game, episode etc." ;
        rdfs:label    "production company" .

sdo:Genetic  rdfs:comment  "A specific branch of medical science that pertains to hereditary transmission and the variation of inherited characteristics and disorders." ;
        rdfs:label    "Genetic" .

sdo:NotInForce  rdfs:comment  "Indicates that a legislation is currently not in force." ;
        rdfs:label    "NotInForce" .

sdo:returnShippingFeesAmount
        rdfs:comment  "Amount of shipping costs for product returns (for any reason). Applicable when property [[returnFees]] equals [[ReturnShippingFees]]." ;
        rdfs:label    "return shippingFeesAmount" .

sdo:acquireLicensePage
        rdfs:comment  "Indicates a page documenting how licenses can be purchased or otherwise acquired, for the current item." ;
        rdfs:label    "acquire licensePage" .

sdo:permitAudience  rdfs:comment  "The target audience for this permit." ;
        rdfs:label    "permit audience" .

sdo:translator  rdfs:comment  "Organization or person who adapts a creative work to different languages, regional differences and technical requirements of a target market, or that translates during some event." ;
        rdfs:label    "translator" .

sdo:PrimaryCare  rdfs:comment  "The medical care by a physician, or other health-care professional, who is the patient's first contact with the health-care system and who may recommend a specialist if necessary." ;
        rdfs:label    "PrimaryCare" .

sdo:specialCommitments
        rdfs:comment  "Any special commitments associated with this job posting. Valid entries include VeteranCommit, MilitarySpouseCommit, etc." ;
        rdfs:label    "special commitments" .

sdo:numberOfPartialBathrooms
        rdfs:comment  "Number of partial bathrooms - The total number of half and ¼ bathrooms in an [[Accommodation]]. This corresponds to the [BathroomsPartial field in RESO](https://ddwiki.reso.org/display/DDW17/BathroomsPartial+Field). " ;
        rdfs:label    "number ofPartialBathrooms" .

sdo:Report  rdfs:comment  "A Report generated by governmental or non-governmental organization." ;
        rdfs:label    "Report" .

sdo:itemLocation  rdfs:comment  "Current location of the item."@en ;
        rdfs:label    "item location"@en .

sdo:guidelineDate  rdfs:comment  "Date on which this guideline's recommendation was made." ;
        rdfs:label    "guideline date" .

sdo:ReservationHold  rdfs:comment  "The status of a reservation on hold pending an update like credit card number or flight changes." ;
        rdfs:label    "ReservationHold" .

sdo:knownVehicleDamages
        rdfs:comment  "A textual description of known damages, both repaired and unrepaired." ;
        rdfs:label    "known vehicleDamages" .

sdo:StatisticalPopulation
        rdfs:comment  "A StatisticalPopulation is a set of instances of a certain given type that satisfy some set of constraints. The property [[populationType]] is used to specify the type. Any property that can be used on instances of that type can appear on the statistical population. For example, a [[StatisticalPopulation]] representing all [[Person]]s with a [[homeLocation]] of East Podunk California, would be described by applying the appropriate [[homeLocation]] and [[populationType]] properties to a [[StatisticalPopulation]] item that stands for that set of people.\nThe properties [[numConstraints]] and [[constrainingProperty]] are used to specify which of the populations properties are used to specify the population. Note that the sense of \"population\" used here is the general sense of a statistical\npopulation, and does not imply that the population consists of people. For example, a [[populationType]] of [[Event]] or [[NewsArticle]] could be used. See also [[Observation]], and the [data and datasets](/docs/data-and-datasets.html) overview for more details.\n  " ;
        rdfs:label    "StatisticalPopulation" .

sdo:returnPolicySeasonalOverride
        rdfs:comment  "Seasonal override of a return policy." ;
        rdfs:label    "return policySeasonalOverride" .

sdo:Bone  rdfs:comment  "Rigid connective tissue that comprises up the skeletal structure of the human body." ;
        rdfs:label    "Bone" .

sdo:CommentAction  rdfs:comment  "The act of generating a comment about a subject." ;
        rdfs:label    "CommentAction" .

sdo:CriticReview  rdfs:comment  "A [[CriticReview]] is a more specialized form of Review written or published by a source that is recognized for its reviewing activities. These can include online columns, travel and food guides, TV and radio shows, blogs and other independent Web sites. [[CriticReview]]s are typically more in-depth and professionally written. For simpler, casually written user/visitor/viewer/customer reviews, it is more appropriate to use the [[UserReview]] type. Review aggregator sites such as Metacritic already separate out the site's user reviews from selected critic reviews that originate from third-party sources." ;
        rdfs:label    "CriticReview" .

sdo:uploadDate  rdfs:comment  "Date when this media object was uploaded to this site." ;
        rdfs:label    "upload date" .

sdo:VideoGameClip  rdfs:comment  "A short segment/part of a video game." ;
        rdfs:label    "VideoGameClip" .

sdo:GasStation  rdfs:comment  "A gas station." ;
        rdfs:label    "GasStation" .

sdo:WatchAction  rdfs:comment  "The act of consuming dynamic/moving visual content." ;
        rdfs:label    "WatchAction" .

sdo:UserCheckins  rdfs:comment  "UserInteraction and its subtypes is an old way of talking about users interacting with pages. It is generally better to use [[Action]]-based vocabulary, alongside types such as [[Comment]]." ;
        rdfs:label    "UserCheckins" .

sdo:foundingDate  rdfs:comment  "The date that this organization was founded." ;
        rdfs:label    "founding date" .

sdo:dateRead  rdfs:comment  "The date/time at which the message has been read by the recipient if a single recipient exists." ;
        rdfs:label    "date read" .

sdo:collection  rdfs:comment  "A sub property of object. The collection target of the action." ;
        rdfs:label    "collection" .

sdo:NLNonprofitType  rdfs:comment  "NLNonprofitType: Non-profit organization type originating from the Netherlands." ;
        rdfs:label    "NLNonprofitType" .

sdo:TheaterGroup  rdfs:comment  "A theater group or company, for example, the Royal Shakespeare Company or Druid Theatre." ;
        rdfs:label    "TheaterGroup" .

sdo:SelfStorage  rdfs:comment  "A self-storage facility." ;
        rdfs:label    "SelfStorage" .

sdo:ReportageNewsArticle
        rdfs:comment  "The [[ReportageNewsArticle]] type is a subtype of [[NewsArticle]] representing\n news articles which are the result of journalistic news reporting conventions.\n\nIn practice many news publishers produce a wide variety of article types, many of which might be considered a [[NewsArticle]] but not a [[ReportageNewsArticle]]. For example, opinion pieces, reviews, analysis, sponsored or satirical articles, or articles that combine several of these elements.\n\nThe [[ReportageNewsArticle]] type is based on a stricter ideal for \"news\" as a work of journalism, with articles based on factual information either observed or verified by the author, or reported and verified from knowledgeable sources.  This often includes perspectives from multiple viewpoints on a particular issue (distinguishing news reports from public relations or propaganda).  News reports in the [[ReportageNewsArticle]] sense de-emphasize the opinion of the author, with commentary and value judgements typically expressed elsewhere.\n\nA [[ReportageNewsArticle]] which goes deeper into analysis can also be marked with an additional type of [[AnalysisNewsArticle]].\n" ;
        rdfs:label    "ReportageNewsArticle" .

sdo:lodgingUnitType  rdfs:comment  "Textual description of the unit type (including suite vs. room, size of bed, etc.)." ;
        rdfs:label    "lodging unitType" .

sdo:partySize  rdfs:comment  "Number of people the reservation should accommodate." ;
        rdfs:label    "party size" .

sdo:instructor  rdfs:comment  "A person assigned to instruct or provide instructional assistance for the [[CourseInstance]]." ;
        rdfs:label    "instructor" .

sdo:Apartment  rdfs:comment  "An apartment (in American English) or flat (in British English) is a self-contained housing unit (a type of residential real estate) that occupies only part of a building (Source: Wikipedia, the free encyclopedia, see <a href=\"http://en.wikipedia.org/wiki/Apartment\">http://en.wikipedia.org/wiki/Apartment</a>)." ;
        rdfs:label    "Apartment" .

sdo:MerchantReturnEnumeration
        rdfs:comment  "Enumerates several kinds of product return policies." ;
        rdfs:label    "MerchantReturnEnumeration" .

sdo:gender  rdfs:comment  "Gender of something, typically a [[Person]], but possibly also fictional characters, animals, etc. While https://schema.org/Male and https://schema.org/Female may be used, text strings are also acceptable for people who do not identify as a binary gender. The [[gender]] property can also be used in an extended sense to cover e.g. the gender of sports teams. As with the gender of individuals, we do not try to enumerate all possibilities. A mixed-gender [[SportsTeam]] can be indicated with a text value of \"Mixed\"." ;
        rdfs:label    "gender" .

sdo:acrissCode  rdfs:comment  "The ACRISS Car Classification Code is a code used by many car rental companies, for classifying vehicles. ACRISS stands for Association of Car Rental Industry Systems and Standards." ;
        rdfs:label    "acriss code" .

sdo:requiredMaxAge  rdfs:comment  "Audiences defined by a person's maximum age." ;
        rdfs:label    "required maxAge" .

sdo:Hardcover  rdfs:comment  "Book format: Hardcover." ;
        rdfs:label    "Hardcover" .

sdo:financialAidEligible
        rdfs:comment  "A financial aid type or program which students may use to pay for tuition or fees associated with the program." ;
        rdfs:label    "financial aidEligible" .

sdo:SpecialAnnouncement
        rdfs:comment  "A SpecialAnnouncement combines a simple date-stamped textual information update\n      with contextualized Web links and other structured data.  It represents an information update made by a\n      locally-oriented organization, for example schools, pharmacies, healthcare providers,  community groups, police,\n      local government.\n\nFor work in progress guidelines on Coronavirus-related markup see [this doc](https://docs.google.com/document/d/14ikaGCKxo50rRM7nvKSlbUpjyIk2WMQd3IkB1lItlrM/edit#).\n\nThe motivating scenario for SpecialAnnouncement is the [Coronavirus pandemic](https://en.wikipedia.org/wiki/2019%E2%80%9320_coronavirus_pandemic), and the initial vocabulary is oriented to this urgent situation. Schema.org\nexpect to improve the markup iteratively as it is deployed and as feedback emerges from use. In addition to our\nusual [Github entry](https://github.com/schemaorg/schemaorg/issues/2490), feedback comments can also be provided in [this document](https://docs.google.com/document/d/1fpdFFxk8s87CWwACs53SGkYv3aafSxz_DTtOQxMrBJQ/edit#).\n\n\nWhile this schema is designed to communicate urgent crisis-related information, it is not the same as an emergency warning technology like [CAP](https://en.wikipedia.org/wiki/Common_Alerting_Protocol), although there may be overlaps. The intent is to cover\nthe kinds of everyday practical information being posted to existing websites during an emergency situation.\n\nSeveral kinds of information can be provided:\n\nWe encourage the provision of \"name\", \"text\", \"datePosted\", \"expires\" (if appropriate), \"category\" and\n\"url\" as a simple baseline. It is important to provide a value for \"category\" where possible, most ideally as a well known\nURL from Wikipedia or Wikidata. In the case of the 2019-2020 Coronavirus pandemic, this should be \"https://en.wikipedia.org/w/index.php?title=2019-20\\_coronavirus\\_pandemic\" or \"https://www.wikidata.org/wiki/Q81068910\".\n\nFor many of the possible properties, values can either be simple links or an inline description, depending on whether a summary is available. For a link, provide just the URL of the appropriate page as the property's value. For an inline description, use a [[WebContent]] type, and provide the url as a property of that, alongside at least a simple \"[[text]]\" summary of the page. It is\nunlikely that a single SpecialAnnouncement will need all of the possible properties simultaneously.\n\nWe expect that in many cases the page referenced might contain more specialized structured data, e.g. contact info, [[openingHours]], [[Event]], [[FAQPage]] etc. By linking to those pages from a [[SpecialAnnouncement]] you can help make it clearer that the events are related to the situation (e.g. Coronavirus) indicated by the [[category]] property of the [[SpecialAnnouncement]].\n\nMany [[SpecialAnnouncement]]s will relate to particular regions and to identifiable local organizations. Use [[spatialCoverage]] for the region, and [[announcementLocation]] to indicate specific [[LocalBusiness]]es and [[CivicStructure]]s. If the announcement affects both a particular region and a specific location (for example, a library closure that serves an entire region), use both [[spatialCoverage]] and [[announcementLocation]].\n\nThe [[about]] property can be used to indicate entities that are the focus of the announcement. We now recommend using [[about]] only\nfor representing non-location entities (e.g. a [[Course]] or a [[RadioStation]]). For places, use [[announcementLocation]] and [[spatialCoverage]]. Consumers of this markup should be aware that the initial design encouraged the use of /about for locations too.\n\nThe basic content of [[SpecialAnnouncement]] is similar to that of an [RSS](https://en.wikipedia.org/wiki/RSS) or [Atom](https://en.wikipedia.org/wiki/Atom_(Web_standard)) feed. For publishers without such feeds, basic feed-like information can be shared by posting\n[[SpecialAnnouncement]] updates in a page, e.g. using JSON-LD. For sites with Atom/RSS functionality, you can point to a feed\nwith the [[webFeed]] property. This can be a simple URL, or an inline [[DataFeed]] object, with [[encodingFormat]] providing\nmedia type information e.g. \"application/rss+xml\" or \"application/atom+xml\".\n" ;
        rdfs:label    "SpecialAnnouncement" .

sdo:potentialUse  rdfs:comment  "Intended use of the BioChemEntity by humans." ;
        rdfs:label    "potential use" .

sdo:candidate  rdfs:comment  "A sub property of object. The candidate subject of this action." ;
        rdfs:label    "candidate" .

sdo:TechArticle  rdfs:comment  "A technical article - Example: How-to (task) topics, step-by-step, procedural troubleshooting, specifications, etc." ;
        rdfs:label    "TechArticle" .

sdo:OfferItemCondition
        rdfs:comment  "A list of possible conditions for the item." ;
        rdfs:label    "OfferItemCondition" .

sdo:inProductGroupWithID
        rdfs:comment  "Indicates the [[productGroupID]] for a [[ProductGroup]] that this product [[isVariantOf]]. " ;
        rdfs:label    "in productGroupWithID" .

sdo:partOfTrip  rdfs:comment  "Identifies that this [[Trip]] is a subTrip of another Trip.  For example Day 1, Day 2, etc. of a multi-day trip." ;
        rdfs:label    "part ofTrip" .

sdo:RadioBroadcastService
        rdfs:comment  "A delivery service through which radio content is provided via broadcast over the air or online." ;
        rdfs:label    "RadioBroadcastService" .

sdo:expectedArrivalFrom
        rdfs:comment  "The earliest date the package may arrive." ;
        rdfs:label    "expected arrivalFrom" .

sdo:gtin13  rdfs:comment  "The GTIN-13 code of the product, or the product to which the offer refers. This is equivalent to 13-digit ISBN codes and EAN UCC-13. Former 12-digit UPC codes can be converted into a GTIN-13 code by simply adding a preceding zero. See [GS1 GTIN Summary](http://www.gs1.org/barcodes/technical/idkeys/gtin) for more details." ;
        rdfs:label    "gtin13" .

sdo:homeTeam  rdfs:comment  "The home team in a sports event." ;
        rdfs:label    "home team" .

sdo:actor  rdfs:comment  "An actor, e.g. in tv, radio, movie, video games etc., or in an event. Actors can be associated with individual items or with a series, episode, clip." ;
        rdfs:label    "actor" .

sdo:wordCount  rdfs:comment  "The number of words in the text of the Article." ;
        rdfs:label    "word count" .

sdo:ImageObjectSnapshot
        rdfs:comment  "A specific and exact (byte-for-byte) version of an [[ImageObject]]. Two byte-for-byte identical files, for the purposes of this type, considered identical. If they have different embedded metadata (e.g. XMP, EXIF) the files will differ. Different external facts about the files, e.g. creator or dateCreated that aren't represented in their actual content, do not affect this notion of identity." ;
        rdfs:label    "ImageObjectSnapshot" .

sdo:musicReleaseFormat
        rdfs:comment  "Format of this release (the type of recording media used, ie. compact disc, digital media, LP, etc.)." ;
        rdfs:label    "music releaseFormat" .

sdo:permissions  rdfs:comment  "Permission(s) required to run the app (for example, a mobile app may require full internet access or may run only on wifi)." ;
        rdfs:label    "permissions" .

sdo:menu  rdfs:comment  "Either the actual menu as a structured representation, as text, or a URL of the menu." ;
        rdfs:label    "menu" .

sdo:relevantOccupation
        rdfs:comment  "The Occupation for the JobPosting." ;
        rdfs:label    "relevant occupation" .

sdo:sha256  rdfs:comment  "The [SHA-2](https://en.wikipedia.org/wiki/SHA-2) SHA256 hash of the content of the item. For example, a zero-length input has value 'e3b0c44298fc1c149afbf4c8996fb92427ae41e4649b934ca495991b7852b855'" ;
        rdfs:label    "sha256" .

sdo:ScheduleAction  rdfs:comment  "Scheduling future actions, events, or tasks.\\n\\nRelated actions:\\n\\n* [[ReserveAction]]: Unlike ReserveAction, ScheduleAction allocates future actions (e.g. an event, a task, etc) towards a time slot / spatial allocation." ;
        rdfs:label    "ScheduleAction" .

sdo:status  rdfs:comment  "The status of the study (enumerated)." ;
        rdfs:label    "status" .

sdo:InformAction  rdfs:comment  "The act of notifying someone of information pertinent to them, with no expectation of a response." ;
        rdfs:label    "InformAction" .

sdo:tourBookingPage  rdfs:comment  "A page providing information on how to book a tour of some [[Place]], such as an [[Accommodation]] or [[ApartmentComplex]] in a real estate setting, as well as other kinds of tours as appropriate." ;
        rdfs:label    "tour bookingPage" .

sdo:medicalAudience  rdfs:comment  "Medical audience for page." ;
        rdfs:label    "medical audience" .

sdo:expectsAcceptanceOf
        rdfs:comment  "An Offer which must be accepted before the user can perform the Action. For example, the user may need to buy a movie before being able to watch it." ;
        rdfs:label    "expects acceptanceOf" .

sdo:ApprovedIndication
        rdfs:comment  "An indication for a medical therapy that has been formally specified or approved by a regulatory body that regulates use of the therapy; for example, the US FDA approves indications for most drugs in the US." ;
        rdfs:label    "ApprovedIndication" .

sdo:ProductGroup  rdfs:comment  "A ProductGroup represents a group of [[Product]]s that vary only in certain well-described ways, such as by [[size]], [[color]], [[material]] etc.\n\nWhile a ProductGroup itself is not directly offered for sale, the various varying products that it represents can be. The ProductGroup serves as a prototype or template, standing in for all of the products who have an [[isVariantOf]] relationship to it. As such, properties (including additional types) can be applied to the ProductGroup to represent characteristics shared by each of the (possibly very many) variants. Properties that reference a ProductGroup are not included in this mechanism; neither are the following specific properties [[variesBy]], [[hasVariant]], [[url]]. " ;
        rdfs:label    "ProductGroup" .

sdo:ElectronicsStore  rdfs:comment  "An electronics store." ;
        rdfs:label    "ElectronicsStore" .

sdo:EntertainmentBusiness
        rdfs:comment  "A business providing entertainment." ;
        rdfs:label    "EntertainmentBusiness" .

sdo:acceptedPaymentMethod
        rdfs:comment  "The payment method(s) accepted by seller for this offer." ;
        rdfs:label    "accepted paymentMethod" .

sdo:discountCode  rdfs:comment  "Code used to redeem a discount." ;
        rdfs:label    "discount code" .

sdo:postalCodePrefix  rdfs:comment  "A defined range of postal codes indicated by a common textual prefix. Used for non-numeric systems such as UK." ;
        rdfs:label    "postal codePrefix" .

sdo:TransformedContent
        rdfs:comment  "Content coded 'transformed content' in a [[MediaReview]], considered in the context of how it was published or shared.\n\nFor a [[VideoObject]] to be 'transformed content':  or all of the video has been manipulated to transform the footage itself. This category includes using tools like the Adobe Suite to change the speed of the video, add or remove visual elements or dub audio. Deepfakes are also a subset of transformation.\n\nFor an [[ImageObject]] to be transformed content': Adding or deleting visual elements to give the image a different meaning with the intention to mislead.\n\nFor an [[ImageObject]] with embedded text to be 'transformed content': Adding or deleting visual elements to give the image a different meaning with the intention to mislead.\n\nFor an [[AudioObject]] to be 'transformed content': Part or all of the audio has been manipulated to alter the words or sounds, or the audio has been synthetically generated, such as to create a sound-alike voice.\n" ;
        rdfs:label    "TransformedContent" .

sdo:CreditCard  rdfs:comment  "A card payment method of a particular brand or name.  Used to mark up a particular payment method and/or the financial product/service that supplies the card account.\\n\\nCommonly used values:\\n\\n* http://purl.org/goodrelations/v1#AmericanExpress\\n* http://purl.org/goodrelations/v1#DinersClub\\n* http://purl.org/goodrelations/v1#Discover\\n* http://purl.org/goodrelations/v1#JCB\\n* http://purl.org/goodrelations/v1#MasterCard\\n* http://purl.org/goodrelations/v1#VISA\n       " ;
        rdfs:label    "CreditCard" .

sdo:contentUrl  rdfs:comment  "Actual bytes of the media object, for example the image file or video file." ;
        rdfs:label    "content url" .

sdo:partOfSeries  rdfs:comment  "The series to which this episode or season belongs." ;
        rdfs:label    "part ofSeries" .

sdo:jobStartDate  rdfs:comment  "The date on which a successful applicant for this job would be expected to start work. Choose a specific date in the future or use the jobImmediateStart property to indicate the position is to be filled as soon as possible." ;
        rdfs:label    "job startDate" .

sdo:EndorsementRating
        rdfs:comment  "An EndorsementRating is a rating that expresses some level of endorsement, for example inclusion in a \"critic's pick\" blog, a\n\"Like\" or \"+1\" on a social network. It can be considered the [[result]] of an [[EndorseAction]] in which the [[object]] of the action is rated positively by\nsome [[agent]]. As is common elsewhere in schema.org, it is sometimes more useful to describe the results of such an action without explicitly describing the [[Action]].\n\nAn [[EndorsementRating]] may be part of a numeric scale or organized system, but this is not required: having an explicit type for indicating a positive,\nendorsement rating is particularly useful in the absence of numeric scales as it helps consumers understand that the rating is broadly positive.\n" ;
        rdfs:label    "EndorsementRating" .

sdo:album  rdfs:comment  "A music album." ;
        rdfs:label    "album" .

sdo:musicGroupMember  rdfs:comment  "A member of a music group&#x2014;for example, John, Paul, George, or Ringo." ;
        rdfs:label    "music groupMember" .

sdo:HighSchool  rdfs:comment  "A high school." ;
        rdfs:label    "HighSchool" .

sdo:reservedTicket  rdfs:comment  "A ticket associated with the reservation." ;
        rdfs:label    "reserved ticket" .

sdo:EventReservation  rdfs:comment  "A reservation for an event like a concert, sporting event, or lecture.\\n\\nNote: This type is for information about actual reservations, e.g. in confirmation emails or HTML pages with individual confirmations of reservations. For offers of tickets, use [[Offer]]." ;
        rdfs:label    "EventReservation" .

sdo:line  rdfs:comment  "A line is a point-to-point path consisting of two or more points. A line is expressed as a series of two or more point objects separated by space." ;
        rdfs:label    "line" .

sdo:sizeGroup  rdfs:comment  "The size group (also known as \"size type\") for a product's size. Size groups are common in the fashion industry to define size segments and suggested audiences for wearable products. Multiple values can be combined, for example \"men's big and tall\", \"petite maternity\" or \"regular\"" ;
        rdfs:label    "size group" .

sdo:PercutaneousProcedure
        rdfs:comment  "A type of medical procedure that involves percutaneous techniques, where access to organs or tissue is achieved via needle-puncture of the skin. For example, catheter-based procedures like stent delivery." ;
        rdfs:label    "PercutaneousProcedure" .

sdo:BodyMeasurementUnderbust
        rdfs:comment  "Girth of body just below the bust. Used, for example, to fit women's swimwear." ;
        rdfs:label    "BodyMeasurementUnderbust" .

sdo:orderNumber  rdfs:comment  "The identifier of the transaction." ;
        rdfs:label    "order number" .

sdo:AddAction  rdfs:comment  "The act of editing by adding an object to a collection." ;
        rdfs:label    "AddAction" .

sdo:accessMode  rdfs:comment  "The human sensory perceptual system or cognitive faculty through which a person may process or perceive information. Expected values include: auditory, tactile, textual, visual, colorDependent, chartOnVisual, chemOnVisual, diagramOnVisual, mathOnVisual, musicOnVisual, textOnVisual.\n      " ;
        rdfs:label    "access mode" .

sdo:actionStatus  rdfs:comment  "Indicates the current disposition of the Action." ;
        rdfs:label    "action status" .

sdo:priceComponentType
        rdfs:comment  "Identifies a price component (for example, a line item on an invoice), part of the total price for an offer." ;
        rdfs:label    "price componentType" .

sdo:FoodEvent  rdfs:comment  "Event type: Food event." ;
        rdfs:label    "FoodEvent" .

sdo:issueNumber  rdfs:comment  "Identifies the issue of publication; for example, \"iii\" or \"2\"." ;
        rdfs:label    "issue number" .

sdo:doseUnit  rdfs:comment  "The unit of the dose, e.g. 'mg'." ;
        rdfs:label    "dose unit" .

sdo:about  rdfs:comment  "The subject matter of the content." ;
        rdfs:label    "about" .

sdo:episodeNumber  rdfs:comment  "Position of the episode within an ordered group of episodes." ;
        rdfs:label    "episode number" .

sdo:costCurrency  rdfs:comment  "The currency (in 3-letter of the drug cost. See: http://en.wikipedia.org/wiki/ISO_4217. " ;
        rdfs:label    "cost currency" .

sdo:geoRadius  rdfs:comment  "Indicates the approximate radius of a GeoCircle (metres unless indicated otherwise via Distance notation)." ;
        rdfs:label    "geo radius" .

sdo:healthPlanNetworkTier
        rdfs:comment  "The tier(s) for this network." ;
        rdfs:label    "health planNetworkTier" .

sdo:BusOrCoach  rdfs:comment  "A bus (also omnibus or autobus) is a road vehicle designed to carry passengers. Coaches are luxury busses, usually in service for long distance travel." ;
        rdfs:label    "BusOrCoach" .

sdo:signOrSymptom  rdfs:comment  "A sign or symptom of this condition. Signs are objective or physically observable manifestations of the medical condition while symptoms are the subjective experience of the medical condition." ;
        rdfs:label    "sign orSymptom" .

sdo:sharedContent  rdfs:comment  "A CreativeWork such as an image, video, or audio clip shared as part of this posting." ;
        rdfs:label    "shared content" .

sdo:PetStore  rdfs:comment  "A pet store." ;
        rdfs:label    "PetStore" .

sdo:VisualArtwork  rdfs:comment  "A work of art that is primarily visual in character." ;
        rdfs:label    "VisualArtwork" .

sdo:MedicalSpecialty  rdfs:comment  "Any specific branch of medical science or practice. Medical specialities include clinical specialties that pertain to particular organ systems and their respective disease states, as well as allied health specialties. Enumerated type." ;
        rdfs:label    "MedicalSpecialty" .

sdo:WearableSizeSystemEN13402
        rdfs:comment  "EN 13402 (joint European standard for size labelling of clothes)." ;
        rdfs:label    "WearableSizeSystemEN13402" .

sdo:secondaryPrevention
        rdfs:comment  "A preventative therapy used to prevent reoccurrence of the medical condition after an initial episode of the condition." ;
        rdfs:label    "secondary prevention" .

sdo:Audiobook  rdfs:comment  "An audiobook." ;
        rdfs:label    "Audiobook" .

sdo:breadcrumb  rdfs:comment  "A set of links that can help a user understand and navigate a website hierarchy." ;
        rdfs:label    "breadcrumb" .

sdo:layoutImage  rdfs:comment  "A schematic image showing the floorplan layout." ;
        rdfs:label    "layout image" .

sdo:availableTest  rdfs:comment  "A diagnostic test or procedure offered by this lab." ;
        rdfs:label    "available test" .

sdo:availableStrength
        rdfs:comment  "An available dosage strength for the drug." ;
        rdfs:label    "available strength" .

sdo:Car  rdfs:comment  "A car is a wheeled, self-powered motor vehicle used for transportation." ;
        rdfs:label    "Car" .

sdo:legislationType  rdfs:comment  "The type of the legislation. Examples of values are \"law\", \"act\", \"directive\", \"decree\", \"regulation\", \"statutory instrument\", \"loi organique\", \"règlement grand-ducal\", etc., depending on the country." ;
        rdfs:label    "legislation type" .

sdo:baseSalary  rdfs:comment  "The base salary of the job or of an employee in an EmployeeRole." ;
        rdfs:label    "base salary" .

sdo:hasMeasurement  rdfs:comment  "A product measurement, for example the inseam of pants, the wheel size of a bicycle, or the gauge of a screw. Usually an exact measurement, but can also be a range of measurements for adjustable products, for example belts and ski bindings." ;
        rdfs:label    "has measurement" .

sdo:priceSpecification
        rdfs:comment  "One or more detailed price specifications, indicating the unit price and delivery or payment charges." ;
        rdfs:label    "price specification" .

sdo:schemaVersion  rdfs:comment  "Indicates (by URL or string) a particular version of a schema used in some CreativeWork. This property was created primarily to\n    indicate the use of a specific schema.org release, e.g. ```10.0``` as a simple string, or more explicitly via URL, ```https://schema.org/docs/releases.html#v10.0```. There may be situations in which other schemas might usefully be referenced this way, e.g. ```http://dublincore.org/specifications/dublin-core/dces/1999-07-02/``` but this has not been carefully explored in the community." ;
        rdfs:label    "schema version" .

sdo:BeautySalon  rdfs:comment  "Beauty salon." ;
        rdfs:label    "BeautySalon" .

sdo:ReimbursementCap  rdfs:comment  "The drug's cost represents the maximum reimbursement paid by an insurer for the drug." ;
        rdfs:label    "ReimbursementCap" .

sdo:constrainingProperty
        rdfs:comment  "Indicates a property used as a constraint to define a [[StatisticalPopulation]] with respect to the set of entities\n  corresponding to an indicated type (via [[populationType]])." ;
        rdfs:label    "constraining property" .

sdo:AMRadioChannel  rdfs:comment  "A radio channel that uses AM." ;
        rdfs:label    "AMRadioChannel" .

sdo:InfectiousDisease
        rdfs:comment  "An infectious disease is a clinically evident human disease resulting from the presence of pathogenic microbial agents, like pathogenic viruses, pathogenic bacteria, fungi, protozoa, multicellular parasites, and prions. To be considered an infectious disease, such pathogens are known to be able to cause this disease." ;
        rdfs:label    "InfectiousDisease" .

sdo:GeoCircle  rdfs:comment  "A GeoCircle is a GeoShape representing a circular geographic area. As it is a GeoShape\n          it provides the simple textual property 'circle', but also allows the combination of postalCode alongside geoRadius.\n          The center of the circle can be indicated via the 'geoMidpoint' property, or more approximately using 'address', 'postalCode'.\n       " ;
        rdfs:label    "GeoCircle" .

sdo:transFatContent  rdfs:comment  "The number of grams of trans fat." ;
        rdfs:label    "trans fatContent" .

sdo:includesAttraction
        rdfs:comment  "Attraction located at destination." ;
        rdfs:label    "includes attraction" .

sdo:valueReference  rdfs:comment  "A secondary value that provides additional information on the original value, e.g. a reference temperature or a type of measurement." ;
        rdfs:label    "value reference" .

sdo:positiveNotes  rdfs:comment  "Indicates, in the context of a [[Review]] (e.g. framed as 'pro' vs 'con' considerations), positive considerations - either as unstructured text, or a list." ;
        rdfs:label    "positive notes" .

sdo:requirements  rdfs:comment  "Component dependency requirements for application. This includes runtime environments and shared libraries that are not included in the application distribution package, but required to run the application (Examples: DirectX, Java or .NET runtime)." ;
        rdfs:label    "requirements" .

sdo:ReceiveAction  rdfs:comment  "The act of physically/electronically taking delivery of an object that has been transferred from an origin to a destination. Reciprocal of SendAction.\\n\\nRelated actions:\\n\\n* [[SendAction]]: The reciprocal of ReceiveAction.\\n* [[TakeAction]]: Unlike TakeAction, ReceiveAction does not imply that the ownership has been transfered (e.g. I can receive a package, but it does not mean the package is now mine)." ;
        rdfs:label    "ReceiveAction" .

sdo:GeoShape  rdfs:comment  "The geographic shape of a place. A GeoShape can be described using several properties whose values are based on latitude/longitude pairs. Either whitespace or commas can be used to separate latitude and longitude; whitespace should be used when writing a list of several such points." ;
        rdfs:label    "GeoShape" .

sdo:WearableSizeGroupBig
        rdfs:comment  "Size group \"Big\" for wearables." ;
        rdfs:label    "WearableSizeGroupBig" .

sdo:educationalRole  rdfs:comment  "An educationalRole of an EducationalAudience." ;
        rdfs:label    "educational role" .

sdo:marginOfError  rdfs:comment  "A marginOfError for an [[Observation]]." ;
        rdfs:label    "margin ofError" .

sdo:cvdNumTotBeds  rdfs:comment  "numtotbeds - ALL HOSPITAL BEDS: Total number of all Inpatient and outpatient beds, including all staffed,ICU, licensed, and overflow (surge) beds used for inpatients or outpatients." ;
        rdfs:label    "cvd numTotBeds" .

sdo:characterName  rdfs:comment  "The name of a character played in some acting or performing role, i.e. in a PerformanceRole." ;
        rdfs:label    "character name" .

sdo:State  rdfs:comment  "A state or province of a country." ;
        rdfs:label    "State" .

rdfs:member  rdfs:label  "member" .

rdfs:ContainerMembershipProperty
        rdfs:label  "ContainerMembershipProperty" .

<https://purl.org/NET/rdflicense/cc-by4.0>
        rdfs:label  "Creative Commons BY 4.0" .
