PREFIX cs: <https://gswa.vocabs.kurrawong.ai/borehole-configuration>
PREFIX dcat: <http://www.w3.org/ns/dcat#>
PREFIX dcterms: <http://purl.org/dc/terms/>
PREFIX ex: <https://gswa.vocabs.kurrawong.ai/borehole-design/>
PREFIX isoroles: <http://def.isotc211.org/iso19115/-1/2018/CitationAndResponsiblePartyInformation/code/CI_RoleCode/>
PREFIX owl: <http://www.w3.org/2002/07/owl#>
PREFIX prov: <http://www.w3.org/ns/prov#>
PREFIX rdfs: <http://www.w3.org/2000/01/rdf-schema#>
PREFIX skos: <http://www.w3.org/2004/02/skos/core#>
PREFIX xsd: <http://www.w3.org/2001/XMLSchema#> 

<http://linked.data.gov.au/def/borehole-design/inclineddown>
    a skos:Concept ;
    dcterms:source "http://linked.data.gov.au/def/borehole-design/inclineddown"^^xsd:anyURI ;
    rdfs:isDefinedBy <https://linked.data.gov.au/def/borehole-design> ;
    skos:altLabel "downhole"@en ;
    skos:definition "A borehole drilled from the start point at a pre-set nonvertical angle below horizontal (drilled downwards)."@en ;
    skos:historyNote "mineral industry concept" ;
    skos:inScheme cs: ;
    skos:narrower
        <http://linked.data.gov.au/def/borehole-design/inclineddown> ,
        <http://linked.data.gov.au/def/borehole-design/inclinedup> ;
    skos:prefLabel "inclined down updated"@en ;
.

<http://linked.data.gov.au/def/borehole-design/inclinedup>
    a skos:Concept ;
    dcterms:source "http://linked.data.gov.au/def/borehole-design/inclinedup"^^xsd:anyURI ;
    rdfs:isDefinedBy <https://linked.data.gov.au/def/borehole-design> ;
    skos:altLabel "uphole"@en ;
    skos:definition "A borehole drilled from the start point at a pre-set nonvertical angle above horizontal (drilled upwards)."@en ;
    skos:historyNote "mineral industry concept" ;
    skos:inScheme cs: ;
    skos:prefLabel "inclined up updated"@en ;
.

<http://linked.data.gov.au/def/borehole-design/vertical>
    a skos:Concept ;
    dcterms:source """http://linked.data.gov.au/def/borehole-design/vertical
https://coringmagazine.com/article/directional-diamond-drilling-definitions-terms-simple-calculations/"""^^xsd:anyURI ;
    rdfs:isDefinedBy <https://linked.data.gov.au/def/borehole-design> ;
    skos:definition "A borehole drilled in a vertical downwards direction with the intent of maintaining a vertical trajectory. Deviations up to 2° from the vertical line are usually accepted as 'vertical’."@en ;
    skos:historyNote "resource industry concept" ;
    skos:inScheme cs: ;
    skos:prefLabel "vertical"@en ;
    skos:topConceptOf cs: ;
.

ex:directional
    a skos:Concept ;
    dcterms:source """https://glossary.americangeosciences.org/term/directionaldrilling
https://glossary.slb.com/en/terms/d/directional_well
https://linked.data.gov.au/def/borehole-design/deviated
https://coringmagazine.com/article/directional-diamond-drilling-definitions-terms-simple-calculations/"""^^xsd:anyURI ;
    skos:closeMatch <https://linked.data.gov.au/def/borehole-design/deviated> ;
    skos:definition "A borehole intentionally drilled at controlled departures from the vertical or parent borehole trajectory and at controlled azimuths, achieved with the use of geosteering equipment or via other methods (e.g. directional wedge). The main purpose is usually to establish multiple boreholes from a single location and/or to intersect a target or zone of interest. Note that the term 'deviated' is not recommended as an alternate label of 'directional', as it can be used to refer to a borehole that unintentionally deviates from the intended trajectory."@en ;
    skos:historyNote "energy and mineral industry concept" ;
    skos:inScheme cs: ;
    skos:narrower
        ex:extended-reach ,
        ex:lateral ;
    skos:prefLabel "directional"@en ;
    skos:topConceptOf cs: ;
.

ex:extended-reach-well
    a skos:Concept ;
    dcterms:source """https://petrowiki.spe.org/Extended_reach_wells
https://glossary.slb.com/en/terms/e/extended-reach_drilling"""^^xsd:anyURI ;
    skos:definition "A directional well in which the ratio of the measured depth (MD) vs the true vertical depth (TVD) is at least 2:1."@en ;
    skos:historyNote "energy industry concept" ;
    skos:inScheme cs: ;
    skos:prefLabel "extended-reach"@en ;
    skos:topConceptOf cs: ;
.

ex:horizontal
    a skos:Concept ;
    dcterms:source """https://glossary.slb.com/en/terms/h/horizontal_drilling
https://petrowiki.spe.org/Horizontal_wells"""^^xsd:anyURI ;
    skos:definition "A borehole drilled in a horizontal direction. In the energy industry, this is achieved with geosteering equipment and applies to boreholes where the departure from vertical exceeds about 80°. In the mineral industry, horizontal drilling is typically carried out from an underground location or on the wall of an open pit."@en ;
    skos:historyNote "resource industry concept" ;
    skos:inScheme cs: ;
    skos:prefLabel "horizontal"@en ;
    skos:relatedMatch <http://linked.data.gov.au/def/borehole-design/lateral> ;
    skos:topConceptOf cs: ;
.

ex:inclined
    a skos:Concept ;
    skos:altLabel "angled"@en ;
    skos:definition "A borehole drilled from the start point at a pre-set nonvertical angle above or below horizontal."@en ;
    skos:historyNote "mineral industry concept" ;
    skos:inScheme cs: ;
    skos:prefLabel "inclined"@en ;
    skos:topConceptOf cs: ;
.

ex:lateral
    a skos:Concept ;
    dcterms:source "https://glossary.americangeosciences.org/term/lateraldrill"^^xsd:anyURI ;
    skos:closeMatch <http://linked.data.gov.au/def/borehole-design/lateral> ;
    skos:definition "A borehole drilled with geosteering equipment with the intent of controlling the trajectory to drill laterally within a targeted stratigraphic interval or intervals. Usually, but not always, drilled close to horizontal and for relatively short distances."@en ;
    skos:historyNote "energy industry concept" ;
    skos:inScheme cs: ;
    skos:prefLabel "lateral"@en ;
.

ex:vertical-uphole
    a skos:Concept ;
    skos:definition "A borehole drilled underground from the start point in a pre-set vertical upwards direction."@en ;
    skos:historyNote "resource industry concept" ;
    skos:inScheme cs: ;
    skos:prefLabel "vertical uphole"@en ;
    skos:topConceptOf cs: ;
.

<https://linked.data.gov.au/org/gswa>
    a prov:Agent ;
    rdfs:label "Gswa" ;
.

cs:
    a skos:ConceptScheme ;
    dcterms:created "2023-09-01"^^xsd:date ;
    dcterms:creator <https://linked.data.gov.au/org/gswa> ;
    dcterms:identifier "borehole-configuration"^^xsd:token ;
    dcterms:modified "2023-09-01"^^xsd:date ;
    dcterms:publisher <https://linked.data.gov.au/org/gswa> ;
    owl:versionIRI <https://gswa.vocabs.kurrawong.ai/borehole-configuration/1> ;
    owl:versionInfo "1" ;
    skos:definition "A description of the intended configuration and trajectory of a borehole, covering concepts from the energy and mineral resources industry. Note that most of the concepts in this vocabulary apply to both the process of drilling (e.g. directional drilling), as well as to an actual borehole (e.g. directional well), even if the definitions in this vocabulary focus specifically on the latter."@en ;
    skos:hasTopConcept
        <http://linked.data.gov.au/def/borehole-design/vertical> ,
        ex:directional ,
        ex:extended-reach-well ,
        ex:horizontal ,
        ex:inclined ,
        ex:vertical-uphole ;
    skos:historyNote "Terms and definitions are predominantly sourced from the Geological Survey of Queensland's Borehole start point vocabulary (https://linked.data.gov.au/def/borehole-design), with some modifications and additional concepts from [WAPIMS].[dbo].(BoreholeReason] and [WAPIMS].[dbo].[Keywords]."@en ;
    skos:prefLabel "Borehole configuration"@en ;
    prov:qualifiedAttribution [
            dcat:hadRole isoroles:custodian ;
            prov:agent [
                    a prov:Agent ;
                    rdfs:label " Erin Gray"
                ]
        ] ;
.
